<?xml version="1.0" encoding="UTF-8"?>
<rdf:RDF xmlns:owl="http://www.w3.org/2002/07/owl#"
         xmlns:rdfs="http://www.w3.org/2000/01/rdf-schema#"
         xmlns:rdf="http://www.w3.org/1999/02/22-rdf-syntax-ns#"
         xmlns:skos="http://www.w3.org/2004/02/skos/core#"
         xmlns:office="urn:oasis:names:tc:opendocument:xmlns:office:1.0"
         xmlns:style="urn:oasis:names:tc:opendocument:xmlns:style:1.0"
         xmlns:text="urn:oasis:names:tc:opendocument:xmlns:text:1.0"
         xmlns:table="urn:oasis:names:tc:opendocument:xmlns:table:1.0"
         xmlns:draw="urn:oasis:names:tc:opendocument:xmlns:drawing:1.0"
         xmlns:fo="urn:oasis:names:tc:opendocument:xmlns:xsl-fo-compatible:1.0"
         xmlns:xlink="http://www.w3.org/1999/xlink"
         xmlns:dc="http://purl.org/dc/elements/1.1/"
         xmlns:meta="urn:oasis:names:tc:opendocument:xmlns:meta:1.0"
         xmlns:number="urn:oasis:names:tc:opendocument:xmlns:datastyle:1.0"
         xmlns:svg="urn:oasis:names:tc:opendocument:xmlns:svg-compatible:1.0"
         xmlns:chart="urn:oasis:names:tc:opendocument:xmlns:chart:1.0"
         xmlns:dr3d="urn:oasis:names:tc:opendocument:xmlns:dr3d:1.0"
         xmlns:math="http://www.w3.org/1998/Math/MathML"
         xmlns:form="urn:oasis:names:tc:opendocument:xmlns:form:1.0"
         xmlns:script="urn:oasis:names:tc:opendocument:xmlns:script:1.0"
         xmlns:ooo="http://openoffice.org/2004/office"
         xmlns:ooow="http://openoffice.org/2004/writer"
         xmlns:oooc="http://openoffice.org/2004/calc"
         xmlns:dom="http://www.w3.org/2001/xml-events"
         xmlns:xforms="http://www.w3.org/2002/xforms"
         xmlns:xsd="http://www.w3.org/2001/XMLSchema"
         xmlns:xsi="http://www.w3.org/2001/XMLSchema-instance"
         xmlns:rpt="http://openoffice.org/2005/report"
         xmlns:of="urn:oasis:names:tc:opendocument:xmlns:of:1.2"
         xmlns:xhtml="http://www.w3.org/1999/xhtml"
         xmlns:grddl="http://www.w3.org/2003/g/data-view#"
         xmlns:tableooo="http://openoffice.org/2009/table"
         xmlns:textooo="http://openoffice.org/2013/office"
         xmlns:field="urn:openoffice:names:experimental:ooo-ms-interop:xmlns:field:1.0"><!--

	- - FRVRoo V2.4 Draft November 2015   - converted from http://www.cidoc-crm.org/docs/frbr_oo/frbr_docs/FRBRoo_V2.4.docx
        	-->
   <owl:Ontology rdf:about="">
      <rdfs:label xml:lang="en"/>
      <owl:versionInfo rdf:datatype="xsd:string">This is a version of the FRBRoo 2.4 specifications in OWL that is based on the structure of the current efrbroo and the text file (odt), realised by Biblissima April 2O16</owl:versionInfo>
   </owl:Ontology>
   <!--

	- - Annotation properties

        	-->
   <!-- http://www.w3.org/2004/02/skos/core#notation -->
   <owl:AnnotationProperty rdf:about="skos:notation"/>
   <!--

	- - Classes

        	-->
   <!--F1_Work-->
   <owl:Class rdf:about="http://erlangen-crm.org/efrbroo/F1_Work">
      <rdfs:label xml:lang="en">F1 Work</rdfs:label>
      <rdfs:subClassOf rdf:resource="http://erlangen-crm.org/current/E89_Propositional_Object"/>
      <rdfs:superClassOf rdf:resource="http://erlangen-crm.org/efrbroo/F14_Individual_Work"/>
      <rdfs:superClassOf rdf:resource="http://erlangen-crm.org/efrbroo/F15_Complex_Work"/>
      <rdfs:superClassOf rdf:resource="http://erlangen-crm.org/efrbroo/F16_Container_Work"/>
      <rdfs:superClassOf rdf:resource="http://erlangen-crm.org/efrbroo/F21_Recording_Work"/>
      <rdfs:comment>Scope note:
This class comprises distinct concepts or combinations of concepts identified in artistic and intellectual expressions, such as poems, stories or musical compositions. Such concepts may appear in the course of the coherent evolution of an original idea into one or more expressions that are dominated by the original idea. A Work may be elaborated by one or more Actors simultaneously or over time. The substance of Work is ideas. A Work may have members that are works in their own right.
A Work can be either individual or complex. If it is individual its concept is completely realised in a single F22 Self-Contained Expression. If it is complex its concept is embedded in an F15 Complex Work. An F15 Complex Work consists of alternative members that are either F15 Complex Works themselves or F14 Individual Works.
A Work is the product of an intellectual process of one or more persons, yet only indirect evidence about it is at our hands. This can be contextual information such as the existence of an order for a work, reflections of the creators themselves that are documented somewhere, and finally the expressions of the work created. As ideas normally take shape during discussion, elaboration and implementation, it is not reasonable to assume that a work starts with a complete concept. In some cases, it can be very difficult or impossible to define the whole of the concept of a work at a particular time. The objective evidence for such a notion can only be based on a stage of expressions at a given time. In this sense, the sets of ideas that constitute particular self-contained expressions may be regarded as a kind of “snap-shot” of a work.
A Work may include the concept of aggregating expressions of other works into a new expression. For instance, an anthology of poems is regarded as a work in its own right that makes use of expressions of the individual poems that have been selected and ordered as part of an intellectual process. This does not make the contents of the aggregated expressions part of this work, but only parts of the resulting expression.

</rdfs:comment>
      <rdfs:comment>Examples:
Abstract content of Giovanni Battista Piranesi’s ‘Carcere XVI: the pier with chains: 1st state’ (F14)
‘La Porte de l’Enfer’ by Auguste Rodin conceived between 1880 and 1917 (F15)
‘Hamlet’ by William Shakespeare (F15)

</rdfs:comment>
      <rdfs:comment>Properties:
R1 is logical successor of (has successor): F1 Work
R2 is derivative of (has derivative): F1 Work
(R2.1 has type: E55 Type)
R3 is realised in (realises): F22 Self-Contained Expression
R40 has representative expression (is representative expression for): F22 Self-Contained Expression

</rdfs:comment>
      <rdfs:subClassOf>
         <owl:Restriction>
            <owl:onProperty>
               <owl:ObjectProperty rdf:about="http://erlangen-crm.org/efrbroo/R1_is_logical_successor_of"/>
            </owl:onProperty>
            <owl:someValuesFrom rdf:resource="http://erlangen-crm.org/efrbroo/F1_Work"/>
         </owl:Restriction>
      </rdfs:subClassOf>
      <rdfs:subClassOf>
         <owl:Restriction>
            <owl:onProperty>
               <owl:ObjectProperty rdf:about="http://erlangen-crm.org/efrbroo/R2_is_derivative_of"/>
            </owl:onProperty>
            <owl:someValuesFrom rdf:resource="http://erlangen-crm.org/efrbroo/F1_Work"/>
         </owl:Restriction>
      </rdfs:subClassOf>
      <rdfs:subClassOf>
         <owl:Restriction>
            <owl:onProperty>
               <owl:ObjectProperty rdf:about="http://erlangen-crm.org/efrbroo/R3_is_realised_in"/>
            </owl:onProperty>
            <owl:someValuesFrom rdf:resource="http://erlangen-crm.org/efrbroo/F1_Work"/>
         </owl:Restriction>
      </rdfs:subClassOf>
      <rdfs:subClassOf>
         <owl:Restriction>
            <owl:onProperty>
               <owl:ObjectProperty rdf:about="http://erlangen-crm.org/efrbroo/R40_has_representative_expression"/>
            </owl:onProperty>
            <owl:someValuesFrom rdf:resource="http://erlangen-crm.org/efrbroo/F1_Work"/>
         </owl:Restriction>
      </rdfs:subClassOf>
   </owl:Class>
   <!--F2_Expression-->
   <owl:Class rdf:about="http://erlangen-crm.org/efrbroo/F2_Expression">
      <rdfs:label xml:lang="en">F2 Expression</rdfs:label>
      <rdfs:subClassOf rdf:resource="http://erlangen-crm.org/current/E73_Information_Object"/>
      <rdfs:superClassOf rdf:resource="http://erlangen-crm.org/efrbroo/F22_Self-Contained_Expression"/>
      <rdfs:superClassOf rdf:resource="http://erlangen-crm.org/efrbroo/F23_Expression_Fragment"/>
      <rdfs:superClassOf rdf:resource="http://erlangen-crm.org/efrbroo/F34_KOS"/>
      <rdfs:superClassOf rdf:resource="http://erlangen-crm.org/efrbroo/F35_Nomen_Use_Statement"/>
      <rdfs:superClassOf rdf:resource="http://erlangen-crm.org/efrbroo/F43_Identifier_Rule"/>
      <rdfs:comment>Scope note:
This class comprises the intellectual or artistic realisations of works in the form of identifiable immaterial objects, such as texts, poems, jokes, musical or choreographic notations, movement pattern, sound pattern, images, multimedia objects, or any combination of such forms that have objectively recognisable structures. The substance of F2 Expression is signs.
Expressions cannot exist without a physical carrier, but do not depend on a specific physical carrier and can exist on one or more carriers simultaneously. Carriers may include human memory.
Inasmuch as the form of F2 Expression is an inherent characteristic of the F2 Expression, any change in form (e.g., from alpha-numeric notation to spoken word, a poem created in capitals and rendered in lower case) is a new F2 Expression. Similarly, changes in the intellectual conventions or instruments that are employed to express a work (e.g., translation from one language to another) result in the creation of a new F2 Expression. Thus, if a text is revised or modified, the resulting F2 Expression is considered to be a new F2 Expression. Minor changes, such as corrections of spelling and punctuation, etc., are normally considered variations within the same F2 Expression. On a practical level, the degree to which distinctions are made between variant expressions of a work will depend to some extent on the nature of the F1 Work itself, and on the anticipated needs of users.
The genre of the work may provide an indication of which features are essential to the expression. In some cases, aspects of physical form, such as typeface and page layout, are not integral to the intellectual or artistic realisation of the work as such, and therefore are not distinctive criteria for the respective expressions. For another work, features such as layout may be essential. For instance, the author or a graphic designer may wrap a poem around an image.
An expression of a work may include expressions of other works within it. For instance, an anthology of poems is regarded as a work in its own right that makes use of expressions of the individual poems that have been selected and ordered as part of an intellectual process. This does not make the contents of the aggregated expressions part of this work, but only parts of the resulting expression.
If an instance of F2 Expression is of a specific form, such as text, image, etc., it may be simultaneously instantiated in the specific classes representing these forms in CIDOC CRM. Thereby one can make use of the more specific properties of these classes, such as language (which is applicable to instances of E33 Linguistic Object only).

</rdfs:comment>
      <rdfs:comment>Examples:
The Italian text of Dante’s ‘Divina Commedia’ as found in the authoritative critical edition ‘La Commedia secondo l’antica vulgata a cura di Giorgio Petrocchi’, Milano: Mondadori, 1966-67 (= Le Opere di Dante Alighieri, Edizione Nazionale a cura della Società Dantesca Italiana, VII, 1-4) (F22 and E33)
The Italian text of Dante’s ‘Inferno’ as found in the same edition (F22 and E33)
‘Nel mezzo del cammin di nostra vitami ritrovai per una selva oscuraché la diritta via era smarrita’ [the Italian text of the first stanza of Dante’s ‘Inferno’ and ‘Divina Commedia’] (F23 and E33)
The signs which make up Christian Morgenstern’s ‘Fisches Nachtgesang’ [a poem consisting simply of ‘—’ and ‘˘’ signs, arranged in a determined combination] (F22)

</rdfs:comment>
      <rdfs:comment>Properties:
R4 carriers provided by (comprises carriers of): F3 Manifestation Product Type
R5 has component (is component of): F22 Self-Contained Expression
R15 has fragment (is fragment of): F23 Expression Fragment
R41 has representative manifestation product type (is representative manifestation product type for): F3 Manifestation Product Type

</rdfs:comment>
      <rdfs:subClassOf>
         <owl:Restriction>
            <owl:onProperty>
               <owl:ObjectProperty rdf:about="http://erlangen-crm.org/efrbroo/R4_carriers_provided_by"/>
            </owl:onProperty>
            <owl:minCardinality rdf:datatype="http://www.w3.org/2001/XMLSchema#nonNegativeInteger">1</owl:minCardinality>
         </owl:Restriction>
      </rdfs:subClassOf>
      <rdfs:subClassOf>
         <owl:Restriction>
            <owl:onProperty>
               <owl:ObjectProperty rdf:about="http://erlangen-crm.org/efrbroo/R5_has_component"/>
            </owl:onProperty>
            <owl:someValuesFrom rdf:resource="http://erlangen-crm.org/efrbroo/F2_Expression"/>
         </owl:Restriction>
      </rdfs:subClassOf>
      <rdfs:subClassOf>
         <owl:Restriction>
            <owl:onProperty>
               <owl:ObjectProperty rdf:about="http://erlangen-crm.org/efrbroo/R15_has_fragment"/>
            </owl:onProperty>
            <owl:someValuesFrom rdf:resource="http://erlangen-crm.org/efrbroo/F2_Expression"/>
         </owl:Restriction>
      </rdfs:subClassOf>
      <rdfs:subClassOf>
         <owl:Restriction>
            <owl:onProperty>
               <owl:ObjectProperty rdf:about="http://erlangen-crm.org/efrbroo/R41_has_representative_manifestation_product_type"/>
            </owl:onProperty>
            <owl:someValuesFrom rdf:resource="http://erlangen-crm.org/efrbroo/F2_Expression"/>
         </owl:Restriction>
      </rdfs:subClassOf>
   </owl:Class>
   <!--F3_Manifestation_Product_Type-->
   <owl:Class rdf:about="http://erlangen-crm.org/efrbroo/F3_Manifestation_Product_Type">
      <rdfs:label xml:lang="en">F3 Manifestation Product Type</rdfs:label>
      <rdfs:subClassOf rdf:resource="http://erlangen-crm.org/current/E55_Type"/>
      <rdfs:subClassOf rdf:resource="http://erlangen-crm.org/current/E72_Legal_Object"/>
      <rdfs:comment>Scope note:
This class comprises the definitions of publication products.
An instance of F3 Manifestation Product Type is the “species”, and all copies of a given object are “specimens” of it. An instance of F3 Manifestation Product Type defines all of the features or traits that instances of F5 Item normally display in order that they may be recognised as copies of a particular publication. However, due to production problems or subsequent events, one or more instances of F5 Item may not exhibit all these features or traits; yet such instances still retain their relationship to the same instance of F3 Manifestation Product Type.
The features that characterise a given instance of F3 Manifestation Product Type include: one instance of F24 Publication Expression, containing one or more than one instance of F2 Expression, reflecting the authors’ content of the manifestation and all additional input by the publisher; and the appropriate types of physical features for that form of the object. For example, hardcover and paperback are two distinct publications (i.e. two distinct instances of F3 Manifestation Product Type) even though authorial and editorial content are otherwise identical in both publications. The activity of cataloguing aims at the most accurate listing of features or traits of an instance of F3 Manifestation Product Type that are sufficient to distinguish it from another instance of F3 Manifestation Product Type.

</rdfs:comment>
      <rdfs:comment>Examples:
The publication product containing the text entitled ‘Harmonie universelle’ (authored by the person named ‘Marin Mersenne’), issued in 1636 in Paris by the publisher named ‘Sébastien Cramoisy’
The publication product containing a modern reprint of Marin Mersenne’s ‘Harmonie universelle’, issued in 1986 in Paris by the publisher named ‘Les éditions du CNRS’, and identified by ISBN ‘2-222-00835-2’
The publication product containing the third edition of the combination of texts and graphics titled ‘Codex Manesse: die Miniaturen der großen Heidelberger Liederhandschrift, herausgegeben und erläutert von Ingo F. Walther unter Mitarbeit von Gisela Siebert’, issued by the publisher named ‘Insel-Verlag’ in 1988
The publication product containing the cartographic resource titled ‘Ordnance Survey Explorer Map 213, Aberystwyth &amp; Cwm Rheidol’, issued in May 2005 by the publisher named ‘Ordnance Survey’ and identified by ISBN ‘0-319-23640-4’ (folded), 1:25,000 scale
The publication product containing the recordings of musical works performed by the person named ‘Florence Foster Jenkins’ gathered under the title ‘The Glory (????) of the human voice’, identified by label and label number ‘RCA Victor Gold Seal GD61175’ (Note: the four question marks within parentheses belong to the title itself)

</rdfs:comment>
      <rdfs:comment>Properties:
CLP2 should have type (should be type of): E55 Type
CLP43 should have dimension (should be dimension of): E54 Dimension
CLP45 should consist of (should be incorporated in): E57 Material
CLP46 should be composed of (may form part of): F3 Manifestation Product Type
CLP57 should have number of parts: E60 Number
CLP104 subject to (applies to): E30 Right
CLP105 right held by (right on): E39 Actor
CLR6 should carry (should be carried by): F24 Publication Expression

</rdfs:comment>
      <rdfs:subClassOf>
         <owl:Restriction>
            <owl:onProperty>
               <owl:ObjectProperty rdf:about="http://erlangen-crm.org/efrbroo/CLP2_should_have_type"/>
            </owl:onProperty>
            <owl:someValuesFrom rdf:resource="http://erlangen-crm.org/efrbroo/F3_Manifestation_Product_Type"/>
         </owl:Restriction>
      </rdfs:subClassOf>
      <rdfs:subClassOf>
         <owl:Restriction>
            <owl:onProperty>
               <owl:ObjectProperty rdf:about="http://erlangen-crm.org/efrbroo/CLP43_should_have_dimension"/>
            </owl:onProperty>
            <owl:minCardinality rdf:datatype="http://www.w3.org/2001/XMLSchema#nonNegativeInteger">1</owl:minCardinality>
         </owl:Restriction>
      </rdfs:subClassOf>
      <rdfs:subClassOf>
         <owl:Restriction>
            <owl:onProperty>
               <owl:ObjectProperty rdf:about="http://erlangen-crm.org/efrbroo/CLP45_should_consist_of"/>
            </owl:onProperty>
            <owl:someValuesFrom rdf:resource="http://erlangen-crm.org/efrbroo/F3_Manifestation_Product_Type"/>
         </owl:Restriction>
      </rdfs:subClassOf>
      <rdfs:subClassOf>
         <owl:Restriction>
            <owl:onProperty>
               <owl:ObjectProperty rdf:about="http://erlangen-crm.org/efrbroo/CLP46_should_be_composed_of"/>
            </owl:onProperty>
            <owl:someValuesFrom rdf:resource="http://erlangen-crm.org/efrbroo/F3_Manifestation_Product_Type"/>
         </owl:Restriction>
      </rdfs:subClassOf>
      <rdfs:subClassOf>
         <owl:Restriction>
            <owl:cardinality rdf:datatype="http://www.w3.org/2001/XMLSchema#nonNegativeInteger">1</owl:cardinality>
            <owl:onProperty>
               <owl:ObjectProperty rdf:about="http://erlangen-crm.org/efrbroo/CLP57_should_have_number_of_parts"/>
            </owl:onProperty>
         </owl:Restriction>
      </rdfs:subClassOf>
      <rdfs:subClassOf>
         <owl:Restriction>
            <owl:onProperty>
               <owl:ObjectProperty rdf:about="http://erlangen-crm.org/efrbroo/CLP104_subject_to"/>
            </owl:onProperty>
            <owl:someValuesFrom rdf:resource="http://erlangen-crm.org/efrbroo/F3_Manifestation_Product_Type"/>
         </owl:Restriction>
      </rdfs:subClassOf>
      <rdfs:subClassOf>
         <owl:Restriction>
            <owl:onProperty>
               <owl:ObjectProperty rdf:about="http://erlangen-crm.org/efrbroo/CLP105_right_held_by"/>
            </owl:onProperty>
            <owl:someValuesFrom rdf:resource="http://erlangen-crm.org/efrbroo/F3_Manifestation_Product_Type"/>
         </owl:Restriction>
      </rdfs:subClassOf>
      <rdfs:subClassOf>
         <owl:Restriction>
            <owl:cardinality rdf:datatype="http://www.w3.org/2001/XMLSchema#nonNegativeInteger">1</owl:cardinality>
            <owl:onProperty>
               <owl:ObjectProperty rdf:about="http://erlangen-crm.org/efrbroo/CLR6_should_carry"/>
            </owl:onProperty>
         </owl:Restriction>
      </rdfs:subClassOf>
   </owl:Class>
   <!--F4_Manifestation_Singleton-->
   <owl:Class rdf:about="http://erlangen-crm.org/efrbroo/F4_Manifestation_Singleton">
      <rdfs:label xml:lang="en">F4 Manifestation Singleton</rdfs:label>
      <rdfs:subClassOf rdf:resource="http://erlangen-crm.org/current/E24_Physical_Man-Made_Thing"/>
      <rdfs:comment>Scope note:
This class comprises physical objects that each carry an instance of F2 Expression, and that were produced as unique objects, with no siblings intended in the course of their production. It should be noted that if all but one copy of a given publication are destroyed, then that copy does not become an instance of F4 Manifestation Singleton, because it was produced together with sibling copies, even though it now happens to be unique. Examples of instances of F4 Manifestation Singleton include manuscripts, preparatory sketches and the final clean draft sent by an author or a composer to a publisher.

</rdfs:comment>
      <rdfs:comment>Examples:
The manuscript known as ‘The Book of Kells’
The manuscript score of Charles Racquet’s ‘Organ fantasy’, included in Marin Mersenne’s personal copy of his own ‘Harmonie universelle’ [Marin Mersenne planned a second edition of his ‘Harmonie universelle’ after it had been first published in 1636, and he asked the composer Charles Racquet to compose his organ fantasy especially for that planned second edition; but Mersenne died before he could finish and publish the second edition and Racquet’s score remained until the 20th century as a manuscript addition to Mersenne’s copy, held in Paris by the Library of the Conservatoire national des arts et métiers]
Marin Mersenne’s personal copy, held in Paris by the Library of the Conservatoire national des arts et métiers, of his own ‘Harmonie universelle’, containing all of his manuscript additions for a planned second edition that never took place before his death, but that served as a basis for the modern reprint published in 1986

</rdfs:comment>
      <rdfs:comment>Properties:
R42 is representative manifestation singleton for (has representative manifestation singleton): F2 Expression

</rdfs:comment>
      <rdfs:subClassOf>
         <owl:Restriction>
            <owl:onProperty>
               <owl:ObjectProperty rdf:about="http://erlangen-crm.org/efrbroo/R42_is_representative_manifestation_singleton_for"/>
            </owl:onProperty>
            <owl:someValuesFrom rdf:resource="http://erlangen-crm.org/efrbroo/F4_Manifestation_Singleton"/>
         </owl:Restriction>
      </rdfs:subClassOf>
   </owl:Class>
   <!--F5_Item-->
   <owl:Class rdf:about="http://erlangen-crm.org/efrbroo/F5_Item">
      <rdfs:label xml:lang="en">F5 Item</rdfs:label>
      <rdfs:subClassOf rdf:resource="http://erlangen-crm.org/efrbroo/F54_Utilised_Information_Carrier"/>
      <rdfs:comment>Scope note:
This class comprises physical objects (printed books, scores, CDs, DVDs, CD-ROMS, etc.) that carry a F24 Publication Expression and were produced by an industrial process involving an F3 Manifestation Product Type.

</rdfs:comment>
      <rdfs:comment>Examples:
Marin Mersenne’s personal copy of his own ‘Harmonie universelle’ without any manuscript addition and without Charles Racquet’s manuscript score, as a mere witness of the 1st edition of ‘Harmonie universelle’, Paris, 1636 [the same physical object can be regarded at the same time as an instance of F5 Item inasmuch as it is a witness of a publication, and as an instance of F4 Manifestation Singleton inasmuch as it contains manuscript annotations and additions and as it served as the basis for a subsequent production process]
Any other copy of the original edition of Marin Mersenne’s ‘Harmonie universelle’, Paris, 1636
Any copy of the modern reprint publication of Marin Mersenne’s ‘Harmonie universelle’, Paris, 1986, ISBN ‘2-222-00835-2’

</rdfs:comment>
      <rdfs:comment>Properties:
R7 is example of (has example): F3 Manifestation Product Type

</rdfs:comment>
      <rdfs:subClassOf>
         <owl:Restriction>
            <owl:cardinality rdf:datatype="http://www.w3.org/2001/XMLSchema#nonNegativeInteger">1</owl:cardinality>
            <owl:onProperty>
               <owl:ObjectProperty rdf:about="http://erlangen-crm.org/efrbroo/R7_is_example_of"/>
            </owl:onProperty>
         </owl:Restriction>
      </rdfs:subClassOf>
   </owl:Class>
   <!--F6_Concept-->
   <owl:Class rdf:about="http://erlangen-crm.org/efrbroo/F6_Concept">
      <rdfs:label xml:lang="en">F6 Concept</rdfs:label>
      <owl:equivalentClass rdf:resource="http://erlangen-crm.org/current/E28_Conceptual_Object"/>
      <rdfs:comment>Equal to:
E28 Conceptual Object
</rdfs:comment>
      <rdfs:comment>Scope note:
An abstract notion or idea. [FRBRER] Includes fields of knowledge, disciplines, schools of thought (philosophies, religions, political ideologies, etc.), etc. Includes theories, processes, techniques, practices, etc. [Definition from the FRAD model, unchanged]
This class comprises non-material products of our minds and other human produced data that have become objects of a discourse about their identity, circumstances of creation or historical implication. The production of such information may have been supported by the use of technical devices such as cameras or computers.
Characteristically, instances of this class are created, invented or thought by someone, and then may be documented or communicated between persons. Instances of E28 Conceptual Object have the ability to exist on more than one particular carrier at the same time, such as paper, electronic signals, marks, audio media, paintings, photos, human memories, etc.
They cannot be destroyed. They exist as long as they can be found on at least one carrier or in at least one human memory. Their existence ends when the last carrier and the last memory are lost. [Scope note for E28 Conceptual Object in CIDOC CRM version 5.0.1]

</rdfs:comment>
      <rdfs:comment>Examples:
Natural history of whales
Cultural history of Wales
The appreciation of Victor Hugo’s works in Germany between 1870 and 1914

</rdfs:comment>
   </owl:Class>
   <!--F7_Object-->
   <owl:Class rdf:about="http://erlangen-crm.org/efrbroo/F7_Object">
      <rdfs:label xml:lang="en">F7 Object</rdfs:label>
      <owl:equivalentClass rdf:resource="http://erlangen-crm.org/current/E18_Physical_Thing"/>
      <rdfs:comment>Equal to:
E18 Physical Thing
</rdfs:comment>
      <rdfs:comment>Scope note:
This class comprises all persistent physical items with a relatively stable form, man-made or natural.
[This is the beginning of scope note for E18 Physical Object in CIDOC CRM version 5.0.1]

</rdfs:comment>
      <rdfs:comment>Examples:
Buckingham Palace
The Lusitania
Apollo 11
The Eiffel Tower

</rdfs:comment>
   </owl:Class>
   <!--F8_Event-->
   <owl:Class rdf:about="http://erlangen-crm.org/efrbroo/F8_Event">
      <rdfs:label xml:lang="en">F8 Event</rdfs:label>
      <owl:equivalentClass rdf:resource="http://erlangen-crm.org/current/E4_Period"/>
      <rdfs:comment>Equal to:
E4 Period
</rdfs:comment>
      <rdfs:comment>Scope note:
This class comprises sets of coherent phenomena or cultural manifestations bounded in time and space.
It is the social or physical coherence of these phenomena that identify an E4 Period and not the associated spatio-temporal bounds. These bounds are a mere approximation of the actual process of growth, spread and retreat. Consequently, different periods can overlap and coexist in time and space, such as when a nomadic culture exists in the same area as a sedentary culture.
Typically this class is used to describe prehistoric or historic periods such as the ‘Neolithic Period’, the ‘Ming Dynasty’ or the ‘McCarthy Era’. There are however no assumptions about the scale of the associated phenomena. In particular all events are seen as synthetic processes consisting of coherent phenomena. Therefore E4 Period is a superclass of E5 Event. For example, a modern clinical E67 Birth can be seen as both an atomic E5 Event and as an E4 Period that consists of multiple activities performed by multiple instances of E39 Actor.
There are two different conceptualisations of “artistic style”, defined either by physical features or by historical context. For example, Impressionism can be viewed as a period lasting from approximately 1870 to 1905 during which paintings with particular characteristics were produced by a group of artists that included (among others) Monet, Renoir, Pissarro, Sisley and Degas. Alternatively, it can be regarded as a style applicable to all paintings sharing the characteristics of the works produced by the Impressionist painters, regardless of historical context. The first interpretation is an E4 Period, and the second defines morphological object types that fall under E55 Type.

Another specific case of an E4 Period is the set of activities and phenomena associated with a settlement, such as the populated period of Nineveh.
[This is the Scope note for E4 Period in CIDOC CRM version 5.0.1]
[Note that in CIDOC CRM, E12 Production, E13 Attribute Assignment, and E65 Creation are indirect subclasses of E4 Period = F8 Event; as a consequence, F8 Event is an indirect superclass of: F27 Work Conception, F28 Expression Creation, F40 Identifier Assignment, F41 Representative Manifestation Assignment, F42 Representative Expression Assignment, F32 Carrier Production Event, F33 Reproduction Event, and F30 Publication Event]

</rdfs:comment>
      <rdfs:comment>Examples:
The battle of Trafalgar
Printing for the publisher named ‘Doubleday’ in 2003 all the copies of the first print run of the novel entitled ‘Da Vinci Code’ (F32)
Having the initial idea that eventually resulted in the existence of the opera entitled ‘Der fliegende Holländer’ (F27)
Creating for Mozart’s 41st symphony the controlled access point that was thereafter consistently used to refer unambiguously to that symphony everywhere in the Library of Congress’s catalogue (F40)

</rdfs:comment>
   </owl:Class>
   <!--F9_Place-->
   <owl:Class rdf:about="http://erlangen-crm.org/efrbroo/F9_Place">
      <rdfs:label xml:lang="en">F9 Place</rdfs:label>
      <owl:equivalentClass rdf:resource="http://erlangen-crm.org/current/E53_Place"/>
      <rdfs:comment>Equal to:
E53 Place
</rdfs:comment>
      <rdfs:comment>Scope note:
This class comprises extents in space, in particular on the surface of the Earth, in the pure sense of physics: independent from temporal phenomena and matter. The instances of E53 Place are usually determined by reference to the position of immobile objects such as buildings, cities, mountains, rivers, or dedicated geodetic marks. A Place can be determined by combining a frame of reference and a location with respect to this frame. It may be identified by one or more instances of E44 Place Appellation.
It is sometimes argued that instances of E53 Place are best identified by global coordinates or absolute reference systems. However, relative references are often more relevant in the context of cultural documentation and tend to be more precise. In particular, we are often interested in position in relation to large, mobile objects, such as ships. For example, the Place at which Nelson died is known with reference to a large mobile object – H.M.S Victory. A resolution of this Place in terms of absolute coordinates would require knowledge of the movements of the vessel and the precise time of death, either of which may be revised, and the result would lack historical and cultural relevance.
Any object can serve as a frame of reference for E53 Place determination. The model foresees the notion of a section of an E19 Physical Object as a valid E53 Place determination. [Scope note for E53 Place in CIDOC CRM version 5.0.1]
Note that Places may be determined by the location of historical or contemporary objects, geographic features, events or geo-political units.

</rdfs:comment>
      <rdfs:comment>Examples:
The area referred to as ‘Lutèce’
The area referred to as ‘verso of the title page of the Library of Congress’s copy of the 1st edition of the novel entitled ‘Da Vinci Code’’

</rdfs:comment>
   </owl:Class>
   <!--F10_Person-->
   <owl:Class rdf:about="http://erlangen-crm.org/efrbroo/F10_Person">
      <rdfs:label xml:lang="en">F10 Person</rdfs:label>
      <owl:equivalentClass rdf:resource="http://erlangen-crm.org/current/E21_Person"/>
      <rdfs:comment>Equal to:
E21 Person
</rdfs:comment>
      <rdfs:comment>Scope note:
This class comprises real persons who live or are assumed to have lived. Bibliographic identities or personae assumed by an individual or a group should be modelled as F12 Nomen and connected to the relevant person or group with an instance of F35 Nomen Use Statement, even if nothing more can be said about this person or group. In a bibliographic context, a name presented following the conventions usually employed for personal names will be assumed to correspond to an actual real person (F10 Person), unless evidence is available to indicate that this is not the case. The fact that a persona may erroneously be classified as an instance of F10 Person does not imply that the concept comprises personae.

</rdfs:comment>
      <rdfs:comment>Examples:
Margaret Atwood
Hans Christian Andersen
Queen Victoria

</rdfs:comment>
   </owl:Class>
   <!--F11_Corporate_Body-->
   <owl:Class rdf:about="http://erlangen-crm.org/efrbroo/F11_Corporate_Body">
      <rdfs:label xml:lang="en">F11 Corporate Body</rdfs:label>
      <rdfs:subClassOf rdf:resource="http://erlangen-crm.org/current/E74_Group"/>
      <rdfs:superClassOf rdf:resource="http://erlangen-crm.org/current/E40_Legal_Body"/>
      <rdfs:comment>Scope note:
This class comprises organisations and groups of two or more people and/or organisations acting as a unit.
To be considered an F11 Corporate Body a gathering of people needs to bear a name and exhibit organisational characteristics sufficient to allow the body as a whole to participate in the creation, modification or production of an E73 Information Object. Groups such as conferences, congresses, expeditions, exhibitions, festivals, fairs, etc. are modelled as F11 Corporate Bodies when they are named and can take collective action, such as approving a report or publishing their proceedings.

</rdfs:comment>
      <rdfs:comment>Examples:
The International Machaut Society
The British Library
The Jackson Five
The Regional Municipality of Ottawa-Carleton
Symposium on Glaucoma

</rdfs:comment>
   </owl:Class>
   <!--F12_Nomen-->
   <owl:Class rdf:about="http://erlangen-crm.org/efrbroo/F12_Nomen">
      <rdfs:label xml:lang="en">F12 Nomen</rdfs:label>
      <rdfs:subClassOf rdf:resource="http://erlangen-crm.org/current/E41_Appellation"/>
      <rdfs:superClassOf rdf:resource="http://erlangen-crm.org/efrbroo/F13_Identifier"/>
      <rdfs:comment>Scope note:
This class comprises any sign or arrangements of signs following a specific syntax (sequences of alphanumeric characters, chemical structure symbols, sound symbols, ideograms etc.) that are used or can be used to refer to and identify a specific instance of some class or category within a certain context. The scripts or type sets for the types of symbols used to compose an instance of F12 Nomen have to be explicitly specified. The identity of an instance of F12 Nomen is given by the order of its symbols and their individual role with respect to their scripts, regardless of the semantics of the larger structural components it may be built from. Structural tags occurring in the nomen string are regarded as symbols constituting the nomen. Spelling variants are regarded as different nomina, whereas the use of different fonts (visual representation variants) or different digital encodings do not change the identity.

</rdfs:comment>
      <rdfs:comment>Examples:
‘杜甫’[the name of a Chinese poet of the 8th century, in simplified Chinese characters]
‘Du Fu’ [Pinyin romanised form of the name of a Chinese poet of the 8th century]
‘Tu Fu’ [another romanised form of the name of a Chinese poet of the 8th century]
‘Thơ Ðô Phủ’ [Vietnamese form of the name of a Chinese poet of the 8th century]
‘جامعة صفاقس’ [Arabic name of the Sfax University (Tunisia), in Arabic script]
‘Ğāmi‘at̀̀ Ṣafāqis’[Arabic name of the Sfax University (Tunisia), transliterated]

‘Université de Sfax’ [French name of the Sfax University (Tunisia)]
‘3-[(2S)-1-methylpyrrolidin-2-yl]pyridine’ [the IUPAC systematic name for nicotine]
‘Murders in the rue Morgue’ [English title of a textual work]
‘Poe, Edgar Allan, 1809-1849. Murders in the rue Morgue’ (F50) [controlled author/title access point for a textual work]
‘modelling’ [not the activity, just the written signs that represent its English name in British spelling]
‘modeling’ [not the activity, just the written signs that represent its English name in American spelling]

</rdfs:comment>
      <rdfs:comment>Properties:
R33 has content: E62 String
(R33.1 has encoding: E55 Type)

</rdfs:comment>
      <rdfs:subClassOf>
         <owl:Restriction>
            <owl:onProperty>
               <owl:ObjectProperty rdf:about="http://erlangen-crm.org/efrbroo/R33_has_content"/>
            </owl:onProperty>
            <owl:minCardinality rdf:datatype="http://www.w3.org/2001/XMLSchema#nonNegativeInteger">1</owl:minCardinality>
         </owl:Restriction>
      </rdfs:subClassOf>
   </owl:Class>
   <!--F13_Identifier-->
   <owl:Class rdf:about="http://erlangen-crm.org/efrbroo/F13_Identifier">
      <rdfs:label xml:lang="en">F13 Identifier</rdfs:label>
      <rdfs:subClassOf rdf:resource="http://erlangen-crm.org/efrbroo/F12_Nomen"/>
      <rdfs:superClassOf rdf:resource="http://erlangen-crm.org/efrbroo/F50_Controlled_Access_Point"/>
      <owl:equivalentClass rdf:resource="http://erlangen-crm.org/current/E42_Identifier"/>
      <rdfs:comment>Equal to:
E42 Identifier
</rdfs:comment>
      <rdfs:comment>Scope note:
This class comprises strings or codes assigned to instances of E1 CRM Entity in order to identify them uniquely and permanently within the context of one or more organisations. Such codes are often known as inventory numbers, registration codes, etc. and are typically composed of alphanumeric sequences. The class E42 Identifier is not normally used for machine-generated identifiers used for automated processing unless these are also used by human agents. [Adapted from the Scope note of CIDOC CRM E42 Identifier ver. 5.0.1]

</rdfs:comment>
      <rdfs:comment>Examples:
ISSN ‘0041-5278’
ISRC ‘FIFIN8900116’
Shelf mark ‘Res 8 P 10’
‘Guillaume de Machaut (1300?-1377)’ (F50) [a controlled personal name access point that follows the French rules]
‘Guillaume, de Machaut, ca. 1300-1377’ (F50) [a controlled personal name access point that follows the AACR2 rules]
‘Rite of spring (Choreographic work: Bausch)’ (F50) [a controlled access point that follows the AACR2 rules]

</rdfs:comment>
      <rdfs:comment>Properties:
R8 consists of (forms part of): E90 Symbolic Object

</rdfs:comment>
      <rdfs:subClassOf>
         <owl:Restriction>
            <owl:onProperty>
               <owl:ObjectProperty rdf:about="http://erlangen-crm.org/efrbroo/R8_consists_of"/>
            </owl:onProperty>
            <owl:someValuesFrom rdf:resource="http://erlangen-crm.org/efrbroo/F13_Identifier"/>
         </owl:Restriction>
      </rdfs:subClassOf>
   </owl:Class>
   <!--F14_Individual_Work-->
   <owl:Class rdf:about="http://erlangen-crm.org/efrbroo/F14_Individual_Work">
      <rdfs:label xml:lang="en">F14 Individual Work</rdfs:label>
      <rdfs:subClassOf rdf:resource="http://erlangen-crm.org/efrbroo/F1_Work"/>
      <rdfs:superClassOf rdf:resource="http://erlangen-crm.org/efrbroo/F17_Aggregation_Work"/>
      <rdfs:comment>Scope note:
This class comprises works that are realised by one and only one self-contained expression, i.e., works representing the concept as expressed by precisely this expression.
Inherent to the notion of work is the completion of recognisable outcomes of the work. These outcomes, i.e. the Self-Contained Expressions, are regarded as the symbolic equivalents of Individual Works, which form the atoms of a complex work. Normally creators would characterise an outcome of a work as finished. In other cases, one could recognise an outcome of a work as complete from the elaboration or logical coherence of its content, or if there is any historical knowledge about the creator deliberately or accidentally never finishing (completing) that particular expression. In all those cases, one would regard the corresponding expression as equivalent to one Individual Work.

</rdfs:comment>
      <rdfs:comment>Examples:
Abstract content of Giovanni Battista Piranesi’s ‘Carcere XVI: the pier with chains: 1st state’
Abstract content of Giovanni Battista Piranesi’s ‘Carcere XVI: the pier with chains: 2nd state’ [explanation: these are two states of the same etching, but with so many and so significant differences between them that they can scarcely be recognised as conveying the same work; more generally speaking, each individual state of an etching, as a Self-Contained Expression, conveys its own F14 Individual Work (even if the differences are not so blatant as in the case of ‘Carcere XVI’), and is regarded as part of the larger, abstract F15 Complex Work that encompasses all distinct states of the same etching]
Abstract content of the recording made of performances of Johann Sebastian Bach’s ‘Toccata in C minor BWV 911’ by Glenn Gould on May 15 &amp; 16, 1979, in Toronto, Eaton’s Auditorium

</rdfs:comment>
      <rdfs:comment>Properties:
R9 is realised in (realises): F22 Self-Contained Expression

</rdfs:comment>
      <rdfs:subClassOf>
         <owl:Restriction>
            <owl:cardinality rdf:datatype="http://www.w3.org/2001/XMLSchema#nonNegativeInteger">1</owl:cardinality>
            <owl:onProperty>
               <owl:ObjectProperty rdf:about="http://erlangen-crm.org/efrbroo/R9_is_realised_in"/>
            </owl:onProperty>
         </owl:Restriction>
      </rdfs:subClassOf>
   </owl:Class>
   <!--F15_Complex_Work-->
   <owl:Class rdf:about="http://erlangen-crm.org/efrbroo/F15_Complex_Work">
      <rdfs:label xml:lang="en">F15 Complex Work</rdfs:label>
      <rdfs:subClassOf rdf:resource="http://erlangen-crm.org/efrbroo/F1_Work"/>
      <rdfs:superClassOf rdf:resource="http://erlangen-crm.org/efrbroo/F18_Serial_Work"/>
      <rdfs:comment>Scope note:
This class comprises works that have other works as members. The members of a Complex Work may constitute alternatives to, derivatives of, or self-contained components of other members of the same Complex Work.
In practice, no clear line can be drawn between parallel and subsequent processes in the evolution of a work. One part may not be finished when another is already revised. An initially monolithic work may be taken up and evolve in pieces. The member relationship of Work is based on the conceptual relationship, and should not be confused with the internal structural parts of an individual expression. The fact that an expression may contain parts from other work(s) does not make the expressed work complex. For instance, an anthology for which only one version exists is not a complex work.
The boundaries of a Complex Work have nothing to do with the value of the intellectual achievement but only with the dominance of a concept. Thus, derivations such as translations are regarded as belonging to the same Complex Work, even though in addition they constitute an Individual Work themselves. In contrast, a Work that significantly takes up and merges concepts of other works so that it is no longer dominated by the initial concept is regarded as a new work. In cataloguing practice, detailed rules are established prescribing which kinds of derivation should be regarded as crossing the boundaries of a complex work. Adaptation and derivation graphs allow the recognition of distinct sub-units, i.e. a complex work contained in a larger complex work.
As a Complex Work can be taken up by any creator who acquires the spirit of its concept, it is never finished in an absolute sense.

</rdfs:comment>
      <rdfs:comment>Examples:
Work entitled ‘La Porte de l’Enfer’ by Auguste Rodin
Work entitled ‘Hamlet’ by William Shakespeare
Work entitled ‘Der Ring der Nibelungen’ by Richard Wagner
Work entitled ‘Carceri d’invenzione’ by Giovanni Battista Piranesi
Work entitled ‘Mass in B minor BWV 232’ by Johann Sebastian Bach

</rdfs:comment>
      <rdfs:comment>Properties:
R10 has member (is member of): F1 Work

</rdfs:comment>
      <rdfs:subClassOf>
         <owl:Restriction>
            <owl:onProperty>
               <owl:ObjectProperty rdf:about="http://erlangen-crm.org/efrbroo/R10_has_member"/>
            </owl:onProperty>
            <owl:minCardinality rdf:datatype="http://www.w3.org/2001/XMLSchema#nonNegativeInteger">2</owl:minCardinality>
         </owl:Restriction>
      </rdfs:subClassOf>
   </owl:Class>
   <!--F16_Container_Work-->
   <owl:Class rdf:about="http://erlangen-crm.org/efrbroo/F16_Container_Work">
      <rdfs:label xml:lang="en">F16 Container Work</rdfs:label>
      <rdfs:subClassOf rdf:resource="http://erlangen-crm.org/efrbroo/F1_Work"/>
      <rdfs:superClassOf rdf:resource="http://erlangen-crm.org/efrbroo/F17_Aggregation_Work"/>
      <rdfs:superClassOf rdf:resource="http://erlangen-crm.org/efrbroo/F19_Publication_Work"/>
      <rdfs:superClassOf rdf:resource="http://erlangen-crm.org/efrbroo/F20_Performance_Work"/>
      <rdfs:comment>Scope note:
This class comprises works whose essence is to enhance or add value to expressions from one or more other works without altering them, by the selection, arrangement and/or addition of features of different form, such as layout to words, recitation and movement to texts, performance to musical scores etc. This does not make the contents of the incorporated expressions part of the Container Work, but only part of the resulting expression. Container Work may include the addition of new, original parts to the incorporated expressions, such as introductions, graphics, etc.
This class is an “abstract class,” in that it only serves as an umbrella for its three subclasses. As a consequence, it can only be instantiated by instances of any of its subclasses: nothing can be an instance of it, unless it is an instance of either F17 Aggregation Work, F19 Publication Work, or F20 Performance Work.
A new version of a container work does not make the resulting complex work a Container Work as well. The inclusion of expressions from a complex work in a Container Work does not make the Container Work itself complex.

</rdfs:comment>
      <rdfs:comment>Examples:
The aggregation and arrangement concept of the anthology entitled ‘American Women Poets of the Nineteenth Century: An Anthology’, edited by Cheryl Walker and published by Rutgers University Press in July 1992 (F17)
The concept for the layout created by printer Guido Morris for the text of Michael Hamburger’s English translation of 12 poems by Georg Trakl for publication in 1952 (F19)
The concept by the publisher named ‘Dell’ of issuing together, in 2002, three novels entitled ‘The Partner’, ‘The Street Lawyer’, and ‘A time to kill’, by the author named ‘John Grisham’, with just the statement ‘Three #1 bestsellers by John Grisham’ as a collective title (F19)
The concept of Sergei Radlov’s mise-en-scène of a Yiddish translation of the textual work entitled ‘King Lear’ in Moscow in 1935 (F20)
The concept of putting together the English text of ‘King Lear’ and a Spanish translation thereof in a bilingual edition of ‘King Lear’ (F17)

</rdfs:comment>
   </owl:Class>
   <!--F17_Aggregation_Work-->
   <owl:Class rdf:about="http://erlangen-crm.org/efrbroo/F17_Aggregation_Work">
      <rdfs:label xml:lang="en">F17 Aggregation Work</rdfs:label>
      <rdfs:subClassOf rdf:resource="http://erlangen-crm.org/efrbroo/F14_Individual_Work"/>
      <rdfs:subClassOf rdf:resource="http://erlangen-crm.org/efrbroo/F16_Container_Work"/>
      <rdfs:comment>Scope note:
This class comprises works whose essence is the selection and/or arrangement of expressions of one or more other works. This does not make the contents of the aggregated expressions part of this work, but only part of the resulting expression. F17 Aggregation Work may include additional original parts.
An expression of a work may include expressions of other works within it. For instance, an anthology of poems is regarded as a work in its own right that makes use of expressions of the individual poems that have been selected and ordered as part of an intellectual process.
A new version of an aggregate work does not make the resulting complex work an aggregate work as well. The inclusion of expressions from a complex work in an aggregation work does not make the aggregation work itself complex.

</rdfs:comment>
      <rdfs:comment>Examples:
The aggregation and arrangement concept of the anthology entitled ‘American Women Poets of the Nineteenth Century: An Anthology’, edited by Cheryl Walker and published by Rutgers University Press in July 1992
The aggregation and arrangement concept of the Web site named ‘IFLANET’
The aggregation and arrangement concept of the collection of articles entitled ‘Marij Kogoj (1892-1992): zbornik referatov s kolokvija ob stoletnici skladateljevega rojstva 7.10.1992 v Ljubljani = Marij Kogoj (1892-1992): proceedings from the colloquium held in Ljubljana at the centenary of the composer’s birth on October 7th, 1992’ and edited by a person named ‘Ivan Klemenčič’

</rdfs:comment>
   </owl:Class>
   <!--F18_Serial_Work-->
   <owl:Class rdf:about="http://erlangen-crm.org/efrbroo/F18_Serial_Work">
      <rdfs:label xml:lang="en">F18 Serial Work</rdfs:label>
      <rdfs:subClassOf rdf:resource="http://erlangen-crm.org/efrbroo/F15_Complex_Work"/>
      <rdfs:subClassOf rdf:resource="http://erlangen-crm.org/efrbroo/F19_Publication_Work"/>
      <rdfs:comment>Scope note:
This class comprises works that are, or have been, planned to result in sequences of Expressions or Manifestations with common features. Whereas a work can acquire new members during the time it evolves, Expressions and Manifestations are identified with a certain state achieved at a particular point in time. Therefore there is in general no single Expression or Manifestation representing a complete serial work, unless the serial work has ended.
Serial Works may or may not have a plan for an overall expression.
The retrospective reprinting of all issues of a Serial Work at once, in the form of a monograph, is regarded to be another member of a Complex Work, which contains the Serial Work and the Individual Work realised in the monograph. This does not make the monograph part of the Serial Work.

</rdfs:comment>
      <rdfs:comment>Examples:
The periodical entitled ‘The UNESCO Courier’, ISSN ‘0041-5278’
The periodical entitled ‘Courrier de l’UNESCO’, ISSN ‘0304-3118’ [French edition of the periodical titled ‘The UNESCO Courier’, ISSN ‘0041-5278’]
The series entitled ‘L’évolution de l’humanité’, ISSN ‘0755-1843’ [a monograph series comprising volumes that were published from 1920 on, and some of which were reprinted, with different physical features and rearranged in a different order, from 1968 on, in a distinct series also entitled ‘L’évolution de l’humanité’, ISSN ‘0755-1770’]

</rdfs:comment>
      <rdfs:comment>Properties:
R11 has issuing rule (is issuing rule of): E29 Design or Procedure

</rdfs:comment>
      <rdfs:subClassOf>
         <owl:Restriction>
            <owl:onProperty>
               <owl:ObjectProperty rdf:about="http://erlangen-crm.org/efrbroo/R11_has_issuing_rule"/>
            </owl:onProperty>
            <owl:someValuesFrom rdf:resource="http://erlangen-crm.org/efrbroo/F18_Serial_Work"/>
         </owl:Restriction>
      </rdfs:subClassOf>
   </owl:Class>
   <!--F19_Publication_Work-->
   <owl:Class rdf:about="http://erlangen-crm.org/efrbroo/F19_Publication_Work">
      <rdfs:label xml:lang="en">F19 Publication Work</rdfs:label>
      <rdfs:subClassOf rdf:resource="http://erlangen-crm.org/efrbroo/F16_Container_Work"/>
      <rdfs:superClassOf rdf:resource="http://erlangen-crm.org/efrbroo/F18_Serial_Work"/>
      <rdfs:comment>Scope note:
This class comprises works that have been planned to result in a manifestation product type or an electronic publishing service and that pertain to the rendering of expressions from other works.

</rdfs:comment>
      <rdfs:comment>Examples:
The concept of publishing Stephen Crane’s complete poems (as edited by Joseph Katz), which includes the idea that every time a stanza jumps over a page change, the statement ‘[NO STANZA BREAK]’ should be printed as a warning for readers that the new page continues the same stanza
The concept, on behalf of publisher named ‘Verlag Neue Kunsthandlung’, of issuing together, around 1925, three formerly independent publications (‘Emil Orlik’ by Max Osborn – vol. 2 within the series named ‘Graphiker der Gegenwart’, published in 1920; ‘Anders Zorn’ by Paul Friedrich – vol. 10 within the series named ‘Graphiker der Gegenwart’, published in 1924; and ‘Max Slevogt’ by Julius Elias – vol. 11 within the series named ‘Graphiker der Gegenwart’, published in 1923) as one, new publication, entitled ‘102 Bilder aus der Sammlung Graphiker der Gegenwart’
The concept, on behalf of publisher named ‘Dell’, of issuing together in 2002 three novels, titled ‘The partner’, ‘The street lawyer’, and ‘A time to kill’, by author named ‘John Grisham’, with just the statement ‘Three #1 bestsellers by John Grisham’ as a collective title

</rdfs:comment>
   </owl:Class>
   <!--F20_Performance_Work-->
   <owl:Class rdf:about="http://erlangen-crm.org/efrbroo/F20_Performance_Work">
      <rdfs:label xml:lang="en">F20 Performance Work</rdfs:label>
      <rdfs:subClassOf rdf:resource="http://erlangen-crm.org/efrbroo/F16_Container_Work"/>
      <rdfs:comment>Scope note:
This class comprises the sets of concepts for rendering a particular or a series of like performances.
F20 Performance Work is declared as a subclass of F16 Container Work. This implies that the incorporated expressions (such as the text of the staged play, the text of the argument for the ballet, the recorded music to be used for the ballet, or the content of the musical score to be used for a concert, etc.) are not by themselves a part of the expression of this F1 Work. Rather, an expression (F25 Performance Plan) of the instructions the stage production, choreography or musical performance consists of incorporates (P165) that textual or musical content. In other words, the text of ‘Hamlet’ is not a component of the concepts that underlie a given mise-en-scène of ‘Hamlet’, but any staging directions (F25 Performance Plan) that convey a given director’s vision of ‘Hamlet’ must necessarily incorporate the text of ‘Hamlet’.

</rdfs:comment>
      <rdfs:comment>Examples:
The conceptual content of Sergei Radlov’s mise-en-scène of a Yiddish translation of the textual work entitled ‘King Lear’ in Moscow in 1935
The conceptual content of Pina Bausch’s choreography of the ballet entitled ‘Rite of spring’ in Wuppertal in 1975
The conceptual content of Bruno Walter’s performance of Gustav Mahler’s 9th symphony in 1961
The conceptual content of the “performance handbook” for Luigi Nono’s musical work entitled ‘À Pierre’

</rdfs:comment>
      <rdfs:comment>Properties:
R12 is realised in (realises): F25 Performance Plan

</rdfs:comment>
      <rdfs:subClassOf>
         <owl:Restriction>
            <owl:onProperty>
               <owl:ObjectProperty rdf:about="http://erlangen-crm.org/efrbroo/R12_is_realised_in"/>
            </owl:onProperty>
            <owl:someValuesFrom rdf:resource="http://erlangen-crm.org/efrbroo/F20_Performance_Work"/>
         </owl:Restriction>
      </rdfs:subClassOf>
   </owl:Class>
   <!--F21_Recording_Work-->
   <owl:Class rdf:about="http://erlangen-crm.org/efrbroo/F21_Recording_Work">
      <rdfs:label xml:lang="en">F21 Recording Work</rdfs:label>
      <rdfs:subClassOf rdf:resource="http://erlangen-crm.org/efrbroo/F1_Work"/>
      <rdfs:comment>Scope note:
This class comprises works that conceptualise the capturing of features of perdurants. The characteristics of the manifestation of a recording work are those of the product of the capture process. The characteristics of any other works recorded are distinct from those of the recording work itself. In the case where the recorded perdurant expresses some Work, the respective instance of F21 is also an F16 Container Work.
The concept of recording is not necessarily linked to the use of modern devices that allow for mechanical recording, such as tape recorders or cameras. However, in practice, library catalogues tend to regard as recordings only the products of such mechanical devices.
But the concept of recording is very much linked to the notion that there is something that is recorded. In general, photographs or animated images are not to be regarded as instances of F21 Recording Work just because of the use of the medium, but simply as instances of F1 Work (or F15 Complex Work). Only such photographs and animated images that can be used as documentation are to be regarded as recordings.

</rdfs:comment>
      <rdfs:comment>Examples:
The concept of recording the Swedish 17th century warship Vasa in August 1959 to April 1961
The concept of documenting the Live Aid concerts July 13, 1985, London, Philadelphia, Sydney and Moscow
The concept of making a photograph of the three Allied leaders at Yalta in February 1945
Oceania Project’s concept of making a large digital acoustic data archive dedicated to East Australian humpback whale songs
The concept of recording Louise Bourgeois’s activity in the documentary movie entitled ‘Louise Bourgeois: The Spider, the Mistress, and the Tangerine’

</rdfs:comment>
      <rdfs:comment>Properties:
R13 is realised in (realises): F26 Recording

</rdfs:comment>
      <rdfs:subClassOf>
         <owl:Restriction>
            <owl:onProperty>
               <owl:ObjectProperty rdf:about="http://erlangen-crm.org/efrbroo/R13_is_realised_in"/>
            </owl:onProperty>
            <owl:someValuesFrom rdf:resource="http://erlangen-crm.org/efrbroo/F21_Recording_Work"/>
         </owl:Restriction>
      </rdfs:subClassOf>
   </owl:Class>
   <!--F22_Self-Contained_Expression-->
   <owl:Class rdf:about="http://erlangen-crm.org/efrbroo/F22_Self-Contained_Expression">
      <rdfs:label xml:lang="en">F22 Self-Contained Expression</rdfs:label>
      <rdfs:subClassOf rdf:resource="http://erlangen-crm.org/efrbroo/F2_Expression"/>
      <rdfs:superClassOf rdf:resource="http://erlangen-crm.org/efrbroo/F24_Publication_Expression"/>
      <rdfs:superClassOf rdf:resource="http://erlangen-crm.org/efrbroo/F25_Performance_Plan"/>
      <rdfs:superClassOf rdf:resource="http://erlangen-crm.org/efrbroo/F26_Recording"/>
      <rdfs:comment>Scope note:
This class comprises the immaterial realisations of individual works at a particular time that are regarded as a complete whole. The quality of wholeness reflects the intention of its creator that this expression should convey the concept of the work. Such a whole can in turn be part of a larger whole.
Inherent to the notion of work is the completion of recognisable outcomes of the work. These outcomes, i.e. the Self-Contained Expressions, are regarded as the symbolic equivalents of Individual Works, which form the atoms of a complex work. A Self-Contained Expression may contain expressions or parts of expressions from other work, such as citations or items collected in anthologies. Even though they are incorporated in the Self-Contained Expression, they are not regarded as becoming members of the expressed container work by their inclusion in the expression, but are rather regarded as foreign or referred to elements.
F22 Self-Contained Expression can be distinguished from F23 Expression Fragment in that an F23 Expression Fragment was not intended by its creator to make sense by itself. Normally creators would characterise an outcome of a work as finished. In other cases, one could recognise an outcome of a work as complete from the elaboration or logical coherence of its content, or if there is any historical knowledge about the creator deliberately or accidentally never finishing (completing) that particular expression. In all those cases, one would regard an expression as self-contained.

</rdfs:comment>
      <rdfs:comment>Examples:
The Italian text of Dante’s ‘Inferno’ as found in the authoritative critical edition La Commedia secondo l’antica vulgata a cura di Giorgio Petrocchi, Milano: Mondadori, 1966-67 (= Le Opere di Dante Alighieri, Edizione Nazionale a cura della Società Dantesca Italiana, VII, 1-4)
The musical notation of Franz Schubert’s lied known as ‘Ave Maria’
The musical notation of Franz Schubert’s lieder cycle entitled ‘Seven Songs after Walter Scott’s The Lady of the Lake’, of which ‘Ave Maria’ is a distinct part
The musical notation of Franz Liszt’s piano transcription of Franz Schubert’s lied known as ‘Ave Maria’
The musical notation of fragments of the unfinished string quartet sketched by Arnold Schoenberg in 1926

</rdfs:comment>
   </owl:Class>
   <!--F23_Expression_Fragment-->
   <owl:Class rdf:about="http://erlangen-crm.org/efrbroo/F23_Expression_Fragment">
      <rdfs:label xml:lang="en">F23 Expression Fragment</rdfs:label>
      <rdfs:subClassOf rdf:resource="http://erlangen-crm.org/efrbroo/F2_Expression"/>
      <rdfs:comment>Scope note:
This class comprises parts of Expressions and these parts are not Self-Contained Expressions themselves.
The existence of an instance of F23 Expression Fragment can be due to accident, such as loss of material over time, e.g. the only remaining manuscript of an antique text being partially eaten by worms, or due to deliberate isolation, such as excerpts taken from a text by the compiler of a collection of excerpts.
An F23 Expression Fragment is only identified with respect to its occurrence in a known or assumed whole. The size of an instance of F23 Expression Fragment ranges from more than 99% of an instance of F22 Self-Contained Expression to tiny bits (a few words from a text, one bar from a musical composition, one detail from a still image, a two-second clip from a movie, etc.).

</rdfs:comment>
      <rdfs:comment>Examples:
The only remnants of Sappho’s poems

The words ‘Beati pauperes spiritu’ (excerpted from Matthew’s Gospel 5,3 in Latin translation)

</rdfs:comment>
   </owl:Class>
   <!--F24_Publication_Expression-->
   <owl:Class rdf:about="http://erlangen-crm.org/efrbroo/F24_Publication_Expression">
      <rdfs:label xml:lang="en">F24 Publication Expression</rdfs:label>
      <rdfs:subClassOf rdf:resource="http://erlangen-crm.org/efrbroo/F22_Self-Contained_Expression"/>
      <rdfs:comment>Scope note:
This class comprises complete sets of signs present in publications, reflecting publishers’ final decisions as to both selection of content and layout of the publications. Frequently the creation of a Publication Expression includes both adding graphical form and fonts to Expressions consisting of words alone and selecting illustrations and other content. As such, an instance of Publication Expression incorporates all Expressions combined for the resulting final form of rendering, whether visual, audio or tactile. An instance of Publication Expression is one entity regardless of the number of independent Expressions published within it, as long as it represents one unit of release. The published third party content can be associated via the property P165 incorporates (is incorporated in).

</rdfs:comment>
      <rdfs:comment>Examples:
The text, its layout and the textual and graphic (Saur’s logo on p. [i]) content of front and back cover, spine (spine title), and p. [i-iv] of the publication entitled ‘Functional Requirements for Bibliographic Records: final report’, published by K. G. Saur in 1998, identified by ISBN ‘3-598-11382-X’
The overall content of the book identified by ISBN ‘0-8014-9130-4’: the text of Stephen Crane’s complete poems as edited by Joseph Katz, the numbering system introduced by Joseph Katz in order to identify each individual poem by Stephen Crane, page numbers, the text of Joseph Katz’s dedication, preface, acknowledgements, and introduction, the table of contents, the index of first lines, the statements found on title page, back of title page (including CIP bibliographic record), cover front, back front, and spine, and the layout of the publication; for one of Stephen Crane’s longer poems, printed on p. 142-143, a statement reads at bottom of p. 142: ‘[NO STANZA BREAK]’: obviously, this statement does not belong to the Self-Contained Expression intended by Stephen Crane, and presumably not to the one intended by editor Joseph Katz either, but was more probably added by the publishing team, due to characteristics of the layout of the publication: a cautious reader can easily interpret ‘[NO STANZA BREAK]’ as non-belonging to the poem itself, but an OCR process would not make the distinction between the text of the poem and the statement made by the publisher; ‘[NO STANZA BREAK]’ belongs to the Publication Expression, although it does not belong to the Self-Contained Expression intended by Stephen Crane and Joseph Katz
The overall content of the LP sound recording identified by label and label number ‘CBS 34-61237’: a recorded performance of Terry Riley’s musical work ‘In C’, the text of liner notes by Paul Williams translated into French by Bernard Weinberg, technical statements such as ‘Stereo,’ publisher’s logo, series logo, title and statement of responsibility on front, back, and spine of the cover and on the recording itself, duration statement, cover art by G. Joly, overall layout, etc.; a special, shunting sound was added at the end of side one and beginning of side two, as Terry Riley’s work is in the form of a continuous musical flow without any interruption and the technical possibilities of vinyl LPs did not allow the complete performance to be contained on just one side: that special, shunting sound was not intended in Riley’s score nor in the performance but was added by the publisher (with or without Riley’s consent, this detail is not documented), and as such it is part of the Publication Expression although it is not part of the composer’s and the performers’ Self-Contained Expression (this shunting sound was no longer needed in subsequent releases on CD)
The overall content of the DVD entitled ‘The Aviator (2-Disc Full Screen Edition)’, released in 2004: Martin Scorsese’s movie itself; layout of the box and the two DVDs contained in the box; pictures on the DVDs themselves; English, Spanish, and French subtitles; English and French audio tracks; and bonuses: commentaries by director Martin Scorsese, editor Thelma Schoonmaker, and producer Michael Mann; a deleted scene (‘Howard Tells Ava About His Car Accident’); and featurettes ‘A Life Without Limits: The Making of The Aviator’; ‘The Role of Howard Hughes in Aviation History’; ‘Modern Marvels: Howard Hughes, A Documentary by the History Channel’; ‘The Visual Effects of The Aviator’; ‘The Affliction of Howard Hughes: Obsessive Compulsive Disorder’; ‘The Age of Glamour: The Hair And Makeup of The Aviator’; ‘Costuming The Aviator: The Work of Sandy Powell’; ‘Constructing The Aviator: The Work of Dante Ferretti’; ‘An evening with Leonardo DiCaprio and Alan Alda’; ‘OCD Panel Discussion With Leonardo DiCaprio, Martin Scorsese, and Howard Hughes’ Widow Terry Moore’; ‘Still Gallery’; ‘Scoring The Aviator: The Work Of Howard Shore’; and ‘The Wainwright Family – Loudon, Rufus and Martha’

</rdfs:comment>
   </owl:Class>
   <!--F25_Performance_Plan-->
   <owl:Class rdf:about="http://erlangen-crm.org/efrbroo/F25_Performance_Plan">
      <rdfs:label xml:lang="en">F25 Performance Plan</rdfs:label>
      <rdfs:subClassOf rdf:resource="http://erlangen-crm.org/efrbroo/F22_Self-Contained_Expression"/>
      <rdfs:subClassOf rdf:resource="http://erlangen-crm.org/current/E29_Design_or_Procedure"/>
      <rdfs:comment>Scope note:
This class comprises sets of directions to which individual performances of theatrical, choreographic, or musical works and their combinations should conform.
In the case of theatrical performances, such directions incorporate, but are not limited nor reducible to, the text of a given version of the play performed (e.g., a translated text, some passages of which are deliberately omitted, with some rephrased lines, etc.).
In the case of choreographic performances, such directions may incorporate, but are neither limited nor reducible to, the notation of choreographic movements in systems such as labanotation.
In the case of musical performances, such directions may incorporate, but are neither limited nor reducible to, the musical score. In case of electronic music, they may incorporate software instructions.
These directions may or may not completely determine the form of the intended performance. Depending on the nature of the directions, the form of the intended performance, such as the sets of movements or the sound characteristics, may or may not be predictable from the directions.
Note that a performance plan may be more or less elaborate, and may even foresee just improvisation.

</rdfs:comment>
      <rdfs:comment>Examples:
The set of instructions for the production of a Yiddish translation of the textual work entitled ‘King Lear’, as directed by Sergei Radlov in Moscow in 1935
The set of instructions for the production of the ballet entitled ‘Rite of spring’, as choreographed by Pina Bausch in Wuppertal in 1975
The set of instructions by Bruno Walter for performing Gustav Mahler’s 9th symphony, delivered by him to the Columbia Symphony Orchestra during rehearsals in Hollywood in 1961 (as partially documented in the CD entitled ‘Bruno Walter conducts and talks about Mahler symphony No. 9: rehearsal &amp; performance’)
The set of instructions contained in the “performance handbook” for Luigi Nono’s musical work entitled ‘À Pierre’

</rdfs:comment>
   </owl:Class>
   <!--F26_Recording-->
   <owl:Class rdf:about="http://erlangen-crm.org/efrbroo/F26_Recording">
      <rdfs:label xml:lang="en">F26 Recording</rdfs:label>
      <rdfs:subClassOf rdf:resource="http://erlangen-crm.org/efrbroo/F22_Self-Contained_Expression"/>
      <rdfs:comment>Scope note:
This class comprises expressions which are created in instances of F29 Recording Event. A recording is intended to convey (and preserve) the features of one or more perdurants.

</rdfs:comment>
      <rdfs:comment>Examples:
The set of signs that make up the third alternate take of the musical work entitled ‘Blue Hawaii’ as performed by Elvis Presley in Hollywood, Calif., Radio Recorders, on March 22nd, 1961
The set of signs that make up the famous photograph of the three Allied leaders at Yalta in February 1945
The set of signs that make up the sound recording of an East Australian humpback whale song in 1994
The set of signs that make up the sequences from the documentary movie entitled ‘Louise Bourgeois: The Spider, the Mistress, and the Tangerine’ in which Louise Bourgeois is seen at work

</rdfs:comment>
   </owl:Class>
   <!--F27_Work_Conception-->
   <owl:Class rdf:about="http://erlangen-crm.org/efrbroo/F27_Work_Conception">
      <rdfs:label xml:lang="en">F27 Work Conception</rdfs:label>
      <rdfs:subClassOf rdf:resource="http://erlangen-crm.org/current/E65_Creation"/>
      <rdfs:comment>Scope note:
This class comprises beginnings of evolutions of works.
An instance of F27 Work Conception marks the initiation of the creation of a work. The work, as an intellectual construction, evolves from this point on, until the last known expression of it. The instance of E39 Actor with which a work is associated through the chain of properties F1 Work R16i was initiated by F27 Work Conception P14 carried out by E39 Actor corresponds to the notion of the “creator” of the work. In the case of commissioned works, it is not the commissioning that is regarded as the work conception, but the acceptance of the commission.
This event does not always correlate with the date assigned in common library practice to the work, which is usually a later event (such as the date of completion of the first clean draft).
In addition, F27 Work Conception can serve to document the circumstances that surrounded the appearance of the original idea for a work, when these are known.

</rdfs:comment>
      <rdfs:comment>Examples:
Ludwig van Beethoven’s having the first ideas for his fifth symphony
Pablo Picasso’s acceptance, in 1930, of Ambroise Vollard’s commission for a set of 100 etchings, now known as the ‘Vollard Suite’
René Goscinny’s and Albert Uderzo’s first collaborative ideas for the comic book entitled ‘Asterix in Britain’ [comment: Goscinny wrote the script and Uderzo made the drawings; both are regarded as co-creators of that collaborative, at the same level of creative input, and no attempt is made to ascertain whether the ideas for the script preceded the ideas for the drawings, or vice-versa]
The combination of activities, carried out, among others, by Alfred Hitchcock, that began the process which eventually resulted in the movie entitled ‘Psycho’ coming into being
Oscar Wilde’s having by May 1897 the initial idea of writing his poem entitled ‘The ballad of the Reading gaol’, inspired by his stay in the Reading prison from November 20, 1895 to May 18, 1897, and the execution of Charles Thomas Woolridge on July 7, 1896

</rdfs:comment>
      <rdfs:comment>Properties:
R16 initiated (was initiated by): F1 Work

</rdfs:comment>
      <rdfs:subClassOf>
         <owl:Restriction>
            <owl:onProperty>
               <owl:ObjectProperty rdf:about="http://erlangen-crm.org/efrbroo/R16_initiated"/>
            </owl:onProperty>
            <owl:minCardinality rdf:datatype="http://www.w3.org/2001/XMLSchema#nonNegativeInteger">1</owl:minCardinality>
         </owl:Restriction>
      </rdfs:subClassOf>
   </owl:Class>
   <!--F28_Expression_Creation-->
   <owl:Class rdf:about="http://erlangen-crm.org/efrbroo/F28_Expression_Creation">
      <rdfs:label xml:lang="en">F28 Expression Creation</rdfs:label>
      <rdfs:subClassOf rdf:resource="http://erlangen-crm.org/current/E12_Production"/>
      <rdfs:subClassOf rdf:resource="http://erlangen-crm.org/current/E65_Creation"/>
      <rdfs:superClassOf rdf:resource="http://erlangen-crm.org/efrbroo/F29_Recording_Event"/>
      <rdfs:superClassOf rdf:resource="http://erlangen-crm.org/efrbroo/F30_Publication_Event"/>
      <rdfs:comment>Scope note:
This class comprises activities that result in instances of F2 Expression coming into existence. This class characterises the externalisation of an Individual Work.
Although F2 Expression is an abstract entity, a conceptual object, the creation of an expression inevitably also affects the physical world: when you scribble the first draft of a poem on a sheet of paper, you produce an instance of F4 Manifestation Singleton; F28 Expression Creation is a subclass of E12 Production because the recording of the expression causes a physical modification of the carrying E18 Physical Thing. The work becomes manifest by being expressed on a physical carrier different from the creator’s brain. The spatio-temporal circumstances under which the expression is created are necessarily the same spatio-temporal circumstances under which the first instance of F4 Manifestation Singleton is produced. The mechanisms through which oral tradition (of myths, tales, music, etc.) operates are not further investigated in this model. As far as bibliographic practice is concerned, only those instances of F2 Expression that are externalised on physical carriers other than both the creator’s brain and the auditor’s brain are taken into account (for a discussion of the modelling of oral traditions, see: Nicolas, Yann. ‘Folklore Requirements for Bibliographic Records: oral traditions and FRBR.’ In: Cataloging &amp; Classification Quarterly (2005). Vol. 39, No. 3-4. P. 179-195).
It is possible to use the P2 has type (is type of) property in order to specify that the creation of a given expression of a given work played a particular role with regard to the overall bibliographic history of that work (e.g., that it was the creation of the progenitor expression on which all other expressions of the same work are based; or that it was the creation of the critical edition that served as the basis for canonical references to the work).

</rdfs:comment>
      <rdfs:comment>Examples:
The creation of the original manuscript score of ‘Uwertura tragiczna’ by Andrzej Panufnik in 1942 in Warsaw
The reconstruction from memory of the manuscript score of ‘Uwertura tragiczna’ by Andrzej Panufnik in 1945 after the original score was destroyed during the war
The creation, by Lord Byron, of the English text of his work entitled ‘Manfred’ (P2 has type E55 Type {major original contribution})
The creation, by Woldemar Starke, of his German translation of Lord Byron’s text entitled ‘Manfred’ (P2 has type E55 Type {translation})
The recording of the third alternate take of ‘Blue Hawaii’ performed by Elvis Presley in Hollywood, Calif., Radio Recorders, on March 22nd, 1961 [each individual take is a distinct instance of F2 Expression]

</rdfs:comment>
      <rdfs:comment>Properties:
R17 created (was created by): F2 Expression
R18 created (was created by): F4 Manifestation Singleton
R19 created a realisation of (was realised through): F1 Work

</rdfs:comment>
      <rdfs:subClassOf>
         <owl:Restriction>
            <owl:cardinality rdf:datatype="http://www.w3.org/2001/XMLSchema#nonNegativeInteger">1</owl:cardinality>
            <owl:onProperty>
               <owl:ObjectProperty rdf:about="http://erlangen-crm.org/efrbroo/R17_created"/>
            </owl:onProperty>
         </owl:Restriction>
      </rdfs:subClassOf>
      <rdfs:subClassOf>
         <owl:Restriction>
            <owl:onProperty>
               <owl:ObjectProperty rdf:about="http://erlangen-crm.org/efrbroo/R18_created"/>
            </owl:onProperty>
            <owl:minCardinality rdf:datatype="http://www.w3.org/2001/XMLSchema#nonNegativeInteger">1</owl:minCardinality>
         </owl:Restriction>
      </rdfs:subClassOf>
      <rdfs:subClassOf>
         <owl:Restriction>
            <owl:onProperty>
               <owl:ObjectProperty rdf:about="http://erlangen-crm.org/efrbroo/R19_created_a_realisation_of"/>
            </owl:onProperty>
            <owl:minCardinality rdf:datatype="http://www.w3.org/2001/XMLSchema#nonNegativeInteger">1</owl:minCardinality>
         </owl:Restriction>
      </rdfs:subClassOf>
   </owl:Class>
   <!--F29_Recording_Event-->
   <owl:Class rdf:about="http://erlangen-crm.org/efrbroo/F29_Recording_Event">
      <rdfs:label xml:lang="en">F29 Recording Event</rdfs:label>
      <rdfs:subClassOf rdf:resource="http://erlangen-crm.org/efrbroo/F28_Expression_Creation"/>
      <rdfs:comment>Scope note:
This class comprises activities that intend to convey (and preserve) the features of perdurants in a recording, such as a live recording of a performance, a documentary, or other capture of a perdurant. Such activities may follow the directions of a recording plan. They may include postproduction.

</rdfs:comment>
      <rdfs:comment>Examples:
The making of the recording of the third alternate take of the musical work titled ‘Blue Hawaii’ as performed by Elvis Presley in Hollywood, Calif., Radio Recorders, on March 22nd, 1961
The making of the photograph of the three Allied leaders at Yalta in February 1945
The making of the recording of an East Australian humpback whale song in 1994 in the framework of the Oceania Project
Filming Louise Bourgeois at work in the context of the shooting of the documentary movie entitled ‘Louise Bourgeois: The Spider, the Mistress, and the Tangerine’

</rdfs:comment>
      <rdfs:comment>Properties:
R20 recorded (was recorded through): E2 Temporal Entity
R21 created (was created through): F26 Recording
R22 created a realisation of (was realised through): F21 Recording Work
R65 recorded aspects of (had aspects recorded through): E18 Physical Thing

</rdfs:comment>
      <rdfs:subClassOf>
         <owl:Restriction>
            <owl:onProperty>
               <owl:ObjectProperty rdf:about="http://erlangen-crm.org/efrbroo/R20_recorded"/>
            </owl:onProperty>
            <owl:minCardinality rdf:datatype="http://www.w3.org/2001/XMLSchema#nonNegativeInteger">1</owl:minCardinality>
         </owl:Restriction>
      </rdfs:subClassOf>
      <rdfs:subClassOf>
         <owl:Restriction>
            <owl:onProperty>
               <owl:ObjectProperty rdf:about="http://erlangen-crm.org/efrbroo/R21_created"/>
            </owl:onProperty>
            <owl:minCardinality rdf:datatype="http://www.w3.org/2001/XMLSchema#nonNegativeInteger">1</owl:minCardinality>
         </owl:Restriction>
      </rdfs:subClassOf>
      <rdfs:subClassOf>
         <owl:Restriction>
            <owl:onProperty>
               <owl:ObjectProperty rdf:about="http://erlangen-crm.org/efrbroo/R22_created_a_realisation_of"/>
            </owl:onProperty>
            <owl:maxCardinality rdf:datatype="http://www.w3.org/2001/XMLSchema#nonNegativeInteger">1</owl:maxCardinality>
         </owl:Restriction>
      </rdfs:subClassOf>
      <rdfs:subClassOf>
         <owl:Restriction>
            <owl:onProperty>
               <owl:ObjectProperty rdf:about="http://erlangen-crm.org/efrbroo/R65_recorded_aspects_of"/>
            </owl:onProperty>
            <owl:someValuesFrom rdf:resource="http://erlangen-crm.org/efrbroo/F29_Recording_Event"/>
         </owl:Restriction>
      </rdfs:subClassOf>
   </owl:Class>
   <!--F30_Publication_Event-->
   <owl:Class rdf:about="http://erlangen-crm.org/efrbroo/F30_Publication_Event">
      <rdfs:label xml:lang="en">F30 Publication Event</rdfs:label>
      <rdfs:subClassOf rdf:resource="http://erlangen-crm.org/efrbroo/F28_Expression_Creation"/>
      <rdfs:comment>Scope note:
This class comprises the activities of publishing. Such an event includes the creation of an F24 Publication Expression and setting up the means of production. The end of this event is regarded as the date of publication, regardless of whether the carrier production is started. Publishing can be either physical or electronic. Electronic publishing is regarded as making an instance of F24 Publication Expression available in electronic form on a public network. Electronic Publishing does not mean producing a physical instance of F5 Item by partially electronic means. Making an electronic file available on a physical carrier can be regarded as equivalent to setting up the means of production; downloading the file is regarded as the electronic equivalent of F32 Carrier Production Event.

</rdfs:comment>
      <rdfs:comment>Examples:
Publishing Amerigo Vespucci’s ‘Mundus novus’ in Paris ca. 1503-1504
Establishing in 1972 the layout, features, and prototype for the publication of ‘The complete poems of Stephen Crane, edited with an introduction by Joseph Katz’ (ISBN ‘0-8014-9130-4’), which served for a second print run in 1978
Making available online the article by Allen Renear, Christopher Phillippe, Pat Lawton, and David Dubin, entitled ‘An XML document corresponds to which FRBR Group 1 entity?’ &lt;http://conferences.idealliance.org/extreme/html/2003/Lawton01/EML2003Lawton01.html&gt;

</rdfs:comment>
      <rdfs:comment>Properties:
R23 created a realisation of (was realised through): F19 Publication Work
R24 created (was created through): F24 Publication Expression

</rdfs:comment>
      <rdfs:subClassOf>
         <owl:Restriction>
            <owl:onProperty>
               <owl:ObjectProperty rdf:about="http://erlangen-crm.org/efrbroo/R23_created_a_realisation_of"/>
            </owl:onProperty>
            <owl:maxCardinality rdf:datatype="http://www.w3.org/2001/XMLSchema#nonNegativeInteger">1</owl:maxCardinality>
         </owl:Restriction>
      </rdfs:subClassOf>
      <rdfs:subClassOf>
         <owl:Restriction>
            <owl:onProperty>
               <owl:ObjectProperty rdf:about="http://erlangen-crm.org/efrbroo/R24_created"/>
            </owl:onProperty>
            <owl:minCardinality rdf:datatype="http://www.w3.org/2001/XMLSchema#nonNegativeInteger">1</owl:minCardinality>
         </owl:Restriction>
      </rdfs:subClassOf>
   </owl:Class>
   <!--F31_Performance-->
   <owl:Class rdf:about="http://erlangen-crm.org/efrbroo/F31_Performance">
      <rdfs:label xml:lang="en">F31 Performance</rdfs:label>
      <rdfs:subClassOf rdf:resource="http://erlangen-crm.org/current/E7_Activity"/>
      <rdfs:comment>Scope note:
This class comprises activities that follow the directions of a performance plan, such as a theatrical play, an expression of a choreographic work or a musical work; i.e., they are intended to communicate directly or indirectly to an audience.
Such activities can be identified at various levels of granularity, and can be contiguous or not. Any individual performance (with or without intermissions) is a single instance of F31 Performance. In addition, a complete run of performances can also be seen as an instance of F31 Performance, with individual performances as parts. A complete run of performances may comprise an original run plus any of its extensions and tours.
Note that a performance plan may be more or less elaborate, and may even foresee just improvisation.

</rdfs:comment>
      <rdfs:comment>Examples:
Performing the first performance of a Yiddish translation of the textual work entitled ‘King Lear’, as directed by Sergei Radlov, in Moscow, at the Moscow State Jewish Theatre, on February 10, 1935 [individual performance]
Performing the ballet entitled ‘Rite of spring’, as choreographed by Pina Bausch, in Avignon, at the Popes’ Palace, on July 7, 1995 [individual performance]
Performing the operatic work entitled ‘Dido and Aeneas’, as directed by Edward Gordon Craig and conducted by Martin Shaw, in London, Hampstead Conservatoire, on May 17, 18, and 19, 1900 [run of performances]

</rdfs:comment>
      <rdfs:comment>Properties:
R25 performed (was performed in): F25 Performance Plan
R66 included performed version of (had a performed version through): E89 Propositional Object

</rdfs:comment>
      <rdfs:subClassOf>
         <owl:Restriction>
            <owl:onProperty>
               <owl:ObjectProperty rdf:about="http://erlangen-crm.org/efrbroo/R25_performed"/>
            </owl:onProperty>
            <owl:someValuesFrom rdf:resource="http://erlangen-crm.org/efrbroo/F31_Performance"/>
         </owl:Restriction>
      </rdfs:subClassOf>
      <rdfs:subClassOf>
         <owl:Restriction>
            <owl:onProperty>
               <owl:ObjectProperty rdf:about="http://erlangen-crm.org/efrbroo/R66_included_performed_version_of"/>
            </owl:onProperty>
            <owl:someValuesFrom rdf:resource="http://erlangen-crm.org/efrbroo/F31_Performance"/>
         </owl:Restriction>
      </rdfs:subClassOf>
   </owl:Class>
   <!--F32_Carrier_Production_Event-->
   <owl:Class rdf:about="http://erlangen-crm.org/efrbroo/F32_Carrier_Production_Event">
      <rdfs:label xml:lang="en">F32 Carrier Production Event</rdfs:label>
      <rdfs:subClassOf rdf:resource="http://erlangen-crm.org/current/E12_Production"/>
      <rdfs:comment>Scope note:
This class comprises activities that result in instances of F54 Utilised Information Carrier coming into existence. Both the production of a series of physical objects (printed books, scores, CDs, DVDs, CD-ROMS, etc.) and the creation of a new copy of a file on an electronic carrier are regarded as instances of F32 Carrier Production Event.
Typically, the production of copies of a publication (no matter whether it is a book, a sound recording, a DVD, a cartographic resource, etc.) strives to produce items all as similar as possible to a prototype that displays all the features that all the copies of the publication should also display, which is reflected in property R27 used as source material F24 Publication Expression.

</rdfs:comment>
      <rdfs:comment>Examples:
The printing of copies of the 3rd edition of ‘Codex Manesse: die Miniaturen der großen Heidelberger Liederhandschrift, herausgegeben und erläutert von Ingo F. Walther unter Mitarbeit von Gisela Siebert’, Insel-Verlag, 1988 [a fac-simile edition of an illuminated mediaeval manuscript]
The printing of copies of the ‘Ordnance Survey Explorer Map 213, Aberystwyth &amp; Cwm Rheidol’, ISBN 0-319-23640-4 (folded), 1:25,000 scale, released in May 2005 [a cartographic resource]
The production of copies of the sound recording titled ‘The Glory (????) of the human voice’, RCA Victor Gold Seal GD61175, containing recordings of musical works performed by Florence Foster Jenkins [a sound recording; the question marks in parentheses belong to the original title]
My clicking now on the link &lt;http://cidoc.ics.forth.gr/docs/cidoc_crm_version_4.0.pdf&gt;, and thus downloading on my PC a reproduction of the electronic file titled ‘Definition of the CIDOC Conceptual Reference Model… version 4.0’ that is stored on the ICS FORTH’s servers in Heraklion, Crete
The second print run, in 1978, of ‘The complete poems of Stephen Crane, edited with an introduction by Joseph Katz’ (ISBN ‘0-8014-9130-4’), a publication dated 1972 [publication of a printed text]

</rdfs:comment>
      <rdfs:comment>Properties:
R26 produced things of type (was produced by): F3 Manifestation Product Type
R27 used as source material (was used by): F24 Publication Expression
R28 produced (was produced by): F54 Utilised Information Carrier

</rdfs:comment>
      <rdfs:subClassOf>
         <owl:Restriction>
            <owl:onProperty>
               <owl:ObjectProperty rdf:about="http://erlangen-crm.org/efrbroo/R26_produced_things_of_type"/>
            </owl:onProperty>
            <owl:minCardinality rdf:datatype="http://www.w3.org/2001/XMLSchema#nonNegativeInteger">1</owl:minCardinality>
         </owl:Restriction>
      </rdfs:subClassOf>
      <rdfs:subClassOf>
         <owl:Restriction>
            <owl:onProperty>
               <owl:ObjectProperty rdf:about="http://erlangen-crm.org/efrbroo/R27_used_as_source_material"/>
            </owl:onProperty>
            <owl:someValuesFrom rdf:resource="http://erlangen-crm.org/efrbroo/F32_Carrier_Production_Event"/>
         </owl:Restriction>
      </rdfs:subClassOf>
      <rdfs:subClassOf>
         <owl:Restriction>
            <owl:onProperty>
               <owl:ObjectProperty rdf:about="http://erlangen-crm.org/efrbroo/R28_produced"/>
            </owl:onProperty>
            <owl:someValuesFrom rdf:resource="http://erlangen-crm.org/efrbroo/F32_Carrier_Production_Event"/>
         </owl:Restriction>
      </rdfs:subClassOf>
   </owl:Class>
   <!--F33_Reproduction_Event-->
   <owl:Class rdf:about="http://erlangen-crm.org/efrbroo/F33_Reproduction_Event">
      <rdfs:label xml:lang="en">F33 Reproduction Event</rdfs:label>
      <rdfs:subClassOf rdf:resource="http://erlangen-crm.org/current/E12_Production"/>
      <rdfs:comment>Scope note:
This class comprises activities that consist in making copies, more or less mechanically, of an instance of E84 Information Carrier (such as an F5 Item or an F4 Manifestation Singleton which is also instance of E84 Information Carrier), preserving the expression carried by it. A Reproduction Event results in new instances of E84 Information Carrier coming into existence. In general, the copy will have different attributes from the original and they are therefore not regarded as siblings.
This class makes it possible to account for the legal distinction between private copying for the purpose of “fair use,” and mass production for the purpose of dissemination.
It can prove difficult to determine where to draw the line between F33 Reproduction Event and F32 Carrier Production Event in cases where multiple copies are produced. In this case, the copies, but not the original, may be regarded as instances of F5 Item. It is the existence of an explicit production plan that makes the difference. As a consequence, F33 Reproduction Event and F32 Carrier Production Event are not declared as disjoint, which makes it possible to account for such situations that could be regarded as instances of both Production Event and Reproduction Event.

</rdfs:comment>
      <rdfs:comment>Examples:
My photocopying now for my own private use an exemplar of the article entitled ‘Federal Court’s Ruling Against Photocopying Chain Will Not Destroy “Fair Use”’ by Kenneth D. Crews, issued in ‘Chronicle of higher education’, 17 April 1991, A48
The BnF’s producing in 1997 the microfilm identified by call number ‘Microfilm M-12169’ of the exemplar identified by shelf mark ‘Res 8 P 10’ of Amerigo Vespucci’s ‘Mundus novus’ published in Paris ca. 1503-1504
The BnF’s reproducing in 2001 the exemplar identified by call number ‘NC His Master’s Voice HC 20’ of a 78 rpm phonogram released by Gramophone in 1932, as part of the CD identified by call number ‘SDCR 2120’
The BnF’s making in 2003 a digitisation, identified by call number ‘IFN 7701015’, of the collection of drawings (held by the BnF) that were made by Étienne-Louis Boullée in 1784 for his project of a ‘Newton Cenotaph’

</rdfs:comment>
      <rdfs:comment>Properties:
R29 reproduced (was reproduced by): E84 Information Carrier
R30 produced (was produced by): E84 Information Carrier

</rdfs:comment>
      <rdfs:subClassOf>
         <owl:Restriction>
            <owl:onProperty>
               <owl:ObjectProperty rdf:about="http://erlangen-crm.org/efrbroo/R29_reproduced"/>
            </owl:onProperty>
            <owl:minCardinality rdf:datatype="http://www.w3.org/2001/XMLSchema#nonNegativeInteger">1</owl:minCardinality>
         </owl:Restriction>
      </rdfs:subClassOf>
      <rdfs:subClassOf>
         <owl:Restriction>
            <owl:onProperty>
               <owl:ObjectProperty rdf:about="http://erlangen-crm.org/efrbroo/R30_produced"/>
            </owl:onProperty>
            <owl:minCardinality rdf:datatype="http://www.w3.org/2001/XMLSchema#nonNegativeInteger">1</owl:minCardinality>
         </owl:Restriction>
      </rdfs:subClassOf>
   </owl:Class>
   <!--F34_KOS-->
   <owl:Class rdf:about="http://erlangen-crm.org/efrbroo/F34_KOS">
      <rdfs:label xml:lang="en">F34 KOS</rdfs:label>
      <rdfs:subClassOf rdf:resource="http://erlangen-crm.org/current/E32_Authority_Document"/>
      <rdfs:subClassOf rdf:resource="http://erlangen-crm.org/current/E29_Design_or_Procedure"/>
      <rdfs:subClassOf rdf:resource="http://erlangen-crm.org/efrbroo/F2_Expression"/>
      <rdfs:comment>Scope note:
This class comprises documents that establish controlled terminology (nomina) for consistent use. They may also describe relationships between entities and controlled terminology and relationships between entities. Note that any meaningful change in a Knowledge Organisation System (KOS) that affects the validity status of its elements defines a new release (Expression) of the KOS. Note that identifiers created following a rule in a KOS are to be regarded as being taken from this KOS, even though not explicitly spelled out. This definition of KOS reflects current library practice and not the use of the term in general.

</rdfs:comment>
      <rdfs:comment>Examples:
LCSH February 20 to March 19 2012
DDC 19 [19th English edition, published only in print by Forest Press in 1979]

</rdfs:comment>
      <rdfs:comment>Properties:
R34 has validity period (is validity period of): E52 Time-Span

</rdfs:comment>
      <rdfs:subClassOf>
         <owl:Restriction>
            <owl:cardinality rdf:datatype="http://www.w3.org/2001/XMLSchema#nonNegativeInteger">1</owl:cardinality>
            <owl:onProperty>
               <owl:ObjectProperty rdf:about="http://erlangen-crm.org/efrbroo/R34_has_validity_period"/>
            </owl:onProperty>
         </owl:Restriction>
      </rdfs:subClassOf>
   </owl:Class>
   <!--F35_Nomen_Use_Statement-->
   <owl:Class rdf:about="http://erlangen-crm.org/efrbroo/F35_Nomen_Use_Statement">
      <rdfs:label xml:lang="en">F35 Nomen Use Statement</rdfs:label>
      <rdfs:subClassOf rdf:resource="http://erlangen-crm.org/efrbroo/F2_Expression"/>
      <rdfs:subClassOf rdf:resource="http://erlangen-crm.org/current/E29_Design_or_Procedure"/>
      <rdfs:comment>Scope note:
This class comprises statements relating a Thema with a particular Nomen and its usage in the context of a common Complex Work realized by one or more KOS.

</rdfs:comment>
      <rdfs:comment>Examples:
‘010 __ |a sh 85082387’…‘150 __ |a Maxwell equations’ [MARC 21 encoding of the preferred subject access point from LCSH, http://lccn.loc.gov/sh85082387, as of 19 November 2012]
‘010 __ |a sh 85082387’…‘450 __ |a Equations, Maxwell’ [MARC 21 encoding of a variant subject access point, from the same source]
‘PTBNP|20891’…‘200 1‎‡a Whitman,‏ ‎‡b Walt,‏ ‎‡f 1819-1892‏’ [UNIMARC encoding of the preferred access point for a personal name, from the authority file of the National Library of Portugal, as found on VIAF, http://www.viaf.org/processed/PTBNP%7C20891, on 28 September 2015]
‘001  FRBNF119547493’…‘100  w.0..barus.$aGončarova$mNatalʹâ Sergeevna$d1881-1962’ [INTERMARC encoding of the preferred access point for a personal name, from the authority file of the National Library of France, http://catalogue.bnf.fr/ark:/12148/cb119547494/ INTERMARC, as of 15 June 2012]
‘001  FRBNF119547493’…‘100  w.0..c.rus.$aГончарова$mНаталья Сергеевна$d1881-1962’ [INTERMARC encoding of a parallel access point from the same source]
‘001  FRBNF119547493’…‘400  $w....b.eng.$aGoncharova$mNatalia$d1881-1962’ [INTERMARC encoding of a variant access point from the same source]
‘&lt;eac-cpf […]&gt; &lt;control&gt; &lt;recordId&gt;beinecke.7h44jbj&lt;/recordId&gt; […] &lt;/control&gt;’ … ‘&lt;cpfDescription&gt; &lt;identity&gt; &lt;entityType&gt;family&lt;/entityType&gt; &lt;nameEntry xml:lang="eng" scriptCode="Latn"&gt;&lt;part localType="100a"&gt;Boswell family&lt;/part&gt; […] &lt;/nameEntry&gt; […] &lt;/identity&gt; &lt;/cpfDescription&gt; […] &lt;/eac-cpf&gt;’ [EAC encoding of the preferred access point for a family]

</rdfs:comment>
      <rdfs:comment>Properties:
R32 is warranted by (warrants): F52 Name Use Activity
R35 is specified by (specifies): F34 KOS

(R35.1 has status: E55 Type)
R36 uses script conversion (is script conversion used in): F36 Script Conversion
R37 states as nomen (is stated as nomen in): F12 Nomen
R38 refers to thema (is thema of): E1 CRM Entity
R39 is intended for (is target audience in): E74 Group
R54 has nomen language (is language of nomen in): E56 Language
R55 has nomen form (is nomen form in): E55 Type
R56 has related use (is related use for): F35 Nomen Use Statement
(R56.1 has type: E55 Type)

</rdfs:comment>
      <rdfs:subClassOf>
         <owl:Restriction>
            <owl:onProperty>
               <owl:ObjectProperty rdf:about="http://erlangen-crm.org/efrbroo/R32_is_warranted_by"/>
            </owl:onProperty>
            <owl:someValuesFrom rdf:resource="http://erlangen-crm.org/efrbroo/F35_Nomen_Use_Statement"/>
         </owl:Restriction>
      </rdfs:subClassOf>
      <rdfs:subClassOf>
         <owl:Restriction>
            <owl:cardinality rdf:datatype="http://www.w3.org/2001/XMLSchema#nonNegativeInteger">1</owl:cardinality>
            <owl:onProperty>
               <owl:ObjectProperty rdf:about="http://erlangen-crm.org/efrbroo/R35_is_specified_by"/>
            </owl:onProperty>
         </owl:Restriction>
      </rdfs:subClassOf>
      <rdfs:subClassOf>
         <owl:Restriction>
            <owl:onProperty>
               <owl:ObjectProperty rdf:about="http://erlangen-crm.org/efrbroo/R36_uses_script_conversion"/>
            </owl:onProperty>
            <owl:maxCardinality rdf:datatype="http://www.w3.org/2001/XMLSchema#nonNegativeInteger">1</owl:maxCardinality>
         </owl:Restriction>
      </rdfs:subClassOf>
      <rdfs:subClassOf>
         <owl:Restriction>
            <owl:cardinality rdf:datatype="http://www.w3.org/2001/XMLSchema#nonNegativeInteger">1</owl:cardinality>
            <owl:onProperty>
               <owl:ObjectProperty rdf:about="http://erlangen-crm.org/efrbroo/R37_states_as_nomen"/>
            </owl:onProperty>
         </owl:Restriction>
      </rdfs:subClassOf>
      <rdfs:subClassOf>
         <owl:Restriction>
            <owl:cardinality rdf:datatype="http://www.w3.org/2001/XMLSchema#nonNegativeInteger">1</owl:cardinality>
            <owl:onProperty>
               <owl:ObjectProperty rdf:about="http://erlangen-crm.org/efrbroo/R38_refers_to_thema"/>
            </owl:onProperty>
         </owl:Restriction>
      </rdfs:subClassOf>
      <rdfs:subClassOf>
         <owl:Restriction>
            <owl:onProperty>
               <owl:ObjectProperty rdf:about="http://erlangen-crm.org/efrbroo/R39_is_intended_for"/>
            </owl:onProperty>
            <owl:someValuesFrom rdf:resource="http://erlangen-crm.org/efrbroo/F35_Nomen_Use_Statement"/>
         </owl:Restriction>
      </rdfs:subClassOf>
      <rdfs:subClassOf>
         <owl:Restriction>
            <owl:onProperty>
               <owl:ObjectProperty rdf:about="http://erlangen-crm.org/efrbroo/R54_has_nomen_language"/>
            </owl:onProperty>
            <owl:someValuesFrom rdf:resource="http://erlangen-crm.org/efrbroo/F35_Nomen_Use_Statement"/>
         </owl:Restriction>
      </rdfs:subClassOf>
      <rdfs:subClassOf>
         <owl:Restriction>
            <owl:onProperty>
               <owl:ObjectProperty rdf:about="http://erlangen-crm.org/efrbroo/R55_has_nomen_form"/>
            </owl:onProperty>
            <owl:maxCardinality rdf:datatype="http://www.w3.org/2001/XMLSchema#nonNegativeInteger">1</owl:maxCardinality>
         </owl:Restriction>
      </rdfs:subClassOf>
      <rdfs:subClassOf>
         <owl:Restriction>
            <owl:onProperty>
               <owl:ObjectProperty rdf:about="http://erlangen-crm.org/efrbroo/R56_has_related_use"/>
            </owl:onProperty>
            <owl:someValuesFrom rdf:resource="http://erlangen-crm.org/efrbroo/F35_Nomen_Use_Statement"/>
         </owl:Restriction>
      </rdfs:subClassOf>
   </owl:Class>
   <!--F36_Script_Conversion-->
   <owl:Class rdf:about="http://erlangen-crm.org/efrbroo/F36_Script_Conversion">
      <rdfs:label xml:lang="en">F36 Script Conversion</rdfs:label>
      <rdfs:subClassOf rdf:resource="http://erlangen-crm.org/current/E29_Design_or_Procedure"/>
      <rdfs:comment>Scope note:
This class comprises rule sets for converting signs or arrangements of signs from one script or type set to another.

</rdfs:comment>
      <rdfs:comment>Examples:
ISO 9:1995

</rdfs:comment>
   </owl:Class>
   <!--F38_Character-->
   <owl:Class rdf:about="http://erlangen-crm.org/efrbroo/F38_Character">
      <rdfs:label xml:lang="en">F38 Character</rdfs:label>
      <rdfs:subClassOf rdf:resource="http://erlangen-crm.org/current/E28_Conceptual_Object"/>
      <rdfs:comment>Scope note:
This class comprises fictional or iconographic individuals or groups of individuals (including families) appearing in works in a way relevant as subjects. Characters may be purely fictitious or based on real persons or groups, but as characters they may exhibit properties that would be inconsistent with a real person or group. Rather than merging characters with real persons, they should be described as disjoint, but related entities.

</rdfs:comment>
      <rdfs:comment>Examples:
Harry Potter [in J.K. Rowling’s series of novels and the films based on them]
Sinuhe the Egyptian [in Mika Waltari’s novel]
The Knights of the Round Table [in fiction]

</rdfs:comment>
      <rdfs:comment>Properties:
R57 is based on (is basis for): E39 Actor
R58 has fictional member (is fictional member of): F38 Character

</rdfs:comment>
      <rdfs:subClassOf>
         <owl:Restriction>
            <owl:onProperty>
               <owl:ObjectProperty rdf:about="http://erlangen-crm.org/efrbroo/R57_is_based_on"/>
            </owl:onProperty>
            <owl:someValuesFrom rdf:resource="http://erlangen-crm.org/efrbroo/F38_Character"/>
         </owl:Restriction>
      </rdfs:subClassOf>
      <rdfs:subClassOf>
         <owl:Restriction>
            <owl:onProperty>
               <owl:ObjectProperty rdf:about="http://erlangen-crm.org/efrbroo/R58_has_fictional_member"/>
            </owl:onProperty>
            <owl:someValuesFrom rdf:resource="http://erlangen-crm.org/efrbroo/F38_Character"/>
         </owl:Restriction>
      </rdfs:subClassOf>
   </owl:Class>
   <!--F39_Family-->
   <owl:Class rdf:about="http://erlangen-crm.org/efrbroo/F39_Family">
      <rdfs:label xml:lang="en">F39 Family</rdfs:label>
      <rdfs:subClassOf rdf:resource="http://erlangen-crm.org/current/E74_Group"/>
      <rdfs:comment>Scope note:
This class comprises groups of two or more persons presented as a family justified by relationships of birth, marriage, adoption, civil union, or similar social or legal status and an assumed common tradition, including examples such as royal families, dynasties, houses of nobility, etc.

</rdfs:comment>
      <rdfs:comment>Examples:
House of Tudor
The Grimm brothers

</rdfs:comment>
   </owl:Class>
   <!--F40_Identifier_Assignment-->
   <owl:Class rdf:about="http://erlangen-crm.org/efrbroo/F40_Identifier_Assignment">
      <rdfs:label xml:lang="en">F40 Identifier Assignment</rdfs:label>
      <owl:equivalentClass rdf:resource="http://erlangen-crm.org/current/E15_Identifier_Assignment"/>
      <rdfs:comment>Equal to:
E15 Identifier Assignment
</rdfs:comment>
      <rdfs:comment>Scope note:
This class comprises activities that result in the allocation of an identifier to an instance of any subclass of E1 CRM Entity. An F40 Identifier Assignment may include the creation of the identifier from multiple constituents. Explicit reference to the used constituents can be made using the property P142 used constituent (was used in). The syntax of the identifier and the kinds of constituents to be used in constructing it may be declared in a rule. The construction of controlled access points for the names of persons, families and corporate bodies following specific cataloguing rules is a typical library application of identifier assignment. F40 Identifier Assignment also includes the assignment of controlled access points for works or expressions.

</rdfs:comment>
      <rdfs:comment>Examples:
Assigning the controlled access point ‘William, Prince, Duke of Cambridge, 1982-’ as a controlled access point for a personal name, using the Anglo-American Cataloguing Rules, 2nd edition
Assigning the controlled access point ‘Library and Archives Canada’ as an authorised controlled access point for a corporate body name, using the Anglo-American Cataloguing Rules, 2nd edition
Assigning the controlled access point ‘Bibliothèque et Archives Canada’ as an authorised controlled access point for a corporate body name, using the Règles de catalogage anglo-américaines, 2e édition
Assigning the controlled access point ‘Goethe, Johann Wolfgang von, 1749-1832. Faust. 1. Theil.’ as an authorised controlled access point for a work
Assigning the controlled access point ‘Bible. English. American Standard’ as an authorised controlled access point for an expression

</rdfs:comment>
      <rdfs:comment>Properties:
R45 assigned to (was assigned by): E1 CRM Entity
R46 assigned (was assigned by): F13 Identifier
R52 used rule (was the rule used in): F43 Identifier Rule

</rdfs:comment>
      <rdfs:subClassOf>
         <owl:Restriction>
            <owl:cardinality rdf:datatype="http://www.w3.org/2001/XMLSchema#nonNegativeInteger">1</owl:cardinality>
            <owl:onProperty>
               <owl:ObjectProperty rdf:about="http://erlangen-crm.org/efrbroo/R45_assigned_to"/>
            </owl:onProperty>
         </owl:Restriction>
      </rdfs:subClassOf>
      <rdfs:subClassOf>
         <owl:Restriction>
            <owl:cardinality rdf:datatype="http://www.w3.org/2001/XMLSchema#nonNegativeInteger">1</owl:cardinality>
            <owl:onProperty>
               <owl:ObjectProperty rdf:about="http://erlangen-crm.org/efrbroo/R46_assigned"/>
            </owl:onProperty>
         </owl:Restriction>
      </rdfs:subClassOf>
      <rdfs:subClassOf>
         <owl:Restriction>
            <owl:onProperty>
               <owl:ObjectProperty rdf:about="http://erlangen-crm.org/efrbroo/R52_used_rule"/>
            </owl:onProperty>
            <owl:someValuesFrom rdf:resource="http://erlangen-crm.org/efrbroo/F40_Identifier_Assignment"/>
         </owl:Restriction>
      </rdfs:subClassOf>
   </owl:Class>
   <!--F41_Representative_Manifestation_Assignment-->
   <owl:Class rdf:about="http://erlangen-crm.org/efrbroo/F41_Representative_Manifestation_Assignment">
      <rdfs:label xml:lang="en">F41 Representative Manifestation Assignment</rdfs:label>
      <rdfs:subClassOf rdf:resource="http://erlangen-crm.org/current/E13_Attribute_Assignment"/>
      <rdfs:comment>Scope note:
This class comprises activities through which an Agency declares (implicitly or explicitly) that a given instance of F3 Manifestation Product Type or F4 Manifestation Singleton is representative for a given F2 Expression, i.e., that some features found on that instance of F3 Manifestation Product Type or F4 Manifestation Singleton (most prominently, information about the title) can be inferred to also apply to that instance of F2 Expression, no matter within which manifestation it is embodied.
The reasoning behind is that the Work title is known through the title of an Expression that is deemed representative of the Work, and the title of the representative Expression is known through the title proper of a Manifestation that is deemed representative of the Expression representative of the Work.

</rdfs:comment>
      <rdfs:comment>Examples:
Selecting the 1775 edition of Richard Brinsley Sheridan’s textual work entitled ‘St. Patrick’s Day’ as the representative manifestation for the text of Richard Brinsley Sheridan’s textual work entitled ‘St. Patrick’s Day’ and citing that publication as the source for the authority record created by the Library of Congress for that work
Selecting the 2007 edition of John Tavener’s musical work entitled ‘The Eternal Sun’ as the representative manifestation for the notation of John Tavener’s musical work entitled ‘The Eternal Sun’ and citing that publication as the source for the authority record created by the National Library of France for that work
Selecting the 1983 edition of Stanley Karnow’s textual work entitled ‘Vietnam, the war nobody won’ as the representative manifestation for a partial expression of the series entitled ‘Headline series’ and citing that publication as the source for the authority record created by the Library of Congress for that series
Selecting the issue dated October 2002 of the periodical entitled ‘The New Courier’ as the representative manifestation for a partial expression of the periodical entitled ‘The New Courier’ and citing that publication as the source for the bibliographic record created by the National Library of France for that periodical
Selecting the manuscript identified by shelfmark ‘MS-8282’ within the collections of the National Library of France, Department for Music, as representative for the notation of Stanislas Champein’s musical work entitled ‘Vichnou’ and citing that manuscript as the source for the authority record created by the National Library of France for that work

</rdfs:comment>
      <rdfs:comment>Properties:
R43 carried out by (performed): F44 Bibliographic Agency
R48 assigned to (was assigned by): F2 Expression
R49 assigned (was assigned by): F3 Manifestation Product Type
R53 assigned (was assigned by): F4 Manifestation Singleton

</rdfs:comment>
      <rdfs:subClassOf>
         <owl:Restriction>
            <owl:cardinality rdf:datatype="http://www.w3.org/2001/XMLSchema#nonNegativeInteger">1</owl:cardinality>
            <owl:onProperty>
               <owl:ObjectProperty rdf:about="http://erlangen-crm.org/efrbroo/R43_carried_out_by"/>
            </owl:onProperty>
         </owl:Restriction>
      </rdfs:subClassOf>
      <rdfs:subClassOf>
         <owl:Restriction>
            <owl:cardinality rdf:datatype="http://www.w3.org/2001/XMLSchema#nonNegativeInteger">1</owl:cardinality>
            <owl:onProperty>
               <owl:ObjectProperty rdf:about="http://erlangen-crm.org/efrbroo/R48_assigned_to"/>
            </owl:onProperty>
         </owl:Restriction>
      </rdfs:subClassOf>
      <rdfs:subClassOf>
         <owl:Restriction>
            <owl:onProperty>
               <owl:ObjectProperty rdf:about="http://erlangen-crm.org/efrbroo/R49_assigned"/>
            </owl:onProperty>
            <owl:someValuesFrom rdf:resource="http://erlangen-crm.org/efrbroo/F41_Representative_Manifestation_Assignment"/>
         </owl:Restriction>
      </rdfs:subClassOf>
      <rdfs:subClassOf>
         <owl:Restriction>
            <owl:onProperty>
               <owl:ObjectProperty rdf:about="http://erlangen-crm.org/efrbroo/R53_assigned"/>
            </owl:onProperty>
            <owl:someValuesFrom rdf:resource="http://erlangen-crm.org/efrbroo/F41_Representative_Manifestation_Assignment"/>
         </owl:Restriction>
      </rdfs:subClassOf>
   </owl:Class>
   <!--F42_Representative_Expression_Assignment-->
   <owl:Class rdf:about="http://erlangen-crm.org/efrbroo/F42_Representative_Expression_Assignment">
      <rdfs:label xml:lang="en">F42 Representative Expression Assignment</rdfs:label>
      <rdfs:subClassOf rdf:resource="http://erlangen-crm.org/current/E13_Attribute_Assignment"/>
      <rdfs:comment>Scope note:
This class comprises activities through which an Agency declares (implicitly or explicitly) that a given instance of F2 Expression is representative for a given F15 Complex Work, i.e., that some attributes of that instance of F2 Expression (most prominently, information about the title) can be inferred to also apply to that instance of F15 Complex Work, no matter in which particular expression it is realised.
The reasoning behind this is that the Work title is known through the title of an Expression that is deemed representative of the Work, and the title of the representative Expression is known through the title of a Manifestation that is deemed representative of the Expression that is representative of the Work.
For instance, by using the qualified controlled access point ‘Poe, Edgar Allan, 1809-1849. Murders in the rue Morgue (French)’ for the French rendition of Poe’s ‘Murders in the rue Morgue’ by Baudelaire, an Agency implicitly states that the French text does not constitute a representative F2 Expression for Poe’s F1 Work, however the original English text does constitute a representative F2 Expression for Poe’s F1 Work.

</rdfs:comment>
      <rdfs:comment>Examples:
Selecting the text embodied in the 1775 edition of Richard Brinsley Sheridan’s textual work entitled ‘St. Patrick’s Day’ as the representative expression for Richard Brinsley Sheridan’s textual work entitled ‘St. Patrick’s Day’ and citing that publication as the source for the authority record created by the Library of Congress for that work
Selecting the musical notation embodied in the 2007 edition of John Tavener’s musical work entitled ‘The Eternal Sun’ as the representative expression for John Tavener’s musical work entitled ‘The Eternal Sun’ and citing that publication as the source for the authority record created by the National Library of France for that work
Selecting the publication expression of the 1983 edition of Stanley Karnow’s textual work entitled ‘Vietnam, the war nobody won’ as the representative expression for the series entitled ‘Headline series’ and citing that publication as the source for the authority record created by the Library of Congress for that series
Selecting the publication expression of the issue dated October 2002 of the periodical entitled ‘The New Courier’ as the representative expression of the periodical entitled ‘The New Courier’ and citing that publication as the source for the bibliographic record created by the National Library of France for that periodical
Selecting the content of the manuscript identified by shelfmark ‘MS-8282’ within the collections of the National Library of France, Department for Music, as the representative expression of Stanislas Champein’s musical work entitled ‘Vichnou’ and citing that manuscript as the source for the authority record created by the National Library of France for that work

</rdfs:comment>
      <rdfs:comment>Properties:
R44 carried out by (performed): F44 Bibliographic Agency
R50 assigned to (was assigned by): F15 Complex Work
R51 assigned (was assigned by): F2 Expression

</rdfs:comment>
      <rdfs:subClassOf>
         <owl:Restriction>
            <owl:cardinality rdf:datatype="http://www.w3.org/2001/XMLSchema#nonNegativeInteger">1</owl:cardinality>
            <owl:onProperty>
               <owl:ObjectProperty rdf:about="http://erlangen-crm.org/efrbroo/R44_carried_out_by"/>
            </owl:onProperty>
         </owl:Restriction>
      </rdfs:subClassOf>
      <rdfs:subClassOf>
         <owl:Restriction>
            <owl:cardinality rdf:datatype="http://www.w3.org/2001/XMLSchema#nonNegativeInteger">1</owl:cardinality>
            <owl:onProperty>
               <owl:ObjectProperty rdf:about="http://erlangen-crm.org/efrbroo/R50_assigned_to"/>
            </owl:onProperty>
         </owl:Restriction>
      </rdfs:subClassOf>
      <rdfs:subClassOf>
         <owl:Restriction>
            <owl:onProperty>
               <owl:ObjectProperty rdf:about="http://erlangen-crm.org/efrbroo/R51_assigned"/>
            </owl:onProperty>
            <owl:minCardinality rdf:datatype="http://www.w3.org/2001/XMLSchema#nonNegativeInteger">1</owl:minCardinality>
         </owl:Restriction>
      </rdfs:subClassOf>
   </owl:Class>
   <!--F43_Identifier_Rule-->
   <owl:Class rdf:about="http://erlangen-crm.org/efrbroo/F43_Identifier_Rule">
      <rdfs:label xml:lang="en">F43 Identifier Rule</rdfs:label>
      <rdfs:subClassOf rdf:resource="http://erlangen-crm.org/current/E29_Design_or_Procedure"/>
      <rdfs:subClassOf rdf:resource="http://erlangen-crm.org/efrbroo/F2_Expression"/>
      <rdfs:comment>Scope note:
This class comprises sets of instructions relating to the formulation of a unique identifier.

</rdfs:comment>
      <rdfs:comment>Examples:
AACR2R 25.25-25.35F1
RAK-Musik (Revidierte Ausgabe 2003), Chapter 6
AFNOR Z 44-079

</rdfs:comment>
   </owl:Class>
   <!--F44_Bibliographic_Agency-->
   <owl:Class rdf:about="http://erlangen-crm.org/efrbroo/F44_Bibliographic_Agency">
      <rdfs:label xml:lang="en">F44 Bibliographic Agency</rdfs:label>
      <rdfs:subClassOf rdf:resource="http://erlangen-crm.org/current/E40_Legal_Body"/>
      <rdfs:comment>Scope note:
This class comprises agents who create the bibliographic description of publications and perform the authority control associated with such descriptions, for the description of copies of such publications actually held by libraries, and for the description of unique documents (manuscripts, objects…) held by libraries.
The activity of creating such descriptions implies that one has to make decisions (as to the controlled access point for a work, as to whether an arrangement still belongs to the same work or is definitely a new work, etc.). Since such decisions always are debatable and different agencies can make different decisions about the same real-world entities, it is important to document which agency made which decision.

</rdfs:comment>
      <rdfs:comment>Examples:
The National Library of France, identified in bibliographic and authority records by the code ‘FRBNF’ at the beginning of INTERMARC field 001
The National Library of Portugal, identified in bibliographic and authority records by the code ‘PTBNP’ at the beginning of UNIMARC field 001
The Beinecke Rare Book and Manuscript Library, Yale University, identified in EAC files through the following elements: &lt;maintenanceAgency&gt; &lt;agencyCode&gt;US-CtY-BR&lt;/agencyCode&gt; &lt;agencyName&gt;Beinecke Rare Book and Manuscript Library, Yale University&lt;/agencyName&gt; &lt;/maintenanceAgency&gt;

</rdfs:comment>
   </owl:Class>
   <!--F50_Controlled_Access_Point-->
   <owl:Class rdf:about="http://erlangen-crm.org/efrbroo/F50_Controlled_Access_Point">
      <rdfs:label xml:lang="en">F50 Controlled Access Point</rdfs:label>
      <rdfs:subClassOf rdf:resource="http://erlangen-crm.org/efrbroo/F13_Identifier"/>
      <rdfs:comment>Scope note:
This class comprises identifiers that are not only designed to be unique for the thing they identify, but also to ensure, by following adequate rules based on widely known and accepted properties for their generation, that an independent agency using the same rule would create the same identifier for the same thing.
F50 Controlled Access Point covers the notion of both “preferred” and “variant” forms. It does not cover the notion of “cross references”. A cross reference may not uniquely identify one entity, but can be shared by two or more entities, regardless of whether it displays the same structural characteristics as preferred controlled access points.

</rdfs:comment>
      <rdfs:comment>Examples:
‘Maxwell equations’ [preferred subject access point from LCSH, http://lccn.loc.gov/sh85082387, as of 19 November 2012]
‘Equations, Maxwell’ [variant subject access point, from the same source]
‘Gončarova, Natalʹâ Sergeevna (1881-1962)’ [preferred access point for a personal name, from the authority file of the National Library of France, http://catalogue.bnf.fr/ark:/12148/cb119547494/PUBLIC, as of 15 June 2012]

‘Гончарова, Наталья Сергеевна (1881-1962)’ [parallel access point from the same source]
‘Goncharova, Natalia (1881-1962)’ [variant access point from the same source]

</rdfs:comment>
   </owl:Class>
   <!--F51_Pursuit-->
   <owl:Class rdf:about="http://erlangen-crm.org/efrbroo/F51_Pursuit">
      <rdfs:label xml:lang="en">F51 Pursuit</rdfs:label>
      <rdfs:subClassOf rdf:resource="http://erlangen-crm.org/current/E7_Activity"/>
      <rdfs:comment>Scope note:
This class comprises periods of continuous activity of an Actor in a specific professional or creative domain or field.

</rdfs:comment>
      <rdfs:comment>Examples:
Natalya Goncharova working as a set and costume designer, painter, illustrator and poet in Russia and France in the first half of the 20th century
Satyajit Ray working as a filmmaker, writer, composer and graphic designer in India in the second half of the 20th century
Folger Shakespeare Library in Washington studying the works of William Shakespeare
M. &amp; N. Hanhart working in lithographic publishing (1839-1882)

</rdfs:comment>
      <rdfs:comment>Properties:
R59 had typical subject (was typical subject of): E1 CRM Entity
R60 used to use language (was language used by): E56 Language
(R60.1 has type of use: E55 Type)

</rdfs:comment>
      <rdfs:subClassOf>
         <owl:Restriction>
            <owl:onProperty>
               <owl:ObjectProperty rdf:about="http://erlangen-crm.org/efrbroo/R59_had_typical_subject"/>
            </owl:onProperty>
            <owl:someValuesFrom rdf:resource="http://erlangen-crm.org/efrbroo/F51_Pursuit"/>
         </owl:Restriction>
      </rdfs:subClassOf>
      <rdfs:subClassOf>
         <owl:Restriction>
            <owl:onProperty>
               <owl:ObjectProperty rdf:about="http://erlangen-crm.org/efrbroo/R60_used_to_use_language"/>
            </owl:onProperty>
            <owl:someValuesFrom rdf:resource="http://erlangen-crm.org/efrbroo/F51_Pursuit"/>
         </owl:Restriction>
      </rdfs:subClassOf>
   </owl:Class>
   <!--F52_Name_Use_Activity-->
   <owl:Class rdf:about="http://erlangen-crm.org/efrbroo/F52_Name_Use_Activity">
      <rdfs:label xml:lang="en">F52 Name Use Activity</rdfs:label>
      <rdfs:subClassOf rdf:resource="http://erlangen-crm.org/current/E13_Attribute_Assignment"/>
      <rdfs:comment>Scope note:
This class comprises periods of continuous use of a specific instance of E41 Appellation for a particular instance of E1 CRM Entity by an E39 Actor. It includes in particular the use of the name by its carrier. Characteristically, actors performing an activity may choose a particular appellation for themselves in the context of this activity. Such cases should be modelled by additionally classifying these activities as instances of F52 Name Use Activity.
It is possible to specify the type of name use, through the P2 has type property, e.g.: use of a pseudonym, use of a married name, use of a birth name, use of a blended name, use of a religious name, etc.

</rdfs:comment>
      <rdfs:comment>Examples:
Using the pseudonym ‘Prince’ until 1993, and again from 2000 on
Using the pseudonym ‘Love Symbol’ from 1993 to 2000
Using the pseudonym ‘Lewis Carroll’ when authoring works of fiction (P2 has type E55 Type {use of a pseudonym})
Using the name ‘Charles Dodgson’ when authoring works of mathematics and logics (P2 has type E55 Type {use of a birth name})
Using the name ‘Mother Teresa’ instead of ‘Agnes Gonxha Bojaxhiu’ when becoming head of the Missionaries of Charity (P2 has type E55 Type {use of a religious name})
Using the name ‘Elizabeth Barrett Browning’ instead of ‘Elizabeth Barrett Barrett’ after marrying Robert Browning (P2 has type E55 Type {use of a married name})
Using the name ‘Antonio Villaraigosa’ instead of ‘Antonio Villar’ after marrying Corina Raigosa (P2 has type E55 Type {use of a blended name}) [comment: when former mayor of Los Angeles Antonio Villar and Corina Raigosa got married in 1987, the two spouses decided they would merge their two last names into one]

</rdfs:comment>
      <rdfs:comment>Properties:
R61 occurred in kind of context (was kind of context for): E55 Type
R62 was used for membership in (was context for): E74 Group
R63 named (was named by): E1 CRM Entity
R64 used name (was name used by): E41 Appellation

</rdfs:comment>
      <rdfs:subClassOf>
         <owl:Restriction>
            <owl:onProperty>
               <owl:ObjectProperty rdf:about="http://erlangen-crm.org/efrbroo/R61_occurred_in_kind_of_context"/>
            </owl:onProperty>
            <owl:someValuesFrom rdf:resource="http://erlangen-crm.org/efrbroo/F52_Name_Use_Activity"/>
         </owl:Restriction>
      </rdfs:subClassOf>
      <rdfs:subClassOf>
         <owl:Restriction>
            <owl:onProperty>
               <owl:ObjectProperty rdf:about="http://erlangen-crm.org/efrbroo/R62_was_used_for_membership_in"/>
            </owl:onProperty>
            <owl:someValuesFrom rdf:resource="http://erlangen-crm.org/efrbroo/F52_Name_Use_Activity"/>
         </owl:Restriction>
      </rdfs:subClassOf>
      <rdfs:subClassOf>
         <owl:Restriction>
            <owl:cardinality rdf:datatype="http://www.w3.org/2001/XMLSchema#nonNegativeInteger">1</owl:cardinality>
            <owl:onProperty>
               <owl:ObjectProperty rdf:about="http://erlangen-crm.org/efrbroo/R63_named"/>
            </owl:onProperty>
         </owl:Restriction>
      </rdfs:subClassOf>
      <rdfs:subClassOf>
         <owl:Restriction>
            <owl:cardinality rdf:datatype="http://www.w3.org/2001/XMLSchema#nonNegativeInteger">1</owl:cardinality>
            <owl:onProperty>
               <owl:ObjectProperty rdf:about="http://erlangen-crm.org/efrbroo/R64_used_name"/>
            </owl:onProperty>
         </owl:Restriction>
      </rdfs:subClassOf>
   </owl:Class>
   <!--F53_Material_Copy-->
   <owl:Class rdf:about="http://erlangen-crm.org/efrbroo/F53_Material_Copy">
      <rdfs:label xml:lang="en">F53 Material Copy</rdfs:label>
      <rdfs:subClassOf rdf:resource="http://erlangen-crm.org/efrbroo/F54_Utilised_Information_Carrier"/>
      <rdfs:subClassOf rdf:resource="http://erlangen-crm.org/current/E25_Man-Made_Feature"/>
      <rdfs:comment>Scope note:
This class comprises the features created on an instance of E84 Information Carrier when an F24 Publication Expression is copied to it by an F32 Carrier Production Event. This is the typical result of an electronic publishing process.

</rdfs:comment>
      <rdfs:comment>Examples:
The physical features created on my PC’s hard drive when I clicked on the link &lt;http://cidoc.ics.forth.gr/docs/cidoc_crm_version_4.0.pdf&gt;, and thus downloaded a reproduction of the electronic file titled ‘Definition of the CIDOC Conceptual Reference Model… version 4.0’ that is stored on the ICS FORTH’s servers in Heraklion, Crete

</rdfs:comment>
   </owl:Class>
   <!--F54_Utilised_Information_Carrier-->
   <owl:Class rdf:about="http://erlangen-crm.org/efrbroo/F54_Utilised_Information_Carrier">
      <rdfs:label xml:lang="en">F54 Utilised Information Carrier</rdfs:label>
      <rdfs:subClassOf rdf:resource="http://erlangen-crm.org/current/E84_Information_Carrier"/>
      <rdfs:superClassOf rdf:resource="http://erlangen-crm.org/efrbroo/F53_Material_Copy"/>
      <rdfs:superClassOf rdf:resource="http://erlangen-crm.org/efrbroo/F5_Item"/>
      <rdfs:comment>Scope note:
This class comprises physical objects that carry one or more instances of F24 Publication Expression.

</rdfs:comment>
      <rdfs:comment>Examples:
The physical features created on my PC’s hard drive when I clicked on the link &lt;http://cidoc.ics.forth.gr/docs/cidoc_crm_version_4.0.pdf&gt;, and thus downloaded a reproduction of the electronic file titled ‘Definition of the CIDOC Conceptual Reference Model… version 4.0’ that is stored on the ICS FORTH’s servers in Heraklion, Crete (F53)
Any copy of the modern reprint publication of Marin Mersenne’s ‘Harmonie universelle’, Paris, 1986, ISBN ‘2-222-00835-2’ (F5)

</rdfs:comment>
      <rdfs:comment>Properties:
R6 carries (is carried by): F24 Publication Expression



</rdfs:comment>
      <rdfs:subClassOf>
         <owl:Restriction>
            <owl:cardinality rdf:datatype="http://www.w3.org/2001/XMLSchema#nonNegativeInteger">1</owl:cardinality>
            <owl:onProperty>
               <owl:ObjectProperty rdf:about="http://erlangen-crm.org/efrbroo/R6_carries"/>
            </owl:onProperty>
         </owl:Restriction>
      </rdfs:subClassOf>
   </owl:Class>
   <!--E1_CRM_Entity-->
   <owl:Class rdf:about="http://erlangen-crm.org/current/E1_CRM_Entity">
      <rdfs:label xml:lang="en">E1 CRM Entity</rdfs:label>
      <rdfs:superClassOf rdf:resource="http://erlangen-crm.org/current/E2_Temporal_Entity"/>
      <rdfs:superClassOf rdf:resource="http://erlangen-crm.org/current/E52_Time-Span"/>
      <rdfs:superClassOf rdf:resource="http://erlangen-crm.org/current/E53_Place"/>
      <rdfs:superClassOf rdf:resource="http://erlangen-crm.org/current/E54_Dimension"/>
      <rdfs:superClassOf rdf:resource="http://erlangen-crm.org/current/E77_Persistent_Item"/>
      <rdfs:comment>Scope note:
This class comprises all things in the universe of discourse of the CIDOC Conceptual Reference Model.

It is an abstract concept providing for three general properties:
Identification by name or appellation, and in particular by a preferred identifier Classification by type, allowing further refinement of the specific subclass an instance belongs to Attachment of free text for the expression of anything not captured by formal properties

With the exception of E59 Primitive Value, all other classes within the CRM are directly or indirectly specialisations of E1 CRM Entity.


</rdfs:comment>
      <rdfs:comment>Examples:

the earthquake in Lisbon 1755 (E5)


</rdfs:comment>
      <rdfs:comment>Properties:

P1 is identified by (identifies): E41 Appellation
P2 has type (is type of): E55 Type
P3 has note: E62 String
(P3.1 has type: E55 Type)
P48 has preferred identifier (is preferred identifier of): E42 Identifier
P137 exemplifies (is exemplified by): E55 Type

</rdfs:comment>
      <rdfs:subClassOf>
         <owl:Restriction>
            <owl:onProperty>
               <owl:ObjectProperty rdf:about="http://erlangen-crm.org/current/P1_is_identified_by"/>
            </owl:onProperty>
            <owl:someValuesFrom rdf:resource="http://erlangen-crm.org/current/E1_CRM_Entity"/>
         </owl:Restriction>
      </rdfs:subClassOf>
      <rdfs:subClassOf>
         <owl:Restriction>
            <owl:onProperty>
               <owl:ObjectProperty rdf:about="http://erlangen-crm.org/current/P2_has_type"/>
            </owl:onProperty>
            <owl:someValuesFrom rdf:resource="http://erlangen-crm.org/current/E1_CRM_Entity"/>
         </owl:Restriction>
      </rdfs:subClassOf>
      <rdfs:subClassOf>
         <owl:Restriction>
            <owl:onProperty>
               <owl:ObjectProperty rdf:about="http://erlangen-crm.org/current/P3_has_note"/>
            </owl:onProperty>
            <owl:someValuesFrom rdf:resource="http://erlangen-crm.org/current/E1_CRM_Entity"/>
         </owl:Restriction>
      </rdfs:subClassOf>
   </owl:Class>
   <!--E2_Temporal_Entity-->
   <owl:Class rdf:about="http://erlangen-crm.org/current/E2_Temporal_Entity">
      <rdfs:label xml:lang="en">E2 Temporal Entity</rdfs:label>
      <rdfs:subClassOf rdf:resource="http://erlangen-crm.org/current/E1_CRM_Entity"/>
      <rdfs:superClassOf rdf:resource="http://erlangen-crm.org/current/Ε3_Condition_State"/>
      <rdfs:superClassOf rdf:resource="http://erlangen-crm.org/current/E4_Period"/>
      <rdfs:comment>Scope note:
This class comprises all phenomena, such as the instances of E4 Periods, E5 Events and states, which happen over a limited extent in time.

In some contexts, these are also called perdurants. This class is disjoint from E77 Persistent Item. This is an abstract class and has no direct instances. E2 Temporal Entity is specialized into E4 Period, which applies to a particular geographic area (defined with a greater or lesser degree of precision), and E3 Condition State, which applies to instances of E18 Physical Thing.

</rdfs:comment>
      <rdfs:comment>Examples:

Bronze Age (E4) the earthquake in Lisbon 1755 (E5) the Peterhof Palace near Saint Petersburg being in ruins from 1944 – 1946 (E3)

</rdfs:comment>
      <rdfs:comment>Properties:

P4 has time-span (is time-span of): E52 Time-Span
P114 is equal in time to: E2 Temporal Entity
P115 finishes (is finished by): E2 Temporal Entity
P116 starts (is started by): E2 Temporal Entity
P117 occurs during (includes): E2 Temporal Entity
P118 overlaps in time with (is overlapped in time by): E2 Temporal Entity
P119 meets in time with (is met in time by): E2 Temporal Entity
P120 occurs before (occurs after): E2 Temporal Entity

</rdfs:comment>
      <rdfs:subClassOf>
         <owl:Restriction>
            <owl:cardinality rdf:datatype="http://www.w3.org/2001/XMLSchema#nonNegativeInteger">1</owl:cardinality>
            <owl:onProperty>
               <owl:ObjectProperty rdf:about="http://erlangen-crm.org/current/P4_has_time-span"/>
            </owl:onProperty>
         </owl:Restriction>
      </rdfs:subClassOf>
   </owl:Class>
   <!--E3_Condition_State-->
   <owl:Class rdf:about="http://erlangen-crm.org/current/E3_Condition_State">
      <rdfs:label xml:lang="en">E3 Condition State</rdfs:label>
      <rdfs:subClassOf rdf:resource="http://erlangen-crm.org/current/E2_Temporal_Entity"/>
      <rdfs:comment>Scope note:
This class comprises the states of objects characterised by a certain condition over a time-span.
An instance of this class describes the prevailing physical condition of any material object or feature during a specific E52 Time Span. In general, the time-span for which a certain condition can be asserted may be shorter than the real time-span, for which this condition held.
The nature of that condition can be described using P2 has type. For example, the E3 Condition State “condition of the SS Great Britain between 22 September 1846 and 27 August 1847” can be characterized as E55 Type “wrecked”.

</rdfs:comment>
      <rdfs:comment>Examples:

the “Amber Room” in Tsarskoje Selo being completely reconstructed from summer 2003 until now the Peterhof Palace near Saint Petersburg being in ruins from 1944 – 1946 the state of my turkey in the oven at 14:30 on 25 December, 2002 (P2 has type: E55 Type “still not cooked”)

</rdfs:comment>
      <rdfs:comment>Properties:

P5 consists of (forms part of): E3 Condition State

</rdfs:comment>
   </owl:Class>
   <!--E4_Period-->
   <owl:Class rdf:about="http://erlangen-crm.org/current/E4_Period">
      <rdfs:label xml:lang="en">E4 Period</rdfs:label>
      <rdfs:subClassOf rdf:resource="http://erlangen-crm.org/current/E2_Temporal_Entity"/>
      <rdfs:superClassOf rdf:resource="http://erlangen-crm.org/current/E5_Event"/>
      <rdfs:comment>Scope note:
This class comprises sets of coherent phenomena or cultural manifestations bounded in time and space.
It is the social or physical coherence of these phenomena that identify an E4 Period and not the associated spatio-temporal bounds. These bounds are a mere approximation of the actual process of growth, spread and retreat. Consequently, different periods can overlap and coexist in time and space, such as when a nomadic culture exists in the same area as a sedentary culture.
Typically this class is used to describe prehistoric or historic periods such as the “Neolithic Period”, the “Ming Dynasty” or the “McCarthy Era”. There are however no assumptions about the scale of the associated phenomena. In particular all events are seen as synthetic processes consisting of coherent phenomena. Therefore E4 Period is a superclass of E5 Event. For example, a modern clinical E67 Birth can be seen as both an atomic E5 Event and as an E4 Period that consists of multiple activities performed by multiple instances of E39 Actor.
There are two different conceptualisations of ‘artistic style’, defined either by physical features or by historical context. For example, “Impressionism” can be viewed as a period lasting from approximately 1870 to 1905 during which paintings with particular characteristics were produced by a group of artists that included (among others) Monet, Renoir, Pissarro, Sisley and Degas. Alternatively, it can be regarded as a style applicable to all paintings sharing the characteristics of the works produced by the Impressionist painters, regardless of historical context. The first interpretation is an E4 Period, and the second defines morphological object types that fall under E55 Type.
Another specific case of an E4 Period is the set of activities and phenomena associated with a settlement, such as the populated period of Nineveh.

</rdfs:comment>
      <rdfs:comment>Examples:

Jurassic European Bronze Age Italian Renaissance Thirty Years War Sturm und Drang Cubism

</rdfs:comment>
      <rdfs:comment>Properties:

P7 took place at (witnessed): E53 Place
P8 took place on or within (witnessed): E19 Physical Object
P9 consists of (forms part of): E4 Period
P10 falls within (contains): E4 Period
P132 overlaps with: E4 Period
P133 is separated from: E4 Period

</rdfs:comment>
      <rdfs:subClassOf>
         <owl:Restriction>
            <owl:onProperty>
               <owl:ObjectProperty rdf:about="http://erlangen-crm.org/current/P7_took_place_at"/>
            </owl:onProperty>
            <owl:minCardinality rdf:datatype="http://www.w3.org/2001/XMLSchema#nonNegativeInteger">1</owl:minCardinality>
         </owl:Restriction>
      </rdfs:subClassOf>
      <rdfs:subClassOf>
         <owl:Restriction>
            <owl:onProperty>
               <owl:ObjectProperty rdf:about="http://erlangen-crm.org/current/P9_consists_of"/>
            </owl:onProperty>
            <owl:someValuesFrom rdf:resource="http://erlangen-crm.org/current/E4_Period"/>
         </owl:Restriction>
      </rdfs:subClassOf>
   </owl:Class>
   <!--E5_Event-->
   <owl:Class rdf:about="http://erlangen-crm.org/current/E5_Event">
      <rdfs:label xml:lang="en">E5 Event</rdfs:label>
      <rdfs:subClassOf rdf:resource="http://erlangen-crm.org/current/E4_Period"/>
      <rdfs:superClassOf rdf:resource="http://erlangen-crm.org/current/E7_Activity"/>
      <rdfs:superClassOf rdf:resource="http://erlangen-crm.org/current/E63_Beginning_of_Existence"/>
      <rdfs:superClassOf rdf:resource="http://erlangen-crm.org/current/E64_End_of_Existence"/>
      <rdfs:comment>Scope note:
This class comprises changes of states in cultural, social or physical systems, regardless of scale, brought about by a series or group of coherent physical, cultural, technological or legal phenomena. Such changes of state will affect instances of E77 Persistent Item or its subclasses.
The distinction between an E5 Event and an E4 Period is partly a question of the scale of observation. Viewed at a coarse level of detail, an E5 Event is an ‘instantaneous’ change of state. At a fine level, the E5 Event can be analysed into its component phenomena within a space and time frame, and as such can be seen as an E4 Period. The reverse is not necessarily the case: not all instances of E4 Period give rise to a noteworthy change of state.

</rdfs:comment>
      <rdfs:comment>Examples:

the birth of Cleopatra (E67) the destruction of Herculaneum by volcanic eruption in 79 AD (E6) World War II (E7) the Battle of Stalingrad (E7) the Yalta Conference (E7) my birthday celebration 28-6-1995 (E7) the falling of a tile from my roof last Sunday the CIDOC Conference 2003 (E7)

</rdfs:comment>
      <rdfs:comment>Properties:

P11 had participant (participated in): E39 Actor
P12 occurred in the presence of (was present at): E77 Persistent Item

</rdfs:comment>
      <rdfs:subClassOf>
         <owl:Restriction>
            <owl:onProperty>
               <owl:ObjectProperty rdf:about="http://erlangen-crm.org/current/P12_occurred_in_the_presence_of"/>
            </owl:onProperty>
            <owl:minCardinality rdf:datatype="http://www.w3.org/2001/XMLSchema#nonNegativeInteger">1</owl:minCardinality>
         </owl:Restriction>
      </rdfs:subClassOf>
   </owl:Class>
   <!--E7_Activity-->
   <owl:Class rdf:about="http://erlangen-crm.org/current/E7_Activity">
      <rdfs:label xml:lang="en">E7 Activity</rdfs:label>
      <rdfs:subClassOf rdf:resource="http://erlangen-crm.org/current/E5_Event"/>
      <rdfs:superClassOf rdf:resource="http://erlangen-crm.org/current/E8_Acquisition"/>
      <rdfs:superClassOf rdf:resource="http://erlangen-crm.org/current/E9_Move"/>
      <rdfs:superClassOf rdf:resource="http://erlangen-crm.org/current/E10_Transfer_of_Custody"/>
      <rdfs:superClassOf rdf:resource="http://erlangen-crm.org/current/E11_Modification"/>
      <rdfs:superClassOf rdf:resource="http://erlangen-crm.org/current/E13_Attribute_Assignment"/>
      <rdfs:superClassOf rdf:resource="http://erlangen-crm.org/current/E65_Creation"/>
      <rdfs:superClassOf rdf:resource="http://erlangen-crm.org/current/E66_Formation"/>
      <rdfs:superClassOf rdf:resource="http://erlangen-crm.org/current/E85_Joining"/>
      <rdfs:superClassOf rdf:resource="http://erlangen-crm.org/current/E86_Leaving"/>
      <rdfs:superClassOf rdf:resource="http://erlangen-crm.org/current/E87_Curation_Activity"/>
      <rdfs:comment>Scope note:
This class comprises actions intentionally carried out by instances of E39 Actor that result in changes of state in the cultural, social, or physical systems documented.
This notion includes complex, composite and long-lasting actions such as the building of a settlement or a war, as well as simple, short-lived actions such as the opening of a door.

</rdfs:comment>
      <rdfs:comment>Examples:

the Battle of Stalingrad the Yalta Conference my birthday celebration 28-6-1995 the writing of “Faust” by Goethe (E65) the formation of the Bauhaus 1919 (E66) calling the place identified by TGN ‘7017998’ ‘Quyunjig’ by the people of Iraq

</rdfs:comment>
      <rdfs:comment>Properties:

P14 carried out by (performed): E39 Actor
(P14.1 in the role of: E55 Type)
P15 was influenced by (influenced): E1 CRM Entity
P16 used specific object (was used for): E70 Thing
(P16.1 mode of use: E55 Type)
P17 was motivated by (motivated): E1 CRM Entity
P19 was intended use of (was made for): E71 Man-Made Thing
(P19.1 mode of use: E55 Type)
P20 had specific purpose (was purpose of): E5 Event
P21 had general purpose (was purpose of): E55 Type
P32 used general technique (was technique of): E55 Type
P33 used specific technique (was used by): E29 Design or Procedure
P125 used object of type (was type of object used in): E55 Type
P134 continued (was continued by): E7 Activity

</rdfs:comment>
      <rdfs:subClassOf>
         <owl:Restriction>
            <owl:onProperty>
               <owl:ObjectProperty rdf:about="http://erlangen-crm.org/current/P14_carried_out_by"/>
            </owl:onProperty>
            <owl:minCardinality rdf:datatype="http://www.w3.org/2001/XMLSchema#nonNegativeInteger">1</owl:minCardinality>
         </owl:Restriction>
      </rdfs:subClassOf>
      <rdfs:subClassOf>
         <owl:Restriction>
            <owl:onProperty>
               <owl:ObjectProperty rdf:about="http://erlangen-crm.org/current/P15_was_influenced_by"/>
            </owl:onProperty>
            <owl:someValuesFrom rdf:resource="http://erlangen-crm.org/current/E7_Activity"/>
         </owl:Restriction>
      </rdfs:subClassOf>
      <rdfs:subClassOf>
         <owl:Restriction>
            <owl:onProperty>
               <owl:ObjectProperty rdf:about="http://erlangen-crm.org/current/P16_used_specific_object"/>
            </owl:onProperty>
            <owl:someValuesFrom rdf:resource="http://erlangen-crm.org/current/E7_Activity"/>
         </owl:Restriction>
      </rdfs:subClassOf>
      <rdfs:subClassOf>
         <owl:Restriction>
            <owl:onProperty>
               <owl:ObjectProperty rdf:about="http://erlangen-crm.org/current/P33_used_specific_technique"/>
            </owl:onProperty>
            <owl:someValuesFrom rdf:resource="http://erlangen-crm.org/current/E7_Activity"/>
         </owl:Restriction>
      </rdfs:subClassOf>
      <rdfs:subClassOf>
         <owl:Restriction>
            <owl:onProperty>
               <owl:ObjectProperty rdf:about="http://erlangen-crm.org/current/P125_used_object_of_type"/>
            </owl:onProperty>
            <owl:someValuesFrom rdf:resource="http://erlangen-crm.org/current/E7_Activity"/>
         </owl:Restriction>
      </rdfs:subClassOf>
   </owl:Class>
   <!--E11_Modification-->
   <owl:Class rdf:about="http://erlangen-crm.org/current/E11_Modification">
      <rdfs:label xml:lang="en">E11 Modification</rdfs:label>
      <rdfs:subClassOf rdf:resource="http://erlangen-crm.org/current/E7_Activity"/>
      <rdfs:superClassOf rdf:resource="http://erlangen-crm.org/current/E12_Production"/>
      <rdfs:superClassOf rdf:resource="http://erlangen-crm.org/current/E79_Part_Addition"/>
      <rdfs:superClassOf rdf:resource="http://erlangen-crm.org/current/E80_Part_Removal"/>
      <rdfs:comment>Scope note:
This class comprises all instances of E7 Activity that create, alter or change E24 Physical Man-Made Thing.
This class includes the production of an item from raw materials, and other so far undocumented objects, and the preventive treatment or restoration of an object for conservation.
Since the distinction between modification and production is not always clear, modification is regarded as the more generally applicable concept. This implies that some items may be consumed or destroyed in a Modification, and that others may be produced as a result of it. An event should also be documented using E81 Transformation if it results in the destruction of one or more objects and the simultaneous production of others using parts or material from the originals. In this case, the new items have separate identities.
If the instance of the E29 Design or Procedure utilized for the modification prescribes the use of specific materials, they should be documented using property P68 foresees use of (use foreseen by): E57 Material of E29 Design or Procedure, rather than via P126 employed (was employed in): E57 Material.

</rdfs:comment>
      <rdfs:comment>Examples:

the construction of the SS Great Britain (E12) the impregnation of the Vasa warship in Stockholm for preservation after 1956 the transformation of the Enola Gay into a museum exhibit by the National Air and Space Museum in Washington DC between 1993 and 1995 (E12, E81) the last renewal of the gold coating of the Toshogu shrine in Nikko, Japan

</rdfs:comment>
      <rdfs:comment>Properties:

P31 has modified (was modified by): E24 Physical Man-Made Thing
P126 employed (was employed in): E57 Material

</rdfs:comment>
      <rdfs:subClassOf>
         <owl:Restriction>
            <owl:onProperty>
               <owl:ObjectProperty rdf:about="http://erlangen-crm.org/current/P31_has_modified"/>
            </owl:onProperty>
            <owl:minCardinality rdf:datatype="http://www.w3.org/2001/XMLSchema#nonNegativeInteger">1</owl:minCardinality>
         </owl:Restriction>
      </rdfs:subClassOf>
   </owl:Class>
   <!--E12_Production-->
   <owl:Class rdf:about="http://erlangen-crm.org/current/E12_Production">
      <rdfs:label xml:lang="en">E12 Production</rdfs:label>
      <rdfs:subClassOf rdf:resource="http://erlangen-crm.org/current/E11_Modification"/>
      <rdfs:subClassOf rdf:resource="http://erlangen-crm.org/current/E63_Beginning_of_Existence"/>
      <rdfs:comment>Scope note:
This class comprises activities that are designed to, and succeed in, creating one or more new items.
It specializes the notion of modification into production. The decision as to whether or not an object is regarded as new is context sensitive. Normally, items are considered “new” if there is no obvious overall similarity between them and the consumed items and material used in their production. In other cases, an item is considered “new” because it becomes relevant to documentation by a modification. For example, the scribbling of a name on a potsherd may make it a voting token. The original potsherd may not be worth documenting, in contrast to the inscribed one.
This entity can be collective: the printing of a thousand books, for example, would normally be considered a single event.
An event should also be documented using E81 Transformation if it results in the destruction of one or more objects and the simultaneous production of others using parts or material from the originals. In this case, the new items have separate identities and matter is preserved, but identity is not.

</rdfs:comment>
      <rdfs:comment>Examples:

the construction of the SS Great Britain the first casting of the Little Mermaid from the harbour of Copenhagen Rembrandt’s creating of the seventh state of his etching “Woman sitting half dressed beside a stove”, 1658, identified by Bartsch Number 197 (E12,E65,E81)

</rdfs:comment>
      <rdfs:comment>Properties:

P108 has produced (was produced by): E24 Physical Man-Made Thing

</rdfs:comment>
      <rdfs:subClassOf>
         <owl:Restriction>
            <owl:onProperty>
               <owl:ObjectProperty rdf:about="http://erlangen-crm.org/current/P108_has_produced"/>
            </owl:onProperty>
            <owl:minCardinality rdf:datatype="http://www.w3.org/2001/XMLSchema#nonNegativeInteger">1</owl:minCardinality>
         </owl:Restriction>
      </rdfs:subClassOf>
   </owl:Class>
   <!--E13_Attribute_Assignment-->
   <owl:Class rdf:about="http://erlangen-crm.org/current/E13_Attribute_Assignment">
      <rdfs:label xml:lang="en">E13 Attribute Assignment</rdfs:label>
      <rdfs:subClassOf rdf:resource="http://erlangen-crm.org/current/E7_Activity"/>
      <rdfs:superClassOf rdf:resource="http://erlangen-crm.org/current/E14_Condition_Assessment"/>
      <rdfs:superClassOf rdf:resource="http://erlangen-crm.org/current/E15_Identifier_Assignment"/>
      <rdfs:superClassOf rdf:resource="http://erlangen-crm.org/current/E16_Measurement"/>
      <rdfs:superClassOf rdf:resource="http://erlangen-crm.org/current/E17_Type_Assignment"/>
      <rdfs:comment>Scope note:
This class comprises the actions of making assertions about properties of an object or any relation between two items or concepts.
This class allows the documentation of how the respective assignment came about, and whose opinion it was. All the attributes or properties assigned in such an action can also be seen as directly attached to the respective item or concept, possibly as a collection of contradictory values. All cases of properties in this model that are also described indirectly through an action are characterised as “shortcuts” of this action. This redundant modelling of two alternative views is preferred because many implementations may have good reasons to model either the action or the shortcut, and the relation between both alternatives can be captured by simple rules.
In particular, the class describes the actions of people making propositions and statements during certain museum procedures, e.g. the person and date when a condition statement was made, an identifier was assigned, the museum object was measured, etc. Which kinds of such assignments and statements need to be documented explicitly in structures of a schema rather than free text, depends on if this information should be accessible by structured queries.

</rdfs:comment>
      <rdfs:comment>Examples:

the assessment of the current ownership of Martin Doerr’s silver cup in February 1997

</rdfs:comment>
      <rdfs:comment>Properties:

P140 assigned attribute to (was attributed by): E1 CRM Entity
P141 assigned (was assigned by): E1 CRM Entity

</rdfs:comment>
      <rdfs:subClassOf>
         <owl:Restriction>
            <owl:onProperty>
               <owl:ObjectProperty rdf:about="http://erlangen-crm.org/current/P140_assigned_attribute_to"/>
            </owl:onProperty>
            <owl:someValuesFrom rdf:resource="http://erlangen-crm.org/current/E13_Attribute_Assignment"/>
         </owl:Restriction>
      </rdfs:subClassOf>
      <rdfs:subClassOf>
         <owl:Restriction>
            <owl:onProperty>
               <owl:ObjectProperty rdf:about="http://erlangen-crm.org/current/P141_assigned"/>
            </owl:onProperty>
            <owl:someValuesFrom rdf:resource="http://erlangen-crm.org/current/E13_Attribute_Assignment"/>
         </owl:Restriction>
      </rdfs:subClassOf>
   </owl:Class>
   <!--E15_Identifier_Assignment-->
   <owl:Class rdf:about="http://erlangen-crm.org/current/E15_Identifier_Assignment">
      <rdfs:label xml:lang="en">E15 Identifier Assignment</rdfs:label>
      <rdfs:subClassOf rdf:resource="http://erlangen-crm.org/current/E13_Attribute_Assignment"/>
      <rdfs:comment>Scope note:
This class comprises activities that result in the allocation of an identifier to an instance of E1 CRM Entity. An E15 Identifier Assignment may include the creation of the identifier from multiple constituents, which themselves may be instances of E41 Appellation. The syntax and kinds of constituents to be used may be declared in a rule constituting an instance of E29 Design or Procedure.

Examples of such identifiers include Find Numbers, Inventory Numbers, uniform titles in the sense of librarianship and Digital Object Identifiers (DOI). Documenting the act of identifier assignment and deassignment is especially useful when objects change custody or the identification system of an organization is changed. In order to keep track of the identity of things in such cases, it is important to document by whom, when and for what purpose an identifier is assigned to an item.


The fact that an identifier is a preferred one for an organisation can be expressed by using the property E1 CRM Entity. P48 has preferred identifier (is preferred identifier of): E42 Identifier. It can better be expressed in a context independent form by assigning a suitable E55 Type, such as “preferred identifier assignment”, to the respective instance of E15 Identifier Assignment via the P2 has type property.

</rdfs:comment>
      <rdfs:comment>Examples:

Replacement of the inventory number TA959a by GE34604 for a 17th century lament cloth at the Museum Benaki, Athens Assigning the author-uniform title heading “Goethe, Johann Wolfgang von, 1749-1832. Faust. 1. Theil.” for a work (E28) On June 1, 2001 assigning the personal name heading “Guillaume, de Machaut, ca. 1300-1377” (E42,E82) to Guillaume de Machaut (E21)

</rdfs:comment>
      <rdfs:comment>Properties:

P37 assigned (was assigned by): E42 Identifier
P38 deassigned (was deassigned by): E42 Identifier
P142 used constituent (was used in): E90 Symbolic Object

</rdfs:comment>
      <rdfs:subClassOf>
         <owl:Restriction>
            <owl:onProperty>
               <owl:ObjectProperty rdf:about="http://erlangen-crm.org/current/P37_assigned"/>
            </owl:onProperty>
            <owl:someValuesFrom rdf:resource="http://erlangen-crm.org/current/E15_Identifier_Assignment"/>
         </owl:Restriction>
      </rdfs:subClassOf>
      <rdfs:subClassOf>
         <owl:Restriction>
            <owl:onProperty>
               <owl:ObjectProperty rdf:about="http://erlangen-crm.org/current/P142_used_constituent"/>
            </owl:onProperty>
            <owl:someValuesFrom rdf:resource="http://erlangen-crm.org/current/E15_Identifier_Assignment"/>
         </owl:Restriction>
      </rdfs:subClassOf>
   </owl:Class>
   <!--E18_Physical_Thing-->
   <owl:Class rdf:about="http://erlangen-crm.org/current/E18_Physical_Thing">
      <rdfs:label xml:lang="en">E18 Physical Thing</rdfs:label>
      <rdfs:subClassOf rdf:resource="http://erlangen-crm.org/current/E72_Legal_Object"/>
      <rdfs:superClassOf rdf:resource="http://erlangen-crm.org/current/E19_Physical_Object"/>
      <rdfs:superClassOf rdf:resource="http://erlangen-crm.org/current/E24_Physical_Man-Made_Thing"/>
      <rdfs:superClassOf rdf:resource="http://erlangen-crm.org/current/E26_Physical_Feature"/>
      <rdfs:comment>Scope note:
This class comprises all persistent physical items with a relatively stable form, man-made or natural.
Depending on the existence of natural boundaries of such things, the CRM distinguishes the instances of E19 Physical Object from instances of E26 Physical Feature, such as holes, rivers, pieces of land etc. Most instances of E19 Physical Object can be moved (if not too heavy), whereas features are integral to the surrounding matter.
The CRM is generally not concerned with amounts of matter in fluid or gaseous states.

</rdfs:comment>
      <rdfs:comment>Examples:

the Cullinan Diamond (E19) the cave “Ideon Andron” in Crete (E26) the Mona Lisa (E22)

</rdfs:comment>
      <rdfs:comment>Properties:

P44 has condition (condition of): E3 Condition State
P45 consists of (is incorporated in): E57 Material
P46 is composed of (forms part of): E18 Physical Thing
P49 has former or current keeper (is former or current keeper of): E39 Actor
P50 has current keeper (is current keeper of): E39 Actor
P51 has former or current owner (is former or current owner of): E39 Actor
P52 has current owner (is current owner of): E39 Actor
P53 has former or current location (is former or current location of): E53 Place
P58 has section definition (defines section): E46 Section Definition
P59 has section (is located on or within): E53 Place

</rdfs:comment>
      <rdfs:subClassOf>
         <owl:Restriction>
            <owl:onProperty>
               <owl:ObjectProperty rdf:about="http://erlangen-crm.org/current/P45_consists_of"/>
            </owl:onProperty>
            <owl:minCardinality rdf:datatype="http://www.w3.org/2001/XMLSchema#nonNegativeInteger">1</owl:minCardinality>
         </owl:Restriction>
      </rdfs:subClassOf>
      <rdfs:subClassOf>
         <owl:Restriction>
            <owl:onProperty>
               <owl:ObjectProperty rdf:about="http://erlangen-crm.org/current/P46_is_composed_of"/>
            </owl:onProperty>
            <owl:someValuesFrom rdf:resource="http://erlangen-crm.org/current/E18_Physical_Thing"/>
         </owl:Restriction>
      </rdfs:subClassOf>
      <rdfs:subClassOf>
         <owl:Restriction>
            <owl:onProperty>
               <owl:ObjectProperty rdf:about="http://erlangen-crm.org/current/P49_has_former_or_current_keeper"/>
            </owl:onProperty>
            <owl:someValuesFrom rdf:resource="http://erlangen-crm.org/current/E18_Physical_Thing"/>
         </owl:Restriction>
      </rdfs:subClassOf>
      <rdfs:subClassOf>
         <owl:Restriction>
            <owl:onProperty>
               <owl:ObjectProperty rdf:about="http://erlangen-crm.org/current/P50_has_current_keeper"/>
            </owl:onProperty>
            <owl:someValuesFrom rdf:resource="http://erlangen-crm.org/current/E18_Physical_Thing"/>
         </owl:Restriction>
      </rdfs:subClassOf>
      <rdfs:subClassOf>
         <owl:Restriction>
            <owl:onProperty>
               <owl:ObjectProperty rdf:about="http://erlangen-crm.org/current/P51_has_former_or_current_owner"/>
            </owl:onProperty>
            <owl:someValuesFrom rdf:resource="http://erlangen-crm.org/current/E18_Physical_Thing"/>
         </owl:Restriction>
      </rdfs:subClassOf>
      <rdfs:subClassOf>
         <owl:Restriction>
            <owl:onProperty>
               <owl:ObjectProperty rdf:about="http://erlangen-crm.org/current/P59_has_section"/>
            </owl:onProperty>
            <owl:someValuesFrom rdf:resource="http://erlangen-crm.org/current/E18_Physical_Thing"/>
         </owl:Restriction>
      </rdfs:subClassOf>
   </owl:Class>
   <!--E19_Physical_Object-->
   <owl:Class rdf:about="http://erlangen-crm.org/current/E19_Physical_Object">
      <rdfs:label xml:lang="en">E19 Physical Object</rdfs:label>
      <rdfs:subClassOf rdf:resource="http://erlangen-crm.org/current/E18_Physical_Thing"/>
      <rdfs:superClassOf rdf:resource="http://erlangen-crm.org/current/E20_Biological_Object"/>
      <rdfs:superClassOf rdf:resource="http://erlangen-crm.org/current/E22_Man-Made_Object"/>
      <rdfs:comment>Scope note:
This class comprises items of a material nature that are units for documentation and have physical boundaries that separate them completely in an objective way from other objects.

The class also includes all aggregates of objects made for functional purposes of whatever kind, independent of physical coherence, such as a set of chessmen. Typically, instances of E19 Physical Object can be moved (if not too heavy).

In some contexts, such objects, except for aggregates, are also called “bona fide objects” (Smith &amp; Varzi, 2000, pp.401-420), i.e. naturally defined objects.

The decision as to what is documented as a complete item, rather than by its parts or components, may be a purely administrative decision or may be a result of the order in which the item was acquired.

</rdfs:comment>
      <rdfs:comment>Examples:

John Smith Aphrodite of Milos the Palace of Knossos the Cullinan Diamond Apollo 13 at the time of launch

</rdfs:comment>
      <rdfs:comment>Properties:

P54 has current permanent location (is current permanent location of): E53 Place
P55 has current location (currently holds): E53 Place
P56 bears feature (is found on): E26 Physical Feature
P57 has number of parts: E60 Number

</rdfs:comment>
      <rdfs:subClassOf>
         <owl:Restriction>
            <owl:onProperty>
               <owl:ObjectProperty rdf:about="http://erlangen-crm.org/current/P57_has_number_of_parts"/>
            </owl:onProperty>
            <owl:maxCardinality rdf:datatype="http://www.w3.org/2001/XMLSchema#nonNegativeInteger">1</owl:maxCardinality>
         </owl:Restriction>
      </rdfs:subClassOf>
   </owl:Class>
   <!--E21_Person-->
   <owl:Class rdf:about="http://erlangen-crm.org/current/E21_Person">
      <rdfs:label xml:lang="en">E21 Person</rdfs:label>
      <rdfs:subClassOf rdf:resource="http://erlangen-crm.org/current/E20_Biological_Object"/>
      <rdfs:subClassOf rdf:resource="http://erlangen-crm.org/current/E39_Actor"/>
      <rdfs:comment>Scope note:
This class comprises real persons who live or are assumed to have lived.
Legendary figures that may have existed, such as Ulysses and King Arthur, fall into this class if the documentation refers to them as historical figures. In cases where doubt exists as to whether several persons are in fact identical, multiple instances can be created and linked to indicate their relationship. The CRM does not propose a specific form to support reasoning about possible identity.

</rdfs:comment>
      <rdfs:comment>Examples:

Tut-Ankh-Amun Nelson Mandela

</rdfs:comment>
   </owl:Class>
   <!--E22_Man-Made_Object-->
   <owl:Class rdf:about="http://erlangen-crm.org/current/E22_Man-Made_Object">
      <rdfs:label xml:lang="en">E22 Man-Made Object</rdfs:label>
      <rdfs:subClassOf rdf:resource="http://erlangen-crm.org/current/E19_Physical_Object"/>
      <rdfs:subClassOf rdf:resource="http://erlangen-crm.org/current/E24_Physical_Man-Made_Thing"/>
      <rdfs:superClassOf rdf:resource="http://erlangen-crm.org/current/E84_Information_Carrier"/>
      <rdfs:comment>Scope note:
This class comprises physical objects purposely created by human activity.


No assumptions are made as to the extent of modification required to justify regarding an object as man-made. For example, an inscribed piece of rock or a preserved butterfly are both regarded as instances of E22 Man-Made Object.

</rdfs:comment>
      <rdfs:comment>Examples:

Mallard (the World’s fastest steam engine) the Portland Vase the Coliseum

</rdfs:comment>
   </owl:Class>
   <!--E24_Physical_Man-Made_Thing-->
   <owl:Class rdf:about="http://erlangen-crm.org/current/E24_Physical_Man-Made_Thing">
      <rdfs:label xml:lang="en">E24 Physical Man-Made Thing</rdfs:label>
      <rdfs:subClassOf rdf:resource="http://erlangen-crm.org/current/E18_Physical_Thing"/>
      <rdfs:subClassOf rdf:resource="http://erlangen-crm.org/current/E71_Man-Made_Thing"/>
      <rdfs:superClassOf rdf:resource="http://erlangen-crm.org/current/E22_Man-Made_Object"/>
      <rdfs:superClassOf rdf:resource="http://erlangen-crm.org/current/E25_Man-Made_Feature"/>
      <rdfs:superClassOf rdf:resource="http://erlangen-crm.org/current/E78_Collection"/>
      <rdfs:comment>Scope note:
This class comprises all persistent physical items that are purposely created by human activity.
This class comprises man-made objects, such as a swords, and man-made features, such as rock art. No assumptions are made as to the extent of modification required to justify regarding an object as man-made. For example, a “cup and ring” carving on bedrock is regarded as instance of E24 Physical Man-Made Thing.

</rdfs:comment>
      <rdfs:comment>Examples:

the Forth Railway Bridge (E22) the Channel Tunnel (E25) the Historical Collection of the Museum Benaki in Athens (E78)

</rdfs:comment>
      <rdfs:comment>Properties:

P62 depicts (is depicted by): E1 CRM Entity
(P62.1 mode of depiction: E55 Type)
P65 shows visual item (is shown by): E36 Visual Item
P128 carries (is carried by): E73 Information Object

</rdfs:comment>
      <rdfs:subClassOf>
         <owl:Restriction>
            <owl:onProperty>
               <owl:ObjectProperty rdf:about="http://erlangen-crm.org/current/P65_shows_visual_item"/>
            </owl:onProperty>
            <owl:someValuesFrom rdf:resource="http://erlangen-crm.org/current/E24_Physical_Man-Made_Thing"/>
         </owl:Restriction>
      </rdfs:subClassOf>
      <rdfs:subClassOf>
         <owl:Restriction>
            <owl:onProperty>
               <owl:ObjectProperty rdf:about="http://erlangen-crm.org/current/P128_carries"/>
            </owl:onProperty>
            <owl:someValuesFrom rdf:resource="http://erlangen-crm.org/current/E24_Physical_Man-Made_Thing"/>
         </owl:Restriction>
      </rdfs:subClassOf>
   </owl:Class>
   <!--E25_Man-Made_Feature-->
   <owl:Class rdf:about="http://erlangen-crm.org/current/E25_Man-Made_Feature">
      <rdfs:label xml:lang="en">E25 Man-Made Feature</rdfs:label>
      <rdfs:subClassOf rdf:resource="http://erlangen-crm.org/current/E24_Physical_Man-Made_Thing"/>
      <rdfs:subClassOf rdf:resource="http://erlangen-crm.org/current/E26_Physical_Feature"/>
      <rdfs:comment>Scope note:
This class comprises physical features that are purposely created by human activity, such as scratches, artificial caves, artificial water channels, etc.

No assumptions are made as to the extent of modification required to justify regarding a feature as man-made. For example, rock art or even “cup and ring” carvings on bedrock a regarded as types of E25 Man-Made Feature.

</rdfs:comment>
      <rdfs:comment>Examples:

the Manchester Ship Canal Michael Jackson’s nose following plastic surgery

</rdfs:comment>
   </owl:Class>
   <!--E26_Physical_Feature-->
   <owl:Class rdf:about="http://erlangen-crm.org/current/E26_Physical_Feature">
      <rdfs:label xml:lang="en">E26 Physical Feature</rdfs:label>
      <rdfs:subClassOf rdf:resource="http://erlangen-crm.org/current/E18_Physical_Thing"/>
      <rdfs:superClassOf rdf:resource="http://erlangen-crm.org/current/E25_Man-Made_Feature"/>
      <rdfs:superClassOf rdf:resource="http://erlangen-crm.org/current/E27_Site"/>
      <rdfs:comment>Scope note:
This class comprises identifiable features that are physically attached in an integral way to particular physical objects.

Instances of E26 Physical Feature share many of the attributes of instances of E19 Physical Object. They may have a one-, two- or three-dimensional geometric extent, but there are no natural borders that separate them completely in an objective way from the carrier objects. For example, a doorway is a feature but the door itself, being attached by hinges, is not.

Instances of E26 Physical Feature can be features in a narrower sense, such as scratches, holes, reliefs, surface colours, reflection zones in an opal crystal or a density change in a piece of wood. In the wider sense, they are portions of particular objects with partially imaginary borders, such as the core of the Earth, an area of property on the surface of the Earth, a landscape or the head of a contiguous marble statue. They can be measured and dated, and it is sometimes possible to state who or what is or was responsible for them. They cannot be separated from the carrier object, but a segment of the carrier object may be identified (or sometimes removed) carrying the complete feature.

This definition coincides with the definition of “fiat objects” (Smith &amp; Varzi, 2000, pp.401-420), with the exception of aggregates of “bona fide objects”.

</rdfs:comment>
      <rdfs:comment>Examples:

the temple in Abu Simbel before its removal, which was carved out of solid rock Albrecht Duerer’s signature on his painting of Charles the Great the damage to the nose of the Great Sphinx in Giza Michael Jackson’s nose prior to plastic surgery

</rdfs:comment>
   </owl:Class>
   <!--E27_Site-->
   <owl:Class rdf:about="http://erlangen-crm.org/current/E27_Site">
      <rdfs:label xml:lang="en">E27 Site</rdfs:label>
      <rdfs:subClassOf rdf:resource="http://erlangen-crm.org/current/E26_Physical_Feature"/>
      <rdfs:comment>Scope note:
This class comprises pieces of land or sea floor.
In contrast to the purely geometric notion of E53 Place, this class describes constellations of matter on the surface of the Earth or other celestial body, which can be represented by photographs, paintings and maps.
Instances of E27 Site are composed of relatively immobile material items and features in a particular configuration at a particular location.

</rdfs:comment>
      <rdfs:comment>Examples:

the Amazon river basin Knossos the Apollo 11 landing site Heathrow Airport the submerged harbour of the Minoan settlement of Gournia, Crete

</rdfs:comment>
   </owl:Class>
   <!--E28_Conceptual_Object-->
   <owl:Class rdf:about="http://erlangen-crm.org/current/E28_Conceptual_Object">
      <rdfs:label xml:lang="en">E28 Conceptual Object</rdfs:label>
      <rdfs:subClassOf rdf:resource="http://erlangen-crm.org/current/E71_Man-Made_Thing"/>
      <rdfs:superClassOf rdf:resource="http://erlangen-crm.org/current/E55_Type"/>
      <rdfs:superClassOf rdf:resource="http://erlangen-crm.org/current/E89_Propositional_Object"/>
      <rdfs:superClassOf rdf:resource="http://erlangen-crm.org/current/E90_Symbolic_Object"/>
      <rdfs:comment>Scope note:
This class comprises non-material products of our minds and other human produced data that have become objects of a discourse about their identity, circumstances of creation or historical implication. The production of such information may have been supported by the use of technical devices such as cameras or computers.
Characteristically, instances of this class are created, invented or thought by someone, and then may be documented or communicated between persons. Instances of E28 Conceptual Object have the ability to exist on more than one particular carrier at the same time, such as paper, electronic signals, marks, audio media, paintings, photos, human memories, etc.
They cannot be destroyed. They exist as long as they can be found on at least one carrier or in at least one human memory. Their existence ends when the last carrier and the last memory are lost.

</rdfs:comment>
      <rdfs:comment>Examples:

Beethoven’s ‘Ode an die Freude’ (Ode to Joy), (E73) the definition of “ontology” in the Oxford English Dictionary the knowledge about the victory at Marathon carried by the famous runner

</rdfs:comment>
      <rdfs:comment>Properties:
P149 is identified by (identifies): E75 Conceptual Object Appellation

</rdfs:comment>
   </owl:Class>
   <!--E29_Design_or_Procedure-->
   <owl:Class rdf:about="http://erlangen-crm.org/current/E29_Design_or_Procedure">
      <rdfs:label xml:lang="en">E29 Design or Procedure</rdfs:label>
      <rdfs:subClassOf rdf:resource="http://erlangen-crm.org/current/E73_Information_Object"/>
      <rdfs:comment>Scope note:
This class comprises documented plans for the execution of actions in order to achieve a result of a specific quality, form or contents. In particular it comprises plans for deliberate human activities that may result in the modification or production of instances of E24 Physical Thing.
Instances of E29 Design or Procedure can be structured in parts and sequences or depend on others. This is modelled using P69 is associated with.
Designs or procedures can be seen as one of the following:
A schema for the activities it describes A schema of the products that result from their application. An independent intellectual product that may have never been applied, such as Leonardo da Vinci’s famous plans for flying machines.
Because designs or procedures may never be applied or only partially executed, the CRM models a loose relationship between the plan and the respective product.

</rdfs:comment>
      <rdfs:comment>Examples:

the ISO standardisation procedure the musical notation for Beethoven’s “Ode to Joy” the architectural drawings for the Kölner Dom in Cologne, Germany the drawing on the folio 860 of the Codex Atlanticus from Leonardo da Vinci, 1486-1490, kept in the Biblioteca Ambrosiana in Milan

</rdfs:comment>
      <rdfs:comment>Properties:

P68 foresees use of (use foreseen by): E57 Material
P69 has association with (is associated with): E29 Design or Procedure
(P69.1 has type: E55 Type)

</rdfs:comment>
      <rdfs:subClassOf>
         <owl:Restriction>
            <owl:onProperty>
               <owl:ObjectProperty rdf:about="http://erlangen-crm.org/current/P69_has_association_with"/>
            </owl:onProperty>
            <owl:someValuesFrom rdf:resource="http://erlangen-crm.org/current/E29_Design_or_Procedure"/>
         </owl:Restriction>
      </rdfs:subClassOf>
   </owl:Class>
   <!--E30_Right-->
   <owl:Class rdf:about="http://erlangen-crm.org/current/E30_Right">
      <rdfs:label xml:lang="en">E30 Right</rdfs:label>
      <rdfs:subClassOf rdf:resource="http://erlangen-crm.org/current/E89_Propositional_Object"/>
      <rdfs:comment>Scope note:
This class comprises legal privileges concerning material and immaterial things or their derivatives.
These include reproduction and property rights.

</rdfs:comment>
      <rdfs:comment>Examples:

copyright held by ISO on ISO/CD 21127 ownership of the “Mona Lisa” by the Louvre

</rdfs:comment>
   </owl:Class>
   <!--E31_Document-->
   <owl:Class rdf:about="http://erlangen-crm.org/current/E31_Document">
      <rdfs:label xml:lang="en">E31 Document</rdfs:label>
      <rdfs:subClassOf rdf:resource="http://erlangen-crm.org/current/E73_Information_Object"/>
      <rdfs:superClassOf rdf:resource="http://erlangen-crm.org/current/E32_Authority_Document"/>
      <rdfs:comment>Scope note:
This class comprises identifiable immaterial items that make propositions about reality.

These propositions may be expressed in text, graphics, images, audiograms, videograms or by other similar means. Documentation databases are regarded as a special case of E31 Document. This class should not be confused with the term “document” in Information Technology, which is compatible with E73 Information Object.

</rdfs:comment>
      <rdfs:comment>Examples:

the Encyclopaedia Britannica (E32) the photo of the Allied Leaders at Yalta published by UPI, 1945 the Doomsday Book

</rdfs:comment>
      <rdfs:comment>Properties:

P70 documents (is documented in): E1 CRM Entity

</rdfs:comment>
   </owl:Class>
   <!--E32_Authority_Document-->
   <owl:Class rdf:about="http://erlangen-crm.org/current/E32_Authority_Document">
      <rdfs:label xml:lang="en">E32 Authority Document</rdfs:label>
      <rdfs:subClassOf rdf:resource="http://erlangen-crm.org/current/E31_Document"/>
      <rdfs:comment>Scope note:
This class comprises encyclopaedia, thesauri, authority lists and other documents that define terminology or conceptual systems for consistent use.


</rdfs:comment>
      <rdfs:comment>Examples:

Webster’s Dictionary Getty Art and Architecture Thesaurus the CIDOC Conceptual Reference Model

</rdfs:comment>
      <rdfs:comment>Properties:

P71 lists (is listed in): E1 CRM Entity

</rdfs:comment>
      <rdfs:subClassOf>
         <owl:Restriction>
            <owl:onProperty>
               <owl:ObjectProperty rdf:about="http://erlangen-crm.org/current/P71_lists"/>
            </owl:onProperty>
            <owl:someValuesFrom rdf:resource="http://erlangen-crm.org/current/E32_Authority_Document"/>
         </owl:Restriction>
      </rdfs:subClassOf>
   </owl:Class>
   <!--E33_Linguistic_Object-->
   <owl:Class rdf:about="http://erlangen-crm.org/current/E33_Linguistic_Object">
      <rdfs:label xml:lang="en">E33 Linguistic Object</rdfs:label>
      <rdfs:subClassOf rdf:resource="http://erlangen-crm.org/current/E73_Information_Object"/>
      <rdfs:superClassOf rdf:resource="http://erlangen-crm.org/current/E34_Inscription"/>
      <rdfs:superClassOf rdf:resource="http://erlangen-crm.org/current/E35_Title"/>
      <rdfs:comment>Scope note:
This class comprises identifiable expressions in natural language or languages.
Instances of E33 Linguistic Object can be expressed in many ways: e.g. as written texts, recorded speech or sign language. However, the CRM treats instances of E33 Linguistic Object independently from the medium or method by which they are expressed. Expressions in formal languages, such as computer code or mathematical formulae, are not treated as instances of E33 Linguistic Object by the CRM. These should be modelled as instances of E73 Information Object.
The text of an instance of E33 Linguistic Object can be documented in a note by P3 has note: E62 String

</rdfs:comment>
      <rdfs:comment>Examples:

the text of the Ellesmere Chaucer manuscript the lyrics of the song “Blue Suede Shoes” the text of the Jabberwocky by Lewis Carroll the text of “Doktoro Jekyll kaj Sinjoro Hyde” (an Esperanto translation of Dr Jekyll and Mr Hyde)

</rdfs:comment>
      <rdfs:comment>Properties:

P72 has language (is language of): E56 Language
P73 has translation (is translation of): E33 Linguistic Object

</rdfs:comment>
      <rdfs:subClassOf>
         <owl:Restriction>
            <owl:onProperty>
               <owl:ObjectProperty rdf:about="http://erlangen-crm.org/current/P72_has_language"/>
            </owl:onProperty>
            <owl:someValuesFrom rdf:resource="http://erlangen-crm.org/current/E33_Linguistic_Object"/>
         </owl:Restriction>
      </rdfs:subClassOf>
   </owl:Class>
   <!--E35_Title-->
   <owl:Class rdf:about="http://erlangen-crm.org/current/E35_Title">
      <rdfs:label xml:lang="en">E35 Title</rdfs:label>
      <rdfs:subClassOf rdf:resource="http://erlangen-crm.org/current/E33_Linguistic_Object"/>
      <rdfs:subClassOf rdf:resource="http://erlangen-crm.org/current/E41_Appellation"/>
      <rdfs:comment>Scope note:
This class comprises the names assigned to works, such as texts, artworks or pieces of music.
Titles are proper noun phrases or verbal phrases, and should not be confused with generic object names such as “chair”, “painting” or “book” (the latter are common nouns that stand for instances of E55 Type). Titles may be assigned by the creator of the work itself, or by a social group.

This class also comprises the translations of titles that are used as surrogates for the original titles in different social contexts.


</rdfs:comment>
      <rdfs:comment>Examples:

“The Merchant of Venice” “Mona Lisa” “La Pie or The Magpie” “Lucy in the Sky with Diamonds”

</rdfs:comment>
   </owl:Class>
   <!--E36_Visual_Item-->
   <owl:Class rdf:about="http://erlangen-crm.org/current/E36_Visual_Item">
      <rdfs:label xml:lang="en">E36 Visual Item</rdfs:label>
      <rdfs:subClassOf rdf:resource="http://erlangen-crm.org/current/E73_Information_Object"/>
      <rdfs:superClassOf rdf:resource="http://erlangen-crm.org/current/E37_Mark"/>
      <rdfs:superClassOf rdf:resource="http://erlangen-crm.org/current/E38_Image"/>
      <rdfs:comment>Scope note:
This class comprises the intellectual or conceptual aspects of recognisable marks and images.

This class does not intend to describe the idiosyncratic characteristics of an individual physical embodiment of a visual item, but the underlying prototype. For example, a mark such as the ICOM logo is generally considered to be the same logo when used on any number of publications. The size, orientation and colour may change, but the logo remains uniquely identifiable. The same is true of images that are reproduced many times. This means that visual items are independent of their physical support.

The class E36 Visual Item provides a means of identifying and linking together instances of E24 Physical Man-Made Thing that carry the same visual symbols, marks or images etc. The property P62 depicts (is depicted by) between E24 Physical Man-Made Thing and depicted subjects (E1 CRM Entity) can be regarded as a shortcut of the more fully developed path from E24 Physical Man-Made Thing through P65 shows visual item (is shown by), E36 Visual Item, P138 represents (has representation) to E1CRM Entity, which in addition captures the optical features of the depiction.


</rdfs:comment>
      <rdfs:comment>Examples:

the visual appearance of Monet’s “La Pie” (E38) the Coca-Cola logo (E34) the Chi-Rho (E37) the communist red star (E37)


</rdfs:comment>
      <rdfs:comment>Properties:

P138 represents (has representation): E1 CRM Entity
(P138.1 mode of representation: E55 Type)

</rdfs:comment>
      <rdfs:subClassOf>
         <owl:Restriction>
            <owl:onProperty>
               <owl:ObjectProperty rdf:about="http://erlangen-crm.org/current/P138_represents"/>
            </owl:onProperty>
            <owl:someValuesFrom rdf:resource="http://erlangen-crm.org/current/E36_Visual_Item"/>
         </owl:Restriction>
      </rdfs:subClassOf>
   </owl:Class>
   <!--E37_Mark-->
   <owl:Class rdf:about="http://erlangen-crm.org/current/E37_Mark">
      <rdfs:label xml:lang="en">E37 Mark</rdfs:label>
      <rdfs:subClassOf rdf:resource="http://erlangen-crm.org/current/E36_Visual_Item"/>
      <rdfs:superClassOf rdf:resource="http://erlangen-crm.org/current/E34_Inscription"/>
      <rdfs:comment>Scope note:
This class comprises symbols, signs, signatures or short texts applied to instances of E24 Physical Man-Made Thing by arbitrary techniques in order to indicate the creator, owner, dedications, purpose, etc.
This class specifically excludes features that have no semantic significance, such as scratches or tool marks. These should be documented as instances of E25 Man-Made Feature.

</rdfs:comment>
      <rdfs:comment>Examples:

Minoan double axe mark © 

</rdfs:comment>
   </owl:Class>
   <!--E39_Actor-->
   <owl:Class rdf:about="http://erlangen-crm.org/current/E39_Actor">
      <rdfs:label xml:lang="en">E39 Actor</rdfs:label>
      <rdfs:subClassOf rdf:resource="http://erlangen-crm.org/current/E77_Persistent_Item"/>
      <rdfs:superClassOf rdf:resource="http://erlangen-crm.org/current/E21_Person"/>
      <rdfs:superClassOf rdf:resource="http://erlangen-crm.org/current/E74_Group"/>
      <rdfs:comment>Scope note:
This class comprises people, either individually or in groups, who have the potential to perform intentional actions for which they can be held responsible.
The CRM does not attempt to model the inadvertent actions of such actors. Individual people should be documented as instances of E21 Person, whereas groups should be documented as instances of either E74 Group or its subclass E40 Legal Body.

</rdfs:comment>
      <rdfs:comment>Examples:

London and Continental Railways (E40) the Governor of the Bank of England in 1975 (E21) Sir Ian McKellan (E21)

</rdfs:comment>
      <rdfs:comment>Properties:

P74 has current or former residence (is current or former residence of): E53 Place
P75 possesses (is possessed by): E30 Right
P76 has contact point (provides access to): E51 Contact Point
P131 is identified by (identifies): E82 Actor Appellation

</rdfs:comment>
      <rdfs:subClassOf>
         <owl:Restriction>
            <owl:onProperty>
               <owl:ObjectProperty rdf:about="http://erlangen-crm.org/current/P74_has_current_or_former_residence"/>
            </owl:onProperty>
            <owl:someValuesFrom rdf:resource="http://erlangen-crm.org/current/E39_Actor"/>
         </owl:Restriction>
      </rdfs:subClassOf>
      <rdfs:subClassOf>
         <owl:Restriction>
            <owl:onProperty>
               <owl:ObjectProperty rdf:about="http://erlangen-crm.org/current/P75_possesses"/>
            </owl:onProperty>
            <owl:someValuesFrom rdf:resource="http://erlangen-crm.org/current/E39_Actor"/>
         </owl:Restriction>
      </rdfs:subClassOf>
      <rdfs:subClassOf>
         <owl:Restriction>
            <owl:onProperty>
               <owl:ObjectProperty rdf:about="http://erlangen-crm.org/current/P131_is_identified_by"/>
            </owl:onProperty>
            <owl:someValuesFrom rdf:resource="http://erlangen-crm.org/current/E39_Actor"/>
         </owl:Restriction>
      </rdfs:subClassOf>
   </owl:Class>
   <!--E40_Legal_Body-->
   <owl:Class rdf:about="http://erlangen-crm.org/current/E40_Legal_Body">
      <rdfs:label xml:lang="en">E40 Legal Body</rdfs:label>
      <rdfs:subClassOf rdf:resource="http://erlangen-crm.org/current/E74_Group"/>
      <rdfs:comment>Scope note:
This class comprises institutions or groups of people that have obtained a legal recognition as a group and can act collectively as agents.

This means that they can perform actions, own property, create or destroy things and can be held collectively responsible for their actions like individual people. The term ‘personne morale’ is often used for this in French.

</rdfs:comment>
      <rdfs:comment>Examples:

Greenpeace Paveprime Ltd the National Museum of Denmark

</rdfs:comment>
   </owl:Class>
   <!--E41_Appellation-->
   <owl:Class rdf:about="http://erlangen-crm.org/current/E41_Appellation">
      <rdfs:label xml:lang="en">E41 Appellation</rdfs:label>
      <rdfs:subClassOf rdf:resource="http://erlangen-crm.org/current/E90_Symbolic_Object"/>
      <rdfs:superClassOf rdf:resource="http://erlangen-crm.org/current/E35_Title"/>
      <rdfs:superClassOf rdf:resource="http://erlangen-crm.org/current/E42_Identifier"/>
      <rdfs:superClassOf rdf:resource="http://erlangen-crm.org/current/E44_Place_Appellation"/>
      <rdfs:superClassOf rdf:resource="http://erlangen-crm.org/current/E49_Time_Appellation"/>
      <rdfs:superClassOf rdf:resource="http://erlangen-crm.org/current/E51_Contact_Point"/>
      <rdfs:superClassOf rdf:resource="http://erlangen-crm.org/current/E75_Conceptual_Object_Appellation"/>
      <rdfs:superClassOf rdf:resource="http://erlangen-crm.org/current/E82_Actor_Appellation"/>
      <rdfs:comment>Scope note:
This class comprises signs, either meaningful or not, or arrangements of signs following a specific syntax, that are used or can be used to refer to and identify a specific instance of some class within a certain context.
Instances of E41 Appellation do not identify things by their meaning, even if they happen to have one, but by convention, tradition, or agreement. Instances of E41 Appellation are cultural constructs; as such, they have a context, a history, and a use in time and space by some group of users. A given instance of E41 Appellation can have alternative forms, i.e., other instances of E41 Appellation that are always regarded as equivalent independent from the thing it denotes.
Specific subclasses of E41 Appellation should be used when instances of E41 Appellation of a characteristic form are used for particular objects. Instances of E49 Time Appellation, for example, which take the form of instances of E50 Date, can be easily recognised.
E41 Appellation should not be confused with the act of naming something. Cf. E15 Identifier Assignment

</rdfs:comment>
      <rdfs:comment>Examples:

“Martin” “the Forth Bridge” “the Merchant of Venice” (E35) “Spigelia marilandica (L.) L.” [not the species, just the name] “information science” [not the science itself, but the name through which we refer to it in an English-speaking context] “安” [Chinese “an”, meaning “peace”]

</rdfs:comment>
      <rdfs:comment>Properties:

P139 has alternative form: E41 Appellation
P139.1 has type: E55 Type

</rdfs:comment>
   </owl:Class>
   <!--E42_Identifier-->
   <owl:Class rdf:about="http://erlangen-crm.org/current/E42_Identifier">
      <rdfs:label xml:lang="en">E42 Identifier</rdfs:label>
      <rdfs:subClassOf rdf:resource="http://erlangen-crm.org/current/E41_Appellation"/>
      <rdfs:comment>Scope note:
This class comprises strings or codes assigned to instances of E1 CRM Entity in order to identify them uniquely and permanently within the context of one or more organisations. Such codes are often known as inventory numbers, registration codes, etc. and are typically composed of alphanumeric sequences. The class E42 Identifier is not normally used for machine-generated identifiers used for automated processing unless these are also used by human agents.

</rdfs:comment>
      <rdfs:comment>Examples:

“MM.GE.195” “13.45.1976” “OXCMS: 1997.4.1” ISSN “0041-5278” ISRC “FIFIN8900116” Shelf mark “Res 8 P 10” “Guillaume de Machaut (1300?-1377)” [a controlled personal name heading that follows the French rules]

</rdfs:comment>
   </owl:Class>
   <!--E44_Place_Appellation-->
   <owl:Class rdf:about="http://erlangen-crm.org/current/E44_Place_Appellation">
      <rdfs:label xml:lang="en">E44 Place Appellation</rdfs:label>
      <rdfs:subClassOf rdf:resource="http://erlangen-crm.org/current/E41_Appellation"/>
      <rdfs:superClassOf rdf:resource="http://erlangen-crm.org/current/E45_Address"/>
      <rdfs:superClassOf rdf:resource="http://erlangen-crm.org/current/E46_Section_Definition"/>
      <rdfs:superClassOf rdf:resource="http://erlangen-crm.org/current/E47_Spatial_Coordinates"/>
      <rdfs:superClassOf rdf:resource="http://erlangen-crm.org/current/E48_Place_Name"/>
      <rdfs:comment>Scope note:
This class comprises any sort of identifier characteristically used to refer to an E53 Place.
Instances of E44 Place Appellation may vary in their degree of precision and their meaning may vary over time – the same instance of E44 Place Appellation may be used to refer to several places, either because of cultural shifts, or because objects used as reference points have moved around. Instances of E44 Place Appellation can be extremely varied in form: postal addresses, instances of E47 Spatial Coordinate, and parts of buildings can all be considered as instances of E44 Place Appellation.

</rdfs:comment>
      <rdfs:comment>Examples:

“Vienna” “CH-1211, Genève” “Aquae Sulis Minerva” “Bath” “Cambridge” “the Other Place” “the City”

</rdfs:comment>
   </owl:Class>
   <!--E47_Spatial_Coordinates-->
   <owl:Class rdf:about="http://erlangen-crm.org/current/E47_Spatial_Coordinates">
      <rdfs:label xml:lang="en">E47 Spatial Coordinates</rdfs:label>
      <rdfs:subClassOf rdf:resource="http://erlangen-crm.org/current/E44_Place_Appellation"/>
      <rdfs:comment>Scope note:
This class comprises the textual or numeric information required to locate specific instances of E53 Place within schemes of spatial identification.
Coordinates are a specific form of E44 Place Appellation, that is, a means of referring to a particular E53 Place. Coordinates are not restricted to longitude, latitude and altitude. Any regular system of reference that maps onto an E19 Physical Object can be used to generate coordinates.

</rdfs:comment>
      <rdfs:comment>Examples:

“6°5’29”N 45°12’13”W” “Black queen’s bishop 4” [chess coordinate]

</rdfs:comment>
   </owl:Class>
   <!--E49_Time_Appellation-->
   <owl:Class rdf:about="http://erlangen-crm.org/current/E49_Time_Appellation">
      <rdfs:label xml:lang="en">E49 Time Appellation</rdfs:label>
      <rdfs:subClassOf rdf:resource="http://erlangen-crm.org/current/E41_Appellation"/>
      <rdfs:superClassOf rdf:resource="http://erlangen-crm.org/current/E50_Date"/>
      <rdfs:comment>Scope note:
This class comprises all forms of names or codes, such as historical periods, and dates, which are characteristically used to refer to a specific E52 Time-Span.
The instances of E49 Time Appellation may vary in their degree of precision, and they may be relative to other time frames, “Before Christ” for example. Instances of E52 Time-Span are often defined by reference to a cultural period or an event e.g. ‘the duration of the Ming Dynasty’.

</rdfs:comment>
      <rdfs:comment>Examples:

“Meiji” [Japanese term for a specific time-span] “1st half of the XX century” “Quaternary” “1215 Hegira” [a date in the Islamic calendar]
“Last century”

</rdfs:comment>
   </owl:Class>
   <!--E50_Date-->
   <owl:Class rdf:about="http://erlangen-crm.org/current/E50_Date">
      <rdfs:label xml:lang="en">E50 Date</rdfs:label>
      <rdfs:subClassOf rdf:resource="http://erlangen-crm.org/current/E49_Time_Appellation"/>
      <rdfs:comment>Scope note:
This class comprises specific forms of E49 Time Appellation.
Dates may vary in their degree of precision.

</rdfs:comment>
      <rdfs:comment>Examples:

“1900” “4-4-1959” “19-MAR-1922”

“19640604”

</rdfs:comment>
   </owl:Class>
   <!--E52_Time-Span-->
   <owl:Class rdf:about="http://erlangen-crm.org/current/E52_Time-Span">
      <rdfs:label xml:lang="en">E52 Time-Span</rdfs:label>
      <rdfs:subClassOf rdf:resource="http://erlangen-crm.org/current/E1_CRM_Entity"/>
      <rdfs:comment>Scope note:
This class comprises abstract temporal extents, in the sense of Galilean physics, having a beginning, an end and a duration.
Time Span has no other semantic connotations. Time-Spans are used to define the temporal extent of instances of E4 Period, E5 Event and any other phenomena valid for a certain time. An E52 Time-Span may be identified by one or more instances of E49 Time Appellation.
Since our knowledge of history is imperfect, instances of E52 Time-Span can best be considered as approximations of the actual Time-Spans of temporal entities. The properties of E52 Time-Span are intended to allow these approximations to be expressed precisely. An extreme case of approximation, might, for example, define an E52 Time-Span having unknown beginning, end and duration. Used as a common E52 Time-Span for two events, it would nevertheless define them as being simultaneous, even if nothing else was known.
Automatic processing and querying of instances of E52 Time-Span is facilitated if data can be parsed into an E61 Time Primitive.

</rdfs:comment>
      <rdfs:comment>Examples:

1961 From 12-17-1993 to 12-8-1996 14h30 – 16h22 4th July 1945 9.30 am 1.1.1999 to 2.00 pm 1.1.1999 duration of the Ming Dynasty

</rdfs:comment>
      <rdfs:comment>Properties:

P78 is identified by (identifies): E49 Time Appellation
P79 beginning is qualified by: E62 String
P80 end is qualified by: E62 String
P81 ongoing throughout: E61 Time Primitive
P82 at some time within: E61 Time Primitive
P83 had at least duration (was minimum duration of): E54 Dimension
P84 had at most duration (was maximum duration of): E54 Dimension
P86 falls within (contains): E52 Time-Span

</rdfs:comment>
      <rdfs:subClassOf>
         <owl:Restriction>
            <owl:onProperty>
               <owl:ObjectProperty rdf:about="http://erlangen-crm.org/current/P78_is_identified_by"/>
            </owl:onProperty>
            <owl:someValuesFrom rdf:resource="http://erlangen-crm.org/current/E52_Time-Span"/>
         </owl:Restriction>
      </rdfs:subClassOf>
      <rdfs:subClassOf>
         <owl:Restriction>
            <owl:cardinality rdf:datatype="http://www.w3.org/2001/XMLSchema#nonNegativeInteger">1</owl:cardinality>
            <owl:onProperty>
               <owl:ObjectProperty rdf:about="http://erlangen-crm.org/current/P82_at_some_time_within"/>
            </owl:onProperty>
         </owl:Restriction>
      </rdfs:subClassOf>
   </owl:Class>
   <!--E53_Place-->
   <owl:Class rdf:about="http://erlangen-crm.org/current/E53_Place">
      <rdfs:label xml:lang="en">E53 Place</rdfs:label>
      <rdfs:subClassOf rdf:resource="http://erlangen-crm.org/current/E1_CRM_Entity"/>
      <rdfs:comment>Scope note:
This class comprises extents in space, in particular on the surface of the Earth, in the pure sense of physics: independent from temporal phenomena and matter.
The instances of E53 Place are usually determined by reference to the position of “immobile” objects such as buildings, cities, mountains, rivers, or dedicated geodetic marks. A Place can be determined by combining a frame of reference and a location with respect to this frame. It may be identified by one or more instances of E44 Place Appellation.
It is sometimes argued that instances of E53 Place are best identified by global coordinates or absolute reference systems. However, relative references are often more relevant in the context of cultural documentation and tend to be more precise. In particular, we are often interested in position in relation to large, mobile objects, such as ships. For example, the Place at which Nelson died is known with reference to a large mobile object – H.M.S Victory. A resolution of this Place in terms of absolute coordinates would require knowledge of the movements of the vessel and the precise time of death, either of which may be revised, and the result would lack historical and cultural relevance.
Any object can serve as a frame of reference for E53 Place determination. The model foresees the notion of a “section” of an E19 Physical Object as a valid E53 Place determination.

</rdfs:comment>
      <rdfs:comment>Examples:

the extent of the UK in the year 2003 the position of the hallmark on the inside of my wedding ring the place referred to in the phrase: “Fish collected at three miles north of the confluence of the Arve and the Rhone” here -&gt; &lt;-

</rdfs:comment>
      <rdfs:comment>Properties:

P87 is identified by (identifies): E44 Place Appellation
P89 falls within (contains): E53 Place
P121 overlaps with: E53 Place
P122 borders with: E53 Place

</rdfs:comment>
      <rdfs:subClassOf>
         <owl:Restriction>
            <owl:onProperty>
               <owl:ObjectProperty rdf:about="http://erlangen-crm.org/current/P87_is_identified_by"/>
            </owl:onProperty>
            <owl:someValuesFrom rdf:resource="http://erlangen-crm.org/current/E53_Place"/>
         </owl:Restriction>
      </rdfs:subClassOf>
   </owl:Class>
   <!--E54_Dimension-->
   <owl:Class rdf:about="http://erlangen-crm.org/current/E54_Dimension">
      <rdfs:label xml:lang="en">E54 Dimension</rdfs:label>
      <rdfs:subClassOf rdf:resource="http://erlangen-crm.org/current/E1_CRM_Entity"/>
      <rdfs:comment>Scope note:
This class comprises quantifiable properties that can be measured by some calibrated means and can be approximated by values, i.e. points or regions in a mathematical or conceptual space, such as natural or real numbers, RGB values etc.
An instance of E54 Dimension represents the true quantity, independent from its numerical approximation, e.g. in inches or in cm. The properties of the class E54 Dimension allow for expressing the numerical approximation of the values of an instance of E54 Dimension. If the true values belong to a non-discrete space, such as spatial distances, it is recommended to record them as approximations by intervals or regions of indeterminacy enclosing the assumed true values. For instance, a length of 5 cm may be recorded as 4.5-5.5 cm, according to the precision of the respective observation. Note, that interoperability of values described in different units depends critically on the representation as value regions.
Numerical approximations in archaic instances of E58 Measurement Unit used in historical records should be preserved. Equivalents corresponding to current knowledge should be recorded as additional instances of E54 Dimension as appropriate.

</rdfs:comment>
      <rdfs:comment>Examples:

currency: £26.00 length: 3.9-4.1 cm diameter 26 mm weight 150 lbs density: 0.85 gm/cc luminescence: 56 ISO lumens tin content: 0.46 % taille au garot: 5 hands calibrated C14 date: 2460-2720 years, etc

</rdfs:comment>
      <rdfs:comment>Properties:

P90 has value: E60 Number
P91 has unit (is unit of): E58 Measurement Unit

</rdfs:comment>
   </owl:Class>
   <!--E55_Type-->
   <owl:Class rdf:about="http://erlangen-crm.org/current/E55_Type">
      <rdfs:label xml:lang="en">E55 Type</rdfs:label>
      <rdfs:subClassOf rdf:resource="http://erlangen-crm.org/current/E28_Conceptual_Object"/>
      <rdfs:superClassOf rdf:resource="http://erlangen-crm.org/current/E56_Language"/>
      <rdfs:superClassOf rdf:resource="http://erlangen-crm.org/current/E57_Material"/>
      <rdfs:superClassOf rdf:resource="http://erlangen-crm.org/current/E58_Measurement_Unit"/>
      <rdfs:comment>Scope note:
This class comprises concepts denoted by terms from thesauri and controlled vocabularies used to characterize and classify instances of CRM classes. Instances of E55 Type represent concepts in contrast to instances of E41 Appellation which are used to name instances of CRM classes.
E55 Type is the CRM’s interface to domain specific ontologies and thesauri. These can be represented in the CRM as subclasses of E55 Type, forming hierarchies of terms, i.e. instances of E55 Type linked via P127 has broader term (has narrower term). Such hierarchies may be extended with additional properties.

</rdfs:comment>
      <rdfs:comment>Examples:

weight, length, depth [types of E54] portrait, sketch, animation [types of E38] French, English, German [E56] excellent, good, poor [types of E3] Ford Model T, chop stick [types of E22] cave, doline, scratch [types of E26] poem, short story [types of E33] wedding, earthquake, skirmish [types of E5]

</rdfs:comment>
      <rdfs:comment>Properties:

P127 has broader term (has narrower term): E55 Type
P150 defines typical parts of (define typical wholes for): E55 Type

</rdfs:comment>
      <rdfs:subClassOf>
         <owl:Restriction>
            <owl:onProperty>
               <owl:ObjectProperty rdf:about="http://erlangen-crm.org/current/P127_has_broader_term"/>
            </owl:onProperty>
            <owl:someValuesFrom rdf:resource="http://erlangen-crm.org/current/E55_Type"/>
         </owl:Restriction>
      </rdfs:subClassOf>
   </owl:Class>
   <!--E56_Language-->
   <owl:Class rdf:about="http://erlangen-crm.org/current/E56_Language">
      <rdfs:label xml:lang="en">E56 Language</rdfs:label>
      <rdfs:subClassOf rdf:resource="http://erlangen-crm.org/current/E55_Type"/>
      <rdfs:comment>Scope note:
This class is a specialization of E55 Type and comprises the natural languages in the sense of concepts.
This type is used categorically in the model without reference to instances of it, i.e. the Model does not foresee the description of instances of instances of E56 Language, e.g.: “instances of Mandarin Chinese”.
It is recommended that internationally or nationally agreed codes and terminology are used to denote instances of E56 Language, such as those defined in ISO 639:1988.

</rdfs:comment>
      <rdfs:comment>Examples:

el [Greek] en [English] eo [Esperanto] es [Spanish] fr [French]

</rdfs:comment>
   </owl:Class>
   <!--E57_Material-->
   <owl:Class rdf:about="http://erlangen-crm.org/current/E57_Material">
      <rdfs:label xml:lang="en">E57 Material</rdfs:label>
      <rdfs:subClassOf rdf:resource="http://erlangen-crm.org/current/E55_Type"/>
      <rdfs:comment>Scope note:
This class is a specialization of E55 Type and comprises the concepts of materials.
Instances of E57 Material may denote properties of matter before its use, during its use, and as incorporated in an object, such as ultramarine powder, tempera paste, reinforced concrete. Discrete pieces of raw-materials kept in museums, such as bricks, sheets of fabric, pieces of metal, should be modelled individually in the same way as other objects. Discrete used or processed pieces, such as the stones from Nefer Titi’s temple, should be modelled as parts (cf. P46 is composed of).
This type is used categorically in the model without reference to instances of it, i.e. the Model does not foresee the description of instances of instances of E57 Material, e.g.: “instances of gold”.
It is recommended that internationally or nationally agreed codes and terminology are used.

</rdfs:comment>
      <rdfs:comment>Examples:

brick gold aluminium polycarbonate resin

</rdfs:comment>
   </owl:Class>
   <!--E59_Primitive_Value-->
   <owl:Class rdf:about="http://erlangen-crm.org/current/E59_Primitive_Value">
      <rdfs:label xml:lang="en">E59 Primitive Value</rdfs:label>
      <rdfs:superClassOf rdf:resource="http://erlangen-crm.org/current/E60_Number"/>
      <rdfs:superClassOf rdf:resource="http://erlangen-crm.org/current/E61_Time_Primitive"/>
      <rdfs:superClassOf rdf:resource="http://erlangen-crm.org/current/E62_String"/>
      <rdfs:comment>Scope note:
This class comprises primitive values used as documentation elements, which are not further elaborated upon within the model.

As such they are not considered as elements within our universe of discourse. No specific implementation recommendations are made. It is recommended that the primitive value system from the implementation platform be used to substitute for this class and its subclasses.

</rdfs:comment>
      <rdfs:comment>Examples:

ABCDEFG (E62) 3.14 (E60) 0 1921-01-01 (E61)

</rdfs:comment>
   </owl:Class>
   <!--E60_Number-->
   <owl:Class rdf:about="http://erlangen-crm.org/current/E60_Number">
      <rdfs:label xml:lang="en">E60 Number</rdfs:label>
      <rdfs:subClassOf rdf:resource="http://erlangen-crm.org/current/E59_Primitive_Value"/>
      <rdfs:comment>Scope note:
This class comprises any encoding of computable (algebraic) values such as integers, real numbers, complex numbers, vectors, tensors etc., including intervals of these values to express limited precision.
Numbers are fundamentally distinct from identifiers in continua, such as instances of E50 Date and E47 Spatial Coordinate, even though their encoding may be similar. Instances of E60 Number can be combined with each other in algebraic operations to yield other instances of E60 Number, e.g., 1+1=2. Identifiers in continua may be combined with numbers expressing distances to yield new identifiers, e.g., 1924-01-31 + 2 days = 1924-02-02. Cf. E54 Dimension.

</rdfs:comment>
      <rdfs:comment>Examples:

5 3+2i 1.5e-04 (0.5, - 0.7,88)

</rdfs:comment>
   </owl:Class>
   <!--E61_Time_Primitive-->
   <owl:Class rdf:about="http://erlangen-crm.org/current/E61_Time_Primitive">
      <rdfs:label xml:lang="en">E61 Time Primitive</rdfs:label>
      <rdfs:subClassOf rdf:resource="http://erlangen-crm.org/current/E59_Primitive_Value"/>
      <rdfs:comment>Scope note:
This class comprises instances of E59 Primitive Value for time that should be implemented with appropriate validation, precision and interval logic to express date ranges relevant to cultural documentation.
E61 Time Primitive is not further elaborated upon within the model.

</rdfs:comment>
      <rdfs:comment>Examples:

1994 – 1997 13 May 1768 2000/01/01 00:00:59.7 85th century BC

</rdfs:comment>
   </owl:Class>
   <!--E62_String-->
   <owl:Class rdf:about="http://erlangen-crm.org/current/E62_String">
      <rdfs:label xml:lang="en">E62 String</rdfs:label>
      <rdfs:subClassOf rdf:resource="http://erlangen-crm.org/current/E59_Primitive_Value"/>
      <rdfs:comment>Scope note:
This class comprises the instances of E59 Primitive Values used for documentation such as free text strings, bitmaps, vector graphics, etc.
E62 String is not further elaborated upon within the model.

</rdfs:comment>
      <rdfs:comment>Examples:

the Quick Brown Fox Jumps Over the Lazy Dog 6F 6E 54 79 70 31 0D 9E

</rdfs:comment>
   </owl:Class>
   <!--E63_Beginning_of_Existence-->
   <owl:Class rdf:about="http://erlangen-crm.org/current/E63_Beginning_of_Existence">
      <rdfs:label xml:lang="en">E63 Beginning of Existence</rdfs:label>
      <rdfs:subClassOf rdf:resource="http://erlangen-crm.org/current/E5_Event"/>
      <rdfs:superClassOf rdf:resource="http://erlangen-crm.org/current/E12_Production"/>
      <rdfs:superClassOf rdf:resource="http://erlangen-crm.org/current/E65_Creation"/>
      <rdfs:superClassOf rdf:resource="http://erlangen-crm.org/current/E66_Formation"/>
      <rdfs:superClassOf rdf:resource="http://erlangen-crm.org/current/E67_Birth"/>
      <rdfs:superClassOf rdf:resource="http://erlangen-crm.org/current/E81_Transformation"/>
      <rdfs:comment>Scope note:
This class comprises events that bring into existence any E77 Persistent Item.

It may be used for temporal reasoning about things (intellectual products, physical items, groups of people, living beings) beginning to exist; it serves as a hook for determination of a terminus post quem and ante quem.


</rdfs:comment>
      <rdfs:comment>Examples:

the birth of my child the birth of Snoopy, my dog the calving of the iceberg that sank the Titanic the construction of the Eiffel Tower

</rdfs:comment>
      <rdfs:comment>Properties:

P92 brought into existence (was brought into existence by): E77 Persistent Item

</rdfs:comment>
   </owl:Class>
   <!--E64_End_of_Existence-->
   <owl:Class rdf:about="http://erlangen-crm.org/current/E64_End_of_Existence">
      <rdfs:label xml:lang="en">E64 End of Existence</rdfs:label>
      <rdfs:subClassOf rdf:resource="http://erlangen-crm.org/current/E5_Event"/>
      <rdfs:superClassOf rdf:resource="http://erlangen-crm.org/current/E6_Destruction"/>
      <rdfs:superClassOf rdf:resource="http://erlangen-crm.org/current/E68_Dissolution"/>
      <rdfs:superClassOf rdf:resource="http://erlangen-crm.org/current/E69_Death"/>
      <rdfs:superClassOf rdf:resource="http://erlangen-crm.org/current/E81_Transformation"/>
      <rdfs:comment>Scope note:
This class comprises events that end the existence of any E77 Persistent Item.

It may be used for temporal reasoning about things (physical items, groups of people, living beings) ceasing to exist; it serves as a hook for determination of a terminus postquem and antequem. In cases where substance from a Persistent Item continues to exist in a new form, the process would be documented by E81 Transformation.

</rdfs:comment>
      <rdfs:comment>Examples:

the death of Snoopy, my dog the melting of the snowman the burning of the Temple of Artemis in Ephesos by Herostratos in 356BC

</rdfs:comment>
      <rdfs:comment>Properties:

P93 took out of existence (was taken out of existence by): E77 Persistent Item

</rdfs:comment>
   </owl:Class>
   <!--E65_Creation-->
   <owl:Class rdf:about="http://erlangen-crm.org/current/E65_Creation">
      <rdfs:label xml:lang="en">E65 Creation</rdfs:label>
      <rdfs:subClassOf rdf:resource="http://erlangen-crm.org/current/E7_Activity"/>
      <rdfs:subClassOf rdf:resource="http://erlangen-crm.org/current/E63_Beginning_of_Existence"/>
      <rdfs:superClassOf rdf:resource="http://erlangen-crm.org/current/E83_Type_Creation"/>
      <rdfs:comment>Scope note:
This class comprises events that result in the creation of conceptual items or immaterial products, such as legends, poems, texts, music, images, movies, laws, types etc.

</rdfs:comment>
      <rdfs:comment>Examples:

the framing of the U.S. Constitution the drafting of U.N. resolution 1441

</rdfs:comment>
      <rdfs:comment>Properties:

P94 has created (was created by): E28 Conceptual Object

</rdfs:comment>
      <rdfs:subClassOf>
         <owl:Restriction>
            <owl:onProperty>
               <owl:ObjectProperty rdf:about="http://erlangen-crm.org/current/P94_has_created"/>
            </owl:onProperty>
            <owl:minCardinality rdf:datatype="http://www.w3.org/2001/XMLSchema#nonNegativeInteger">1</owl:minCardinality>
         </owl:Restriction>
      </rdfs:subClassOf>
   </owl:Class>
   <!--E66_Formation-->
   <owl:Class rdf:about="http://erlangen-crm.org/current/E66_Formation">
      <rdfs:label xml:lang="en">E66 Formation</rdfs:label>
      <rdfs:subClassOf rdf:resource="http://erlangen-crm.org/current/E7_Activity"/>
      <rdfs:subClassOf rdf:resource="http://erlangen-crm.org/current/E63_Beginning_of_Existence"/>
      <rdfs:comment>Scope note:
This class comprises events that result in the formation of a formal or informal E74 Group of people, such as a club, society, association, corporation or nation.

E66 Formation does not include the arbitrary aggregation of people who do not act as a collective.
The formation of an instance of E74 Group does not mean that the group is populated with members at the time of formation. In order to express the joining of members at the time of formation, the respective activity should be simultaneously an instance of both E66 Formation and E85 Joining.

</rdfs:comment>
      <rdfs:comment>Examples:

the formation of the CIDOC CRM Special Interest Group the formation of the Soviet Union the conspiring of the murderers of Caesar

</rdfs:comment>
      <rdfs:comment>Properties:

P95 has formed (was formed by): E74 Group
P151 was formed from (participated in): E74 Group

</rdfs:comment>
      <rdfs:subClassOf>
         <owl:Restriction>
            <owl:onProperty>
               <owl:ObjectProperty rdf:about="http://erlangen-crm.org/current/P95_has_formed"/>
            </owl:onProperty>
            <owl:minCardinality rdf:datatype="http://www.w3.org/2001/XMLSchema#nonNegativeInteger">1</owl:minCardinality>
         </owl:Restriction>
      </rdfs:subClassOf>
      <rdfs:subClassOf>
         <owl:Restriction>
            <owl:onProperty>
               <owl:ObjectProperty rdf:about="http://erlangen-crm.org/current/P151_was_formed_from"/>
            </owl:onProperty>
            <owl:someValuesFrom rdf:resource="http://erlangen-crm.org/current/E66_Formation"/>
         </owl:Restriction>
      </rdfs:subClassOf>
   </owl:Class>
   <!--E67_Birth-->
   <owl:Class rdf:about="http://erlangen-crm.org/current/E67_Birth">
      <rdfs:label xml:lang="en">E67 Birth</rdfs:label>
      <rdfs:subClassOf rdf:resource="http://erlangen-crm.org/current/E63_Beginning_of_Existence"/>
      <rdfs:comment>Scope note:
This class comprises the births of human beings. E67 Birth is a biological event focussing on the context of people coming into life. (E63 Beginning of Existence comprises the coming into life of any living beings).
Twins, triplets etc. are brought into life by the same E67 Birth event. The introduction of the E67 Birth event as a documentation element allows the description of a range of family relationships in a simple model. Suitable extensions may describe more details and the complexity of motherhood with the intervention of modern medicine. In this model, the biological father is not seen as a necessary participant in the E67 Birth event.

</rdfs:comment>
      <rdfs:comment>Examples:

the birth of Alexander the Great

</rdfs:comment>
      <rdfs:comment>Properties:

P96 by mother (gave birth): E21 Person
P97 from father (was father for): E21 Person
P98 brought into life (was born): E21 Person

</rdfs:comment>
      <rdfs:subClassOf>
         <owl:Restriction>
            <owl:onProperty>
               <owl:ObjectProperty rdf:about="http://erlangen-crm.org/current/P98_brought_into_life"/>
            </owl:onProperty>
            <owl:someValuesFrom rdf:resource="http://erlangen-crm.org/current/E67_Birth"/>
         </owl:Restriction>
      </rdfs:subClassOf>
   </owl:Class>
   <!--E69_Death-->
   <owl:Class rdf:about="http://erlangen-crm.org/current/E69_Death">
      <rdfs:label xml:lang="en">E69 Death</rdfs:label>
      <rdfs:subClassOf rdf:resource="http://erlangen-crm.org/current/E64_End_of_Existence"/>
      <rdfs:comment>Scope note:
This class comprises the deaths of human beings.
If a person is killed, their death should be instantiated as E69 Death and as E7 Activity. The death or perishing of other living beings should be documented using E64 End of Existence.

</rdfs:comment>
      <rdfs:comment>Examples:

the murder of Julius Caesar (E69, E7) the death of Senator Paul Wellstone

</rdfs:comment>
      <rdfs:comment>Properties:

P100 was death of (died in): E21 Person

</rdfs:comment>
      <rdfs:subClassOf>
         <owl:Restriction>
            <owl:onProperty>
               <owl:ObjectProperty rdf:about="http://erlangen-crm.org/current/P100_was_death_of"/>
            </owl:onProperty>
            <owl:minCardinality rdf:datatype="http://www.w3.org/2001/XMLSchema#nonNegativeInteger">1</owl:minCardinality>
         </owl:Restriction>
      </rdfs:subClassOf>
   </owl:Class>
   <!--E70_Thing-->
   <owl:Class rdf:about="http://erlangen-crm.org/current/E70_Thing">
      <rdfs:label xml:lang="en">E70 Thing</rdfs:label>
      <rdfs:subClassOf rdf:resource="http://erlangen-crm.org/current/E77_Persistent_Item"/>
      <rdfs:superClassOf rdf:resource="http://erlangen-crm.org/current/E71_Man-Made_Thing"/>
      <rdfs:superClassOf rdf:resource="http://erlangen-crm.org/current/E72_Legal_Object"/>
      <rdfs:comment>Scope note:
This general class comprises usable discrete, identifiable, instances of E77 Persistent Item that are documented as single units.
They can be either intellectual products or physical things, and are characterized by relative stability. They may for instance either have a solid physical form, an electronic encoding, or they may be logical concept or structure.

</rdfs:comment>
      <rdfs:comment>Examples:

my photograph collection (E78) the bottle of milk in my refrigerator (E22) the plan of the Strassburger Muenster (E29) the thing on the top of Otto Hahn’s desk (E19) the form of the no-smoking sign (E36)
the cave of Dirou, Mani, Greece (E27)

</rdfs:comment>
      <rdfs:comment>Properties:

P43 has dimension (is dimension of): E54 Dimension
P101 had as general use (was use of): E55 Type
P130 shows features of (features are also found on): E70 Thing
(P130.1 kind of similarity: E55 Type)

</rdfs:comment>
      <rdfs:subClassOf>
         <owl:Restriction>
            <owl:onProperty>
               <owl:ObjectProperty rdf:about="http://erlangen-crm.org/current/P43_has_dimension"/>
            </owl:onProperty>
            <owl:someValuesFrom rdf:resource="http://erlangen-crm.org/current/E70_Thing"/>
         </owl:Restriction>
      </rdfs:subClassOf>
      <rdfs:subClassOf>
         <owl:Restriction>
            <owl:onProperty>
               <owl:ObjectProperty rdf:about="http://erlangen-crm.org/current/P130_shows_features_of"/>
            </owl:onProperty>
            <owl:someValuesFrom rdf:resource="http://erlangen-crm.org/current/E70_Thing"/>
         </owl:Restriction>
      </rdfs:subClassOf>
   </owl:Class>
   <!--E71_Man-Made_Thing-->
   <owl:Class rdf:about="http://erlangen-crm.org/current/E71_Man-Made_Thing">
      <rdfs:label xml:lang="en">E71 Man-Made Thing</rdfs:label>
      <rdfs:subClassOf rdf:resource="http://erlangen-crm.org/current/E70_Thing"/>
      <rdfs:superClassOf rdf:resource="http://erlangen-crm.org/current/E24_Physical_Man-Made_Thing"/>
      <rdfs:superClassOf rdf:resource="http://erlangen-crm.org/current/E28_Conceptual_Object"/>
      <rdfs:comment>Scope note:
This class comprises discrete, identifiable man-made items that are documented as single units.

These items are either intellectual products or man-made physical things, and are characterized by relative stability. They may for instance have a solid physical form, an electronic encoding, or they may be logical concepts or structures.

</rdfs:comment>
      <rdfs:comment>Examples:

Beethoven’s 5th Symphony (E73) Michelangelo’s David Einstein’s Theory of General Relativity (E73) the taxon ‘Fringilla coelebs Linnaeus,1758’ (E55)

</rdfs:comment>
      <rdfs:comment>Properties:

P102 has title (is title of): E35 Title
(P102.1 has type: E55 Type)
P103 was intended for (was intention of): E55 Type

</rdfs:comment>
      <rdfs:subClassOf>
         <owl:Restriction>
            <owl:onProperty>
               <owl:ObjectProperty rdf:about="http://erlangen-crm.org/current/P102_has_title"/>
            </owl:onProperty>
            <owl:someValuesFrom rdf:resource="http://erlangen-crm.org/current/E71_Man-Made_Thing"/>
         </owl:Restriction>
      </rdfs:subClassOf>
      <rdfs:subClassOf>
         <owl:Restriction>
            <owl:onProperty>
               <owl:ObjectProperty rdf:about="http://erlangen-crm.org/current/P103_was_intended_for"/>
            </owl:onProperty>
            <owl:someValuesFrom rdf:resource="http://erlangen-crm.org/current/E71_Man-Made_Thing"/>
         </owl:Restriction>
      </rdfs:subClassOf>
   </owl:Class>
   <!--E72_Legal_Object-->
   <owl:Class rdf:about="http://erlangen-crm.org/current/E72_Legal_Object">
      <rdfs:label xml:lang="en">E72 Legal Object</rdfs:label>
      <rdfs:subClassOf rdf:resource="http://erlangen-crm.org/current/E70_Thing"/>
      <rdfs:superClassOf rdf:resource="http://erlangen-crm.org/current/E18_Physical_Thing"/>
      <rdfs:superClassOf rdf:resource="http://erlangen-crm.org/current/E90_Symbolic_Object"/>
      <rdfs:comment>Scope note:
This class comprises those material or immaterial items to which instances of E30 Right, such as the right of ownership or use, can be applied.
This is true for all E18 Physical Thing. In the case of instances of E28 Conceptual Object, however, the identity of the E28 Conceptual Object or the method of its use may be too ambiguous to reliably establish instances of E30 Right, as in the case of taxa and inspirations. Ownership of corporations is currently regarded as out of scope of the CRM.

</rdfs:comment>
      <rdfs:comment>Examples:

the Cullinan diamond (E19) definition of the CIDOC Conceptual Reference Model Version 2.1 (E73)

</rdfs:comment>
      <rdfs:comment>Properties:

P104 is subject to (applies to): E30 Right
P105 right held by (has right on): E39 Actor

</rdfs:comment>
      <rdfs:subClassOf>
         <owl:Restriction>
            <owl:onProperty>
               <owl:ObjectProperty rdf:about="http://erlangen-crm.org/current/P104_is_subject_to"/>
            </owl:onProperty>
            <owl:someValuesFrom rdf:resource="http://erlangen-crm.org/current/E72_Legal_Object"/>
         </owl:Restriction>
      </rdfs:subClassOf>
      <rdfs:subClassOf>
         <owl:Restriction>
            <owl:onProperty>
               <owl:ObjectProperty rdf:about="http://erlangen-crm.org/current/P105_right_held_by"/>
            </owl:onProperty>
            <owl:someValuesFrom rdf:resource="http://erlangen-crm.org/current/E72_Legal_Object"/>
         </owl:Restriction>
      </rdfs:subClassOf>
   </owl:Class>
   <!--E73_Information_Object-->
   <owl:Class rdf:about="http://erlangen-crm.org/current/E73_Information_Object">
      <rdfs:label xml:lang="en">E73 Information Object</rdfs:label>
      <rdfs:subClassOf rdf:resource="http://erlangen-crm.org/current/E89_Propositional_Object"/>
      <rdfs:subClassOf rdf:resource="http://erlangen-crm.org/current/E90_Symbolic_Object"/>
      <rdfs:superClassOf rdf:resource="http://erlangen-crm.org/current/E29_Design_or_Procedure"/>
      <rdfs:superClassOf rdf:resource="http://erlangen-crm.org/current/E31_Document"/>
      <rdfs:superClassOf rdf:resource="http://erlangen-crm.org/current/E33_Linguistic_Object"/>
      <rdfs:superClassOf rdf:resource="http://erlangen-crm.org/current/E36_Visual_Item"/>
      <rdfs:comment>Scope note:
This class comprises identifiable immaterial items, such as a poems, jokes, data sets, images, texts, multimedia objects, procedural prescriptions, computer program code, algorithm or mathematical formulae, that have an objectively recognizable structure and are documented as single units.
An E73 Information Object does not depend on a specific physical carrier, which can include human memory, and it can exist on one or more carriers simultaneously.
Instances of E73 Information Object of a linguistic nature should be declared as instances of the E33 Linguistic Object subclass. Instances of E73 Information Object of a documentary nature should be declared as instances of the E31 Document subclass. Conceptual items such as types and classes are not instances of E73 Information Object, nor are ideas without a reproducible expression.

</rdfs:comment>
      <rdfs:comment>Examples:

image BM000038850.JPG from the Clayton Herbarium in London E. A. Poe’s “The Raven” the movie “The Seven Samurai” by Akira Kurosawa the Maxwell Equations

</rdfs:comment>
      <rdfs:comment>Properties:
P165 incorporates (is incorporated in): E90 Symbolic Object

</rdfs:comment>
      <rdfs:subClassOf>
         <owl:Restriction>
            <owl:onProperty>
               <owl:ObjectProperty rdf:about="http://erlangen-crm.org/current/P165_incorporates"/>
            </owl:onProperty>
            <owl:someValuesFrom rdf:resource="http://erlangen-crm.org/current/E73_Information_Object"/>
         </owl:Restriction>
      </rdfs:subClassOf>
   </owl:Class>
   <!--E74_Group-->
   <owl:Class rdf:about="http://erlangen-crm.org/current/E74_Group">
      <rdfs:label xml:lang="en">E74 Group</rdfs:label>
      <rdfs:subClassOf rdf:resource="http://erlangen-crm.org/current/E39_Actor"/>
      <rdfs:superClassOf rdf:resource="http://erlangen-crm.org/current/E40_Legal_Body"/>
      <rdfs:comment>Scope note:
This class comprises any gatherings or organizations of two or more people that act collectively or in a similar way due to any form of unifying relationship. In the wider sense this class also comprises official positions which used to be regarded in certain contexts as one actor, independent of the current holder of the office, such as the president of a country.
A gathering of people becomes an E74 Group when it exhibits organizational characteristics usually typified by a set of ideas or beliefs held in common, or actions performed together. These might be communication, creating some common 109ulgate109, a common purpose such as study, worship, business, sports, etc. Nationality can be 109ulgate109 as membership in an E74 Group (cf. HumanML markup). Married couples and other concepts of family are regarded as particular examples of E74 Group.

</rdfs:comment>
      <rdfs:comment>Examples:

the impressionists the Navajo the Greeks the peace protestors in New York City on February 15 2003 Exxon-Mobil King Solomon and his wives The President of the Swiss Confederation

</rdfs:comment>
      <rdfs:comment>Properties:

P107 has current or former member (is current or former member of): E39 Actor
(P107.1 kind of member: E55 Type)

</rdfs:comment>
      <rdfs:subClassOf>
         <owl:Restriction>
            <owl:onProperty>
               <owl:ObjectProperty rdf:about="http://erlangen-crm.org/current/P107_has_current_or_former_member"/>
            </owl:onProperty>
            <owl:someValuesFrom rdf:resource="http://erlangen-crm.org/current/E74_Group"/>
         </owl:Restriction>
      </rdfs:subClassOf>
   </owl:Class>
   <!--E77_Persistent_Item-->
   <owl:Class rdf:about="http://erlangen-crm.org/current/E77_Persistent_Item">
      <rdfs:label xml:lang="en">E77 Persistent Item</rdfs:label>
      <rdfs:subClassOf rdf:resource="http://erlangen-crm.org/current/E1_CRM_Entity"/>
      <rdfs:superClassOf rdf:resource="http://erlangen-crm.org/current/E39_Actor"/>
      <rdfs:superClassOf rdf:resource="http://erlangen-crm.org/current/E70_Thing"/>
      <rdfs:comment>Scope note:
This class comprises items that have a persistent identity, sometimes known as “endurants” in philosophy.

They can be repeatedly recognized within the duration of their existence by identity criteria rather than by continuity or observation. Persistent Items can be either physical entities, such as people, animals or things, or conceptual entities such as ideas, concepts, products of the imagination or common names.

The criteria that determine the identity of an item are often difficult to establish; the decision depends largely on the judgement of the observer. For example, a building is regarded as no longer existing if it is dismantled and the materials reused in a different configuration. On the other hand, human beings go through radical and profound changes during their life-span, affecting both material composition and form, yet preserve their identity by other criteria. Similarly, inanimate objects may be subject to exchange of parts and matter. The class E77 Persistent Item does not take any position about the nature of the applicable identity criteria and if actual knowledge about identity of an instance of this class exists. There may be cases, where the identity of an E77 Persistent Item is not decidable by a certain state of knowledge.
The main classes of objects that fall outside the scope the E77 Persistent Item class are temporal objects such as periods, events and acts, and descriptive properties.

</rdfs:comment>
      <rdfs:comment>Examples:

Leonard da Vinci Stonehenge the hole in the ozone layer the First Law of Thermodynamics the Bermuda Triangle

</rdfs:comment>
   </owl:Class>
   <!--E82_Actor_Appellation-->
   <owl:Class rdf:about="http://erlangen-crm.org/current/E82_Actor_Appellation">
      <rdfs:label xml:lang="en">E82 Actor Appellation</rdfs:label>
      <rdfs:subClassOf rdf:resource="http://erlangen-crm.org/current/E41_Appellation"/>
      <rdfs:comment>Scope note:
This class comprises any sort of name, number, code or symbol characteristically used to identify an E39 Actor.
An E39 Actor will typically have more than one E82 Actor Appellation, and instances of E82 Actor Appellation in turn may have alternative representations. The distinction between corporate and personal names, which is particularly important in library applications, should be made by explicitly linking the E82 Actor Appellation to an instance of either E21 Person or E74 Group/E40 Legal Body. If this is not possible, the distinction can be made through the use of the P2 has type mechanism.

</rdfs:comment>
      <rdfs:comment>Examples:

“John Doe” “Doe, J” “the U.S. Social Security Number 246-14-2304” “the Artist Formerly Known as Prince” “the Master of the Flemish Madonna” “Raphael’s Workshop” “the Brontë Sisters” “ICOM”
“International Council of Museums”

</rdfs:comment>
   </owl:Class>
   <!--E84_Information_Carrier-->
   <owl:Class rdf:about="http://erlangen-crm.org/current/E84_Information_Carrier">
      <rdfs:label xml:lang="en">E84 Information Carrier</rdfs:label>
      <rdfs:subClassOf rdf:resource="http://erlangen-crm.org/current/E22_Man-Made_Object"/>
      <rdfs:comment>Scope note:
This class comprises all instances of E22 Man-Made Object that are explicitly designed to act as persistent physical carriers for instances of E73 Information Object.
This allows a relationship to be asserted between an E19 Physical Object and its immaterial information contents. An E84 Information Carrier may or may not contain information, e.g., a diskette. Note that any E18 Physical Thing may carry information, such as an E34 Inscription. However, unless it was specifically designed for this purpose, it is not an Information Carrier. Therefore the property P128 carries (is carried by) applies to E18 Physical Thing in general.

</rdfs:comment>
      <rdfs:comment>Examples:

the Rosetta Stone my paperback copy of Crime &amp; Punishment the computer disk at ICS-FORTH that stores the canonical Definition of the CIDOC CRM

</rdfs:comment>
      <rdfs:subClassOf>
         <owl:Restriction>
            <owl:onProperty>
               <owl:ObjectProperty rdf:about="http://erlangen-crm.org/efrbroo/R31_is_reproduction_of"/>
            </owl:onProperty>
            <owl:maxCardinality rdf:datatype="http://www.w3.org/2001/XMLSchema#nonNegativeInteger">1</owl:maxCardinality>
         </owl:Restriction>
      </rdfs:subClassOf>
   </owl:Class>
   <!--E89_Propositional_Object-->
   <owl:Class rdf:about="http://erlangen-crm.org/current/E89_Propositional_Object">
      <rdfs:label xml:lang="en">E89 Propositional Object</rdfs:label>
      <rdfs:subClassOf rdf:resource="http://erlangen-crm.org/current/E28_Conceptual_Object"/>
      <rdfs:superClassOf rdf:resource="http://erlangen-crm.org/current/E73_Information_Object"/>
      <rdfs:superClassOf rdf:resource="http://erlangen-crm.org/current/E30_Right"/>
      <rdfs:comment>Scope note:
This class comprises immaterial items, including but not limited to stories, plots, procedural prescriptions, algorithms, laws of physics or images that are, or represent in some sense, sets of propositions about real or mental things and that are documented as single units or serve as topic of discourse.
This class also comprises items that are “about” something in the sense of a subject. In the wider sense, this class includes expressions of psychological value such as non-figural art and musical themes. However, conceptual items such as types and classes are not instances of E89 Propositional Object. This should not be confused with the definition of a type, which is indeed an instance of E89 Propositional Object.

</rdfs:comment>
      <rdfs:comment>Examples:

Maxwell’s Equations The ideational contents of Aristotle’s book entitled ‘Metaphysics’ as rendered in the Greek texts translated in … Oxford edition… The underlying prototype of any “no-smoking” sign (E36)
The common ideas of the plots of the movie “The Seven Samurai” by Akira Kurosawa and the movie “The Magnificent Seven” by John Sturges The image content of the photo of the Allied Leaders at Yalta 1945 (E38)

</rdfs:comment>
      <rdfs:comment>Properties:

P67 refers to (is referred to by): E1 CRM Entity
(P67.1 has type: E55 Type)
P129 is about (is subject of): E1 CRM Entity
P148 has component (is component of): E89 Propositional Object

</rdfs:comment>
      <rdfs:subClassOf>
         <owl:Restriction>
            <owl:onProperty>
               <owl:ObjectProperty rdf:about="http://erlangen-crm.org/current/P67_refers_to"/>
            </owl:onProperty>
            <owl:someValuesFrom rdf:resource="http://erlangen-crm.org/current/E89_Propositional_Object"/>
         </owl:Restriction>
      </rdfs:subClassOf>
      <rdfs:subClassOf>
         <owl:Restriction>
            <owl:onProperty>
               <owl:ObjectProperty rdf:about="http://erlangen-crm.org/current/P129_is_about"/>
            </owl:onProperty>
            <owl:someValuesFrom rdf:resource="http://erlangen-crm.org/current/E89_Propositional_Object"/>
         </owl:Restriction>
      </rdfs:subClassOf>
      <rdfs:subClassOf>
         <owl:Restriction>
            <owl:onProperty>
               <owl:ObjectProperty rdf:about="http://erlangen-crm.org/current/P148_has_component"/>
            </owl:onProperty>
            <owl:someValuesFrom rdf:resource="http://erlangen-crm.org/current/E89_Propositional_Object"/>
         </owl:Restriction>
      </rdfs:subClassOf>
   </owl:Class>
   <!--E90_Symbolic_Object-->
   <owl:Class rdf:about="http://erlangen-crm.org/current/E90_Symbolic_Object">
      <rdfs:label xml:lang="en">E90 Symbolic Object</rdfs:label>
      <rdfs:subClassOf rdf:resource="http://erlangen-crm.org/current/E28_Conceptual_Object"/>
      <rdfs:subClassOf rdf:resource="http://erlangen-crm.org/current/E72_Legal_Object"/>
      <rdfs:superClassOf rdf:resource="http://erlangen-crm.org/current/E73_Information_Object"/>
      <rdfs:superClassOf rdf:resource="http://erlangen-crm.org/current/E41_Appellation"/>
      <rdfs:comment>Scope note:
This class comprises identifiable symbols and any aggregation of symbols, such as characters, identifiers, traffic signs, emblems, texts, data sets, images, musical scores, multimedia objects, computer program code or mathematical formulae that have an objectively recognizable structure and that are documented as single units.
It includes sets of signs of any nature, which may serve to designate something, or to communicate some propositional content.
An instance of E90 Symbolic Object does not depend on a specific physical carrier, which can include human memory, and it can exist on one or more carriers simultaneously. An instance of E90 Symbolic Object may or may not have a specific meaning, for example an arbitrary character string.
In some cases, the content of an instance of E90 Symbolic Object may completely be represented by a serialized content model, such.. as the property P3 has note allows for describing this content model…P3.1 has type: E55 Type to specify the encoding..

</rdfs:comment>
      <rdfs:comment>Examples:

‘ecognizabl’ The “no-smoking” sign (E36)
‘BM000038850.JPG’ (E75) image BM000038850.JPG from the Clayton Herbarium in London (E38) The distribution of form, tone and colour found on Leonardo da Vinci’s painting named “Mona Lisa” (E38) The Italian text of Dante’s “Divina Commedia” as found in the authoritative critical edition La Commedia secondo l’antica 109ulgate a cura di Giorgio Petrocchi, Milano: Mondadori, 1966-67 (= Le Opere di Dante Alighieri, Edizione Nazionale a cura della Società Dantesca Italiana, VII, 1-4)(E33)

</rdfs:comment>
      <rdfs:comment>Properties:

P106 is composed of (forms part of): E90 Symbolic Object


</rdfs:comment>
      <rdfs:subClassOf>
         <owl:Restriction>
            <owl:onProperty>
               <owl:ObjectProperty rdf:about="http://erlangen-crm.org/current/P106_is_composed_of"/>
            </owl:onProperty>
            <owl:someValuesFrom rdf:resource="http://erlangen-crm.org/current/E90_Symbolic_Object"/>
         </owl:Restriction>
      </rdfs:subClassOf>
   </owl:Class>
   <!--

	- - Properties

        	-->
   <!--http://erlangen-crm.org/efrbroo/R1_is_logical_successor_of-->
   <owl:ObjectProperty rdf:about="http://erlangen-crm.org/efrbroo/R1_is_logical_successor_of">
      <rdfs:label xml:lang="en">R1 is logical successor of</rdfs:label>
      <owl:inverseOf rdf:resource="http://erlangen-crm.org/efrbroo/R1i_has_successor"/>
      <rdfs:domain rdf:resource="http://erlangen-crm.org/efrbroo/F1_Work"/>
      <rdfs:range rdf:resource="http://erlangen-crm.org/efrbroo/F1_Work"/>
      <rdfs:subPropertyOf rdf:resource="http://erlangen-crm.org/current/P130_shows_features_of"/>
      <rdfs:comment>Quantification:
(0,n:0,n)</rdfs:comment>
      <rdfs:comment>Scope note:
This property associates an instance of F1 Work which logically continues the content of another instance of F1 Work with the latter.</rdfs:comment>
      <rdfs:comment>Examples:
Albrecht Dürer’s woodcut from ‘The Large Woodcut Passion’ entitled ‘The Agony in the Garden’ (F1, conceived ca 1496-98) R1 is logical successor of Albrecht Dürer’s woodcut from ‘The Large Woodcut Passion’ entitled ‘The Last Supper’ (F1, dated 1510)The first ‘Star wars’ trilogy (F15, 1977-1983) R1 is logical successor of The second ‘Star wars’ trilogy (F15, 1999-2005) [Note that the logical order does not follow, in either of these two examples, the chronological order]</rdfs:comment>
   </owl:ObjectProperty>
   <!--http://erlangen-crm.org/efrbroo/R2_is_derivative_of-->
   <owl:ObjectProperty rdf:about="http://erlangen-crm.org/efrbroo/R2_is_derivative_of">
      <rdfs:label xml:lang="en">R2 is derivative of</rdfs:label>
      <owl:inverseOf rdf:resource="http://erlangen-crm.org/efrbroo/R2i_has_derivative"/>
      <rdfs:domain rdf:resource="http://erlangen-crm.org/efrbroo/F1_Work"/>
      <rdfs:range rdf:resource="http://erlangen-crm.org/efrbroo/F1_Work"/>
      <rdfs:subPropertyOf rdf:resource="http://erlangen-crm.org/current/P130_shows_features_of"/>
      <rdfs:comment>Quantification:
(0,n:0,n)</rdfs:comment>
      <rdfs:comment>Scope note:
This property associates an instance of F1 Work which modifies the content of another instance of F1 Work with the latter. The property R2.1 has type of this property allows for specifying the kind of derivation, such as adaptation, summarisation etc.</rdfs:comment>
      <rdfs:comment>Examples:
William Schuman’s orchestration of Charles Ives’s ‘Variations on America’ (F15) R2 is derivative of Charles Ives’s ‘Variations on America’ (F15) R2.1 has type orchestration (E55)Charles Ives’s musical work entitled ‘Variations on America’ (F15) R2 is derivative of the musical work titled ‘America’ (F15) R2.1 has type variations (E55)The musical work entitled ‘America’ (F15) R2 is derivative of the musical work entitled ‘God save the King’ (F15) R2.1 has type same tune with different lyrics (E55)Properties:R2.1 has type: E55 Type</rdfs:comment>
   </owl:ObjectProperty>
   <!--http://erlangen-crm.org/efrbroo/R3_is_realised_in-->
   <owl:ObjectProperty rdf:about="http://erlangen-crm.org/efrbroo/R3_is_realised_in">
      <rdfs:label xml:lang="en">R3 is realised in</rdfs:label>
      <owl:inverseOf rdf:resource="http://erlangen-crm.org/efrbroo/R3i_realises"/>
      <rdfs:domain rdf:resource="http://erlangen-crm.org/efrbroo/F1_Work"/>
      <rdfs:range rdf:resource="http://erlangen-crm.org/efrbroo/F22_Self-Contained_Expression"/>
      <rdfs:superPropertyOf rdf:resource="http://erlangen-crm.org/efrbroo/R9_is_realised_in"/>
      <rdfs:superPropertyOf rdf:resource="http://erlangen-crm.org/efrbroo/R12_is_realised_in"/>
      <rdfs:superPropertyOf rdf:resource="http://erlangen-crm.org/efrbroo/R13_is_realised_in"/>
      <rdfs:superPropertyOf rdf:resource="http://erlangen-crm.org/efrbroo/R40_has_representative_expression"/>
      <rdfs:subPropertyOf rdf:resource="http://erlangen-crm.org/current/P130_shows_features_of"/>
      <rdfs:comment>Quantification:
(0,n:1,1)</rdfs:comment>
      <rdfs:comment>Scope note:
This property associates an instance of F22 Self-Contained Expression with an instance of F1 Work.This property expresses the association that exists between an expression (F22) and the work that this expression conveys. The semantics of the association will be different depending on what specific subtype of F1 Work the work is an instance of. If the work is an instance of F14 Individual Work, the F22 Self-Contained Expression completely conveys the individual work. If the work is an instance of F15 Complex Work, the F22 Self-Contained Expression conveys an alternative member of the complex work.Our factual knowledge of how a given work is realised into an expression is often limited and this property makes it possible to express the association between instances of F22 Self-Contained Expression and the work it conveys without using the more developed paths.The property R3.1 has type: E55 Type allows for specifying the role played by the referred to expression in the overall bibliographic history of the work (e.g., ‘progenitor expression’, on which all other expressions of the same work are based; ‘reference for canonical citations’, in the sense of the HuCit ontology developed by Matteo Romanello and Michele Pasin; ‘earliest draft’, ‘intermediate draft’, ‘final clean draft’, ‘princeps edition’, etc.).</rdfs:comment>
      <rdfs:comment>Examples:
Dante’s work entitled ‘Inferno’ (F15) R3 is realised in the Italian text of Dante’s ‘Inferno’ as found in the authoritative critical edition La Commedia secondo l’antica vulgata a cura di Giorgio Petrocchi, Milano: Mondadori, 1966-67 (= Le Opere di Dante Alighieri, Edizione Nazionale a cura della Società Dantesca Italiana, VII, 1-4) (F22) R3.1 has type authoritative critical edition (E55)Mozart’s work entitled ‘Il dissoluto punito ossia il Don Giovanni’ (F15) R3 is realised in the notated music of the Prague version, as found on manuscript Ms 1548 of the National Library of France (F22) R3.1 has type autograph version (E55)Properties:R3.1 has type: E55 Type</rdfs:comment>
   </owl:ObjectProperty>
   <!--http://erlangen-crm.org/efrbroo/R4_carriers_provided_by-->
   <owl:ObjectProperty rdf:about="http://erlangen-crm.org/efrbroo/R4_carriers_provided_by">
      <rdfs:label xml:lang="en">R4 carriers provided by</rdfs:label>
      <owl:inverseOf rdf:resource="http://erlangen-crm.org/efrbroo/R4i_comprises_carriers_of"/>
      <rdfs:domain rdf:resource="http://erlangen-crm.org/efrbroo/F2_Expression"/>
      <rdfs:range rdf:resource="http://erlangen-crm.org/efrbroo/F3_Manifestation_Product_Type"/>
      <rdfs:superPropertyOf rdf:resource="http://erlangen-crm.org/efrbroo/R41_has_representative_manifestation_product_type"/>
      <rdfs:subPropertyOf rdf:resource="http://erlangen-crm.org/current/P128i_is_carried_by"/>
      <rdfs:comment>Quantification:
(1,n:0,n)</rdfs:comment>
      <rdfs:comment>Scope note:
This property associates a publication, i.e. an instance of F3 Manifestation Product Type, with an instance of F2 Expression, which all exemplars of that publication should carry, as long as they are recognised as complete exemplars of that publication. Typically, this property is observed on one exemplar of a publication, and extrapolated to all other exemplars of the same publication.This property is a shortcut of: F2 Expression P165i is incorporated in F24 Publication Expression CLR6i should be carried by F3 Manifestation Product Type.</rdfs:comment>
      <rdfs:comment>Examples:
The text of Marin Mersenne’s ‘Harmonie universelle’ (F22) R4 carriers provided by publication identified by ISBN ‘2-222-00835-2’ (F3)A recording of the Atrium Musicæ Ensemble’s performance of a fragment of Euripides’ textual and musical work entitled ‘Orestes’ (F26) R4 carriers provided by the CD entitled ‘Musique de la Grèce antique = Ancient Greek music = Griechische Musik der Antike’, released in 2000 and identified by UPC/EAN ‘794881601622’ (F3)</rdfs:comment>
   </owl:ObjectProperty>
   <!--http://erlangen-crm.org/efrbroo/R5_has_component-->
   <owl:ObjectProperty rdf:about="http://erlangen-crm.org/efrbroo/R5_has_component">
      <rdfs:label xml:lang="en">R5 has component</rdfs:label>
      <owl:inverseOf rdf:resource="http://erlangen-crm.org/efrbroo/R5i_is_component_of"/>
      <rdfs:domain rdf:resource="http://erlangen-crm.org/efrbroo/F2_Expression"/>
      <rdfs:range rdf:resource="http://erlangen-crm.org/efrbroo/F22_Self-Contained_Expression"/>
      <rdfs:subPropertyOf rdf:resource="http://erlangen-crm.org/current/P148_has_component"/>
      <rdfs:comment>Quantification:
(0,n:0,n)</rdfs:comment>
      <rdfs:comment>Scope note:
This property associates an F2 Expression X with a structural component Y that conveys in itself the complete concept of a work that is member of (R10) the overall work realized by X.It does not cover the relationship that exists between pre-existing expressions that are re-used in a new, larger expression and that new, larger expression. Such a relationship is modelled by P165 incorporates.</rdfs:comment>
      <rdfs:comment>Examples:
The Italian text of Dante’s textual work entitled ‘Divina Commedia’ (F22) R5 has component the Italian text of Dante’s textual work entitled ‘Inferno’ (F22)The musical notation of Mozart’s Singspiel entitled ‘Die Zauberflöte’ (F22) R5 has component the musical notation of Mozart’s aria entitled ‘Der Hölle Rache’, also known as ‘The Queen of the Night’s Aria’ (F22)The visual content of the map entitled ‘Wales – The Midlands – South West England’, scale 1:400,000, issued by Michelin in 2005 (F22) R5 has component the visual content of the inset entitled ‘Liverpool’, scale 1:200,000, set within the compass of the map titled ‘Wales – The Midlands – South West England’, scale 1:400,000, issued by Michelin in 2005 (F22)</rdfs:comment>
   </owl:ObjectProperty>
   <!--http://erlangen-crm.org/efrbroo/R6_carries-->
   <owl:ObjectProperty rdf:about="http://erlangen-crm.org/efrbroo/R6_carries">
      <rdfs:label xml:lang="en">R6 carries</rdfs:label>
      <owl:inverseOf rdf:resource="http://erlangen-crm.org/efrbroo/R6i_is_carried_by"/>
      <rdfs:domain rdf:resource="http://erlangen-crm.org/efrbroo/F54_Utilised_Information_Carrier"/>
      <rdfs:range rdf:resource="http://erlangen-crm.org/efrbroo/F24_Publication_Expression"/>
      <rdfs:subPropertyOf rdf:resource="http://erlangen-crm.org/current/P128_carries"/>
      <rdfs:comment>Quantification:
(1,1:0,n)</rdfs:comment>
      <rdfs:comment>Scope note:
This property associates an instance of F54 Utilised Information Carrier with the unique instance of F24 Publication Expression it carries.</rdfs:comment>
      <rdfs:comment>Examples:
The British Library’s holding identified by shelfmark ‘DSC 9078.177 vol 19’ (F5) R6 carries the entire content (text, layout, publisher logo, etc.) of the publication entitled ‘Functional Requirements for Bibliographic Records: final report’, issued by publisher named ‘K. G. Saur’ in 1998 (F24)</rdfs:comment>
   </owl:ObjectProperty>
   <!--http://erlangen-crm.org/efrbroo/R7_is_example_of-->
   <owl:ObjectProperty rdf:about="http://erlangen-crm.org/efrbroo/R7_is_example_of">
      <rdfs:label xml:lang="en">R7 is example of</rdfs:label>
      <owl:inverseOf rdf:resource="http://erlangen-crm.org/efrbroo/R7i_has_example"/>
      <rdfs:domain rdf:resource="http://erlangen-crm.org/efrbroo/F5_Item"/>
      <rdfs:range rdf:resource="http://erlangen-crm.org/efrbroo/F3_Manifestation_Product_Type"/>
      <rdfs:subPropertyOf rdf:resource="http://erlangen-crm.org/current/P2_has_type"/>
      <rdfs:comment>Quantification:
(1,1:0,n)</rdfs:comment>
      <rdfs:comment>Scope note:
This property associates a publication with one of its exemplars.It is a shortcut of the more developed path: F5 Item R28i was produced by F32 Carrier Production R26 produced things of type (was produced by): F3 Manifestation Product Type.</rdfs:comment>
      <rdfs:comment>Examples:
The item held by the National Library of France and identified by shelf mark ‘Res 8 P 10’ (F5) R7 is example of the edition of Amerigo Vespucci’s textual and cartographic work entitled ‘Mundus novus’ issued in Paris ca. 1503-1504 (F3)</rdfs:comment>
   </owl:ObjectProperty>
   <!--http://erlangen-crm.org/efrbroo/R8_consists_of-->
   <owl:ObjectProperty rdf:about="http://erlangen-crm.org/efrbroo/R8_consists_of">
      <rdfs:label xml:lang="en">R8 consists of</rdfs:label>
      <owl:inverseOf rdf:resource="http://erlangen-crm.org/efrbroo/R8i_forms_part_of"/>
      <rdfs:domain rdf:resource="http://erlangen-crm.org/efrbroo/F13_Identifier"/>
      <rdfs:range rdf:resource="http://erlangen-crm.org/current/E90_Symbolic_Object"/>
      <rdfs:subPropertyOf rdf:resource="http://erlangen-crm.org/current/P106_is_composed_of"/>
      <rdfs:comment>Quantification:
(0,n:0,n)</rdfs:comment>
      <rdfs:comment>Scope note:
This property associates an instance of F13 Identifier with one of the non-syntactic instances of E90 Symbolic Object which form part of it.</rdfs:comment>
      <rdfs:comment>Examples:
Controlled access point ‘The Adoration of the Shepherds (Coventry)’ (F50) R8 consists of ‘The Adoration of the Shepherds’ (E35), and R8 consists of ‘Coventry’ (E48)Controlled access point ‘Rite of spring (Choreographic Work : Bausch)’ (F50) R8 consists of ‘Rite of spring’ (E35), R8 consists of ‘Choreographic Work’ (F12), and R8 consists of ‘Bausch’ (F12)Controlled access point ‘King Kong (1933)’ (F50) R8 consists of ‘King Kong’ (E35), and R8 consists of ‘1933’ (E50)Controlled access point ‘Guillaume, de Machaut, ca. 1300-1377’ (F50) R8 consists of ‘Guillaume, de Machaut’ (F12), and R8 consists of ‘ca. 1300-1377’ (E90)Controlled access point ‘Univerza v Ljubljani. Oddelek za bibliotekarstvo’ (F50) R8 consists of ‘Univerza v Ljubljani’ (F12), and R8 consists of ‘Oddelek za bibliotekarstvo’ (F12)ISBN ‘978-002-002-0’ (F13) R8 consists of ‘978’ (E90) indicating the Nigerian ISBN Agency, R8 consists of ‘002’ (E90) indicating the Nigerian Institute of International Affairs, R8 consists of ‘002’ (E90) used for the publication entitled ‘Nigeria’s international economic relations’, and R8 consists of ‘0’ (E90)</rdfs:comment>
   </owl:ObjectProperty>
   <!--http://erlangen-crm.org/efrbroo/R9_is_realised_in-->
   <owl:ObjectProperty rdf:about="http://erlangen-crm.org/efrbroo/R9_is_realised_in">
      <rdfs:label xml:lang="en">R9 is realised in</rdfs:label>
      <owl:inverseOf rdf:resource="http://erlangen-crm.org/efrbroo/R9i_realises"/>
      <rdfs:domain rdf:resource="http://erlangen-crm.org/efrbroo/F14_Individual_Work"/>
      <rdfs:range rdf:resource="http://erlangen-crm.org/efrbroo/F22_Self-Contained_Expression"/>
      <rdfs:subPropertyOf rdf:resource="http://erlangen-crm.org/efrbroo/R3_is_realised_in"/>
      <rdfs:comment>Quantification:
(1,1:1,1)</rdfs:comment>
      <rdfs:comment>Scope note:
This property associates an F14 Individual Work with the unique F22 Self-Contained Expression that completely conveys it.It is a shortcut for the more developed path: F14 Individual Work R19i was realised through F28 Expression Creation R17 created F22 Self-Contained Expression.</rdfs:comment>
      <rdfs:comment>Examples:
Abstract content of Giovanni Battista Piranesi’s graphic work entitled ‘Carcere XVI: the pier with chains: 2nd state’ (F14) R9 is realised in Giovanni Battista Piranesi’s graphic work entitled ‘Carcere XVI: the pier with chains: 2nd state’ (F22)Abstract content of the English text of the 1855 edition of Walt Whitman’s textual work entitled ‘Leaves of Grass’ (F14) R9 is realised in the English text of the 1855 edition of Walt Whitman’s textual work entitled ‘Leaves of Grass’ (F22)</rdfs:comment>
   </owl:ObjectProperty>
   <!--http://erlangen-crm.org/efrbroo/R10_has_member-->
   <owl:ObjectProperty rdf:about="http://erlangen-crm.org/efrbroo/R10_has_member">
      <rdfs:label xml:lang="en">R10 has member</rdfs:label>
      <owl:inverseOf rdf:resource="http://erlangen-crm.org/efrbroo/R10i_is_member_of"/>
      <rdfs:domain rdf:resource="http://erlangen-crm.org/efrbroo/F15_Complex_Work"/>
      <rdfs:range rdf:resource="http://erlangen-crm.org/efrbroo/F1_Work"/>
      <rdfs:subPropertyOf rdf:resource="http://erlangen-crm.org/current/P148_has_component"/>
      <rdfs:comment>Quantification:
(2,n:0,n)</rdfs:comment>
      <rdfs:comment>Scope note:
This property associates an instance of F15 Complex Work with an instance of F1 Work that forms part of it.</rdfs:comment>
      <rdfs:comment>Examples:
Dante’s textual work entitled ‘Divina Commedia’ (F15) R10 has member Dante’s textual work entitled ‘Inferno’ (F15)Dante’s textual work entitled ‘Inferno’ (F15) R10 has member the abstract content of the pseudo-old French text of Émile Littré’s translation entitled ‘L’Enfer mis en vieux langage françois et en vers’ [a 19th century translation of Dante’s ‘Inferno’ into old French] published in Paris in 1879 (F14)Giovanni Battista Piranesi’s graphic work entitled ‘Carceri’ (F15) R10 has member Giovanni Battista Piranesi’s graphic work entitled ‘Carcere XVI: the pier with chains’ (F15)Giovanni Battista Piranesi’s graphic work entitled ‘Carcere XVI: the pier with chains’ (F15) R10 has member the abstract content of Giovanni Battista Piranesi’s graphic work entitled ‘Carcere XVI: the pier with chains: 2nd state’ (F14)</rdfs:comment>
   </owl:ObjectProperty>
   <!--http://erlangen-crm.org/efrbroo/R11_has_issuing_rule-->
   <owl:ObjectProperty rdf:about="http://erlangen-crm.org/efrbroo/R11_has_issuing_rule">
      <rdfs:label xml:lang="en">R11 has issuing rule</rdfs:label>
      <owl:inverseOf rdf:resource="http://erlangen-crm.org/efrbroo/R11i_is_issuing_rule_of"/>
      <rdfs:domain rdf:resource="http://erlangen-crm.org/efrbroo/F18_Serial_Work"/>
      <rdfs:range rdf:resource="http://erlangen-crm.org/current/E29_Design_or_Procedure"/>
      <rdfs:comment>Quantification:
(0,n:0,n)</rdfs:comment>
      <rdfs:comment>Scope note:
This property associates an instance of F18 Serial Work with the instance of E29 Design or Procedure that specifies the issuing policy planned by this Work, such as sequencing pattern, expected frequency and expected regularity.This property is a shortcut of the full path: F18 Serial Work R23i was realised through F30 Publication Event P16 used specific object E29 Design or Procedure.</rdfs:comment>
      <rdfs:comment>Examples:
The serial entitled ‘Quarterly journal of pure and applied mathematics’, identified by ISSN ‘1549-6724’ (F18) R11 has issuing rule to be issued every three months, on a regular basis, with each issue being numbered according to the pattern ‘Vol. 1, no. 1 (2005)’ that was observed by the Library of Congress’s cataloguers on an exemplar of the first issue (E29)</rdfs:comment>
   </owl:ObjectProperty>
   <!--http://erlangen-crm.org/efrbroo/R12_is_realised_in-->
   <owl:ObjectProperty rdf:about="http://erlangen-crm.org/efrbroo/R12_is_realised_in">
      <rdfs:label xml:lang="en">R12 is realised in</rdfs:label>
      <owl:inverseOf rdf:resource="http://erlangen-crm.org/efrbroo/R12i_realises"/>
      <rdfs:domain rdf:resource="http://erlangen-crm.org/efrbroo/F20_Performance_Work"/>
      <rdfs:range rdf:resource="http://erlangen-crm.org/efrbroo/F25_Performance_Plan"/>
      <rdfs:subPropertyOf rdf:resource="http://erlangen-crm.org/efrbroo/R3_is_realised_in"/>
      <rdfs:comment>Quantification:
(0,n:1,1)</rdfs:comment>
      <rdfs:comment>Scope note:
This property associates an instance of F20 Performance Work with an instance of F25 Performance Plan that consists of signs (words, figures, etc.) which express the directions the instance of F20 Performance Work consists of.</rdfs:comment>
      <rdfs:comment>Examples:
The concept of Sergei Radlov’s mise-en-scène of a Yiddish translation of the textual work entitled ‘King Lear’ in Moscow in 1935 (F20) R12 is realised in the set of instructions for the production of a Yiddish translation of the textual work entitled ‘King Lear’, as directed by Sergei Radlov in Moscow in 1935 (F25)The concept of Pina Bausch’s choreography of the ballet entitled ‘Rite of spring’ in Wuppertal in 1975 (F20) R12 is realised in the set of instructions for the production of the ballet entitled ‘Rite of spring’, as choreographed by Pina Bausch in Wuppertal in 1975 (F25)The concept of Bruno Walter’s performance of Gustav Mahler’s 9th symphony in 1961 (F20) R12 is realised in the set of instructions by Bruno Walter for performing Gustav Mahler’s 9th symphony, delivered by him to the Columbia Symphony Orchestra during rehearsals in Hollywood in 1961 (as partially documented in the CD entitled ‘Bruno Walter conducts and talks about Mahler symphony No. 9: rehearsal &amp; performance’) (F25)The concept of the “performance handbook” for Luigi Nono’s musical work entitled ‘À Pierre’ (F20) R12 is realised in the set of instructions contained in the performance handbook for Luigi Nono’s musical work entitled ‘À Pierre’ (F25)</rdfs:comment>
   </owl:ObjectProperty>
   <!--http://erlangen-crm.org/efrbroo/R13_is_realised_in-->
   <owl:ObjectProperty rdf:about="http://erlangen-crm.org/efrbroo/R13_is_realised_in">
      <rdfs:label xml:lang="en">R13 is realised in</rdfs:label>
      <owl:inverseOf rdf:resource="http://erlangen-crm.org/efrbroo/R13i_realises"/>
      <rdfs:domain rdf:resource="http://erlangen-crm.org/efrbroo/F21_Recording_Work"/>
      <rdfs:range rdf:resource="http://erlangen-crm.org/efrbroo/F26_Recording"/>
      <rdfs:subPropertyOf rdf:resource="http://erlangen-crm.org/efrbroo/R3_is_realised_in"/>
      <rdfs:comment>Quantification:
(0,n:0,1)</rdfs:comment>
      <rdfs:comment>Scope note:
This property associates an instance of F21 Recording Work with an instance of F26 Recording realising the instance of F21 Recording Work.This is a shortcut of the more elaborated path through R22 was realised through, F29 Recording Event and R21 created, which should be used when information about the recording event is available.</rdfs:comment>
      <rdfs:comment>Examples:
The concept of the third alternate take of the musical work entitled ‘Blue Hawaii’ as performed by Elvis Presley in Hollywood, Calif., Radio Recorders, on March 22nd, 1961 (F21) R13 is realised in the set of signs that make up the third alternate take of the musical work entitled ‘Blue Hawaii’ as performed by Elvis Presley in Hollywood, Calif., Radio Recorders, on March 22nd, 1961 (F26)The concept of making a photograph of the three Allied leaders at Yalta in February 1945 (F21) R13 is realised in the visual content of the famous photograph of the three Allied leaders at Yalta in February 1945 (F26)Oceania Project’s concept of making a large digital acoustic data archive dedicated to East Australian humpback whale songs (F21) R13 is realised in the audio content of the album entitled ‘Songlines – Songs of the East Australian Humpback Whales’ released in 2011 (F26)The concept of recording Louise Bourgeois’s artistic activity in the documentary movie entitled ‘Louise Bourgeois: The Spider, the Mistress, and the Tangerine’ (F21) R13 is realised in the audiovisual content of the documentary movie entitled ‘Louise Bourgeois: The Spider, the Mistress, and the Tangerine’ (F26)</rdfs:comment>
   </owl:ObjectProperty>
   <!--http://erlangen-crm.org/efrbroo/R15_has_fragment-->
   <owl:ObjectProperty rdf:about="http://erlangen-crm.org/efrbroo/R15_has_fragment">
      <rdfs:label xml:lang="en">R15 has fragment</rdfs:label>
      <owl:inverseOf rdf:resource="http://erlangen-crm.org/efrbroo/R15i_is_fragment_of"/>
      <rdfs:domain rdf:resource="http://erlangen-crm.org/efrbroo/F2_Expression"/>
      <rdfs:range rdf:resource="http://erlangen-crm.org/efrbroo/F23_Expression_Fragment"/>
      <rdfs:subPropertyOf rdf:resource="http://erlangen-crm.org/current/P106_is_composed_of"/>
      <rdfs:comment>Quantification:
(0,n:0,n)</rdfs:comment>
      <rdfs:comment>Scope note:
This property associates the fragment of an expression and the expression of which it is a fragment.</rdfs:comment>
      <rdfs:comment>Examples:
The ancient Greek text of the four stanzas from an ode by Sappho that were quoted by Pseudo-Longinus in his textual work entitled ‘On the sublime’ (F23) R15 is fragment of the complete ancient Greek text, now irremediably lost, of Sappho’s ode currently identified as Sappho’s poem #2 (F22)The statement ‘fasc. 111’ (abridgement for ‘fascicle no. 111’) indicating the sequential position of the publication identified by ISBN ‘2-7018-0037-4’ within the series entitled ‘Bibliothèque des Écoles françaises d’Athènes et de Rome’ and identified by ISSN ‘0257-4101’ (F23) R15 is fragment of the overall content of the publication identified by ISBN ‘2-7018-0037-4’ (F24)</rdfs:comment>
   </owl:ObjectProperty>
   <!--http://erlangen-crm.org/efrbroo/R16_initiated-->
   <owl:ObjectProperty rdf:about="http://erlangen-crm.org/efrbroo/R16_initiated">
      <rdfs:label xml:lang="en">R16 initiated</rdfs:label>
      <owl:inverseOf rdf:resource="http://erlangen-crm.org/efrbroo/R16i_was_initiated_by"/>
      <rdfs:domain rdf:resource="http://erlangen-crm.org/efrbroo/F27_Work_Conception"/>
      <rdfs:range rdf:resource="http://erlangen-crm.org/efrbroo/F1_Work"/>
      <rdfs:subPropertyOf rdf:resource="http://erlangen-crm.org/current/P94_has_created"/>
      <rdfs:comment>Quantification:
(1,n:1,1)</rdfs:comment>
      <rdfs:comment>Scope note:
This property associates the first conception of a work and the work itself that ensued from a given initial idea.It marks the origin of the causality chain that results in a work’s coming into existence.</rdfs:comment>
      <rdfs:comment>Examples:
Ludwig van Beethoven’s decision to compose a fifth symphony (F27) R16 initiated Ludwig van Beethoven’s Fifth Symphony (F15)Pablo Picasso’s acceptance, in 1930, of Ambroise Vollard’s commission for a set of 100 etchings, now known as the ‘Vollard Suite’ (F27) R16 initiated the ‘Vollard Suite’ (F15)René Goscinny’s and Albert Uderzo’s decision to collaborate on the comic book entitled ‘Asterix in Britain’ (F27) R16 initiated the comic book entitled ‘Asterix in Britain’ (F15)The creative spark that motivated Oscar Wilde, by May 1897, to write a poem inspired by his stay in the Reading prison in 1895-1897 (F27) R16 initiated Oscar Wilde’s poem entitled ‘The ballad of the Reading gaol’ (F15)</rdfs:comment>
   </owl:ObjectProperty>
   <!--http://erlangen-crm.org/efrbroo/R17_created-->
   <owl:ObjectProperty rdf:about="http://erlangen-crm.org/efrbroo/R17_created">
      <rdfs:label xml:lang="en">R17 created</rdfs:label>
      <owl:inverseOf rdf:resource="http://erlangen-crm.org/efrbroo/R17i_was_created_by"/>
      <rdfs:domain rdf:resource="http://erlangen-crm.org/efrbroo/F28_Expression_Creation"/>
      <rdfs:range rdf:resource="http://erlangen-crm.org/efrbroo/F2_Expression"/>
      <rdfs:superPropertyOf rdf:resource="http://erlangen-crm.org/efrbroo/R21_created"/>
      <rdfs:superPropertyOf rdf:resource="http://erlangen-crm.org/efrbroo/R24_created"/>
      <rdfs:subPropertyOf rdf:resource="http://erlangen-crm.org/current/P94_has_created"/>
      <rdfs:comment>Quantification:
(1,1:1,n)</rdfs:comment>
      <rdfs:comment>Scope note:
This property associates the expression that was first externalised during a particular creation event with that particular creation event.</rdfs:comment>
      <rdfs:comment>Examples:
Richard Wagner’s writing the original manuscript of his opera entitled ‘Der fliegende Holländer’ (F28) R17 created the notational content of the original manuscript of Richard Wagner’s opera entitled ‘Der fliegende Holländer’ (F22)Oscar Wilde’s writing the original manuscript of his poem entitled ‘The ballad of the Reading gaol’ (F28) R17 created the English text of Oscar Wilde’s poem entitled ‘The ballad of the Reading gaol’ (F22)</rdfs:comment>
   </owl:ObjectProperty>
   <!--http://erlangen-crm.org/efrbroo/R18_created-->
   <owl:ObjectProperty rdf:about="http://erlangen-crm.org/efrbroo/R18_created">
      <rdfs:label xml:lang="en">R18 created</rdfs:label>
      <owl:inverseOf rdf:resource="http://erlangen-crm.org/efrbroo/R18i_was_created_by"/>
      <rdfs:domain rdf:resource="http://erlangen-crm.org/efrbroo/F28_Expression_Creation"/>
      <rdfs:range rdf:resource="http://erlangen-crm.org/efrbroo/F4_Manifestation_Singleton"/>
      <rdfs:subPropertyOf rdf:resource="http://erlangen-crm.org/current/P108_has_produced"/>
      <rdfs:comment>Quantification:
(1,n:0,1)</rdfs:comment>
      <rdfs:comment>Scope note:
This property associates an instance of F28 Expression Creation with the first physical objects in which the resulting instance of F2 Expression was embodied.</rdfs:comment>
      <rdfs:comment>Examples:
Emily Dickinson’s creating the text of one of the several extant versions of her poem known as ‘Safe in their alabaster chambers’ (F28) R18 created the manuscript now identified as ‘Massachusetts Cambridge Harvard University Houghton Library bMS Am 1118.3 (203c, 203d)’ (F4)Emily Dickinson’s creating the text of another one of the several extant versions of her poem known as ‘Safe in their alabaster chambers’ (F28) R18 created the manuscript now identified as ‘Massachusetts Cambridge Harvard University Houghton Library bMS Am 1118.5 (74c)’ (F4)The recording of the third alternate take of the musical work entitled ‘Blue Hawaii’ performed by Elvis Presley in Hollywood, Calif., Radio Recorders, on March 22nd, 1961 (F28) R18 created the master tape of the 3rd alternate take of the musical work entitled ‘Blue Hawaii’ performed by Elvis Presley in Hollywood, Calif., Radio Recorders, on March 22nd, 1961 (F4) (each individual take is a distinct expression)The resource (a drawing) held by the New York Public Library and identified by call number ‘*MGZGB Far P Cop 1’ (F4) R18i was created by the creation, by the artist named ‘Peter Farmer’, of a costume design for the character named ‘War’ in the Act III Masque of the seasons, in the Festival Ballet of London production of the choreographic work entitled ‘Coppélia’, with choreography by Jack Carter after Petipa (F28)</rdfs:comment>
   </owl:ObjectProperty>
   <!--http://erlangen-crm.org/efrbroo/R19_created_a_realisation_of-->
   <owl:ObjectProperty rdf:about="http://erlangen-crm.org/efrbroo/R19_created_a_realisation_of">
      <rdfs:label xml:lang="en">R19 created a realisation of</rdfs:label>
      <owl:inverseOf rdf:resource="http://erlangen-crm.org/efrbroo/R19i_was_realised_through"/>
      <rdfs:domain rdf:resource="http://erlangen-crm.org/efrbroo/F28_Expression_Creation"/>
      <rdfs:range rdf:resource="http://erlangen-crm.org/efrbroo/F1_Work"/>
      <rdfs:superPropertyOf rdf:resource="http://erlangen-crm.org/efrbroo/R22_created_a_realisation_of"/>
      <rdfs:superPropertyOf rdf:resource="http://erlangen-crm.org/efrbroo/R23_created_a_realisation_of"/>
      <rdfs:subPropertyOf rdf:resource="http://erlangen-crm.org/current/P16_used_specific_object"/>
      <rdfs:comment>Quantification:
(1,n:1,1)</rdfs:comment>
      <rdfs:comment>Scope note:
This property associates an instance of F28 Expression Creation with the corresponding instance of F14 Individual Work or an instance of F15 Complex Work of which the corresponding instance of F14 Individual Work is a member.</rdfs:comment>
      <rdfs:comment>Examples:
Giovanni Battista Piranesi’s creating the image identified as ‘Carcere XVI: the pier with chains: 2nd state’ (F28) R19 created a realisation of the concept of Giovanni Battista Piranesi’s graphic work entitled ‘Carcere XVI: the pier with chains: 2nd state’ (F14)Recording Glenn Gould’s performance of Johann Sebastian Bach’s musical work entitled ‘Toccata in C minor BWV 911’ on May 15 &amp; 16, 1979, in Toronto, Eaton’s Auditorium (F29) R19 created a realisation of the concept of the recorded performance of Johann Sebastian Bach’s musical work entitled ‘Toccata in C minor BWV 911’ by Glenn Gould on May 15 &amp; 16, 1979, in Toronto, Eaton’s Auditorium (F21)</rdfs:comment>
   </owl:ObjectProperty>
   <!--http://erlangen-crm.org/efrbroo/R20_recorded-->
   <owl:ObjectProperty rdf:about="http://erlangen-crm.org/efrbroo/R20_recorded">
      <rdfs:label xml:lang="en">R20 recorded</rdfs:label>
      <owl:inverseOf rdf:resource="http://erlangen-crm.org/efrbroo/R20i_was_recorded_through"/>
      <rdfs:domain rdf:resource="http://erlangen-crm.org/efrbroo/F29_Recording_Event"/>
      <rdfs:range rdf:resource="http://erlangen-crm.org/current/E2_Temporal_Entity"/>
      <rdfs:subPropertyOf rdf:resource="http://erlangen-crm.org/current/P15_was_influenced_by"/>
      <rdfs:comment>Quantification:
(1,n:0,n)</rdfs:comment>
      <rdfs:comment>Scope note:
This property associates an instance of F29 Recording Event with the instance of E2 Temporal Entity which was captured.</rdfs:comment>
      <rdfs:comment>Examples:
The making of the recording of the third alternate take of the musical work entitled ‘Blue Hawaii’ as performed by Elvis Presley in Hollywood, Calif., Radio Recorders, on March 22nd, 1961 (F29) R20 recorded Elvis Presley’s performance of the musical work entitled ‘Blue Hawaii’ in Hollywood, Calif., Radio Recorders, on March 22nd, 1961 (F31)</rdfs:comment>
   </owl:ObjectProperty>
   <!--http://erlangen-crm.org/efrbroo/R21_created-->
   <owl:ObjectProperty rdf:about="http://erlangen-crm.org/efrbroo/R21_created">
      <rdfs:label xml:lang="en">R21 created</rdfs:label>
      <owl:inverseOf rdf:resource="http://erlangen-crm.org/efrbroo/R21i_was_created_through"/>
      <rdfs:domain rdf:resource="http://erlangen-crm.org/efrbroo/F29_Recording_Event"/>
      <rdfs:range rdf:resource="http://erlangen-crm.org/efrbroo/F26_Recording"/>
      <rdfs:subPropertyOf rdf:resource="http://erlangen-crm.org/efrbroo/R17_created"/>
      <rdfs:comment>Quantification:
(1,n:1,n)</rdfs:comment>
      <rdfs:comment>Scope note:
This property associates an instance of F29 Recording Event with the instance of F26 Recording that was created.</rdfs:comment>
      <rdfs:comment>Examples:
The making of the recording of the third alternate take of the musical work entitled ‘Blue Hawaii’ as performed by Elvis Presley in Hollywood, Calif., Radio Recorders, on March 22nd, 1961 (F29) R21 created the set of signs that make up the third alternate take of the musical work entitled ‘Blue Hawaii’ as performed by Elvis Presley in Hollywood, Calif., Radio Recorders, on March 22nd, 1961 (F26)The making of the photograph of the three Allied leaders at Yalta in February 1945 (F29) R21 created the set of signs that make up the famous photograph of the three Allied leaders at Yalta in February 1945 (F26)The making of the recording of an East Australian humpback whale song in 1994 in the framework of the Oceania Project (F29) R21 created the set of signs that make up the sound recording of an East Australian humpback whale song in 1994 (F26)Filming Louise Bourgeois at work in the context of the shooting of the documentary movie entitled ‘Louise Bourgeois: The Spider, the Mistress, and the Tangerine’ (F29) R21 created the set of signs that make up the sequences from the documentary movie entitled ‘Louise Bourgeois: The Spider, the Mistress, and the Tangerine’ in which Louise Bourgeois is seen at work (F26)</rdfs:comment>
   </owl:ObjectProperty>
   <!--http://erlangen-crm.org/efrbroo/R22_created_a_realisation_of-->
   <owl:ObjectProperty rdf:about="http://erlangen-crm.org/efrbroo/R22_created_a_realisation_of">
      <rdfs:label xml:lang="en">R22 created a realisation of</rdfs:label>
      <owl:inverseOf rdf:resource="http://erlangen-crm.org/efrbroo/R22i_was_realised_through"/>
      <rdfs:domain rdf:resource="http://erlangen-crm.org/efrbroo/F29_Recording_Event"/>
      <rdfs:range rdf:resource="http://erlangen-crm.org/efrbroo/F21_Recording_Work"/>
      <rdfs:subPropertyOf rdf:resource="http://erlangen-crm.org/efrbroo/R19_created_a_realisation_of"/>
      <rdfs:comment>Quantification:
(0,1:0,n)</rdfs:comment>
      <rdfs:comment>Scope note:
This property associates an instance of F29 Recording Event with the instance of F21 Recording Work it realised.</rdfs:comment>
      <rdfs:comment>Examples:
The making of the recording of the third alternate take of the musical work entitled ‘Blue Hawaii’ as performed by Elvis Presley in Hollywood, Calif., Radio Recorders, on March 22nd, 1961 (F29) R22 created a realisation of the concept of the third alternate take of the musical work entitled ‘Blue Hawaii’ as performed by Elvis Presley in Hollywood, Calif.The making of the photograph of the three Allied leaders at Yalta in February 1945 (F29) R22 created a realisation of the concept of making a photograph of the three Allied leaders at Yalta in February 1945 (F21)The making of the recording of an East Australian humpback whale song in 1994 in the framework of the Oceania Project (F29) R22 created a realisation of Oceania Project’s concept of making a large digital acoustic data archive dedicated to East Australian humpback whale songs (F21)Filming Louise Bourgeois at work in the context of the shooting of the documentary movie entitled ‘Louise Bourgeois: The Spider, the Mistress, and the Tangerine’ (F29) R22 created a realisation of the concept of recording Louise Bourgeois’s artistic activity in the documentary movie entitled ‘Louise Bourgeois: The Spider, the Mistress, and the Tangerine’ (F21)</rdfs:comment>
   </owl:ObjectProperty>
   <!--http://erlangen-crm.org/efrbroo/R23_created_a_realisation_of-->
   <owl:ObjectProperty rdf:about="http://erlangen-crm.org/efrbroo/R23_created_a_realisation_of">
      <rdfs:label xml:lang="en">R23 created a realisation of</rdfs:label>
      <owl:inverseOf rdf:resource="http://erlangen-crm.org/efrbroo/R23i_was_realised_through"/>
      <rdfs:domain rdf:resource="http://erlangen-crm.org/efrbroo/F30_Publication_Event"/>
      <rdfs:range rdf:resource="http://erlangen-crm.org/efrbroo/F19_Publication_Work"/>
      <rdfs:subPropertyOf rdf:resource="http://erlangen-crm.org/efrbroo/R19_created_a_realisation_of"/>
      <rdfs:comment>Quantification:
(0,1:0,n)</rdfs:comment>
      <rdfs:comment>Scope note:
This property associates an instance of F30 Publication Event with the instance of F19 Publication Work it realised.</rdfs:comment>
      <rdfs:comment>Examples:
Establishing in 1972 the layout, features, and prototype for the publication of Stephen Crane’s complete poems (F30) R23 created a realisation of Cornell University Press’s concepts for an edition of Stephen Crane’s complete poems (F19)</rdfs:comment>
   </owl:ObjectProperty>
   <!--http://erlangen-crm.org/efrbroo/R24_created-->
   <owl:ObjectProperty rdf:about="http://erlangen-crm.org/efrbroo/R24_created">
      <rdfs:label xml:lang="en">R24 created</rdfs:label>
      <owl:inverseOf rdf:resource="http://erlangen-crm.org/efrbroo/R24i_was_created_through"/>
      <rdfs:domain rdf:resource="http://erlangen-crm.org/efrbroo/F30_Publication_Event"/>
      <rdfs:range rdf:resource="http://erlangen-crm.org/efrbroo/F24_Publication_Expression"/>
      <rdfs:subPropertyOf rdf:resource="http://erlangen-crm.org/efrbroo/R17_created"/>
      <rdfs:comment>Quantification:
(1,n:1,n)</rdfs:comment>
      <rdfs:comment>Scope note:
This property associates the instance of F24 Publication Expression that was created during a particular F30 Publication Event with that F30 Publication Event.</rdfs:comment>
      <rdfs:comment>Examples:
Establishing in 1972 the layout, features, and prototype for the publication of Stephen Crane’s complete poems (F30) R24 created the set of signs and instructions as to manufacturing established by Cornell University Press for a publication of Stephen Crane’s complete poems (F24)</rdfs:comment>
   </owl:ObjectProperty>
   <!--http://erlangen-crm.org/efrbroo/R25_performed-->
   <owl:ObjectProperty rdf:about="http://erlangen-crm.org/efrbroo/R25_performed">
      <rdfs:label xml:lang="en">R25 performed</rdfs:label>
      <owl:inverseOf rdf:resource="http://erlangen-crm.org/efrbroo/R25i_was_performed_in"/>
      <rdfs:domain rdf:resource="http://erlangen-crm.org/efrbroo/F31_Performance"/>
      <rdfs:range rdf:resource="http://erlangen-crm.org/efrbroo/F25_Performance_Plan"/>
      <rdfs:subPropertyOf rdf:resource="http://erlangen-crm.org/current/P33_used_specific_technique"/>
      <rdfs:comment>Quantification:
(0,n:0,n)</rdfs:comment>
      <rdfs:comment>Scope note:
This property associates an instance of F31 Performance with the instance of F25 Performance Plan to which all those participating in the performance were supposed to conform.</rdfs:comment>
      <rdfs:comment>Examples:
Performing the first performance of a Yiddish translation of ‘King Lear’, as directed by Sergei Radlov, in Moscow, at the Moscow State Jewish Theatre, on February 10, 1935 (F31) R25 performed the set of instructions for the production of a Yiddish translation of ‘King Lear’, directed by Sergei Radlov in Moscow in 1935 (F25)Performing the ballet ‘Rite of spring’, as choreographed by Pina Bausch, in Avignon, at the Popes’ Palace, on July 7, 1995 (F31) R25 performed the set of instructions for the production of the ballet ‘Rite of spring’, as choreographed by Pina Bausch (F25)</rdfs:comment>
   </owl:ObjectProperty>
   <!--http://erlangen-crm.org/efrbroo/R26_produced_things_of_type-->
   <owl:ObjectProperty rdf:about="http://erlangen-crm.org/efrbroo/R26_produced_things_of_type">
      <rdfs:label xml:lang="en">R26 produced things of type</rdfs:label>
      <owl:inverseOf rdf:resource="http://erlangen-crm.org/efrbroo/R26i_was_produced_by"/>
      <rdfs:domain rdf:resource="http://erlangen-crm.org/efrbroo/F32_Carrier_Production_Event"/>
      <rdfs:range rdf:resource="http://erlangen-crm.org/efrbroo/F3_Manifestation_Product_Type"/>
      <rdfs:subPropertyOf rdf:resource="http://erlangen-crm.org/current/P108_has_produced"/>
      <rdfs:comment>Quantification:
(1,n:0,n)</rdfs:comment>
      <rdfs:comment>Scope note:
This property associates an instance of F32 Carrier Production Event with the instance of F3 Manifestation Product Type it produced items of.</rdfs:comment>
      <rdfs:comment>Examples:
The production of copies of the publication entitled ‘Codex Manesse: die Miniaturen der großen Heidelberger Liederhandschrift, herausgegeben und erläutert von Ingo F. Walther unter Mitarbeit von Gisela Siebert’, 3rd edition, Insel-Verlag, 1988 (F32) R26 produced things of type the publication identified as ‘Codex Manesse: die Miniaturen der großen Heidelberger Liederhandschrift, herausgegeben und erläutert von Ingo F. Walther unter Mitarbeit von Gisela Siebert’, 3rd edition, Insel-Verlag, 1988 (F3)The production of copies of the publication entitled ‘Ordnance Survey Explorer Map 213, Aberystwyth &amp; Cwm Rheidol’, ISBN ‘0-319-23640-4’ (folded), 1:25,000 scale, released in May 2005 (F32) R26 produced things of type the publication identified by ISBN ‘0-319-23640-4’ (F3)The production of copies of the sound recording entitled ‘The Glory (????) of the human voice’, RCA Victor Gold Seal GD61175, containing recordings of musical works performed by Florence Foster Jenkins (F32) R26 produced things of type the publication entitled ‘The Glory (????) of the human voice’ and identified by the label and label number ‘RCA Victor Gold Seal GD61175’ (F3)The production of a second print run, in 1978, of the publication titled ‘The complete poems of Stephen Crane, edited with an introduction by Joseph Katz’ (identified by ISBN ‘0-8014-9130-4’) (F32) R26 produced things of type the publication, dated 1972, entitled ‘The complete poems of Stephen Crane, edited with an introduction by Joseph Katz’ (identified by ISBN ‘0-8014-9130-4’) (F3)</rdfs:comment>
   </owl:ObjectProperty>
   <!--http://erlangen-crm.org/efrbroo/R27_used_as_source_material-->
   <owl:ObjectProperty rdf:about="http://erlangen-crm.org/efrbroo/R27_used_as_source_material">
      <rdfs:label xml:lang="en">R27 used as source material</rdfs:label>
      <owl:inverseOf rdf:resource="http://erlangen-crm.org/efrbroo/R27i_was_used_by"/>
      <rdfs:domain rdf:resource="http://erlangen-crm.org/efrbroo/F32_Carrier_Production_Event"/>
      <rdfs:range rdf:resource="http://erlangen-crm.org/efrbroo/F24_Publication_Expression"/>
      <rdfs:subPropertyOf rdf:resource="http://erlangen-crm.org/current/P16_used_specific_object"/>
      <rdfs:comment>Quantification:
(0,n:0,n)</rdfs:comment>
      <rdfs:comment>Scope note:
This property associates an instance of F32 Carrier Production Event with the set of signs provided by the publisher to be carried by all of the produced items.</rdfs:comment>
      <rdfs:comment>Examples:
The production of copies of the publication identified by ISBN ‘1-86197-612-7’ (F32) R27 used as source material the final set of signs sent by the publisher named ‘Profile Books’ to their printer for the production of copies of the publication identified by ISBN ‘1-86197-612-7’ (F24)</rdfs:comment>
   </owl:ObjectProperty>
   <!--http://erlangen-crm.org/efrbroo/R28_produced-->
   <owl:ObjectProperty rdf:about="http://erlangen-crm.org/efrbroo/R28_produced">
      <rdfs:label xml:lang="en">R28 produced</rdfs:label>
      <owl:inverseOf rdf:resource="http://erlangen-crm.org/efrbroo/R28i_was_produced_by"/>
      <rdfs:domain rdf:resource="http://erlangen-crm.org/efrbroo/F32_Carrier_Production_Event"/>
      <rdfs:range rdf:resource="http://erlangen-crm.org/efrbroo/F54_Utilised_Information_Carrier"/>
      <rdfs:subPropertyOf rdf:resource="http://erlangen-crm.org/current/P108_has_produced"/>
      <rdfs:comment>Quantification:
(0,n:1,1)</rdfs:comment>
      <rdfs:comment>Scope note:
This property associates an instance of F32 Carrier Production Event with any one of the produced items (i.e., the instances of F5 Item or F53 Material Copy).</rdfs:comment>
      <rdfs:comment>Examples:
The production of copies of the publication entitled ‘Codex Manesse: die Miniaturen der großen Heidelberger Liederhandschrift, herausgegeben und erläutert von Ingo F. Walther unter Mitarbeit von Gisela Siebert’, 3rd edition, Insel-Verlag, 1988 (F32) R28 produced the National Library of France’s holding identified by shelf mark ‘C-1604(2)’ (F5)The production of copies of the publication entitled ‘Ordnance Survey Explorer Map 213, Aberystwyth &amp; Cwm Rheidol’, ISBN 0-319-23640-4 (folded), 1:25,000 scale, released in May 2005 (F32) R28 produced the National Library of Wales’ holding identified by holding information ‘MAP, STORFA/STACK ; FLAT MAP, C16 (20/1), Sheet 213, c.135/5/2’ (F5)The production of copies of the sound recording entitled ‘The Glory (????) of the human voice’, RCA Victor Gold Seal GD61175 (F32) R28 produced the London Public Library’s holding identified by call number ‘R J416.Gl’ (F5)The second print run, occurring in 1978, of the publication dated of 1972 and entitled ‘The complete poems of Stephen Crane, edited with an introduction by Joseph Katz’ (identified by ISBN ‘0-8014-9130-4’) (F32) R28 produced Universitätsbibliothek Passau’s holding identified by call number ‘00/HT 4801.978 K2’ (F5)</rdfs:comment>
   </owl:ObjectProperty>
   <!--http://erlangen-crm.org/efrbroo/R29_reproduced-->
   <owl:ObjectProperty rdf:about="http://erlangen-crm.org/efrbroo/R29_reproduced">
      <rdfs:label xml:lang="en">R29 reproduced</rdfs:label>
      <owl:inverseOf rdf:resource="http://erlangen-crm.org/efrbroo/R29i_was_reproduced_by"/>
      <rdfs:domain rdf:resource="http://erlangen-crm.org/efrbroo/F33_Reproduction_Event"/>
      <rdfs:range rdf:resource="http://erlangen-crm.org/current/E84_Information_Carrier"/>
      <rdfs:subPropertyOf rdf:resource="http://erlangen-crm.org/current/P16_used_specific_object"/>
      <rdfs:comment>Quantification:
(1,n:0,n)</rdfs:comment>
      <rdfs:comment>Scope note:
This property associates an instance of F33 Reproduction Event with an instance of E84 Information Carrier it reproduces.</rdfs:comment>
      <rdfs:comment>Examples:
Making a photocopy of an exemplar of Eran Guter’s dissertation entitled ‘Where languages end: Ludwig Wittgenstein at the crossroads of music, language, and the world’ (F33) R29 reproduced one of the original exemplars of Eran Guter’s dissertation (E84)</rdfs:comment>
   </owl:ObjectProperty>
   <!--http://erlangen-crm.org/efrbroo/R30_produced-->
   <owl:ObjectProperty rdf:about="http://erlangen-crm.org/efrbroo/R30_produced">
      <rdfs:label xml:lang="en">R30 produced</rdfs:label>
      <owl:inverseOf rdf:resource="http://erlangen-crm.org/efrbroo/R30i_was_produced_by"/>
      <rdfs:domain rdf:resource="http://erlangen-crm.org/efrbroo/F33_Reproduction_Event"/>
      <rdfs:range rdf:resource="http://erlangen-crm.org/current/E84_Information_Carrier"/>
      <rdfs:subPropertyOf rdf:resource="http://erlangen-crm.org/current/P108_has_produced"/>
      <rdfs:comment>Quantification:
(1,n:0,1)</rdfs:comment>
      <rdfs:comment>Scope note:
This property associates an instance of F33 Reproduction Event with an instance of E84 Information Carrier it produces.</rdfs:comment>
      <rdfs:comment>Examples:
Making a photocopy of an exemplar of Eran Guter’s dissertation entitled ‘Where languages end: Ludwig Wittgenstein at the crossroads of music, language, and the world’ (F33) R30 produced the New York Public Library holding identified by call number ‘JMD 04-1060’ (E84)</rdfs:comment>
   </owl:ObjectProperty>
   <!--http://erlangen-crm.org/efrbroo/R31_is_reproduction_of-->
   <owl:ObjectProperty rdf:about="http://erlangen-crm.org/efrbroo/R31_is_reproduction_of">
      <rdfs:label xml:lang="en">R31 is reproduction of</rdfs:label>
      <owl:inverseOf rdf:resource="http://erlangen-crm.org/efrbroo/R31i_has_reproduction"/>
      <rdfs:domain rdf:resource="http://erlangen-crm.org/current/E84_Information_Carrier"/>
      <rdfs:range rdf:resource="http://erlangen-crm.org/current/E84_Information_Carrier"/>
      <rdfs:subPropertyOf rdf:resource="http://erlangen-crm.org/current/P130_shows_features_of"/>
      <rdfs:comment>Quantification:
(0,1:0,n)</rdfs:comment>
      <rdfs:comment>Scope note:
This property associates an instance of E84 Information Carrier which is a reproduction of another instance of E84 Information Carrier with the latter. It is considered that a reproduction of multiple originals resulting in a single product requires a merging of those objects prior to the reproduction. Therefore an Information Carrier is regarded to be a reproduction of one and only one original. This property is a shortcut of the more fully developed path from E84 Information Carrier through R30 produced (was produced by), F33 Reproduction Event R29 reproduced (was reproduced by) to E84 Information Carrier.</rdfs:comment>
      <rdfs:comment>Examples:
The New York Public Library holding identified by call number ‘JMD 04-1060’ (E84) R31 is reproduction of one of the original exemplars of Eran Guter’s dissertation (E84)</rdfs:comment>
   </owl:ObjectProperty>
   <!--http://erlangen-crm.org/efrbroo/R32_is_warranted_by-->
   <owl:ObjectProperty rdf:about="http://erlangen-crm.org/efrbroo/R32_is_warranted_by">
      <rdfs:label xml:lang="en">R32 is warranted by</rdfs:label>
      <owl:inverseOf rdf:resource="http://erlangen-crm.org/efrbroo/R32i_warrants"/>
      <rdfs:domain rdf:resource="http://erlangen-crm.org/efrbroo/F35_Nomen_Use_Statement"/>
      <rdfs:range rdf:resource="http://erlangen-crm.org/efrbroo/F52_Name_Use_Activity"/>
      <rdfs:subPropertyOf rdf:resource="http://erlangen-crm.org/current/P67_refers_to"/>
      <rdfs:comment>Quantification:
(0,n:0,n)</rdfs:comment>
      <rdfs:comment>Scope note:
This property associates an instance of F35 Nomen Use Statement with an instance of F52 Name Use Activity which provides evidence for the use of the particular nomen in the stated sense. The association between this name use activity and a source for it may be described by the property P70 documents (is documented in).</rdfs:comment>
      <rdfs:comment>Examples:
The variant controlled access point in record n 79021736, tagged in MARC 21 format, ‘400 1_ |a Пруст, Марсель, |d 1871-1922’ found in the Library of Congress authorities as of 15 June 2012 (F35) R32 is warranted by the use of the name ‘Марсель Пруст’ in Cyrillic script (F52), for which evidence can be found in the publication referred to as ‘Andreev, L.G. Marselʹ Prust, 1968’ in the authority record established by the Library of Congress for Marcel ProustThe preferred access point in record sh 85109469, tagged in MARC 21 format, ‘150 __ |a Quantum theory’ found in the Library of Congress authorities as of 15 June 2012 (F35) R32 is warranted by the use of the phrase ‘quantum theory’ in the English language (F52), as attested to by references to the NASA and INSPEC thesauri in the authority record established by the Library of CongressThe preferred access point in record sh 85074230 in the LCSH authority file tagged in MARC 21 in the field ‘150__ |a Lamniformes’ (F35) R32 is warranted by the use of the term ‘Lamniformes’ for mackerel sharks in the entry on page 51 of Fishes of the world by J.S. Nelson published in 1994 (F52)The preferred access point in record n 85118480 in the Library of Congress name authority file as of 19 November 2012 tagged in MARC 21 in the field ‘110 2_ |a Canadian Academic Centre in Italy’ (F35) R32 is warranted by the use of the name ‘Canadian Academic Centre in Italy’ on page 6 of the book ‘Lo Scavo di S. Giovanni di Ruoti ed il periodo tardoantico in Basilicata’ published in 1983</rdfs:comment>
   </owl:ObjectProperty>
   <!--http://erlangen-crm.org/efrbroo/R33_has_content-->
   <owl:ObjectProperty rdf:about="http://erlangen-crm.org/efrbroo/R33_has_content">
      <rdfs:label xml:lang="en">R33 has content</rdfs:label>
      <rdfs:domain rdf:resource="http://erlangen-crm.org/efrbroo/F12_Nomen"/>
      <rdfs:range rdf:resource="http://erlangen-crm.org/current/E62_String"/>
      <rdfs:subPropertyOf rdf:resource="http://erlangen-crm.org/current/P3_has_note"/>
      <rdfs:comment>Quantification:
(1,n:0,n)</rdfs:comment>
      <rdfs:comment>Scope note:
This property associates an instance of F12 Nomen with one or more equivalent serialized content models for it. In digital form the symbol arrangement constituting an instance of F12 Nomen can only be represented through a particular encoding, for example ASCII or Latin1 for the Latin script. We call such a representation a content model. The property R33.1 has encoding: E55 Type allows for specifying the encoding of a particular associated content model. Together with this specification, a content model allows for unambiguously defining a nomen independently from the encoding used for representing the content.</rdfs:comment>
      <rdfs:comment>Examples:
The term ‘earth’ encoded as ASCII (F12) R33 has content ‘0x65 0x61 0x72 0x74 0x68’ (E62) R33.1 has encoding ASCII (E55)The term ‘earth’ encoded as UNICODE UTF16 (F12) R33 has content ‘0x0065 0x0061 0x0072 0x0074 0x0068’ R33.1 has encoding UNICODE UTF16 (E55)The term ‘earth’ in Latin Arial font (F12) R33 has content ‘ ’ (E62) R33.1 has encoding printed Latin Arial (E55)Properties:R33.1 has encoding: E55 Type</rdfs:comment>
   </owl:ObjectProperty>
   <!--http://erlangen-crm.org/efrbroo/R34_has_validity_period-->
   <owl:ObjectProperty rdf:about="http://erlangen-crm.org/efrbroo/R34_has_validity_period">
      <rdfs:label xml:lang="en">R34 has validity period</rdfs:label>
      <owl:inverseOf rdf:resource="http://erlangen-crm.org/efrbroo/R34i_is_validity_period_of"/>
      <rdfs:domain rdf:resource="http://erlangen-crm.org/efrbroo/F34_KOS"/>
      <rdfs:range rdf:resource="http://erlangen-crm.org/current/E52_Time-Span"/>
      <rdfs:comment>Quantification:
(1,1:0,n)</rdfs:comment>
      <rdfs:comment>Scope note:
This property associates an instance of F34 KOS with the instance of E52 Time-Span describing the period for which the particular KOS Expression was regarded as valid by its maintainers. Each change of validity status of a nomen use statement within a KOS should be associated with a release change of the KOS. The individual time-span of a validity state of a nomen would be the union of the time-spans of the KOS in which the Nomen was declared to have the particular validity status (provisional, accepted, obsolete etc...).</rdfs:comment>
      <rdfs:comment>Examples:
LCSH February 20 to March 19 2012 (F34) R34 has validity period February 20 to March 19 2012 (E52)DDC 19 (F34) R34 has validity period 1979 to 1989 (E52)</rdfs:comment>
   </owl:ObjectProperty>
   <!--http://erlangen-crm.org/efrbroo/R35_is_specified_by-->
   <owl:ObjectProperty rdf:about="http://erlangen-crm.org/efrbroo/R35_is_specified_by">
      <rdfs:label xml:lang="en">R35 is specified by</rdfs:label>
      <owl:inverseOf rdf:resource="http://erlangen-crm.org/efrbroo/R35i_specifies"/>
      <rdfs:domain rdf:resource="http://erlangen-crm.org/efrbroo/F35_Nomen_Use_Statement"/>
      <rdfs:range rdf:resource="http://erlangen-crm.org/efrbroo/F34_KOS"/>
      <rdfs:subPropertyOf rdf:resource="http://erlangen-crm.org/current/P148_has_component"/>
      <rdfs:comment>Quantification:
(1,1:1,n)</rdfs:comment>
      <rdfs:comment>Scope note:
This property associates an instance of F35 Nomen Use Statement with an instance of F34 KOS in which the Nomen Use Statement has a given status. The property R35.1 allows for specifying the particular status of the nomen use statement within the KOS. An instance of R35 is specified by should have only one status.</rdfs:comment>
      <rdfs:comment>Examples:
‘acoustic surface wave device’ (F35) R35 is specified by INSPEC Thesaurus version January 1973 (F34) R35.1 has status valid (E55)‘acoustic surface wave device’ (F35) R35 is specified by INSPEC Thesaurus version June 1978 (F34) R35.1 has status obsolete (E55)Properties:R35.1 has status: E55 Type</rdfs:comment>
   </owl:ObjectProperty>
   <!--http://erlangen-crm.org/efrbroo/R36_uses_script_conversion-->
   <owl:ObjectProperty rdf:about="http://erlangen-crm.org/efrbroo/R36_uses_script_conversion">
      <rdfs:label xml:lang="en">R36 uses script conversion</rdfs:label>
      <owl:inverseOf rdf:resource="http://erlangen-crm.org/efrbroo/R36i_is_script_conversion_used_in"/>
      <rdfs:domain rdf:resource="http://erlangen-crm.org/efrbroo/F35_Nomen_Use_Statement"/>
      <rdfs:range rdf:resource="http://erlangen-crm.org/efrbroo/F36_Script_Conversion"/>
      <rdfs:comment>Quantification:
(0,1:0,n)</rdfs:comment>
      <rdfs:comment>Scope note:
This property associates an instance of F35 Nomen Use Statement with the instance of F36 Script Conversion that was used to create the Nomen referred to in the Nomen Use Statement. The source of this conversion may or may not be explicitly mentioned. Is shortcut of: F35 Nomen Use Statement R17 was created by (created) F28 Expression Creation P33 used specific technique (was used by) E29 Design or Procedure.</rdfs:comment>
      <rdfs:comment>Examples:
‘001  FRBNF120864715’…‘100  $w.0..ba....$aDu$mFu$d0712-0770’ [an instance of F35 Nomen Use Statement in INTERMARC format] (F35) R36 uses script conversion Pinyin (F36)‘001  FRBNF119547493’…‘100  w.0..barus.$aGončarova$mNatalʹâ Sergeevna$d1881-1962’ [an instance of F35 Nomen Use Statement in INTERMARC format] (F35) R36 uses script conversion ISO 9:1995 (F36)</rdfs:comment>
   </owl:ObjectProperty>
   <!--http://erlangen-crm.org/efrbroo/R37_states_as_nomen-->
   <owl:ObjectProperty rdf:about="http://erlangen-crm.org/efrbroo/R37_states_as_nomen">
      <rdfs:label xml:lang="en">R37 states as nomen</rdfs:label>
      <owl:inverseOf rdf:resource="http://erlangen-crm.org/efrbroo/R37i_is_stated_as_nomen_in"/>
      <rdfs:domain rdf:resource="http://erlangen-crm.org/efrbroo/F35_Nomen_Use_Statement"/>
      <rdfs:range rdf:resource="http://erlangen-crm.org/efrbroo/F12_Nomen"/>
      <rdfs:subPropertyOf rdf:resource="http://erlangen-crm.org/current/P67_refers_to"/>
      <rdfs:comment>Quantification:
(1,1:0,n)</rdfs:comment>
      <rdfs:comment>Scope note:
This property associates an instance of F35 Nomen Use Statement with the instance of F12 Nomen for which it declares usage.</rdfs:comment>
      <rdfs:comment>Examples:
‘PTBNP|20891’…‘200 1‎‡a Whitman,‏ ‎‡b Walt,‏ ‎‡f 1819-1892‏’ [an instance of F35 Nomen Use Statement in UNIMARC format] (F35) R37 states as nomen ‘Whitman, Walt (1819-1892)’ (F50)‘001  FRBNF120864715’…‘100  $w.0..ba....$aDu$mFu$d0712-0770’ [an instance of F35 Nomen Use Statement in INTERMARC format] (F35) R37 states as nomen ‘Du, Fu (0712-0770)’ (F50)‘001  FRBNF119547493’…‘100  w.0..barus.$aGončarova$mNatalʹâ Sergeevna$d1881-1962’ [an instance of F35 Nomen Use Statement in INTERMARC format] (F35) R37 states as nomen ‘Gončarova, Natalʹâ Sergeevna (1881-1962)’ (F50)‘010 __ |a n 79021736’…‘400 1_ |a Пруст, Марсель, |d 1871-1922’ [an instance of F35 Nomen Use Statement in INTERMARC format] (F35) R37 states as nomen ‘Пруст, Марсель, 1871-1922’ (F50)‘010 __ |a sh 85074230’…‘150__ |a Lamniformes’ [an instance of F35 Nomen Use Statement in MARC 21 format] (F35) R37 states as nomen ‘Lamniformes’ (F12)‘010 __ |a sh 85074230’…‘053 _0 |a QL638.94.L36 |c Zoology’ [an instance of F35 Nomen Use Statement in MARC 21 format] (F35) R37 states as nomen the Library of Congress classification number ‘QL638.94.L36’ (F12)‘ID: 300024668’…‘navaja (C,U,Spanish,UF,U,SN)’ R37 states as nomen ‘navaja’(F12) (“used for” term, Getty Art &amp; Architecture Thesaurus Online, retrieved 19/11/2012)‘ID: 7010879’…‘Candia (H,V,Greek (transliterated),U) ….Venetian corruption of Arabic name, used from 13th cen.’ R37 states as nomen ‘Candia’ (F12) (“historical term”, Getty Thesaurus of Geographic Names Online, retrieved 19/11/2012)‘ID: 7010879’…‘Ērakleion (NA,V,Greek (transliterated),U)’ R37 states as nomen ‘Ērakleion’ (F12) (“not-applicable term”, Getty Thesaurus of Geographic Names Online, retrieved 19/11/2012)‘&lt;eac-cpf […]&gt; &lt;control&gt; &lt;recordId&gt;beinecke.7h44jbj&lt;/recordId&gt; […] &lt;/control&gt;’ … ‘&lt;cpfDescription&gt; &lt;identity&gt; &lt;entityType&gt;family&lt;/entityType&gt; &lt;nameEntry xml:lang="eng" scriptCode="Latn"&gt;&lt;part localType="100a"&gt;Boswell family&lt;/part&gt; […] &lt;/nameEntry&gt; […] &lt;/identity&gt; &lt;/cpfDescription&gt; […] &lt;/eac-cpf&gt;’ [an instance of F35 Nomen Use Statement in EAC] (F35) R37 states as nomen ‘Boswell family’ (F12)</rdfs:comment>
   </owl:ObjectProperty>
   <!--http://erlangen-crm.org/efrbroo/R38_refers_to_thema-->
   <owl:ObjectProperty rdf:about="http://erlangen-crm.org/efrbroo/R38_refers_to_thema">
      <rdfs:label xml:lang="en">R38 refers to thema</rdfs:label>
      <owl:inverseOf rdf:resource="http://erlangen-crm.org/efrbroo/R38i_is_thema_of"/>
      <rdfs:domain rdf:resource="http://erlangen-crm.org/efrbroo/F35_Nomen_Use_Statement"/>
      <rdfs:range rdf:resource="http://erlangen-crm.org/current/E1_CRM_Entity"/>
      <rdfs:comment>Quantification:
(1,1:0,n)</rdfs:comment>
      <rdfs:comment>Scope note:
This property associates an instance of F35 Nomen Use Statement with the instance of E1 CRM Entity for which it declares the usage of a nomen.</rdfs:comment>
      <rdfs:comment>Examples:
‘PTBNP|20891’…‘200 1‎‡a Whitman,‏ ‎‡b Walt,‏ ‎‡f 1819-1892‏’ [an instance of F35 Nomen Use Statement in UNIMARC format] (F35) R38 refers to thema the person who wrote the collection of poems titled ‘Leaves of Grass’ (E21=F10)‘010 __ |a sh 85109469’…‘150 __ |a Quantum theory’ [preferred subject access point from LCSH, in MARC 21 format, http://lccn.loc.gov/sh85109469, as of 15 June 2012] (F35) R38 refers to thema the branch of physics known as quantum theory (F6 = E28)‘&lt;eac-cpf […]&gt; &lt;control&gt; &lt;recordId&gt;beinecke.7h44jbj&lt;/recordId&gt; […] &lt;/control&gt;’ … ‘&lt;cpfDescription&gt; &lt;identity&gt; &lt;entityType&gt;family&lt;/entityType&gt; &lt;nameEntry xml:lang="eng" scriptCode="Latn"&gt;&lt;part localType="100a"&gt;Boswell family&lt;/part&gt; […] &lt;/nameEntry&gt; […] &lt;/identity&gt; &lt;/cpfDescription&gt; […] &lt;/eac-cpf&gt;’ [an instance of F35 Nomen Use Statement in EAC] (F35) R38 refers to thema the family who held the barony of Auchinleck in Scotland from 1504 on (F39)</rdfs:comment>
   </owl:ObjectProperty>
   <!--http://erlangen-crm.org/efrbroo/R39_is_intended_for-->
   <owl:ObjectProperty rdf:about="http://erlangen-crm.org/efrbroo/R39_is_intended_for">
      <rdfs:label xml:lang="en">R39 is intended for</rdfs:label>
      <owl:inverseOf rdf:resource="http://erlangen-crm.org/efrbroo/R39i_is_target_audience_in"/>
      <rdfs:domain rdf:resource="http://erlangen-crm.org/efrbroo/F35_Nomen_Use_Statement"/>
      <rdfs:range rdf:resource="http://erlangen-crm.org/current/E74_Group"/>
      <rdfs:subPropertyOf rdf:resource="http://erlangen-crm.org/current/P67_refers_to"/>
      <rdfs:comment>Quantification:
(0,n:0,n)</rdfs:comment>
      <rdfs:comment>Scope note:
This property associates an instance of F35 Nomen Use Statement with an instance of E74 Group which is the target audience for which the associated nomen use is intended. To indicate that the associated nomen is declared as preferred in all contexts, the instance of E74 Group is ‘mankind’.</rdfs:comment>
      <rdfs:comment>Examples:
‘010 __ |a sj 96004896’…‘150 __ |a Belly button’ [an instance of F35 Nomen Use Statement in MARC 21 format] (F35) R39 is intended for Children (E74)</rdfs:comment>
   </owl:ObjectProperty>
   <!--http://erlangen-crm.org/efrbroo/R40_has_representative_expression-->
   <owl:ObjectProperty rdf:about="http://erlangen-crm.org/efrbroo/R40_has_representative_expression">
      <rdfs:label xml:lang="en">R40 has representative expression</rdfs:label>
      <owl:inverseOf rdf:resource="http://erlangen-crm.org/efrbroo/R40i_is_representative_expression_for"/>
      <rdfs:domain rdf:resource="http://erlangen-crm.org/efrbroo/F1_Work"/>
      <rdfs:range rdf:resource="http://erlangen-crm.org/efrbroo/F22_Self-Contained_Expression"/>
      <rdfs:subPropertyOf rdf:resource="http://erlangen-crm.org/efrbroo/R3_is_realised_in"/>
      <rdfs:comment>Quantification:
(0,n:0,n)</rdfs:comment>
      <rdfs:comment>Scope note:
This property identifies an instance of F22 Self-Contained Expression that has been chosen as the most characteristic expression of the instance of F1 Work of which it is an expression. There is no other semantic implication to this notion of being characteristic than to be an adequate candidate to uniquely identify the Work realized by it. Prototypically, this is the instance of F22 Self-Contained Expression that is deemed characteristic of an instance of F15 Complex Work.Typically, any expression that is not regarded as “representative” for the work it expresses, would require a controlled access point, with qualifiers specifying the differences between that expression and a representative expression, although this may not always be done in practice. The title of a Work may not be one taken from a representative expression.A given work can have more than one representative expression, provided the differences between these expressions are not deemed “substantial.” If the anticipated needs of users are not considered to call for bibliographic distinctions between variant expressions of a work, then even expressions that differ significantly from each other can be regarded as equally representative for the work. (See FRBR: Final Report, p. 19-20).A given expression can be deemed representative for a work with regard to some of its aspects (e.g., the text contained in an edition the title proper of which reads ‘The tragicall historie of HAMLET Prince of Denmarke’, and the language of that text), and not representative for it with regard to some other aspects (e.g., the title proper ‘The tragicall historie of HAMLET Prince of Denmarke’ itself, which, being different from the title that is regarded as “representative” for Shakespeare’s work, will require the use of a controlled access point).R40 has representative expression is a shortcut of the more developed path F1 Work R50i was assigned by F42 Representative Expression Assignment R51 assigned F2 Expression.</rdfs:comment>
      <rdfs:comment>Examples:
Richard Brinsley Sheridan’s textual work entitled ‘St. Patrick’s Day’ (F15) R40 has representative expression the linguistic content of the 1775 edition of Richard Brinsley Sheridan’s textual work entitled ‘St. Patrick’s Day’, mentioned in the ‘Encyclopaedia Britannica’, 15th edition, cited as the source for the authority record created for that work by the Library of Congress (F22)John Tavener’s musical work entitled ‘The Eternal Sun’ (F15) R40 has representative expression the notational content embodied in the 2007 edition of John Tavener’s ‘The Eternal Sun’ cited as the source for the authority record created for that work by the National Library of France (F22)The series entitled ‘Headline series’ (F18) R40 has representative expression the overall content of the publication entitled ‘Vietnam, the war nobody won’ by S. Karnow, which belongs to the series entitled ‘Headline series’ and was used by the Library of Congress as the basis for creating the authority record for that series (F24)The periodical entitled ‘The New Courier’, released by UNESCO, and described by the National Library of France in a bibliographic record that contains the following statement: ‘Notice réd. d’après le n° d’octobre 2002’ (i.e., ‘description based on the issue dated October 2002’) (F18) R40 has representative expression the overall content of the October 2002 issue of UNESCO’s periodical entitled ‘The New Courier’ (F24)</rdfs:comment>
   </owl:ObjectProperty>
   <!--http://erlangen-crm.org/efrbroo/R41_has_representative_manifestation_product_type-->
   <owl:ObjectProperty rdf:about="http://erlangen-crm.org/efrbroo/R41_has_representative_manifestation_product_type">
      <rdfs:label xml:lang="en">R41 has representative manifestation product type</rdfs:label>
      <owl:inverseOf rdf:resource="http://erlangen-crm.org/efrbroo/R41i_is_representative_manifestation_product_type_for"/>
      <rdfs:domain rdf:resource="http://erlangen-crm.org/efrbroo/F2_Expression"/>
      <rdfs:range rdf:resource="http://erlangen-crm.org/efrbroo/F3_Manifestation_Product_Type"/>
      <rdfs:subPropertyOf rdf:resource="http://erlangen-crm.org/efrbroo/R4_carriers_provided_by"/>
      <rdfs:comment>Quantification:
(0,n:0,n)</rdfs:comment>
      <rdfs:comment>Scope note:
This property identifies an instance of F3 Manifestation Product Type that has been chosen as the most characteristic Manifestation Product Type of the instance of F2 Expression of which it is a manifestation.Identifying an instance of F3 Manifestation Product Type that is representative for an instance of F2 Expression makes it possible in turn to identify an instance of F2 Expression that is representative for an instance of F1 Work, and to decide what should be regarded as the title of the work.The title of an Expression may not be one taken from a representative Manifestation Product Type or Manifestation Singleton.A given expression can have more than one Representative Manifestation Product Type.R41 has representative manifestation product type is a shortcut of the more developed path F2 Expression R48i was assigned by F41 Representative Manifestation Assignment R49 assigned F3 Manifestation Product Type.</rdfs:comment>
      <rdfs:comment>Examples:
The original text of Richard Brinsley Sheridan’s textual work entitled ‘St. Patrick’s Day’ (F22) R41 has representative manifestation product type the 1775 edition of Richard Brinsley Sheridan’s textual work entitled ‘St. Patrick’s Day’, mentioned in the ‘Encyclopaedia Britannica’, 15th edition, cited as the source for the authority record created for that work by the Library of Congress (F3)The original notation of John Tavener’s musical work entitled ‘The Eternal Sun’ (F22) R41 has representative manifestation the 2007 edition of John Tavener’s ‘The Eternal Sun’ cited as the source for the authority record created for that work by the National Library of France (F3)The textual content of the series entitled ‘Headline series’ (F2) R41 has representative manifestation the publication entitled ‘Vietnam, the war nobody won’ by S. Karnow, which belongs to the series entitled ‘Headline series’ and was used by the Library of Congress as the basis for creating the authority record for that series (F3)The textual content of the periodical entitled ‘The New Courier’ (F2) R41 has representative manifestation the October 2002 issue of the periodical entitled ‘The New Courier’ (F3), which was used as the source for the bibliographic record created by the National Library of France</rdfs:comment>
   </owl:ObjectProperty>
   <!--http://erlangen-crm.org/efrbroo/R42_is_representative_manifestation_singleton_for-->
   <owl:ObjectProperty rdf:about="http://erlangen-crm.org/efrbroo/R42_is_representative_manifestation_singleton_for">
      <rdfs:label xml:lang="en">R42 is representative manifestation singleton for</rdfs:label>
      <owl:inverseOf rdf:resource="http://erlangen-crm.org/efrbroo/R42i_has_representative_manifestation_singleton"/>
      <rdfs:domain rdf:resource="http://erlangen-crm.org/efrbroo/F4_Manifestation_Singleton"/>
      <rdfs:range rdf:resource="http://erlangen-crm.org/efrbroo/F2_Expression"/>
      <rdfs:subPropertyOf rdf:resource="http://erlangen-crm.org/current/P128_carries"/>
      <rdfs:comment>Quantification:
(0,n:0,n)</rdfs:comment>
      <rdfs:comment>Scope note:
This property identifies an instance of Manifestation Singleton that has been declared as the unique representative for an instance of F2 Expression by some bibliographic agency.This property identifies an instance of F4 Manifestation Singleton that has been chosen as the most characteristic Manifestation Singleton of the instance of F2 Expression of which it is a manifestation.Identifying an instance of F4 Manifestation Singleton that is representative for an instance of F2 Expression makes it possible in turn to identify an instance of F2 Expression that is representative for an instance of F1 Work, and to decide what should be regarded as the title of the work.The title of an Expression may not be one taken from a representative Manifestation Product Type or Manifestation Singleton.A given expression can have more than one representative Manifestation Singleton.It is a shortcut for the more developed path: F2 Expression R48i was assigned by F41 Representative Manifestation Assignment R53 assigned F4 Manifestation Singleton.</rdfs:comment>
      <rdfs:comment>Examples:
The musical text of Stanislas Champein’s opera ‘Vichnou’ (F22) R42 has representative manifestation singleton the manuscript identified by shelfmark ‘MS-8282’ within the collections of the National Library of France, Department for Music (F4) [explanation: the BnF’s Department for Music holds 3 manuscript scores (identified by shelfmarks ‘MS-8282’, ‘MS-13778’, and ‘MS-17321’) for this opera; the title inscribed on MS-8282 is ‘Vichnou’, while MS-13778 and MS-17321 are titled ‘Vistnou’; the authorised form chosen by cataloguers and reference tools such as the Grove Dictionary for Opera is ‘Vichnou’, while ‘Vistnou’ is recorded in the BnF’s authority file as a variant form only]</rdfs:comment>
   </owl:ObjectProperty>
   <!--http://erlangen-crm.org/efrbroo/R43_carried_out_by-->
   <owl:ObjectProperty rdf:about="http://erlangen-crm.org/efrbroo/R43_carried_out_by">
      <rdfs:label xml:lang="en">R43 carried out by</rdfs:label>
      <owl:inverseOf rdf:resource="http://erlangen-crm.org/efrbroo/R43i_performed"/>
      <rdfs:domain rdf:resource="http://erlangen-crm.org/efrbroo/F41_Representative_Manifestation_Assignment"/>
      <rdfs:range rdf:resource="http://erlangen-crm.org/efrbroo/F44_Bibliographic_Agency"/>
      <rdfs:subPropertyOf rdf:resource="http://erlangen-crm.org/current/P14_carried_out_by"/>
      <rdfs:comment>Quantification:
(1,1:0,n)</rdfs:comment>
      <rdfs:comment>Scope note:
This property associates a bibliographic agency (represented by one or more of its cataloguers) and the assigning of which Manifestation (i.e., which instance of F3 Manifestation Product Type or F4 Manifestation Singleton) is representative for a given expression.In cataloguing practice, such a relationship is usually just implicit. However, it can become explicit, for example when a bibliographic agency creates an authority record for a given work and fills the “Source” field with information about the publication that contains the expression that was used by the bibliographic agency to establish the controlled access point for the work realised in that expression.</rdfs:comment>
      <rdfs:comment>Examples:
Assigning the manuscript identified by shelfmark ‘MS-8282’ within the collections of the National Library of France, Department for Music, as representative for the musical text of Stanislas Champein’s opera ‘Vichnou’ (F41) R43 carried out by the National Library of France (F44), identified by code ‘FRBNF’ at the beginning of field 001 in the INTERMARC authority record created for Stanislas Champein’s opera ‘Vichnou’Assigning the 1775 edition of Richard Brinsley Sheridan’s textual work entitled ‘St. Patrick’s Day’ (F41), mentioned in the ‘Encyclopaedia Britannica’, 15th edition, R43 carried out by the Library of Congress (F44), identified by code ‘DLC’ in field 040 of the MARC 21 authority record created for Richard Brinsley Sheridan’s textual work entitled ‘St. Patrick’s Day’</rdfs:comment>
   </owl:ObjectProperty>
   <!--http://erlangen-crm.org/efrbroo/R44_carried_out_by-->
   <owl:ObjectProperty rdf:about="http://erlangen-crm.org/efrbroo/R44_carried_out_by">
      <rdfs:label xml:lang="en">R44 carried out by</rdfs:label>
      <owl:inverseOf rdf:resource="http://erlangen-crm.org/efrbroo/R44i_performed"/>
      <rdfs:domain rdf:resource="http://erlangen-crm.org/efrbroo/F42_Representative_Expression_Assignment"/>
      <rdfs:range rdf:resource="http://erlangen-crm.org/efrbroo/F44_Bibliographic_Agency"/>
      <rdfs:subPropertyOf rdf:resource="http://erlangen-crm.org/current/P14_carried_out_by"/>
      <rdfs:comment>Quantification:
(1,1:0,n)</rdfs:comment>
      <rdfs:comment>Scope note:
This property associates a bibliographic agency (represented by one or more of its cataloguers) and the assigning of which expression is representative for a given Work.In cataloguing practice, such a relationship is usually just implicit. However, it can become explicit, for example when a bibliographic agency creates an authority record for a given work and fills the “Source” field with information about the publication that contains the expression that was used by the bibliographic agency to establish the controlled access point for the work realised in that expression.</rdfs:comment>
      <rdfs:comment>Examples:
Assigning the musical text contained in the manuscript identified by shelfmark ‘MS-8282’ within the collections of the National Library of France, Department for Music, as representative for Stanislas Champein’s opera ‘Vichnou’ (F41) R44 carried out by the National Library of France, identified by code ‘FRBNF’ at the beginning of field 001 in the INTERMARC authority record for Stanislas Champein’s opera ‘Vichnou’ (F44)Assigning the text embodied in the 1775 edition of Richard Brinsley Sheridan’s textual work entitled ‘St. Patrick’s Day’ as the representative expression for Richard Brinsley Sheridan’s textual work entitled ‘St. Patrick’s Day’ (F42) R44 carried out by the bibliographic agency identified, in field 040 of a MARC 21 authority record for Richard Brinsley Sheridan’s textual work entitled ‘St. Patrick’s Day’, by the code ‘DLC’ (i.e., the Library of Congress) (F44)</rdfs:comment>
   </owl:ObjectProperty>
   <!--http://erlangen-crm.org/efrbroo/R45_assigned_to-->
   <owl:ObjectProperty rdf:about="http://erlangen-crm.org/efrbroo/R45_assigned_to">
      <rdfs:label xml:lang="en">R45 assigned to</rdfs:label>
      <owl:inverseOf rdf:resource="http://erlangen-crm.org/efrbroo/R45i_was_assigned_by"/>
      <rdfs:domain rdf:resource="http://erlangen-crm.org/efrbroo/F40_Identifier_Assignment"/>
      <rdfs:range rdf:resource="http://erlangen-crm.org/current/E1_CRM_Entity"/>
      <rdfs:subPropertyOf rdf:resource="http://erlangen-crm.org/current/P140_assigned_attribute_to"/>
      <rdfs:comment>Quantification:
(1,1:0,n)</rdfs:comment>
      <rdfs:comment>Scope note:
This property identifies the entity to which an actor, such as a bibliographic agency, assigned an instance of F13 Identifier.</rdfs:comment>
      <rdfs:comment>Examples:
Assigning the controlled access point ‘The Adoration of the Shepherds (Coventry)’ (F40) R45 assigned to the anonymous textual work otherwise simply known as ‘The Adoration of the Shepherds’ (F15) [assignment of an Identifier to a Work]Assigning the controlled access point ‘Rite of spring (Choreographic Work: Bausch)’ (F40) R45 assigned to Pina Bausch’s choreographic work entitled ‘Rite of spring’ (F15) [assignment of an Identifier to a Work]Assigning the controlled access point ‘King Kong (1933)’ (F40) R45 assigned to the motion picture directed in 1933 by Merian C. Cooper and Ernest B. Schoedsack, entitled ‘King Kong’ (F15) [assignment of an Identifier to a Work]Assigning the controlled access point ‘Guillaume, de Machaut, ca. 1300-1377’ (F40) R45 assigned to Guillaume de Machaut (F10) [assignment of an Identifier to a Person]Assigning the controlled access point ‘Univerza v Ljubljani. Oddelek za bibliotekarstvo’ (F40) R45 assigned to the Department for library science of the University of Ljubljana (F11) [assignment of an Identifier to a Corporate Body]</rdfs:comment>
   </owl:ObjectProperty>
   <!--http://erlangen-crm.org/efrbroo/R46_assigned-->
   <owl:ObjectProperty rdf:about="http://erlangen-crm.org/efrbroo/R46_assigned">
      <rdfs:label xml:lang="en">R46 assigned</rdfs:label>
      <owl:inverseOf rdf:resource="http://erlangen-crm.org/efrbroo/R46i_was_assigned_by"/>
      <rdfs:domain rdf:resource="http://erlangen-crm.org/efrbroo/F40_Identifier_Assignment"/>
      <rdfs:range rdf:resource="http://erlangen-crm.org/efrbroo/F13_Identifier"/>
      <rdfs:comment>Quantification:
(1,1:0,n)</rdfs:comment>
      <rdfs:comment>Scope note:
This property associates the instance of F13 Identifier assigned to an instance of E1 CRM Entity and the event of assigning it.</rdfs:comment>
      <rdfs:comment>Examples:
Assigning a controlled access point to the anonymous textual work known as ‘The Adoration of the Shepherds’, a title shared by another, distinct anonymous textual work (F40) R46 assigned the controlled access point ‘The Adoration of the Shepherds (Coventry)’ (F50)Assigning a controlled access point to Pina Bausch’s choreographic work entitled ‘Rite of spring’ (F40) R46 assigned the controlled access point ‘Rite of spring (Choreographic Work: Bausch)’ (F50)Assigning a controlled access point to the motion picture directed in 1933 by Merian C. Cooper and Ernest B. Schoedsack and entitled ‘King Kong’ (F40) R46 assigned the controlled access point ‘King Kong (1933)’ (F50)Assigning a controlled access point to Guillaume de Machaut (F40) R46 assigned ‘Guillaume, de Machaut, ca. 1300-1377’ (F50)Assigning a controlled access point to the Department for library science of the University of Ljubljana (F40) R46 assigned ‘Univerza v Ljubljani. Oddelek za bibliotekarstvo’ (F50)Assigning a subject heading (in an authority record) to the concept of knowledge representation (F40) R46 assigned ‘Conceptual structures (Information theory)’ (F50)Assigning a subject heading (in a bibliographic record) to the concept of the appreciation of Victor Hugo’s works in Germany between 1870 and 1914 (F40) R46 assigned ‘Hugo, Victor, 1802-1885 – Appreciation – Germany – 1870-1914’ (F13)</rdfs:comment>
   </owl:ObjectProperty>
   <!--http://erlangen-crm.org/efrbroo/R48_assigned_to-->
   <owl:ObjectProperty rdf:about="http://erlangen-crm.org/efrbroo/R48_assigned_to">
      <rdfs:label xml:lang="en">R48 assigned to</rdfs:label>
      <owl:inverseOf rdf:resource="http://erlangen-crm.org/efrbroo/R48i_was_assigned_by"/>
      <rdfs:domain rdf:resource="http://erlangen-crm.org/efrbroo/F41_Representative_Manifestation_Assignment"/>
      <rdfs:range rdf:resource="http://erlangen-crm.org/efrbroo/F2_Expression"/>
      <rdfs:subPropertyOf rdf:resource="http://erlangen-crm.org/current/P140_assigned_attribute_to"/>
      <rdfs:comment>Quantification:
(1,1:0,n)</rdfs:comment>
      <rdfs:comment>Scope note:
This property associates the event of assigning a representative instance of F3 Manifestation Product Type or F4 Manifestation Singleton with the expression to which it was assigned.</rdfs:comment>
      <rdfs:comment>Examples:
Selecting the 1775 edition of Richard Brinsley Sheridan’s textual work entitled ‘St. Patrick’s Day’ as the representative manifestation for the text of Richard Brinsley Sheridan’s textual work entitled ‘St. Patrick’s Day’ (F41) R48 assigned to the text of Richard Brinsley Sheridan’s textual work entitled ‘St. Patrick’s Day’ (F22)Selecting the 2007 edition of John Tavener’s musical work entitled ‘The Eternal Sun’ as the representative manifestation for the notation of John Tavener’s musical work entitled ‘The Eternal Sun’ (F41) R48 assigned to the notation of John Tavener’s musical work entitled ‘The Eternal Sun’ (F22)Selecting the 1983 edition of Stanley Karnow’s textual work entitled ‘Vietnam, the war nobody won’ as the representative manifestation for a partial expression of the series entitled ‘Headline series’ (F41) R48 assigned to the content of the series entitled ‘Headline series’ (F22)Selecting the issue dated October 2002 of the periodical entitled ‘The New Courier’ as the representative manifestation for a partial expression of the periodical entitled ‘The New Courier’ (F41) R48 assigned to the content of the periodical entitled ‘The New Courier’ (F22)Selecting the manuscript held by the National Library of France and identified by shelf mark ‘MS-8282’ as the representative Manifestation Singleton for the notation of Stanislas Champein’s opera ‘Vichnou’ (F41) R48 assigned to the notation of Stanislas Champein’s opera ‘Vichnou’ (F22)</rdfs:comment>
   </owl:ObjectProperty>
   <!--http://erlangen-crm.org/efrbroo/R49_assigned-->
   <owl:ObjectProperty rdf:about="http://erlangen-crm.org/efrbroo/R49_assigned">
      <rdfs:label xml:lang="en">R49 assigned</rdfs:label>
      <owl:inverseOf rdf:resource="http://erlangen-crm.org/efrbroo/R49i_was_assigned_by"/>
      <rdfs:domain rdf:resource="http://erlangen-crm.org/efrbroo/F41_Representative_Manifestation_Assignment"/>
      <rdfs:range rdf:resource="http://erlangen-crm.org/efrbroo/F3_Manifestation_Product_Type"/>
      <rdfs:subPropertyOf rdf:resource="http://erlangen-crm.org/current/P141_assigned"/>
      <rdfs:comment>Quantification:
(0,n:0,n)</rdfs:comment>
      <rdfs:comment>Scope note:
This property associates the event of assigning a representative instance of F3 Manifestation Product Type with the F3 Manifestation Product Type which has been assigned.</rdfs:comment>
      <rdfs:comment>Examples:
Selecting the representative manifestation for the text of Richard Brinsley Sheridan’s textual work entitled ‘St. Patrick’s Day’ (F41) R49 assigned the 1775 edition of Richard Brinsley Sheridan’s textual work entitled ‘St. Patrick’s Day’ (F3)Selecting the representative manifestation for the notation of John Tavener’s musical work entitled ‘The Eternal Sun’ (F41) R49 assigned the 2007 edition of John Tavener’s musical work entitled ‘The Eternal Sun’ (F3)Selecting the representative manifestation for a partial expression of the series entitled ‘Headline series’ (F41) R49 assigned the 1983 edition of Stanley Karnow’s textual work entitled ‘Vietnam, the war nobody won’ (F3)Selecting the representative manifestation for a partial expression of the periodical entitled ‘The New Courier’ (F41) R49 assigned the issue dated October 2002 of the periodical entitled ‘The New Courier’ (F22)</rdfs:comment>
   </owl:ObjectProperty>
   <!--http://erlangen-crm.org/efrbroo/R50_assigned_to-->
   <owl:ObjectProperty rdf:about="http://erlangen-crm.org/efrbroo/R50_assigned_to">
      <rdfs:label xml:lang="en">R50 assigned to</rdfs:label>
      <owl:inverseOf rdf:resource="http://erlangen-crm.org/efrbroo/R50i_was_assigned_by"/>
      <rdfs:domain rdf:resource="http://erlangen-crm.org/efrbroo/F42_Representative_Expression_Assignment"/>
      <rdfs:range rdf:resource="http://erlangen-crm.org/efrbroo/F15_Complex_Work"/>
      <rdfs:subPropertyOf rdf:resource="http://erlangen-crm.org/current/P140_assigned_attribute_to"/>
      <rdfs:comment>Quantification:
(1,1:0,n)</rdfs:comment>
      <rdfs:comment>Scope note:
This property associates the event of assigning a representative instance of F2 Expression with the instance of F15 Complex Work to which it was assigned.</rdfs:comment>
      <rdfs:comment>Examples:
Selecting the text embodied in the 1775 edition of Richard Brinsley Sheridan’s textual work entitled ‘St. Patrick’s Day’ as the representative expression for Richard Brinsley Sheridan’s textual work entitled ‘St. Patrick’s Day’ (F42) R50 assigned to Richard Brinsley Sheridan’s textual work entitled ‘St. Patrick’s Day’ (F15)Selecting the musical notation embodied in the 2007 edition of John Tavener’s musical work entitled ‘The Eternal Sun’ as the representative expression for John Tavener’s musical work entitled ‘The Eternal Sun’ (F42) R50 assigned to John Tavener’s musical work entitled ‘The Eternal Sun’ (F15)Selecting the publication expression of the 1983 edition of Stanley Karnow’s textual work entitled ‘Vietnam, the war nobody won’ as the representative expression for the series entitled ‘Headline series’ (F42) R50 assigned to the series entitled ‘Headline series’ (F18)Selecting the publication expression of the issue dated October 2002 of the periodical entitled ‘The New Courier’ as the representative expression of the periodical entitled ‘The New Courier’ (F42) R50 assigned to the periodical entitled ‘The New Courier’ (F18)Selecting the content of the manuscript identified by shelfmark ‘MS-8282’ within the collections of the National Library of France, Department for Music, as the representative expression of Stanislas Champein’s musical work entitled ‘Vichnou’ (F42) R50 assigned toStanislas Champein’s musical work entitled ‘Vichnou’ (F15)</rdfs:comment>
   </owl:ObjectProperty>
   <!--http://erlangen-crm.org/efrbroo/R51_assigned-->
   <owl:ObjectProperty rdf:about="http://erlangen-crm.org/efrbroo/R51_assigned">
      <rdfs:label xml:lang="en">R51 assigned</rdfs:label>
      <owl:inverseOf rdf:resource="http://erlangen-crm.org/efrbroo/R51i_was_assigned_by"/>
      <rdfs:domain rdf:resource="http://erlangen-crm.org/efrbroo/F42_Representative_Expression_Assignment"/>
      <rdfs:range rdf:resource="http://erlangen-crm.org/efrbroo/F2_Expression"/>
      <rdfs:subPropertyOf rdf:resource="http://erlangen-crm.org/current/P141_assigned"/>
      <rdfs:comment>Quantification:
(1,n:0,n)</rdfs:comment>
      <rdfs:comment>Scope note:
This property associates the event of assigning a representative instance of F2 Expression with the F2 Expression which has been assigned.</rdfs:comment>
      <rdfs:comment>Examples:
Selecting the representative expression for Richard Brinsley Sheridan’s textual work entitled ‘St. Patrick’s Day’ (F42) R51 assigned the text embodied in the 1775 edition of Richard Brinsley Sheridan’s textual work entitled ‘St. Patrick’s Day’ (F22)Selecting the representative expression for John Tavener’s musical work entitled ‘The Eternal Sun’ (F42) R51 assigned the musical notation embodied in the 2007 edition of John Tavener’s musical work entitled ‘The Eternal Sun’ (F15)Selecting the representative expression for the series entitled ‘Headline series’ (F42) R51 assigned the publication expression of the volume of the series entitled ‘Headline series’ that consists of the 1983 edition of Stanley Karnow’s textual work entitled ‘Vietnam, the war nobody won’ (F24)Selecting the representative expression of the periodical entitled ‘The New Courier’ (F42) R51 assigned the publication expression of the issue dated October 2002 of the periodical entitled ‘The New Courier’ (F24)Selecting the representative expression of Stanislas Champein’s musical work entitled ‘Vichnou’ (F42) R51 assigned the content of the manuscript identified by shelfmark ‘MS-8282’ within the collections of the National Library of France, Department for Music (F22)</rdfs:comment>
   </owl:ObjectProperty>
   <!--http://erlangen-crm.org/efrbroo/R52_used_rule-->
   <owl:ObjectProperty rdf:about="http://erlangen-crm.org/efrbroo/R52_used_rule">
      <rdfs:label xml:lang="en">R52 used rule</rdfs:label>
      <owl:inverseOf rdf:resource="http://erlangen-crm.org/efrbroo/R52i_was_the_rule_used_in"/>
      <rdfs:domain rdf:resource="http://erlangen-crm.org/efrbroo/F40_Identifier_Assignment"/>
      <rdfs:range rdf:resource="http://erlangen-crm.org/efrbroo/F43_Identifier_Rule"/>
      <rdfs:subPropertyOf rdf:resource="http://erlangen-crm.org/current/P33_used_specific_technique"/>
      <rdfs:comment>Quantification:
(0,n:0,n)</rdfs:comment>
      <rdfs:comment>Scope note:
This property associates the event of assigning an instance of F13 Identifier with the instructions followed by an actor, such as a Bibliographic Agency, in creating that identifier.</rdfs:comment>
      <rdfs:comment>Examples:
Assigning the controlled access point ‘Bach, Johann Sebastian, 1685-1750. Concertos, violins (2), string orchestra, BWV 1043, D minor’ to Johann Sebastian Bach’s Double Concerto in D minor, BWV 1043 (F40) R52 used rule AACR2R 25.25-25.35F1 (F43)Assigning the controlled access point ‘Bach, Johann Sebastian [Konzerte, Vl 1 2 Orch BWV 1043]’ to Johann Sebastian Bach’s Double Concerto in D minor, BWV 1043 (F40) R52 used rule RAK-Musik (Revidierte Ausgabe 2003), Chapter 6 (F43)Assigning the controlled access point ‘Bach, Johann Sebastian (1685-1750). – [Concertos. Violons (2), orchestre à cordes. BWV 1043. Ré mineur]’ to Johann Sebastian Bach’s Double Concerto in D minor, BWV 1043 (F40) R52 used rule AFNOR Z 44-079 (F43)Assigning the controlled access point ‘Guillaume de Machaut (1300?-1377)’ (F40) R52 used rule AFNOR Z 44-061 (F43)Assigning the controlled access point ‘Guillaume, de Machaut, ca. 1300-1377’ (F40) R52 used rule AACR2R 22 (F43)Assigning the controlled access point ‘Guillaume, de Machaut, approximately 1300-1377’ (F40) R52 used rule RDA 9.19 (F43)</rdfs:comment>
   </owl:ObjectProperty>
   <!--http://erlangen-crm.org/efrbroo/R53_assigned-->
   <owl:ObjectProperty rdf:about="http://erlangen-crm.org/efrbroo/R53_assigned">
      <rdfs:label xml:lang="en">R53 assigned</rdfs:label>
      <owl:inverseOf rdf:resource="http://erlangen-crm.org/efrbroo/R53i_was_assigned_by"/>
      <rdfs:domain rdf:resource="http://erlangen-crm.org/efrbroo/F41_Representative_Manifestation_Assignment"/>
      <rdfs:range rdf:resource="http://erlangen-crm.org/efrbroo/F4_Manifestation_Singleton"/>
      <rdfs:subPropertyOf rdf:resource="http://erlangen-crm.org/current/P141_assigned"/>
      <rdfs:comment>Quantification:
(0,n:0,n)</rdfs:comment>
      <rdfs:comment>Scope note:
This property associates the event of assigning a representative instance of F4 Manifestation Singleton with the F4 Manifestation Singleton which has been assigned.</rdfs:comment>
      <rdfs:comment>Examples:
Selecting the representative Manifestation Singleton for the notation of Stanislas Champein’s opera ‘Vichnou’ (F41) R53 assigned the manuscript held by the National Library of France and identified by shelf mark ‘MS-8282’ (F4)</rdfs:comment>
   </owl:ObjectProperty>
   <!--http://erlangen-crm.org/efrbroo/R54_has_nomen_language-->
   <owl:ObjectProperty rdf:about="http://erlangen-crm.org/efrbroo/R54_has_nomen_language">
      <rdfs:label xml:lang="en">R54 has nomen language</rdfs:label>
      <owl:inverseOf rdf:resource="http://erlangen-crm.org/efrbroo/R54i_is_language_of_nomen_in"/>
      <rdfs:domain rdf:resource="http://erlangen-crm.org/efrbroo/F35_Nomen_Use_Statement"/>
      <rdfs:range rdf:resource="http://erlangen-crm.org/current/E56_Language"/>
      <rdfs:subPropertyOf rdf:resource="http://erlangen-crm.org/current/P67_refers_to"/>
      <rdfs:comment>Quantification:
(0,n:0,n)</rdfs:comment>
      <rdfs:comment>Scope note:
This property associates an instance of F35 Nomen Use Statement with an instance of E56 Language which is a target language for the associated nomen use.</rdfs:comment>
      <rdfs:comment>Examples:
‘001  FRBNF119304566’…‘100  $w.0..b.spa.$aColón$mCristóbal$d1450?-1506’ (F35) R54 has nomen language the language referred to in subfield $w by the ISO code ‘spa,’ i.e., Spanish (E56)‘001  FRBNF119304566’…‘400  $w....b.eng.$aColumbus$mChristopher$d1450?-1506’ (F35) R54 has nomen language the language referred to in subfield $w by the ISO code ‘eng,’ i.e., English (E56)‘001  FRBNF118726828’…‘110  $w20..b.fre.$aConseil international des musées’ (F35) R54 has nomen language the language referred to in subfield $w by the ISO code ‘fre,’ i.e., French (E56)‘001  FRBNF118726828’…‘110  $w20..b.ger.$aInternationaler Museumsrat’ (F35) R54 has nomen language the language referred to in subfield $w by the ISO code ‘ger,’ i.e., German (E56)‘ID: 300024668’…‘navaja (C,U,Spanish,UF,U,SN)’ R54 has nomen language Spanish (E56) (“used for” term, Getty Art &amp; Architecture Thesaurus Online, retrieved 19/11/2012)</rdfs:comment>
   </owl:ObjectProperty>
   <!--http://erlangen-crm.org/efrbroo/R55_has_nomen_form-->
   <owl:ObjectProperty rdf:about="http://erlangen-crm.org/efrbroo/R55_has_nomen_form">
      <rdfs:label xml:lang="en">R55 has nomen form</rdfs:label>
      <owl:inverseOf rdf:resource="http://erlangen-crm.org/efrbroo/R55i_is_nomen_form_in"/>
      <rdfs:domain rdf:resource="http://erlangen-crm.org/efrbroo/F35_Nomen_Use_Statement"/>
      <rdfs:range rdf:resource="http://erlangen-crm.org/current/E55_Type"/>
      <rdfs:subPropertyOf rdf:resource="http://erlangen-crm.org/current/P67_refers_to"/>
      <rdfs:comment>Quantification:
(0,1:0,n)</rdfs:comment>
      <rdfs:comment>Scope note:
This property associates an instance of F35 Nomen Use Statement with the instance of E55 Type that characterizes the Nomen referred to in the Nomen Use Statement, such as abbreviation, full name etc. In the case of abbreviations, the source of this form may or may not be explicitly mentioned.</rdfs:comment>
      <rdfs:comment>Examples:
‘010 __ |a n 78004438’…‘410 2_ |a IFLA’ to refer to the International Federation of Library Associations and Institutions (F35) R55 has nomen form acronym (E55)</rdfs:comment>
   </owl:ObjectProperty>
   <!--http://erlangen-crm.org/efrbroo/R56_has_related_use-->
   <owl:ObjectProperty rdf:about="http://erlangen-crm.org/efrbroo/R56_has_related_use">
      <rdfs:label xml:lang="en">R56 has related use</rdfs:label>
      <owl:inverseOf rdf:resource="http://erlangen-crm.org/efrbroo/R56i_is_related_use_for"/>
      <rdfs:domain rdf:resource="http://erlangen-crm.org/efrbroo/F35_Nomen_Use_Statement"/>
      <rdfs:range rdf:resource="http://erlangen-crm.org/efrbroo/F35_Nomen_Use_Statement"/>
      <rdfs:subPropertyOf rdf:resource="http://erlangen-crm.org/current/P69_has_association_with"/>
      <rdfs:comment>Quantification:
(0,n:0,n)</rdfs:comment>
      <rdfs:comment>Scope note:
This property associates an instance of F35 Nomen Use Statement with another instance of F35 Nomen Use Statement which has a related use in some context, such as alternative, lexical variant, replacing former use etc. The property R56.1 allows for specifying the particular kind of the nomen use statement relationship.</rdfs:comment>
      <rdfs:comment>Examples:
‘001  FRBNF122597517’…‘14506$w.1..b.fre.$aDu sublime’ [an instance of F35 Nomen Use Statement in INTERMARC format] (F35) R56 has related use ‘001  FRBNF122597517’…‘14506$w.0..g.grp $aΠερὶ ὕπσους’ [an instance of F35 Nomen Use Statement in INTERMARC format] (F35) R56.1 has type parallel form (E55)‘001  FRBNF126866954’…‘100  $w.0..b.....$aTyrrell$mGeorge$d1861-1909’ [an instance of F35 Nomen Use Statement in INTERMARC format] (F35) R56 has related use ‘001  FRBNF126866954’…‘466  $w....b     $aTyrell$oAffaire$g1907’ [an instance of F35 Nomen Use Statement in INTERMARC format] (F35) R56.1 has type variant access point for a personal name, intended to be displayed in a subject index only, and not in a personal names index (E55) [Explanation: in the INTERMARC format used at the National Library of France, tag 466 in an authority record for a person serves to introduce a topical term which is displayed as a variant form for the personal name in the subject index, but is not displayed in the name index]‘010 __ |a n 78004438’…‘110 2_ |a International Federation of Library Associations and Institutions’ [an instance of F35 Nomen Use Statement in MARC 21 format] (F35) R56 has related use ‘010 __ |a n 78004438’…‘410 2_ |a IFLA’ [an instance of F35 Nomen Use Statement in MARC 21 format] (F35) R56.1 has type acronym (E55) (in MARC 21 field 410 serves as a reference to the accepted form which appears in field 110)‘PTBNP|20891’…‘200 1‎‡a Whitman,‏ ‎‡b Walt,‏ ‎‡f 1819-1892‏’ (F35) R56 has related use ‘PTBNP|20891’…‘675 ‎‡a 820(73) Whitman, Walt.09‏ ‎‡v BN‏ ‎‡z por‏’ R56.1 has type has associated UDC number (in UNIMARC field 675 serves to associate a UDC number with the accepted form which appears in field 200)‘&lt;eac-cpf […]&gt; &lt;control&gt; &lt;recordId&gt;beinecke.7h44jbj&lt;/recordId&gt; […] &lt;/control&gt;’ … ‘&lt;cpfDescription&gt; &lt;identity&gt; &lt;entityType&gt;family&lt;/entityType&gt; &lt;nameEntry xml:lang="eng" scriptCode="Latn"&gt;&lt;part localType="100a"&gt;Boswell family&lt;/part&gt; […] &lt;/nameEntry&gt; […] &lt;/identity&gt; &lt;/cpfDescription&gt; […] &lt;/eac-cpf&gt;’ [an instance of F35 Nomen Use Statement in EAC] (F35) R56 has related use ‘&lt;eac-cpf […]&gt; &lt;control&gt; &lt;recordId&gt;beinecke.7h44jbj&lt;/recordId&gt; […] &lt;/control&gt;’ … ‘&lt;cpfDescription&gt; &lt;identity&gt; &lt;entityType&gt;family&lt;/entityType&gt; &lt;nameEntry xml:lang="eng" scriptCode="Latn"&gt; &lt;part localType="400a"&gt;Buzwell family &lt;/part&gt; […] &lt;/nameEntry&gt; […] &lt;/identity&gt; &lt;/cpfDescription&gt; […] &lt;/eac-cpf&gt;’ [an instance of F35 Nomen Use Statement in EAC] (F35) R56.1 has type alternative form (E55)Properties:R56.1 has type: E55 Type</rdfs:comment>
   </owl:ObjectProperty>
   <!--http://erlangen-crm.org/efrbroo/R57_is_based_on-->
   <owl:ObjectProperty rdf:about="http://erlangen-crm.org/efrbroo/R57_is_based_on">
      <rdfs:label xml:lang="en">R57 is based on</rdfs:label>
      <owl:inverseOf rdf:resource="http://erlangen-crm.org/efrbroo/R57i_is_basis_for"/>
      <rdfs:domain rdf:resource="http://erlangen-crm.org/efrbroo/F38_Character"/>
      <rdfs:range rdf:resource="http://erlangen-crm.org/current/E39_Actor"/>
      <rdfs:comment>Shortcut of:
F38 Character. P94i was created by (has created): E65 Creation. P17 was motivated by (motivated): E39 Actor</rdfs:comment>
      <rdfs:comment>Quantification:
(0,n:0,n)</rdfs:comment>
      <rdfs:comment>Scope note:
This property associates an instance of F38 Character with an instance of E39 Actor that the character is motivated by or is intended to represent. An instance of F38 Character may be based on a combination of features taken from several actors. This property is a shortcut of the more fully developed path from E28 Conceptual Object, restricted to F38 Character, through the inverse of P94 has created (was created by), E65 Creation P17 was motivated by (motivated) to E1 CRM Entity restricted to E39 Actor.</rdfs:comment>
      <rdfs:comment>Examples:
The Character ‘Sinuhe’ (F38) in Mika Waltari’s ‘Sinuhe the Egyptian: A Novel’ R57 is based on Sinuhe (E21) (documented in the autobiographic narrative in fragments carried by The Ramesside Papyrus, Pap. Berlin 10499, Pap. Berlin 3022, The Amherst fragments (m-q) and other Egyptian sources)The Character ‘Alexander’ (F38) in Mary Renault’s ‘Fire from Heaven’ R57 is based on Alexander the Great of Macedon (356-323) (E21)</rdfs:comment>
   </owl:ObjectProperty>
   <!--http://erlangen-crm.org/efrbroo/R58_has_fictional_member-->
   <owl:ObjectProperty rdf:about="http://erlangen-crm.org/efrbroo/R58_has_fictional_member">
      <rdfs:label xml:lang="en">R58 has fictional member</rdfs:label>
      <owl:inverseOf rdf:resource="http://erlangen-crm.org/efrbroo/R58i_is_fictional_member_of"/>
      <rdfs:domain rdf:resource="http://erlangen-crm.org/efrbroo/F38_Character"/>
      <rdfs:range rdf:resource="http://erlangen-crm.org/efrbroo/F38_Character"/>
      <rdfs:comment>Quantification:
(0,n:0,n)</rdfs:comment>
      <rdfs:comment>Scope note:
This property associates an instance of F38 Character representing a group with another instance of F38 Character that is presented in relevant fiction as a member of the fictional group.</rdfs:comment>
      <rdfs:comment>Examples:
Argonauts (F38) R58 has fictional member Jason (F38)</rdfs:comment>
   </owl:ObjectProperty>
   <!--http://erlangen-crm.org/efrbroo/R59_had_typical_subject-->
   <owl:ObjectProperty rdf:about="http://erlangen-crm.org/efrbroo/R59_had_typical_subject">
      <rdfs:label xml:lang="en">R59 had typical subject</rdfs:label>
      <owl:inverseOf rdf:resource="http://erlangen-crm.org/efrbroo/R59i_was_typical_subject_of"/>
      <rdfs:domain rdf:resource="http://erlangen-crm.org/efrbroo/F51_Pursuit"/>
      <rdfs:range rdf:resource="http://erlangen-crm.org/current/E1_CRM_Entity"/>
      <rdfs:subPropertyOf rdf:resource="http://erlangen-crm.org/current/P94_has_created"/>
      <rdfs:comment>Quantification:
(0,n:0,n)</rdfs:comment>
      <rdfs:comment>Scope note:
This property associates an instance of F51 Pursuit with the instance of E1 CRM Entity that is the typical subject of the associated activity, such as an area of expertise in which the actor is engaged or was engaged.</rdfs:comment>
      <rdfs:comment>Examples:
John Dover Wilson’s activity as a Shakespeare scholar (F51) R59 had typical subject William Shakespeare (F10)</rdfs:comment>
   </owl:ObjectProperty>
   <!--http://erlangen-crm.org/efrbroo/R60_used_to_use_language-->
   <owl:ObjectProperty rdf:about="http://erlangen-crm.org/efrbroo/R60_used_to_use_language">
      <rdfs:label xml:lang="en">R60 used to use language</rdfs:label>
      <owl:inverseOf rdf:resource="http://erlangen-crm.org/efrbroo/R60i_was_language_used_by"/>
      <rdfs:domain rdf:resource="http://erlangen-crm.org/efrbroo/F51_Pursuit"/>
      <rdfs:range rdf:resource="http://erlangen-crm.org/current/E56_Language"/>
      <rdfs:comment>Shortcut of:
E65 Creation. P94 has created (was created by): E33 Linguistic Object. P72 has language (is language of): E56 Language</rdfs:comment>
      <rdfs:comment>Quantification:
(0,n:0,n)</rdfs:comment>
      <rdfs:comment>Scope note:
This property associates an instance of F51 Pursuit with the instance of E56 Language that was characteristically used for the products of the associated activity.The property R60.1 has type of use allows for specifying a particular form of use.</rdfs:comment>
      <rdfs:comment>Examples:
Samuel Beckett’s activity as author of English texts (F51) R60 used to use language English (E56) R60.1 has type of use Authorship (E55)Samuel Beckett’s activity as author of French texts (F51) R60 used to use language French (E56) R60.1 has type of use Authorship (E55)Samuel Beckett’s activity as translator of English texts into French (F51) R60 used to use language French (E56) R60.1 has type of use Translation – target language (E55)Samuel Beckett’s activity as translator of English texts (F51) R60 used to use language English (E56) R60.1 has type of use Translation – source language (E55)Properties:R60.1 has type of use: E55 Type</rdfs:comment>
   </owl:ObjectProperty>
   <!--http://erlangen-crm.org/efrbroo/R61_occurred_in_kind_of_context-->
   <owl:ObjectProperty rdf:about="http://erlangen-crm.org/efrbroo/R61_occurred_in_kind_of_context">
      <rdfs:label xml:lang="en">R61 occurred in kind of context</rdfs:label>
      <owl:inverseOf rdf:resource="http://erlangen-crm.org/efrbroo/R61i_was_kind_of_context_for"/>
      <rdfs:domain rdf:resource="http://erlangen-crm.org/efrbroo/F52_Name_Use_Activity"/>
      <rdfs:range rdf:resource="http://erlangen-crm.org/current/E55_Type"/>
      <rdfs:comment>Shortcut of:
F52 Name Use Activity. P9i forms part of: F51 Pursuit. P2 has type: E55 Type</rdfs:comment>
      <rdfs:comment>Quantification:
(0,n:0,n)</rdfs:comment>
      <rdfs:comment>Scope note:
This property associates an instance of F52 Name Use Activity with the instance of E55 Type that characterises the kind of role or context within which the associated name was used.</rdfs:comment>
      <rdfs:comment>Examples:
Charles Lutwidge Dodgson using the name ‘Lewis Carroll’ (F52) R61 occurred in kind of context writing for children (E55)Charles Lutwidge Dodgson using the name ‘Charles Dodgson’ (F52) R61 occurred in kind of context writing in mathematics (E55)</rdfs:comment>
   </owl:ObjectProperty>
   <!--http://erlangen-crm.org/efrbroo/R62_was_used_for_membership_in-->
   <owl:ObjectProperty rdf:about="http://erlangen-crm.org/efrbroo/R62_was_used_for_membership_in">
      <rdfs:label xml:lang="en">R62 was used for membership in</rdfs:label>
      <owl:inverseOf rdf:resource="http://erlangen-crm.org/efrbroo/R62i_was_context_for"/>
      <rdfs:domain rdf:resource="http://erlangen-crm.org/efrbroo/F52_Name_Use_Activity"/>
      <rdfs:range rdf:resource="http://erlangen-crm.org/current/E74_Group"/>
      <rdfs:comment>Shortcut of:
E7 Activity. P17 was motivated by (motivated): E85 Joining. P144 joined with: E74 Group</rdfs:comment>
      <rdfs:comment>Quantification:
(0,n:0,n)</rdfs:comment>
      <rdfs:comment>Scope note:
This property associates an instance of F52 Name Use Activity with the instance of E74 Group that characterises the context within which the associated name was used for membership in that group.</rdfs:comment>
      <rdfs:comment>Examples:
Using the name ‘John Paul I’ (F52) R62 was used for membership in the corporate body identified in the Library of Congress’s authority file as ‘Catholic Church. Pope’ (F11)</rdfs:comment>
   </owl:ObjectProperty>
   <!--http://erlangen-crm.org/efrbroo/R63_named-->
   <owl:ObjectProperty rdf:about="http://erlangen-crm.org/efrbroo/R63_named">
      <rdfs:label xml:lang="en">R63 named</rdfs:label>
      <owl:inverseOf rdf:resource="http://erlangen-crm.org/efrbroo/R63i_was_named_by"/>
      <rdfs:domain rdf:resource="http://erlangen-crm.org/efrbroo/F52_Name_Use_Activity"/>
      <rdfs:range rdf:resource="http://erlangen-crm.org/current/E1_CRM_Entity"/>
      <rdfs:subPropertyOf rdf:resource="http://erlangen-crm.org/current/P140_assigned_attribute_to"/>
      <rdfs:comment>Quantification:
(1,1:0,n)</rdfs:comment>
      <rdfs:comment>Scope note:
This property associates an instance of F52 Name Use Activity with the instance of E1 CRM Entity that the associated name was used for.</rdfs:comment>
      <rdfs:comment>Examples:
The recording of the MARC 21 field ‘110 2_ |a Canadian Academic Centre in Italy’ (F52) R63 named the instance of F11 Corporate Body represented by the Library of Congress authority record number n 85118480The appearance of the name ‘Centro accademico canadese in Italia’ on the title page of the book ‘Lo Scavo di S. Giovanni di Ruoti ed il periodo tardoantico in Basilicata’ published in 1983 (F52) R63 named the instance of F11 Corporate Body represented by the Library of Congress authority record number n 85118480The statement ‘The International Federation of Library Associations and Institutions (IFLA) is the leading international body representing the interests of library and information services and their users’ cited from the ‘About IFLA’ page of the website http://www.ifla.org/ (F35) R63 named the instance of F11 Corporate Body represented by the Library of Congress authority record number n 78004438</rdfs:comment>
   </owl:ObjectProperty>
   <!--http://erlangen-crm.org/efrbroo/R64_used_name-->
   <owl:ObjectProperty rdf:about="http://erlangen-crm.org/efrbroo/R64_used_name">
      <rdfs:label xml:lang="en">R64 used name</rdfs:label>
      <owl:inverseOf rdf:resource="http://erlangen-crm.org/efrbroo/R64i_was_name_used_by"/>
      <rdfs:domain rdf:resource="http://erlangen-crm.org/efrbroo/F52_Name_Use_Activity"/>
      <rdfs:range rdf:resource="http://erlangen-crm.org/current/E41_Appellation"/>
      <rdfs:subPropertyOf rdf:resource="http://erlangen-crm.org/current/P16_used_specific_object"/>
      <rdfs:comment>Quantification:
(1,1:0,n)</rdfs:comment>
      <rdfs:comment>Scope note:
This property associates an instance of F52 Name Use Activity with the instance of E41 Appellation that was used for the associated entity.</rdfs:comment>
      <rdfs:comment>Examples:
The appearance of the name ‘Lewis Carroll’ on the title page of ‘Le avventure d’Alice nel paese delle meraviglie’, published in 1872 in London by Macmillan and Co. (F52) R64 used name ‘Lewis Carroll’ (E41)The appearance of the name ‘Centro accademico canadese in Italia’ on the title page of the book ‘Lo Scavo di S. Giovanni di Ruoti ed il periodo tardoantico in Basilicata’ published in 1983 (F52) R64 used name ‘Centro accademico canadese in Italia’ (E41)The appearance of the name ‘Canadian Academic Centre in Italy’ on page 6 of the book ‘Lo Scavo di S. Giovanni di Ruoti ed il periodo tardoantico in Basilicata’ published in 1983 (F52) R64 used name ‘Canadian Academic Centre in Italy’ (E41)The appearance of the name ‘IFLA’ as an acronym for ‘The International Federation of Library Associations and Institutions’ in the sentence (F2) ‘The International Federation of Library Associations and Institutions (IFLA) is the leading international body representing the interests of library and information services and their users’ cited from the ‘About IFLA’ page of the website http://www.ifla.org/ (F52) R64 used name ‘IFLA’ (E41)</rdfs:comment>
   </owl:ObjectProperty>
   <!--http://erlangen-crm.org/efrbroo/R65_recorded_aspects_of-->
   <owl:ObjectProperty rdf:about="http://erlangen-crm.org/efrbroo/R65_recorded_aspects_of">
      <rdfs:label xml:lang="en">R65 recorded aspects of</rdfs:label>
      <owl:inverseOf rdf:resource="http://erlangen-crm.org/efrbroo/R65i_had_aspects_recorded_through"/>
      <rdfs:domain rdf:resource="http://erlangen-crm.org/efrbroo/F29_Recording_Event"/>
      <rdfs:range rdf:resource="http://erlangen-crm.org/current/E18_Physical_Thing"/>
      <rdfs:comment>Shortcut of:
F29 Recording Event. R20 recorded: E3 Condition State. P44i is condition of: E18 Physical ThingSubproperty of shortcut of: F29 Recording Event. R20 recorded: E5 Event. P12 occurred in the presence of: E18 Physical Thing</rdfs:comment>
      <rdfs:comment>Quantification:
(0,n:0,n)</rdfs:comment>
      <rdfs:comment>Scope note:
This property associates an instance of F29 Recording Event with an instance of E18 Physical Thing some of whose features, at the time of recording, were recorded in that process.</rdfs:comment>
      <rdfs:comment>Examples:
The making of the photograph of the three Allied leaders at Yalta in February 1945 (F29) R65 recorded aspects of Stalin (E21)Filming Louise Bourgeois at work in the context of the shooting of the documentary movie entitled ‘Louise Bourgeois: The Spider, the Mistress, and the Tangerine’ (F29) R65 recorded aspects of Louise Bourgeois (E21)</rdfs:comment>
   </owl:ObjectProperty>
   <!--http://erlangen-crm.org/efrbroo/R66_included_performed_version_of-->
   <owl:ObjectProperty rdf:about="http://erlangen-crm.org/efrbroo/R66_included_performed_version_of">
      <rdfs:label xml:lang="en">R66 included performed version of</rdfs:label>
      <owl:inverseOf rdf:resource="http://erlangen-crm.org/efrbroo/R66i_had_a_performed_version_through"/>
      <rdfs:domain rdf:resource="http://erlangen-crm.org/efrbroo/F31_Performance"/>
      <rdfs:range rdf:resource="http://erlangen-crm.org/current/E89_Propositional_Object"/>
      <rdfs:subPropertyOf rdf:resource="http://erlangen-crm.org/current/P16_used_specific_object"/>
      <rdfs:comment>Quantification:
(0,n:0,n)</rdfs:comment>
      <rdfs:comment>Scope note:
This property associates an instance of F31 Performance with a product of the mind that was performed in the course of that instance of F31 Performance.According to the level of knowledge available about the performance, the range of this property can actually be specialised as either an instance of F1 Work (if nothing is known as to which specific expression of the work was performed), or of F2 Expression (if there is a reasonable amount of certainty as to which specific expression—e.g., a well identified translation of a play—of the work was performed).In addition to being a subproperty of P16 used specific object (was used for), this property also is a shortcut of the fully developed path that goes from F31 Performance to F1 Work through: R25 performed F25 Performance Plan P165 incorporates F22 Self-Contained Expression R3i realises. In this fully developed path, the specific instance of F22 Self-Contained Expression can be precisely identified and described for its own sake, or it can just be known to have necessarily existed.</rdfs:comment>
      <rdfs:comment>Examples:
The performance of ‘Hamlet’ on 17 June 1909 in Berlin, Deutsches Theater, by Alexander Moissi, directed by Max Reinhardt (F31) R66 included performed version of William Shakespeare’s work ‘Hamlet’ (F15) [Note: the specific German translation that was performed is not mentioned in the documentation available from http://www.glopad.org/pi/en/record/production/1001207]The performance of ‘Hamlet’ on 6 June 1964 in Zurich, Schauspielhaus, by Compagnia Proclemer-Albertazzi, directed by Franco Zeffirelli (F31) R66 included performed version of Gerardo Guerrieri’s Italian translation (F22) of William Shakespeare’s work ‘Hamlet’</rdfs:comment>
   </owl:ObjectProperty>
   <!--http://erlangen-crm.org/efrbroo/CLP2_should_have_type-->
   <owl:ObjectProperty rdf:about="http://erlangen-crm.org/efrbroo/CLP2_should_have_type">
      <rdfs:label xml:lang="en">CLP2 should have type</rdfs:label>
      <owl:inverseOf rdf:resource="http://erlangen-crm.org/efrbroo/CLP2i_should_be_type_of"/>
      <rdfs:domain rdf:resource="http://erlangen-crm.org/efrbroo/F3_Manifestation_Product_Type"/>
      <rdfs:range rdf:resource="http://erlangen-crm.org/current/E55_Type"/>
      <rdfs:comment>Quantification:
(0,n:0,n)</rdfs:comment>
      <rdfs:comment>Scope note:
This property associates a publication, i.e. an instance of F3 Manifestation Product Type, with an instance of E55 Type, which all exemplars of that publication should belong to, as long as they are recognised as exemplars of that publication. Typically, this property is observed on one exemplar of a publication, and extrapolated to all other exemplars of the same publication. This logical inference is an induction along the path that can be modelled as: F3 Manifestation Product Type R7i has example F5 Item P41i was classified by E17 Type Assignment P42 assigned E55 Type.It can happen that a given exemplar, or subset of exemplars, originally produced, or intended to be produced, with that characteristic, accidentally lacks it. This fact should be recorded as a property of F5 Item, and not of F3 Manifestation Product Type.</rdfs:comment>
      <rdfs:comment>Examples:
The sound recording entitled ‘The Glory (????) of the human voice’, identified by label and label number ‘RCA Victor Gold Seal GD61175’, containing recordings of musical works performed by Florence Foster Jenkins (F3) CLP2 should have type sound recording (E55)The sound recording entitled ‘The Glory (????) of the human voice’, identified by label and label number ‘RCA Victor Gold Seal GD61175’, containing recordings of musical works performed by Florence Foster Jenkins (F3) CLP2 should have type kind of sound: monaural (E55)</rdfs:comment>
   </owl:ObjectProperty>
   <!--http://erlangen-crm.org/efrbroo/CLP43_should_have_dimension-->
   <owl:ObjectProperty rdf:about="http://erlangen-crm.org/efrbroo/CLP43_should_have_dimension">
      <rdfs:label xml:lang="en">CLP43 should have dimension</rdfs:label>
      <owl:inverseOf rdf:resource="http://erlangen-crm.org/efrbroo/CLP43i_should_be_dimension_of"/>
      <rdfs:domain rdf:resource="http://erlangen-crm.org/efrbroo/F3_Manifestation_Product_Type"/>
      <rdfs:range rdf:resource="http://erlangen-crm.org/current/E54_Dimension"/>
      <rdfs:comment>Quantification:
(1,n:1,1)</rdfs:comment>
      <rdfs:comment>Scope note:
This property associates a publication, i.e. an instance of F3 Manifestation Product Type, with an instance of E54 Dimension, which all exemplars of that publication should have, as long as they are recognised as exemplars of that publication. Typically, this property is observed on one exemplar of a publication, and extrapolated to all other exemplars of the same publication. This logical inference is an induction along the path that can be modelled as: F3 Manifestation Product Type R7i has example F5 Item P39i was measured by E16 Measurement P40 observed dimension E54 Dimension.It can happen that a given exemplar, or subset of exemplars, originally produced, or intended to be produced, with that characteristic, accidentally lacks it. This fact should be recorded as a property of F5 Item, and not of F3 Manifestation Product Type.</rdfs:comment>
      <rdfs:comment>Examples:
The publication entitled ‘Functional Requirements for Bibliographic Records: final report’, published by K. G. Saur in 1998, identified by ISBN ‘3-598-11382-X’ (F3) CLP43 should have dimension height of the individual copy of ‘Functional Requirements for Bibliographic Records: final report’ that I have at hand and that I observed while describing it (E54) P3 has note ‘24 cm’ (E62) [or, alternatively: P90 has value ‘24’ (E60) and P91 has unit ‘cm’ (E58)]The jigsaw puzzle entitled ‘Map of the New York city subway system’, designed by Stephen J. Voorhies and released around 1954 by the Union Dimes Savings Bank (F3) CLP43 should have dimension length and height of the exemplar held and catalogued by the Library of Congress (E54) P3 has note ‘46 x 29 cm’ (E62)</rdfs:comment>
   </owl:ObjectProperty>
   <!--http://erlangen-crm.org/efrbroo/CLP45_should_consist_of-->
   <owl:ObjectProperty rdf:about="http://erlangen-crm.org/efrbroo/CLP45_should_consist_of">
      <rdfs:label xml:lang="en">CLP45 should consist of</rdfs:label>
      <owl:inverseOf rdf:resource="http://erlangen-crm.org/efrbroo/CLP45i_should_be_incorporated_in"/>
      <rdfs:domain rdf:resource="http://erlangen-crm.org/efrbroo/F3_Manifestation_Product_Type"/>
      <rdfs:range rdf:resource="http://erlangen-crm.org/current/E57_Material"/>
      <rdfs:comment>Quantification:
(0,n:0,n)</rdfs:comment>
      <rdfs:comment>Scope note:
This property associates a publication, i.e. an instance of F3 Manifestation Product Type, with an instance of E57 Material, which all exemplars of that publication should consist of, as long as they are recognised as exemplars of that publication. Typically, this property is observed on one exemplar of a publication, and extrapolated to all other exemplars of the same publication. This logical inference is an induction along the path that can be modelled as: F3 Manifestation Product Type R7i has example F5 Item P41i was classified by E17 Type Assignment P42 assigned E57 Material.It can happen that a given exemplar, or subset of exemplars, originally produced, or intended to be produced, with that characteristic, accidentally lacks it. This fact should be recorded as a property of F5 Item, and not of F3 Manifestation Product Type.</rdfs:comment>
      <rdfs:comment>Examples:
The jigsaw puzzle entitled ‘Map of the New York city subway system’, designed by Stephen J. Voorhies and released around 1954 by the Union Dimes Savings Bank (F3) CLP45 should consist of cardboard (E57)</rdfs:comment>
   </owl:ObjectProperty>
   <!--http://erlangen-crm.org/efrbroo/CLP46_should_be_composed_of-->
   <owl:ObjectProperty rdf:about="http://erlangen-crm.org/efrbroo/CLP46_should_be_composed_of">
      <rdfs:label xml:lang="en">CLP46 should be composed of</rdfs:label>
      <owl:inverseOf rdf:resource="http://erlangen-crm.org/efrbroo/CLP46i_may_form_part_of"/>
      <rdfs:domain rdf:resource="http://erlangen-crm.org/efrbroo/F3_Manifestation_Product_Type"/>
      <rdfs:range rdf:resource="http://erlangen-crm.org/efrbroo/F3_Manifestation_Product_Type"/>
      <rdfs:comment>Quantification:
(0,n:0,n)</rdfs:comment>
      <rdfs:comment>Scope note:
This property associates an instance of F3 Manifestation Product Type which prescribes that all its Items will contain as parts an Item of another instance of F3 Manifestation Product Type with that instance of F3 Manifestation Product Type.</rdfs:comment>
      <rdfs:comment>Examples:
The publication product identified by ISBN ‘0618260587’ and consisting of a 3-volume edition of J.R.R. Tolkien’s ‘The Lord of the rings’ (F3) CLP46 should be composed of the publication product identified by ISBN ‘0618260595’ and consisting of an edition of J.R.R Tolkien’s ‘The two towers’ (F3)The publication product issued by Deutsche Grammophon in 1998 and consisting of a recording of Richard Wagner’s ‘Der fliegende Holländer’ as performed in 1991 by Plácido Domingo, Cheryl Studer et al., and conducted by Giuseppe Sinopoli (F3) CLP46 should be composed of the publication product consisting of printed programme notes and libretto with French and English translations (F3)</rdfs:comment>
   </owl:ObjectProperty>
   <!--http://erlangen-crm.org/efrbroo/CLP57_should_have_number_of_parts-->
   <owl:ObjectProperty rdf:about="http://erlangen-crm.org/efrbroo/CLP57_should_have_number_of_parts">
      <rdfs:label xml:lang="en">CLP57 should have number of parts</rdfs:label>
      <rdfs:domain rdf:resource="http://erlangen-crm.org/efrbroo/F3_Manifestation_Product_Type"/>
      <rdfs:range rdf:resource="http://erlangen-crm.org/current/E60_Number"/>
      <rdfs:comment>Quantification:
(1,1:0,n)</rdfs:comment>
      <rdfs:comment>Scope note:
This property associates a publication, i.e. an instance of F3 Manifestation Product Type, with an instance of E60 Number, which denotes the number of physical units all exemplars of that publication should consist of, as long as they are recognised as complete exemplars of that publication. Typically, this property is observed on one exemplar of a publication, and extrapolated to all other exemplars of the same publication. This logical inference is an induction along the path that can be modelled as: F3 Manifestation Product Type R7i has example F5 Item P57 has number of parts E60 Number.It can happen that a given exemplar, or subset of exemplars, originally produced, or intended to be produced, with that characteristic, accidentally lacks it. This fact should be recorded as a property of F5 Item, and not of F3 Manifestation Product Type.</rdfs:comment>
      <rdfs:comment>Examples:
The jigsaw puzzle entitled ‘Map of the New York city subway system’, designed by Stephen J. Voorhies and released around 1954 by the Union Dimes Savings Bank (F3) CLP57 should have number of parts 76 (E60) [Number of physical units of the exemplar held by the Library of Congress, as observed by a cataloguer from the Library of Congress when he/she catalogued that particular exemplar and recorded the statement: ‘1 jigsaw puzzle (ca. 76 pieces)’]The publication entitled ‘History of costume: in slides, notes, and commentaries’ by Jeanne Button, Patricia Quinn Stuart, and Stephen Sbarge, released by Slide Presentations (New York) ca. 1975 (F3) CLP57 should have number of parts 1,491 (E60) [Number of physical units of the exemplar held by the Gelman Library of the George Washington University, as observed by a cataloguer from the Gelman Library of the George Washington University when he/she catalogued that particular exemplar and recorded the statement: ‘1,491 slides in 14 slide trays + 6 ring binders in cases (30 x 29 cm.)’]</rdfs:comment>
   </owl:ObjectProperty>
   <!--http://erlangen-crm.org/efrbroo/CLP104_subject_to-->
   <owl:ObjectProperty rdf:about="http://erlangen-crm.org/efrbroo/CLP104_subject_to">
      <rdfs:label xml:lang="en">CLP104 subject to</rdfs:label>
      <owl:inverseOf rdf:resource="http://erlangen-crm.org/efrbroo/CLP104i_applies_to"/>
      <rdfs:domain rdf:resource="http://erlangen-crm.org/efrbroo/F3_Manifestation_Product_Type"/>
      <rdfs:range rdf:resource="http://erlangen-crm.org/current/E30_Right"/>
      <rdfs:comment>Quantification:
(0,n:1,1)</rdfs:comment>
      <rdfs:comment>Scope note:
This property associates a publication, i.e. an instance of F3 Manifestation Product Type, with an instance of E30 Right, which applies to all exemplars of that publication, as long as they are recognised as exemplars of that publication.The rights covered by this property may include: acquisition or access authorisation; terms of availability; access restrictions on the Manifestation Product Type; etc.</rdfs:comment>
      <rdfs:comment>Examples:
The publication entitled ‘Recent poems’ by the author named ‘Stephen Spender’, released by the publisher named ‘Anvil Press Poetry’ in 1978 and identified by ISBN ‘0856460516’ (F3) CLP104 subject to availability restricted to Anvil Press Poetry subscribers (E30) [P3 has note ‘This edition […] is available only to Anvil Press Poetry subscribers’ (E62)]</rdfs:comment>
   </owl:ObjectProperty>
   <!--http://erlangen-crm.org/efrbroo/CLP105_right_held_by-->
   <owl:ObjectProperty rdf:about="http://erlangen-crm.org/efrbroo/CLP105_right_held_by">
      <rdfs:label xml:lang="en">CLP105 right held by</rdfs:label>
      <owl:inverseOf rdf:resource="http://erlangen-crm.org/efrbroo/CLP105i_right_on"/>
      <rdfs:domain rdf:resource="http://erlangen-crm.org/efrbroo/F3_Manifestation_Product_Type"/>
      <rdfs:range rdf:resource="http://erlangen-crm.org/current/E39_Actor"/>
      <rdfs:comment>Quantification:
(0,n:0,n)</rdfs:comment>
      <rdfs:comment>Scope note:
This property associates a publication, i.e. an instance of F3 Manifestation Product Type, with an instance of E39 Actor, who holds an instance of E30 Right on all exemplars of that publication, as long as they are recognised as exemplars of that publication.</rdfs:comment>
      <rdfs:comment>Examples:
The publication entitled ‘Recent poems’ by the author named ‘Stephen Spender’, released by the publisher named ‘Anvil Press Poetry’ in 1978 and identified by ISBN ‘0856460516’ (F3) CLP105 right held by Anvil Press Poetry (F11)</rdfs:comment>
   </owl:ObjectProperty>
   <!--http://erlangen-crm.org/efrbroo/CLR6_should_carry-->
   <owl:ObjectProperty rdf:about="http://erlangen-crm.org/efrbroo/CLR6_should_carry">
      <rdfs:label xml:lang="en">CLR6 should carry</rdfs:label>
      <owl:inverseOf rdf:resource="http://erlangen-crm.org/efrbroo/CLR6i_should_be_carried_by"/>
      <rdfs:domain rdf:resource="http://erlangen-crm.org/efrbroo/F3_Manifestation_Product_Type"/>
      <rdfs:range rdf:resource="http://erlangen-crm.org/efrbroo/F24_Publication_Expression"/>
      <rdfs:comment>Quantification:
(1,1:0,n)</rdfs:comment>
      <rdfs:comment>Scope note:
This property associates a publication, i.e. an instance of F3 Manifestation Product Type, with an instance of F24 Publication Expression, which all exemplars of that publication should carry, as long as they are recognised as complete exemplars of that publication. Typically, this property is observed on one exemplar of a publication, and extrapolated to all other exemplars of the same publication. This logical inference is an induction along the path that can be modelled as: F3 Manifestation Product Type R7i has example F5 Item R6 carries F24 Publication Expression.It can happen that a given exemplar, or a subset of exemplars, originally produced, or intended to be produced with that characteristic, accidentally lacks part of the publication expression. This fact should be recorded as a property of F5 Item, and not of F3 Manifestation Product Type.</rdfs:comment>
      <rdfs:comment>Examples:
The publication, dated 1972, entitled ‘The complete poems of Stephen Crane, edited with an introduction by Joseph Katz’ (ISBN ‘0-8014-9130-4’) (F3) CLR6 should carry the overall content of the book identified by ISBN ‘0-8014-9130-4’, i.e.: the text of Stephen Crane’s complete poems as edited by Joseph Katz, the numbering system introduced by Joseph Katz in order to identify each individual poem by Stephen Crane, page numbers, the text of Joseph Katz’s dedication, preface, acknowledgements, and introduction, the table of contents, the index of first lines, the statements found on title page, back of title page (including CIP bibliographic record), cover front, back front, and spine, and the layout of the publication, and the occasional statement ‘[NO STANZA BREAK]’ (F24)</rdfs:comment>
   </owl:ObjectProperty>
   <!--http://erlangen-crm.org/current/P1_is_identified_by-->
   <owl:ObjectProperty rdf:about="http://erlangen-crm.org/current/P1_is_identified_by">
      <rdfs:label xml:lang="en">P1 is identified by</rdfs:label>
      <owl:inverseOf rdf:resource="http://erlangen-crm.org/current/P1i_identifies"/>
      <rdfs:domain rdf:resource="http://erlangen-crm.org/current/E1_CRM_Entity"/>
      <rdfs:range rdf:resource="http://erlangen-crm.org/current/E41_Appellation"/>
      <rdfs:superPropertyOf rdf:resource="http://erlangen-crm.org/current/P48_has_preferred_identifier"/>
      <rdfs:superPropertyOf rdf:resource="http://erlangen-crm.org/current/P78_is_identified_by"/>
      <rdfs:superPropertyOf rdf:resource="http://erlangen-crm.org/current/P87_is_identified_by"/>
      <rdfs:superPropertyOf rdf:resource="http://erlangen-crm.org/current/P102_has_title"/>
      <rdfs:superPropertyOf rdf:resource="http://erlangen-crm.org/current/P131_is_identified_by"/>
      <rdfs:superPropertyOf rdf:resource="http://erlangen-crm.org/current/P149_is_identified_by"/>
      <rdfs:comment>Quantification:
many to many (0,n:0,n)</rdfs:comment>
      <rdfs:comment>Scope note:
This property describes the naming or identification of any real world item by a name or any other identifier.This property is intended for identifiers in general use, which form part of the world the model intends to describe, and not merely for internal database identifiers which are specific to a technical system, unless these latter also have a more general use outside the technical context. This property includes in particular identification by mathematical expressions such as coordinate systems used for the identification of instances of E53 Place. The property does not reveal anything about when, where and by whom this identifier was used. A more detailed representation can be made using the fully developed (i.e. indirect) path through E15 Identifier Assignment.</rdfs:comment>
      <rdfs:comment>Examples:
the capital of Italy (E53) is identified by “Rome” (E48) text 25014–32 (E33) is identified by “The Decline and Fall of the Roman Empire” (E35)</rdfs:comment>
   </owl:ObjectProperty>
   <!--http://erlangen-crm.org/current/P2_has_type-->
   <owl:ObjectProperty rdf:about="http://erlangen-crm.org/current/P2_has_type">
      <rdfs:label xml:lang="en">P2 has type</rdfs:label>
      <owl:inverseOf rdf:resource="http://erlangen-crm.org/current/P2i_is_type_of"/>
      <rdfs:domain rdf:resource="http://erlangen-crm.org/current/E1_CRM_Entity"/>
      <rdfs:range rdf:resource="http://erlangen-crm.org/current/E55_Type"/>
      <rdfs:superPropertyOf rdf:resource="http://erlangen-crm.org/current/P137_exemplifies"/>
      <rdfs:comment>Quantification:
many to many (0,n:0,n)</rdfs:comment>
      <rdfs:comment>Scope note:
This property allows sub typing of CRM entities - a form of specialisation – through the use of a terminological hierarchy, or thesaurus.The CRM is intended to focus on the high-level entities and relationships needed to describe data structures. Consequently, it does not specialise entities any further than is required for this immediate purpose. However, entities in the isA hierarchy of the CRM may by specialised into any number of sub entities, which can be defined in the E55 Type hierarchy. E51 Contact Point, for example, may be specialised into “e-mail address”, “telephone number”, “post office box”, “URL” etc. none of which figures explicitly in the CRM hierarchy. Sub typing obviously requires consistency between the meaning of the terms assigned and the more general intent of the CRM entity in question.</rdfs:comment>
      <rdfs:comment>Examples:
“enquiries@cidoc-crm.org” (E51) has type e-mail address (E55)</rdfs:comment>
   </owl:ObjectProperty>
   <!--http://erlangen-crm.org/current/P3_has_note-->
   <owl:ObjectProperty rdf:about="http://erlangen-crm.org/current/P3_has_note">
      <rdfs:label xml:lang="en">P3 has note</rdfs:label>
      <rdfs:domain rdf:resource="http://erlangen-crm.org/current/E1_CRM_Entity"/>
      <rdfs:range rdf:resource="http://erlangen-crm.org/current/E62_String"/>
      <rdfs:superPropertyOf rdf:resource="http://erlangen-crm.org/current/P79_beginning_is_qualified_by"/>
      <rdfs:superPropertyOf rdf:resource="http://erlangen-crm.org/current/P80_end_is_qualified_by"/>
      <rdfs:comment>Quantification:
one to many (0,n:0,1)</rdfs:comment>
      <rdfs:comment>Scope note:
This property is a container for all informal descriptions about an object that have not been expressed in terms of CRM constructs.In particular it captures the characterisation of the item itself, its internal structures, appearance etc.Like property P2 has type (is type of), this property is a consequence of the restricted focus of the CRM. The aim is not to capture, in a structured form, everything that can be said about an item; indeed, the CRM formalism is not regarded as sufficient to express everything that can be said. Good practice requires use of distinct note fields for different aspects of a characterisation. The P3.1 has type property of P3 has note allows differentiation of specific notes, e.g. “construction”, “decoration” etc.An item may have many notes, but a note is attached to a specific item.</rdfs:comment>
      <rdfs:comment>Examples:
coffee mug – OXCMS:1983.1.1 (E19) has note chipped at edge of handle (E62) has type Condition (E55)Properties:P3.1 has type: E55 Type</rdfs:comment>
   </owl:ObjectProperty>
   <!--http://erlangen-crm.org/current/P4_has_time-span-->
   <owl:ObjectProperty rdf:about="http://erlangen-crm.org/current/P4_has_time-span">
      <rdfs:label xml:lang="en">P4 has time-span</rdfs:label>
      <owl:inverseOf rdf:resource="http://erlangen-crm.org/current/P4i_is_time-span_of"/>
      <rdfs:domain rdf:resource="http://erlangen-crm.org/current/E2_Temporal_Entity"/>
      <rdfs:range rdf:resource="http://erlangen-crm.org/current/E52_Time-Span"/>
      <rdfs:comment>Quantification:
many to one, necessary, dependent (1,1:1,n)</rdfs:comment>
      <rdfs:comment>Scope note:
This property describes the temporal confinement of an instance of an E2 Temporal Entity.The related E52 Time-Span is understood as the real Time-Span during which the phenomena were active, which make up the temporal entity instance. It does not convey any other meaning than a positioning on the “time-line” of chronology. The Time-Span in turn is approximated by a set of dates (E61 Time Primitive). A temporal entity can have in reality only one Time-Span, but there may exist alternative opinions about it, which we would express by assigning multiple Time-Spans. Related temporal entities may share a Time-Span. Time-Spans may have completely unknown dates but other descriptions by which we can infer knowledge.</rdfs:comment>
      <rdfs:comment>Examples:
the Yalta Conference (E7) has time-span Yalta Conference time-span (E52)</rdfs:comment>
   </owl:ObjectProperty>
   <!--http://erlangen-crm.org/current/P7_took_place_at-->
   <owl:ObjectProperty rdf:about="http://erlangen-crm.org/current/P7_took_place_at">
      <rdfs:label xml:lang="en">P7 took place at</rdfs:label>
      <owl:inverseOf rdf:resource="http://erlangen-crm.org/current/P7i_witnessed"/>
      <rdfs:domain rdf:resource="http://erlangen-crm.org/current/E4_Period"/>
      <rdfs:range rdf:resource="http://erlangen-crm.org/current/E53_Place"/>
      <rdfs:superPropertyOf rdf:resource="http://erlangen-crm.org/current/P26_moved_to"/>
      <rdfs:superPropertyOf rdf:resource="http://erlangen-crm.org/current/P27_moved_from"/>
      <rdfs:comment>Quantification:
many to many, necessary (1,n:0,n)</rdfs:comment>
      <rdfs:comment>Scope note:
This property describes the spatial location of an instance of E4 Period.The related E53 Place should be seen as an approximation of the geographical area within which the phenomena that characterise the period in question occurred. P7 took place at (witnessed) does not convey any meaning other than spatial positioning (generally on the surface of the Earth). For example, the period “Révolution française” can be said to have taken place in “France”, the “Victorian” period, may be said to have taken place in “Britain” and its colonies, as well as other parts of Europe and north America.A period can take place at multiple locations.</rdfs:comment>
      <rdfs:comment>Examples:
the period “Révolution française” (E4) took place at France (E53)</rdfs:comment>
   </owl:ObjectProperty>
   <!--http://erlangen-crm.org/current/P9_consists_of-->
   <owl:ObjectProperty rdf:about="http://erlangen-crm.org/current/P9_consists_of">
      <rdfs:label xml:lang="en">P9 consists of</rdfs:label>
      <owl:inverseOf rdf:resource="http://erlangen-crm.org/current/P9i_forms_part_of"/>
      <rdfs:domain rdf:resource="http://erlangen-crm.org/current/E4_Period"/>
      <rdfs:range rdf:resource="http://erlangen-crm.org/current/E4_Period"/>
      <rdfs:comment>Quantification:
one to many, (0,n:0,1)</rdfs:comment>
      <rdfs:comment>Scope note:
This property describes the decomposition of an instance of E4 Period into discrete, subsidiary periods.The sub-periods into which the period is decomposed form a logical whole - although the entire picture may not be completely known - and the sub-periods are constitutive of the general period.</rdfs:comment>
      <rdfs:comment>Examples:
Cretan Bronze Age (E4) consists of Middle Minoan (E4)</rdfs:comment>
   </owl:ObjectProperty>
   <!--http://erlangen-crm.org/current/P12_occurred_in_the_presence_of-->
   <owl:ObjectProperty rdf:about="http://erlangen-crm.org/current/P12_occurred_in_the_presence_of">
      <rdfs:label xml:lang="en">P12 occurred in the presence of</rdfs:label>
      <owl:inverseOf rdf:resource="http://erlangen-crm.org/current/P12i_was_present_at"/>
      <rdfs:domain rdf:resource="http://erlangen-crm.org/current/E5_Event"/>
      <rdfs:range rdf:resource="http://erlangen-crm.org/current/E77_Persistent_Item"/>
      <rdfs:superPropertyOf rdf:resource="http://erlangen-crm.org/current/P11_had_participant"/>
      <rdfs:superPropertyOf rdf:resource="http://erlangen-crm.org/current/P16_used_specific_object"/>
      <rdfs:superPropertyOf rdf:resource="http://erlangen-crm.org/current/P25_moved"/>
      <rdfs:superPropertyOf rdf:resource="http://erlangen-crm.org/current/P31_has_modified"/>
      <rdfs:superPropertyOf rdf:resource="http://erlangen-crm.org/current/P92_brought_into_existence"/>
      <rdfs:superPropertyOf rdf:resource="http://erlangen-crm.org/current/P93_took_out_of_existence"/>
      <rdfs:comment>Quantification:
many to many, necessary (1,n:0,n)</rdfs:comment>
      <rdfs:comment>Scope note:
This property describes the active or passive presence of an E77 Persistent Item in an E5 Event without implying any specific role.It connects the history of a thing with the E53 Place and E50 Date of an event. For example, an object may be the desk, now in a museum on which a treaty was signed. The presence of an immaterial thing implies the presence of at least one of its carriers.</rdfs:comment>
      <rdfs:comment>Examples:
Deckchair 42 (E19) was present at The sinking of the Titanic (E5)</rdfs:comment>
   </owl:ObjectProperty>
   <!--http://erlangen-crm.org/current/P14_carried_out_by-->
   <owl:ObjectProperty rdf:about="http://erlangen-crm.org/current/P14_carried_out_by">
      <rdfs:label xml:lang="en">P14 carried out by</rdfs:label>
      <owl:inverseOf rdf:resource="http://erlangen-crm.org/current/P14i_performed"/>
      <rdfs:domain rdf:resource="http://erlangen-crm.org/current/E7_Activity"/>
      <rdfs:range rdf:resource="http://erlangen-crm.org/current/E39_Actor"/>
      <rdfs:subPropertyOf rdf:resource="http://erlangen-crm.org/current/P11_had_participant"/>
      <rdfs:superPropertyOf rdf:resource="http://erlangen-crm.org/current/P22_transferred_title_to"/>
      <rdfs:superPropertyOf rdf:resource="http://erlangen-crm.org/current/P23_transferred_title_from"/>
      <rdfs:superPropertyOf rdf:resource="http://erlangen-crm.org/current/P28_custody_surrendered_by"/>
      <rdfs:superPropertyOf rdf:resource="http://erlangen-crm.org/current/P29_custody_received_by"/>
      <rdfs:comment>Quantification:
many to many, necessary (1,n:0,n)</rdfs:comment>
      <rdfs:comment>Scope note:
This property describes the active participation of an E39 Actor in an E7 Activity.It implies causal or legal responsibility. The P14.1 in the role of property of the property allows the nature of an Actor’s participation to be specified.</rdfs:comment>
      <rdfs:comment>Examples:
the painting of the Sistine Chapel (E7) carried out by Michaelangelo Buonaroti (E21) in the role of master craftsman (E55)Properties:P14.1 in the role of: E55 Type</rdfs:comment>
   </owl:ObjectProperty>
   <!--http://erlangen-crm.org/current/P15_was_influenced_by-->
   <owl:ObjectProperty rdf:about="http://erlangen-crm.org/current/P15_was_influenced_by">
      <rdfs:label xml:lang="en">P15 was influenced by</rdfs:label>
      <owl:inverseOf rdf:resource="http://erlangen-crm.org/current/P15i_influenced"/>
      <rdfs:domain rdf:resource="http://erlangen-crm.org/current/E7_Activity"/>
      <rdfs:range rdf:resource="http://erlangen-crm.org/current/E1_CRM_Entity"/>
      <rdfs:superPropertyOf rdf:resource="http://erlangen-crm.org/current/P16_used_specific_object"/>
      <rdfs:superPropertyOf rdf:resource="http://erlangen-crm.org/current/P17_was_motivated_by"/>
      <rdfs:superPropertyOf rdf:resource="http://erlangen-crm.org/current/P134_continued"/>
      <rdfs:superPropertyOf rdf:resource="http://erlangen-crm.org/current/P136_was_based_on"/>
      <rdfs:comment>Quantification:
many to many (0,n:0,n)</rdfs:comment>
      <rdfs:comment>Scope note:
This is a high level property, which captures the relationship between an E7 Activity and anything that may have had some bearing upon it.The property has more specific sub properties.</rdfs:comment>
      <rdfs:comment>Examples:
the designing of the Sydney Harbour Bridge (E7) was influenced by the Tyne bridge (E22)</rdfs:comment>
   </owl:ObjectProperty>
   <!--http://erlangen-crm.org/current/P16_used_specific_object-->
   <owl:ObjectProperty rdf:about="http://erlangen-crm.org/current/P16_used_specific_object">
      <rdfs:label xml:lang="en">P16 used specific object</rdfs:label>
      <owl:inverseOf rdf:resource="http://erlangen-crm.org/current/P16i_was_used_for"/>
      <rdfs:domain rdf:resource="http://erlangen-crm.org/current/E7_Activity"/>
      <rdfs:range rdf:resource="http://erlangen-crm.org/current/E70_Thing"/>
      <rdfs:subPropertyOf rdf:resource="http://erlangen-crm.org/current/P12_occurred_in_the_presence_of"/>
      <rdfs:subPropertyOf rdf:resource="http://erlangen-crm.org/current/P15_was_influenced_by"/>
      <rdfs:superPropertyOf rdf:resource="http://erlangen-crm.org/current/P33_used_specific_technique"/>
      <rdfs:superPropertyOf rdf:resource="http://erlangen-crm.org/current/P142_used_constituent"/>
      <rdfs:comment>Quantification:
many to many (0,n:0,n)</rdfs:comment>
      <rdfs:comment>Scope note:
This property describes the use of material or immaterial things in a way essential to the performance or the outcome of an E7 Activity.This property typically applies to tools, instruments, moulds, raw materials and items embedded in a product. It implies that the presence of the object in question was a necessary condition for the action. For example, the activity of writing this text required the use of a computer. An immaterial thing can be used if at least one of its carriers is present. For example, the software tools on a computer.Another example is the use of a particular name by a particular group of people over some span to identify a thing, such as a settlement. In this case, the physical carriers of this name are at least the people understanding its use.</rdfs:comment>
      <rdfs:comment>Examples:
the writing of this scope note (E7) used specific object Nicholas Crofts’ computer (E22) mode of use Typing Tool; Storage Medium (E55) the people of Iraq calling the place identified by TGN ‘7017998’ (E7) used specific object “Quyunjig” (E44) mode of use Current; Vernacular (E55)Properties:P16.1 mode of use: E55 Type</rdfs:comment>
   </owl:ObjectProperty>
   <!--http://erlangen-crm.org/current/P31_has_modified-->
   <owl:ObjectProperty rdf:about="http://erlangen-crm.org/current/P31_has_modified">
      <rdfs:label xml:lang="en">P31 has modified</rdfs:label>
      <owl:inverseOf rdf:resource="http://erlangen-crm.org/current/P31i_was_modified_by"/>
      <rdfs:domain rdf:resource="http://erlangen-crm.org/current/E11_Modification"/>
      <rdfs:range rdf:resource="http://erlangen-crm.org/current/E24_Physical_Man-Made_Thing"/>
      <rdfs:subPropertyOf rdf:resource="http://erlangen-crm.org/current/P12_occurred_in_the_presence_of"/>
      <rdfs:superPropertyOf rdf:resource="http://erlangen-crm.org/current/P108_has_produced"/>
      <rdfs:superPropertyOf rdf:resource="http://erlangen-crm.org/current/P110_augmented"/>
      <rdfs:superPropertyOf rdf:resource="http://erlangen-crm.org/current/P112_diminished"/>
      <rdfs:comment>Quantification:
many to many, necessary (1,n:0,n)</rdfs:comment>
      <rdfs:comment>Scope note:
This property identifies the E24 Physical Man-Made Thing modified in an E11 Modification.If a modification is applied to a non-man-made object, it is regarded as an E22 Man-Made Object from that time onwards.</rdfs:comment>
      <rdfs:comment>Examples:
rebuilding of the Reichstag (E11) has modified the Reichstag in Berlin (E24)</rdfs:comment>
   </owl:ObjectProperty>
   <!--http://erlangen-crm.org/current/P33_used_specific_technique-->
   <owl:ObjectProperty rdf:about="http://erlangen-crm.org/current/P33_used_specific_technique">
      <rdfs:label xml:lang="en">P33 used specific technique</rdfs:label>
      <owl:inverseOf rdf:resource="http://erlangen-crm.org/current/P33i_was_used_by"/>
      <rdfs:domain rdf:resource="http://erlangen-crm.org/current/E7_Activity"/>
      <rdfs:range rdf:resource="http://erlangen-crm.org/current/E29_Design_or_Procedure"/>
      <rdfs:subPropertyOf rdf:resource="http://erlangen-crm.org/current/P16_used_specific_object"/>
      <rdfs:comment>Quantification:
many to many (0,n:0,n)</rdfs:comment>
      <rdfs:comment>Scope note:
This property identifies a specific E29 Design or Procedure in order to carry out an instance of E7 Activity or parts of it.The property differs from P32 used general technique (was technique of) in that the E29 Design or Procedure referred to is specific and documented rather than simply being a term in the E55 Type hierarchy. Typical examples would include intervention plans for conservation.Typical examples would include intervention plans for conservation or the construction plans of a building.</rdfs:comment>
      <rdfs:comment>Examples:
Ornamentation of silver cup 232 (E11) used specific technique ‘Instructions for golden chase work by A N Other’ (E29) Rebuilding of Reichstag (E11) used specific technique Architectural plans by Foster and Partners (E29)</rdfs:comment>
   </owl:ObjectProperty>
   <!--http://erlangen-crm.org/current/P37_assigned-->
   <owl:ObjectProperty rdf:about="http://erlangen-crm.org/current/P37_assigned">
      <rdfs:label xml:lang="en">P37 assigned</rdfs:label>
      <owl:inverseOf rdf:resource="http://erlangen-crm.org/current/P37i_was_assigned_by"/>
      <rdfs:domain rdf:resource="http://erlangen-crm.org/current/E15_Identifier_Assignment"/>
      <rdfs:range rdf:resource="http://erlangen-crm.org/current/E42_Identifier"/>
      <rdfs:subPropertyOf rdf:resource="http://erlangen-crm.org/current/P141_assigned"/>
      <rdfs:comment>Quantification:
many to many (0,n:0,n)</rdfs:comment>
      <rdfs:comment>Scope note:
This property records the identifier that was assigned to an item in an Identifier Assignment activity.The same identifier may be assigned on more than one occasion.An Identifier might be created prior to an assignment.</rdfs:comment>
      <rdfs:comment>Examples:
01 June 1997 Identifier Assignment of the silver cup donated by Martin Doerr (E15) assigned “232” (E42)</rdfs:comment>
   </owl:ObjectProperty>
   <!--http://erlangen-crm.org/current/P43_has_dimension-->
   <owl:ObjectProperty rdf:about="http://erlangen-crm.org/current/P43_has_dimension">
      <rdfs:label xml:lang="en">P43 has dimension</rdfs:label>
      <owl:inverseOf rdf:resource="http://erlangen-crm.org/current/P43i_is_dimension_of"/>
      <rdfs:domain rdf:resource="http://erlangen-crm.org/current/E70_Thing"/>
      <rdfs:range rdf:resource="http://erlangen-crm.org/current/E54_Dimension"/>
      <rdfs:comment>Quantification:
one to many, dependent (0,n:1.1)</rdfs:comment>
      <rdfs:comment>Scope note:
This property records a E54 Dimension of some E70 Thing.It is a shortcut of the more fully developed path from E70 Thing through P39 measured (was measured by), E16 Measurement P40 observed dimension (was observed in) to E54 Dimension. It offers no information about how and when an E54 Dimension was established, nor by whom.An instance of E54 Dimension is specific to an instance of E70 Thing.</rdfs:comment>
      <rdfs:comment>Examples:
silver cup 232 (E22) has dimension height of silver cup 232 (E54) has unit mm (E58), has value 224 (E60)</rdfs:comment>
   </owl:ObjectProperty>
   <!--http://erlangen-crm.org/current/P44_has_condition-->
   <owl:ObjectProperty rdf:about="http://erlangen-crm.org/current/P44_has_condition">
      <rdfs:label xml:lang="en">P44 has condition</rdfs:label>
      <owl:inverseOf rdf:resource="http://erlangen-crm.org/current/P44i_is_condition_of"/>
      <rdfs:domain rdf:resource="http://erlangen-crm.org/current/E18_Physical_Thing"/>
      <rdfs:range rdf:resource="http://erlangen-crm.org/current/E3_Condition_State"/>
      <rdfs:comment>Quantification:
one to many, dependent (0, n: 1,1)</rdfs:comment>
      <rdfs:comment>Scope note:
This property records an E3 Condition State for some E18 Physical Thing.It is a shortcut of the more fully developed path from E18 Physical Thing through P34 concerned (was assessed by), E14 Condition Assessment P35 has identified (identified by) to E3 Condition State. It offers no information about how and when the E3 Condition State was established, nor by whom.An instance of Condition State is specific to an instance of Physical Thing.</rdfs:comment>
      <rdfs:comment>Examples:
silver cup 232 (E22) has condition oxidation traces were present in 1997 (E3) has type oxidation traces (E55)</rdfs:comment>
   </owl:ObjectProperty>
   <!--http://erlangen-crm.org/current/P45_consists_of-->
   <owl:ObjectProperty rdf:about="http://erlangen-crm.org/current/P45_consists_of">
      <rdfs:label xml:lang="en">P45 consists of</rdfs:label>
      <owl:inverseOf rdf:resource="http://erlangen-crm.org/current/P45i_is_incorporated_in"/>
      <rdfs:domain rdf:resource="http://erlangen-crm.org/current/E18_Physical_Thing"/>
      <rdfs:range rdf:resource="http://erlangen-crm.org/current/E57_Material"/>
      <rdfs:comment>Quantification:
many to many, necessary (1,n:0,n)</rdfs:comment>
      <rdfs:comment>Scope note:
This property identifies the instances of E57 Materials of which an instance of E18 Physical Thing is composed.All physical things consist of physical materials. P45 consists of (is incorporated in) allows the different Materials to be recorded. P45 consists of (is incorporated in) refers here to observed Material as opposed to the consumed raw material.A Material, such as a theoretical alloy, may not have any physical instances.</rdfs:comment>
      <rdfs:comment>Examples:
silver cup 232 (E22) consists of silver (E57)</rdfs:comment>
   </owl:ObjectProperty>
   <!--http://erlangen-crm.org/current/P46_is_composed_of-->
   <owl:ObjectProperty rdf:about="http://erlangen-crm.org/current/P46_is_composed_of">
      <rdfs:label xml:lang="en">P46 is composed of</rdfs:label>
      <owl:inverseOf rdf:resource="http://erlangen-crm.org/current/P46i_forms_part_of"/>
      <rdfs:domain rdf:resource="http://erlangen-crm.org/current/E18_Physical_Thing"/>
      <rdfs:range rdf:resource="http://erlangen-crm.org/current/E18_Physical_Thing"/>
      <rdfs:superPropertyOf rdf:resource="http://erlangen-crm.org/current/P56_bears_feature"/>
      <rdfs:comment>Quantification:
many to many (0,n:0,n)</rdfs:comment>
      <rdfs:comment>Scope note:
This property allows instances of E18 Physical Thing to be analysed into component elements.Component elements, since they are themselves instances of E18 Physical Thing, may be further analysed into sub-components, thereby creating a hierarchy of part decomposition. An instance of E18 Physical Thing may be shared between multiple wholes, for example two buildings may share a common wall.This property is intended to describe specific components that are individually documented, rather than general aspects. Overall descriptions of the structure of an instance of E18 Physical Thing are captured by the P3 has note property.The instances of E57 Materials of which an item of E18 Physical Thing is composed should be documented using P45 consists of (is incorporated in).</rdfs:comment>
      <rdfs:comment>Examples:
the Royal carriage (E22) forms part of the Royal train (E22) the “Hog’s Back” (E24) forms part of the “Fosseway” (E24</rdfs:comment>
   </owl:ObjectProperty>
   <!--http://erlangen-crm.org/current/P49_has_former_or_current_keeper-->
   <owl:ObjectProperty rdf:about="http://erlangen-crm.org/current/P49_has_former_or_current_keeper">
      <rdfs:label xml:lang="en">P49 has former or current keeper</rdfs:label>
      <owl:inverseOf rdf:resource="http://erlangen-crm.org/current/P49i_is_former_or_current_keeper_of"/>
      <rdfs:domain rdf:resource="http://erlangen-crm.org/current/E18_Physical_Thing"/>
      <rdfs:range rdf:resource="http://erlangen-crm.org/current/E39_Actor"/>
      <rdfs:superPropertyOf rdf:resource="http://erlangen-crm.org/current/P50_has_current_keeper"/>
      <rdfs:comment>Quantification:
many to many (0,n:0,n)</rdfs:comment>
      <rdfs:comment>Scope note:
This property identifies the E39 Actor or Actors who have or have had custody of an instance of E18 Physical Thing at some time.The distinction with P50 has current keeper (is current keeper of) is that P49 has former or current keeper (is former or current keeper of) leaves open the question as to whether the specified keepers are current.P49 has former or current keeper (is former or current keeper of) is a shortcut for the more detailed path from E18 Physical Thing through P30 transferred custody of (custody transferred through), E10 Transfer of Custody, P28 custody surrendered by (surrendered custody through) or P29 custody received by (received custody through) to E39 Actor.</rdfs:comment>
      <rdfs:comment>Examples:
paintings from The Iveagh Bequest (E18) has former or current keeper Secure Deliveries Inc. (E40)</rdfs:comment>
   </owl:ObjectProperty>
   <!--http://erlangen-crm.org/current/P50_has_current_keeper-->
   <owl:ObjectProperty rdf:about="http://erlangen-crm.org/current/P50_has_current_keeper">
      <rdfs:label xml:lang="en">P50 has current keeper</rdfs:label>
      <owl:inverseOf rdf:resource="http://erlangen-crm.org/current/P50i_is_current_keeper_of"/>
      <rdfs:domain rdf:resource="http://erlangen-crm.org/current/E18_Physical_Thing"/>
      <rdfs:range rdf:resource="http://erlangen-crm.org/current/E39_Actor"/>
      <rdfs:subPropertyOf rdf:resource="http://erlangen-crm.org/current/P49_has_former_or_current_keeper"/>
      <rdfs:comment>Quantification:
many to many (0,n:0,n)</rdfs:comment>
      <rdfs:comment>Scope note:
This property identifies the E39 Actor or Actors who had custody of an instance of E18 Physical Thing at the time this property was recorded.P50 has current keeper (is current keeper of) is a shortcut for the more detailed path from E18 Physical Thing through P30 transferred custody of (custody transferred through), E10 Transfer of Custody, P29 custody received by (received custody through) to E39 Actor.</rdfs:comment>
      <rdfs:comment>Examples:
paintings from The Iveagh Bequest (E18) has current keeper The National Gallery (E40)</rdfs:comment>
   </owl:ObjectProperty>
   <!--http://erlangen-crm.org/current/P51_has_former_or_current_owner-->
   <owl:ObjectProperty rdf:about="http://erlangen-crm.org/current/P51_has_former_or_current_owner">
      <rdfs:label xml:lang="en">P51 has former or current owner</rdfs:label>
      <owl:inverseOf rdf:resource="http://erlangen-crm.org/current/P51i_is_former_or_current_owner_of"/>
      <rdfs:domain rdf:resource="http://erlangen-crm.org/current/E18_Physical_Thing"/>
      <rdfs:range rdf:resource="http://erlangen-crm.org/current/E39_Actor"/>
      <rdfs:superPropertyOf rdf:resource="http://erlangen-crm.org/current/P52_has_current_owner"/>
      <rdfs:comment>Quantification:
many to many (0,n:0,n)</rdfs:comment>
      <rdfs:comment>Scope note:
This property identifies the E39 Actor that is or has been the legal owner (i.e. title holder) of an instance of E18 Physical Thing at some time.The distinction with P52 has current owner (is current owner of) is that P51 has former or current owner (is former or current owner of) does not indicate whether the specified owners are current. P51 has former or current owner (is former or current owner of) is a shortcut for the more detailed path from E18 Physical Thing through P24 transferred title of (changed ownership through), E8 Acquisition, P23 transferred title from (surrendered title through), or P22 transferred title to (acquired title through) to E39 Actor.</rdfs:comment>
      <rdfs:comment>Examples:
paintings from the Iveagh Bequest (E18) has former or current owner Lord Iveagh (E21)</rdfs:comment>
   </owl:ObjectProperty>
   <!--http://erlangen-crm.org/current/P57_has_number_of_parts-->
   <owl:ObjectProperty rdf:about="http://erlangen-crm.org/current/P57_has_number_of_parts">
      <rdfs:label xml:lang="en">P57 has number of parts</rdfs:label>
      <rdfs:domain rdf:resource="http://erlangen-crm.org/current/E19_Physical_Object"/>
      <rdfs:range rdf:resource="http://erlangen-crm.org/current/E60_Number"/>
      <rdfs:comment>Quantification:
many to one (0,1:0,n)</rdfs:comment>
      <rdfs:comment>Scope note:
This property documents the E60 Number of parts of which an instance of E19 Physical Object is composed.This may be used as a method of checking inventory counts with regard to aggregate or collective objects. What constitutes a part or component depends on the context and requirements of the documentation. Normally, the parts documented in this way would not be considered as worthy of individual attention.For a more complete description, objects may be decomposed into their components and constituents using P46 is composed of (forms parts of) and P45 consists of (is incorporated in). This allows each element to be described individually.</rdfs:comment>
      <rdfs:comment>Examples:
chess set 233 (E22) has number of parts 33 (E60)</rdfs:comment>
   </owl:ObjectProperty>
   <!--http://erlangen-crm.org/current/P59_has_section-->
   <owl:ObjectProperty rdf:about="http://erlangen-crm.org/current/P59_has_section">
      <rdfs:label xml:lang="en">P59 has section</rdfs:label>
      <owl:inverseOf rdf:resource="http://erlangen-crm.org/current/P59i_is_located_on_or_within"/>
      <rdfs:domain rdf:resource="http://erlangen-crm.org/current/E18_Physical_Thing"/>
      <rdfs:range rdf:resource="http://erlangen-crm.org/current/E53_Place"/>
      <rdfs:comment>Quantification:
one to many (0,n:0,1)</rdfs:comment>
      <rdfs:comment>Scope note:
This property links an area to the instance of E18 Physical Thing upon which it is found.It is typically used when a named E46 Section Definition is not appropriate.E18 Physical Thing may be subdivided into arbitrary regions.P59 has section (is located on or within) is a shortcut. If the E53 Place is identified by a Section Definition, a more detailed representation can make use of the fully developed (i.e. indirect) path from E18 Physical Thing through P58 has section definition (defines section), E46 Section Definition, P87 is identified by (identifies) to E53 Place. A Place can only be located on or within one Physical Object.</rdfs:comment>
      <rdfs:comment>Examples:
HMS Victory (E22) has section HMS Victory section B347.6 (E53)</rdfs:comment>
   </owl:ObjectProperty>
   <!--http://erlangen-crm.org/current/P65_shows_visual_item-->
   <owl:ObjectProperty rdf:about="http://erlangen-crm.org/current/P65_shows_visual_item">
      <rdfs:label xml:lang="en">P65 shows visual item</rdfs:label>
      <owl:inverseOf rdf:resource="http://erlangen-crm.org/current/P65i_is_shown_by"/>
      <rdfs:domain rdf:resource="http://erlangen-crm.org/current/E24_Physical_Man-Made_Thing"/>
      <rdfs:range rdf:resource="http://erlangen-crm.org/current/E36_Visual_Item"/>
      <rdfs:subPropertyOf rdf:resource="http://erlangen-crm.org/current/P128_carries"/>
      <rdfs:comment>Quantification:
many to many (0,n:0,n)</rdfs:comment>
      <rdfs:comment>Scope note:
This property documents an E36 Visual Item shown by an instance of E24 Physical Man-Made Thing.This property is similar to P62 depicts (is depicted by) in that it associates an item of E24 Physical Man-Made Thing with a visual representation. However, P65 shows visual item (is shown by) differs from the P62 depicts (is depicted by) property in that it makes no claims about what the E36 Visual Item is deemed to represent. E36 Visual Item identifies a recognisable image or visual symbol, regardless of what this image may or may not represent.For example, all recent British coins bear a portrait of Queen Elizabeth II, a fact that is correctly documented using P62 depicts (is depicted by). Different portraits have been used at different periods, however. P65 shows visual item (is shown by) can be used to refer to a particular portrait.P65 shows visual item (is shown by) may also be used for Visual Items such as signs, marks and symbols, for example the 'Maltese Cross' or the 'copyright symbol’ that have no particular representational content.This property is part of the fully developed path from E24 Physical Man-Made Thing through P65 shows visual item (is shown by), E36 Visual Item, P138 represents (has representation) to E1 CRM Entity which is shortcut by, P62 depicts (is depicted by).</rdfs:comment>
      <rdfs:comment>Examples:
My T-Shirt (E22) shows visual item Mona Lisa (E38)</rdfs:comment>
   </owl:ObjectProperty>
   <!--http://erlangen-crm.org/current/P67_refers_to-->
   <owl:ObjectProperty rdf:about="http://erlangen-crm.org/current/P67_refers_to">
      <rdfs:label xml:lang="en">P67 refers to</rdfs:label>
      <owl:inverseOf rdf:resource="http://erlangen-crm.org/current/P67i_is_referred_to_by"/>
      <rdfs:domain rdf:resource="http://erlangen-crm.org/current/E89_Propositional_Object"/>
      <rdfs:range rdf:resource="http://erlangen-crm.org/current/E1_CRM_Entity"/>
      <rdfs:superPropertyOf rdf:resource="http://erlangen-crm.org/current/P70_documents"/>
      <rdfs:superPropertyOf rdf:resource="http://erlangen-crm.org/current/P71_lists"/>
      <rdfs:superPropertyOf rdf:resource="http://erlangen-crm.org/current/P129_is_about"/>
      <rdfs:superPropertyOf rdf:resource="http://erlangen-crm.org/current/P138_represents"/>
      <rdfs:superPropertyOf rdf:resource="http://erlangen-crm.org/current/P68_foresees_use_of"/>
      <rdfs:comment>Quantification:
many to many (0,n:0,n)</rdfs:comment>
      <rdfs:comment>Scope note:
This property documents that an E89 Propositional Object makes a statement about an instance of E1 CRM Entity. P67 refers to (is referred to by) has the P67.1 has type link to an instance of E55 Type. This is intended to allow a more detailed description of the type of reference. This differs from P129 is about (is subject of), which describes the primary subject or subjects of the E89 Propositional Object.</rdfs:comment>
      <rdfs:comment>Examples:
the eBay auction listing of 4 July 2002 (E73) refers to silver cup 232 (E22) has type item for sale (E55)Properties:P67.1 has type: E55 Type</rdfs:comment>
   </owl:ObjectProperty>
   <!--http://erlangen-crm.org/current/P69_has_association_with-->
   <owl:ObjectProperty rdf:about="http://erlangen-crm.org/current/P69_has_association_with">
      <rdfs:label xml:lang="en">P69 has association with</rdfs:label>
      <owl:inverseOf rdf:resource="http://erlangen-crm.org/current/P69i_is_associated_with"/>
      <rdfs:domain rdf:resource="http://erlangen-crm.org/current/E29_Design_or_Procedure"/>
      <rdfs:range rdf:resource="http://erlangen-crm.org/current/E29_Design_or_Procedure"/>
      <rdfs:comment>Quantification:
many to many (0,n:0,n)</rdfs:comment>
      <rdfs:comment>Scope note:
This symmetric property describes the association of an E29 Design or Procedure with other Designs or Procedures.Any instance of E29 Design or Procedure may be associated with other designs or procedures.The P69.1 has type property of P69 is associated with allows the nature of the association to be specified; examples of types of association between instances of E29 Design or Procedure include: whole-part, sequence, prerequisite, etc</rdfs:comment>
      <rdfs:comment>Examples:
procedure for glass blowing (E29) has association with procedure for glass heating (E29)Properties:P69.1 has type: E55 Type</rdfs:comment>
   </owl:ObjectProperty>
   <!--http://erlangen-crm.org/current/P71_lists-->
   <owl:ObjectProperty rdf:about="http://erlangen-crm.org/current/P71_lists">
      <rdfs:label xml:lang="en">P71 lists</rdfs:label>
      <owl:inverseOf rdf:resource="http://erlangen-crm.org/current/P71i_is_listed_in"/>
      <rdfs:domain rdf:resource="http://erlangen-crm.org/current/E32_Authority_Document"/>
      <rdfs:range rdf:resource="http://erlangen-crm.org/current/E1_CRM_Entity"/>
      <rdfs:subPropertyOf rdf:resource="http://erlangen-crm.org/current/P67_refers_to"/>
      <rdfs:comment>Quantification:
many to many (0,n:0,n)</rdfs:comment>
      <rdfs:comment>Scope note:
This property documents a source E32 Authority Document for an instance of an E1 CRM Entity.</rdfs:comment>
      <rdfs:comment>Examples:
the Art &amp; Architecture Thesaurus (E32) lists alcazars (E55)</rdfs:comment>
   </owl:ObjectProperty>
   <!--http://erlangen-crm.org/current/P72_has_language-->
   <owl:ObjectProperty rdf:about="http://erlangen-crm.org/current/P72_has_language">
      <rdfs:label xml:lang="en">P72 has language</rdfs:label>
      <owl:inverseOf rdf:resource="http://erlangen-crm.org/current/P72i_is_language_of"/>
      <rdfs:domain rdf:resource="http://erlangen-crm.org/current/E33_Linguistic_Object"/>
      <rdfs:range rdf:resource="http://erlangen-crm.org/current/E56_Language"/>
      <rdfs:comment>Quantification:
many to many, necessary (0,n:0,n)</rdfs:comment>
      <rdfs:comment>Scope note:
This property describes the E56 Language of an E33 Linguistic Object.Linguistic Objects are composed in one or more human Languages. This property allows these languages to be documented.</rdfs:comment>
      <rdfs:comment>Examples:
the American Declaration of Independence (E33) has language 18th Century English (E56)</rdfs:comment>
   </owl:ObjectProperty>
   <!--http://erlangen-crm.org/current/P74_has_current_or_former_residence-->
   <owl:ObjectProperty rdf:about="http://erlangen-crm.org/current/P74_has_current_or_former_residence">
      <rdfs:label xml:lang="en">P74 has current or former residence</rdfs:label>
      <owl:inverseOf rdf:resource="http://erlangen-crm.org/current/P74i_is_current_or_former_residence_of"/>
      <rdfs:domain rdf:resource="http://erlangen-crm.org/current/E39_Actor"/>
      <rdfs:range rdf:resource="http://erlangen-crm.org/current/E53_Place"/>
      <rdfs:comment>Quantification:
many to many (0,n:0,n)</rdfs:comment>
      <rdfs:comment>Scope note:
This property describes the current or former E53 Place of residence of an E39 Actor.The residence may be either the Place where the Actor resides, or a legally registered address of any kind.</rdfs:comment>
      <rdfs:comment>Examples:
Queen Elizabeth II (E39) has current or former residence Buckingham Palace (E53)</rdfs:comment>
   </owl:ObjectProperty>
   <!--http://erlangen-crm.org/current/P75_possesses-->
   <owl:ObjectProperty rdf:about="http://erlangen-crm.org/current/P75_possesses">
      <rdfs:label xml:lang="en">P75 possesses</rdfs:label>
      <owl:inverseOf rdf:resource="http://erlangen-crm.org/current/P75i_is_possessed_by"/>
      <rdfs:domain rdf:resource="http://erlangen-crm.org/current/E39_Actor"/>
      <rdfs:range rdf:resource="http://erlangen-crm.org/current/E30_Right"/>
      <rdfs:comment>Quantification:
many to many (0,n:0,n)</rdfs:comment>
      <rdfs:comment>Scope note:
This property identifies former or current instances of E30 Rights held by an E39 Actor.</rdfs:comment>
      <rdfs:comment>Examples:
Michael Jackson (E21) possesses Intellectual property rights on the Beatles’ back catalogue (E30)</rdfs:comment>
   </owl:ObjectProperty>
   <!--http://erlangen-crm.org/current/P78_is_identified_by-->
   <owl:ObjectProperty rdf:about="http://erlangen-crm.org/current/P78_is_identified_by">
      <rdfs:label xml:lang="en">P78 is identified by</rdfs:label>
      <owl:inverseOf rdf:resource="http://erlangen-crm.org/current/P78i_identifies"/>
      <rdfs:domain rdf:resource="http://erlangen-crm.org/current/E52_Time-Span"/>
      <rdfs:range rdf:resource="http://erlangen-crm.org/current/E49_Time_Appellation"/>
      <rdfs:subPropertyOf rdf:resource="http://erlangen-crm.org/current/P1_is_identified_by"/>
      <rdfs:comment>Quantification:
many to many (0,n:0,n)</rdfs:comment>
      <rdfs:comment>Scope note:
This property identifies an E52 Time-Span using an E49Time Appellation.</rdfs:comment>
      <rdfs:comment>Examples:
the time span 1926 to 1988 (E52) is identified by “Showa” (Japanese time appellation) (E49)</rdfs:comment>
   </owl:ObjectProperty>
   <!--http://erlangen-crm.org/current/P82_at_some_time_within-->
   <owl:ObjectProperty rdf:about="http://erlangen-crm.org/current/P82_at_some_time_within">
      <rdfs:label xml:lang="en">P82 at some time within</rdfs:label>
      <rdfs:domain rdf:resource="http://erlangen-crm.org/current/E52_Time-Span"/>
      <rdfs:range rdf:resource="http://erlangen-crm.org/current/E61_Time_Primitive"/>
      <rdfs:comment>Quantification:
many to one, necessary (1,1:0,n)</rdfs:comment>
      <rdfs:comment>Scope note:
This property describes the maximum period of time within which an E52 Time-Span falls.Since Time-Spans may not have precisely known temporal extents, the CRM supports statements about the minimum and maximum temporal extents of Time-Spans. This property allows a Time-Span’s maximum temporal extent (i.e. its outer boundary) to be assigned an E61 Time Primitive value. Time Primitives are treated by the CRM as application or system specific date intervals, and are not further analysed.</rdfs:comment>
      <rdfs:comment>Examples:
the time-span of the development of the CIDOC CRM (E52) at some time within 1992-infinity (E61)</rdfs:comment>
   </owl:ObjectProperty>
   <!--http://erlangen-crm.org/current/P87_is_identified_by-->
   <owl:ObjectProperty rdf:about="http://erlangen-crm.org/current/P87_is_identified_by">
      <rdfs:label xml:lang="en">P87 is identified by</rdfs:label>
      <owl:inverseOf rdf:resource="http://erlangen-crm.org/current/P87i_identifies"/>
      <rdfs:domain rdf:resource="http://erlangen-crm.org/current/E53_Place"/>
      <rdfs:range rdf:resource="http://erlangen-crm.org/current/E44_Place_Appellation"/>
      <rdfs:subPropertyOf rdf:resource="http://erlangen-crm.org/current/P1_is_identified_by"/>
      <rdfs:comment>Quantification:
many to many (0,n:0,n)</rdfs:comment>
      <rdfs:comment>Scope note:
This property identifies an E53 Place using an E44 Place Appellation.Examples of Place Appellations used to identify Places include instances of E48 Place Name, addresses, E47 Spatial Coordinates etc.</rdfs:comment>
      <rdfs:comment>Examples:
the location of the Duke of Wellington’s House (E53) is identified by “No 1 London” (E45)</rdfs:comment>
   </owl:ObjectProperty>
      <!--http://erlangen-crm.org/current/P91_has_unit-->
      <owl:ObjectProperty rdf:about="http://erlangen-crm.org/current/P91_has_unit">
         <rdfs:label xml:lang="en">P87 is identified by</rdfs:label>
         <owl:inverseOf rdf:resource="http://erlangen-crm.org/current/P91i_is_unit_of"/>
         <rdfs:domain rdf:resource="http://erlangen-crm.org/current/E54_Dimension"/>
         <rdfs:range rdf:resource="http://erlangen-crm.org/current/E58_Measurement_Unit"/>
         <rdfs:comment>Quantification:
   many to one, necessary (1,1:0,n)</rdfs:comment>
         <rdfs:comment>Scope note:
   </rdfs:comment>
         <rdfs:comment>Examples:
   </rdfs:comment>
      </owl:ObjectProperty>
      <!--http://erlangen-crm.org/current/P93_took_out_of_existence-->
      <owl:ObjectProperty rdf:about="http://erlangen-crm.org/current/P93_took_out_of_existence">
         <rdfs:label xml:lang="en">P93 took out of existence</rdfs:label>
         <owl:inverseOf rdf:resource="http://erlangen-crm.org/current/P93i_was_taken_out_of_existence_by"/>
         <rdfs:domain rdf:resource="http://erlangen-crm.org/current/E64_End_of_Existence"/>
         <rdfs:range rdf:resource="http://erlangen-crm.org/current/E77_Persistent_Item"/>
         <rdfs:subPropertyOf rdf:resource="http://erlangen-crm.org/current/P12_occurred_in_the_presence_of"/>
         <rdfs:superPropertyOf rdf:resource="http://erlangen-crm.org/current/P13_destroyed"/>
         <rdfs:superPropertyOf rdf:resource="http://erlangen-crm.org/current/P99_dissolved"/>
         <rdfs:superPropertyOf rdf:resource="http://erlangen-crm.org/current/P100_was_death_of"/>
         <rdfs:superPropertyOf rdf:resource="http://erlangen-crm.org/current/P124_transformed"/>
         <rdfs:comment>Quantification:
   one to many, necessary (1,n:0,1)</rdfs:comment>
         <rdfs:comment>Scope note:
   </rdfs:comment>
         <rdfs:comment>Examples:
   </rdfs:comment>
      </owl:ObjectProperty>
   <!--http://erlangen-crm.org/current/P94_has_created-->
   <owl:ObjectProperty rdf:about="http://erlangen-crm.org/current/P94_has_created">
      <rdfs:label xml:lang="en">P94 has created</rdfs:label>
      <owl:inverseOf rdf:resource="http://erlangen-crm.org/current/P94i_was_created_by"/>
      <rdfs:domain rdf:resource="http://erlangen-crm.org/current/E65_Creation"/>
      <rdfs:range rdf:resource="http://erlangen-crm.org/current/E28_Conceptual_Object"/>
      <rdfs:subPropertyOf rdf:resource="http://erlangen-crm.org/current/P92_brought_into_existence"/>
      <rdfs:superPropertyOf rdf:resource="http://erlangen-crm.org/current/P135_created_type"/>
      <rdfs:comment>Quantification:
one to many, necessary, dependent (1,n:1,1)</rdfs:comment>
      <rdfs:comment>Scope note:
This property allows a conceptual E65 Creation to be linked to the E28 Conceptual Object created by it.It represents the act of conceiving the intellectual content of the E28 Conceptual Object. It does not represent the act of creating the first physical carrier of the E28 Conceptual Object. As an example, this is the composition of a poem, not its commitment to paper.</rdfs:comment>
      <rdfs:comment>Examples:
the composition of “The Four Friends” by A. A. Milne (E65) has created “The Four Friends” by A. A. Milne (E28)</rdfs:comment>
   </owl:ObjectProperty>
   <!--http://erlangen-crm.org/current/P95_has_formed-->
   <owl:ObjectProperty rdf:about="http://erlangen-crm.org/current/P95_has_formed">
      <rdfs:label xml:lang="en">P95 has formed</rdfs:label>
      <owl:inverseOf rdf:resource="http://erlangen-crm.org/current/P95i_was_formed_by"/>
      <rdfs:domain rdf:resource="http://erlangen-crm.org/current/E66_Formation"/>
      <rdfs:range rdf:resource="http://erlangen-crm.org/current/E74_Group"/>
      <rdfs:subPropertyOf rdf:resource="http://erlangen-crm.org/current/P92_brought_into_existence"/>
      <rdfs:comment>Quantification:
one to many, necessary, dependent (1,n:1,1)</rdfs:comment>
      <rdfs:comment>Scope note:
This property links the founding or E66 Formation for an E74 Group with the Group itself.</rdfs:comment>
      <rdfs:comment>Examples:
the formation of the CIDOC CRM SIG at the August 2000 CIDOC Board meeting (E66) has formed the CIDOC CRM Special Interest Group (E74)</rdfs:comment>
   </owl:ObjectProperty>
   <!--http://erlangen-crm.org/current/P98_brought_into_life-->
   <owl:ObjectProperty rdf:about="http://erlangen-crm.org/current/P98_brought_into_life">
      <rdfs:label xml:lang="en">P98 brought into life</rdfs:label>
      <owl:inverseOf rdf:resource="http://erlangen-crm.org/current/P98i_was_born"/>
      <rdfs:domain rdf:resource="http://erlangen-crm.org/current/E67_Birth"/>
      <rdfs:range rdf:resource="http://erlangen-crm.org/current/E21_Person"/>
      <rdfs:subPropertyOf rdf:resource="http://erlangen-crm.org/current/P92_brought_into_existence"/>
      <rdfs:comment>Quantification:
one to many, dependent (0,n:1,1)</rdfs:comment>
      <rdfs:comment>Scope note:
This property links an E67 Birth event to an E21 Person in the role of offspring.Twins, triplets etc. are brought into life by the same Birth event. This is not intended for use with general Natural History material, only people. There is no explicit method for modelling conception and gestation except by using extensions.</rdfs:comment>
      <rdfs:comment>Examples:
the Birth of Queen Elizabeth II (E67) brought into life Queen Elizabeth II (E21)</rdfs:comment>
   </owl:ObjectProperty>
   <!--http://erlangen-crm.org/current/P100_was_death_of-->
   <owl:ObjectProperty rdf:about="http://erlangen-crm.org/current/P100_was_death_of">
      <rdfs:label xml:lang="en">P100 was death of</rdfs:label>
      <owl:inverseOf rdf:resource="http://erlangen-crm.org/current/P100i_died_in"/>
      <rdfs:domain rdf:resource="http://erlangen-crm.org/current/E69_Death"/>
      <rdfs:range rdf:resource="http://erlangen-crm.org/current/E21_Person"/>
      <rdfs:subPropertyOf rdf:resource="http://erlangen-crm.org/current/P93_took_out_of_existence"/>
      <rdfs:comment>Quantification:
one to many, necessary (1,n:0,n)</rdfs:comment>
      <rdfs:comment>Scope note:
This property links an E69 Death event to the E21 Person that died.A Death event may involve multiple people, for example in the case of a battle or disaster.This is not intended for use with general Natural History material, only people.</rdfs:comment>
      <rdfs:comment>Examples:
Mozart’s death (E69) was death of Mozart (E21)</rdfs:comment>
   </owl:ObjectProperty>
   <!--http://erlangen-crm.org/current/P102_has_title-->
   <owl:ObjectProperty rdf:about="http://erlangen-crm.org/current/P102_has_title">
      <rdfs:label xml:lang="en">P102 has title</rdfs:label>
      <owl:inverseOf rdf:resource="http://erlangen-crm.org/current/P102i_is_title_of"/>
      <rdfs:domain rdf:resource="http://erlangen-crm.org/current/E71_Man-Made_Thing"/>
      <rdfs:range rdf:resource="http://erlangen-crm.org/current/E35_Title"/>
      <rdfs:subPropertyOf rdf:resource="http://erlangen-crm.org/current/P1_is_identified_by"/>
      <rdfs:comment>Quantification:
many to many (0,n:0,n)</rdfs:comment>
      <rdfs:comment>Scope note:
This property describes the E35 Title applied to an instance of E71 Man-Made Thing. The E55 Type of Title is assigned in a sub property.The P102.1 has type property of the P102 has title (is title of) property enables the relationship between the Title and the thing to be further clarified, for example, if the Title was a given Title, a supplied Title etc.It allows any man-made material or immaterial thing to be given a Title. It is possible to imagine a Title being created without a specific object in mind.</rdfs:comment>
      <rdfs:comment>Examples:
the first book of the Old Testament (E33) has title “Genesis” (E35)has type translated (E55)Properties:P102.1 has type: E55 Type</rdfs:comment>
   </owl:ObjectProperty>
   <!--http://erlangen-crm.org/current/P103_was_intended_for-->
   <owl:ObjectProperty rdf:about="http://erlangen-crm.org/current/P103_was_intended_for">
      <rdfs:label xml:lang="en">P103 was intended for</rdfs:label>
      <owl:inverseOf rdf:resource="http://erlangen-crm.org/current/P103i_was_intention_of"/>
      <rdfs:domain rdf:resource="http://erlangen-crm.org/current/E71_Man-Made_Thing"/>
      <rdfs:range rdf:resource="http://erlangen-crm.org/current/E55_Type"/>
      <rdfs:comment>Quantification:
many to many (0,n:0,n)</rdfs:comment>
      <rdfs:comment>Scope note:
This property links an instance of E71 Man-Made Thing to an E55 Type of usage.It creates a property between specific man-made things, both physical and immaterial, to Types of intended methods and techniques of use. Note: A link between specific man-made things and a specific use activity should be expressed using P19 was intended use of (was made for).</rdfs:comment>
      <rdfs:comment>Examples:
this plate (E22) was intended for being destroyed at wedding reception (E55)</rdfs:comment>
   </owl:ObjectProperty>
   <!--http://erlangen-crm.org/current/P104_is_subject_to-->
   <owl:ObjectProperty rdf:about="http://erlangen-crm.org/current/P104_is_subject_to">
      <rdfs:label xml:lang="en">P104 is subject to</rdfs:label>
      <owl:inverseOf rdf:resource="http://erlangen-crm.org/current/P104i_applies_to"/>
      <rdfs:domain rdf:resource="http://erlangen-crm.org/current/E72_Legal_Object"/>
      <rdfs:range rdf:resource="http://erlangen-crm.org/current/E30_Right"/>
      <rdfs:comment>Quantification:
many to many (0,n:0,n)</rdfs:comment>
      <rdfs:comment>Scope note:
This property links a particular E72 Legal Object to the instances of E30 Right to which it is subject.The Right is held by an E39 Actor as described by P75 possesses (is possessed by).</rdfs:comment>
      <rdfs:comment>Examples:
Beatles back catalogue (E72) is subject to reproduction right on Beatles back catalogue (E30)</rdfs:comment>
   </owl:ObjectProperty>
   <!--http://erlangen-crm.org/current/P105_right_held_by-->
   <owl:ObjectProperty rdf:about="http://erlangen-crm.org/current/P105_right_held_by">
      <rdfs:label xml:lang="en">P105 right held by</rdfs:label>
      <owl:inverseOf rdf:resource="http://erlangen-crm.org/current/P105i_has_right_on"/>
      <rdfs:domain rdf:resource="http://erlangen-crm.org/current/E72_Legal_Object"/>
      <rdfs:range rdf:resource="http://erlangen-crm.org/current/E39_Actor"/>
      <rdfs:superPropertyOf rdf:resource="http://erlangen-crm.org/current/P52_has_current_owner"/>
      <rdfs:comment>Quantification:
many to many (0,n:0,n)</rdfs:comment>
      <rdfs:comment>Scope note:
This property identifies the E39 Actor who holds the instances of E30 Right to an E72 Legal Object.It is a superproperty of P52 has current owner (is current owner of) because ownership is a right that is held on the owned object.P105 right held by (has right on) is a shortcut of the fully developed path from E72 Legal Object through P104 is subject to (applies to), E30 Right, P75 possesses (is possessed by) to E39 Actor.</rdfs:comment>
      <rdfs:comment>Examples:
Beatles back catalogue (E73) right held by Michael Jackson (E21)</rdfs:comment>
   </owl:ObjectProperty>
   <!--http://erlangen-crm.org/current/P106_is_composed_of-->
   <owl:ObjectProperty rdf:about="http://erlangen-crm.org/current/P106_is_composed_of">
      <rdfs:label xml:lang="en">P106 is composed of</rdfs:label>
      <owl:inverseOf rdf:resource="http://erlangen-crm.org/current/P106i_forms_part_of"/>
      <rdfs:domain rdf:resource="http://erlangen-crm.org/current/E90_Symbolic_Object"/>
      <rdfs:range rdf:resource="http://erlangen-crm.org/current/E90_Symbolic_Object"/>
      <rdfs:comment>Quantification:
many to many (0,n:0,n)</rdfs:comment>
      <rdfs:comment>Scope note:
This property associates an instance of E90 Symbolic Object with a part of it that is by itself an instance of E90 Symbolic Object, such as fragments of texts or clippings from an image.</rdfs:comment>
      <rdfs:comment>Examples:
This Scope note (E33) P106 is composed of ‘fragments of texts’ (E33) ‘recognizable’ (E90) P106 is composed of ‘ecognizabl’ (E90)</rdfs:comment>
   </owl:ObjectProperty>
   <!--http://erlangen-crm.org/current/P107_has_current_or_former_member-->
   <owl:ObjectProperty rdf:about="http://erlangen-crm.org/current/P107_has_current_or_former_member">
      <rdfs:label xml:lang="en">P107 has current or former member</rdfs:label>
      <owl:inverseOf rdf:resource="http://erlangen-crm.org/current/P107i_is_current_or_former_member_of"/>
      <rdfs:domain rdf:resource="http://erlangen-crm.org/current/E74_Group"/>
      <rdfs:range rdf:resource="http://erlangen-crm.org/current/E39_Actor"/>
      <rdfs:comment>Quantification:
many to many (0,n:0,n)</rdfs:comment>
      <rdfs:comment>Scope note:
This property relates an E39 Actor to the E74 Group of which that E39 Actor is a member.Groups, Legal Bodies and Persons, may all be members of Groups. A Group necessarily consists of more than one member.This property is a shortcut of the more fully developed path from E74 Group through P144 joined with (gained member by), E85 Joining, P143 joined (was joined by) to E39 Actor.The property P107.1 kind of member can be used to specify the type of membership or the role the member has in the group.</rdfs:comment>
      <rdfs:comment>Examples:
Moholy Nagy (E21) is current or former member of Bauhaus (E74) National Museum of Science and Industry (E40) has current or former member The National Railway Museum (E40) The married couple Queen Elisabeth and Prince Phillip (E74) has current or former member Prince Phillip (E21) with P107.1 kind of member husband (E55 Type)Properties:P107.1 kind of member: E55 Type</rdfs:comment>
   </owl:ObjectProperty>
   <!--http://erlangen-crm.org/current/P108_has_produced-->
   <owl:ObjectProperty rdf:about="http://erlangen-crm.org/current/P108_has_produced">
      <rdfs:label xml:lang="en">P108 has produced</rdfs:label>
      <owl:inverseOf rdf:resource="http://erlangen-crm.org/current/P108i_was_produced_by"/>
      <rdfs:domain rdf:resource="http://erlangen-crm.org/current/E12_Production"/>
      <rdfs:range rdf:resource="http://erlangen-crm.org/current/E24_Physical_Man-Made_Thing"/>
      <rdfs:subPropertyOf rdf:resource="http://erlangen-crm.org/current/P31_has_modified"/>
      <rdfs:subPropertyOf rdf:resource="http://erlangen-crm.org/current/P92_brought_into_existence"/>
      <rdfs:comment>Quantification:
one to many, necessary, dependent (1,n:1,1)</rdfs:comment>
      <rdfs:comment>Scope note:
This property identifies the E24 Physical Man-Made Thing that came into existence as a result of an E12 Production.The identity of an instance of E24 Physical Man-Made Thing is not defined by its matter, but by its existence as a subject of documentation. An E12 Production can result in the creation of multiple instances of E24 Physical Man-Made Thing.</rdfs:comment>
      <rdfs:comment>Examples:
The building of Rome (E12) has produced Τhe Colosseum (E22)</rdfs:comment>
   </owl:ObjectProperty>
   <!--http://erlangen-crm.org/current/P125_used_object_of_type-->
   <owl:ObjectProperty rdf:about="http://erlangen-crm.org/current/P125_used_object_of_type">
      <rdfs:label xml:lang="en">P125 used object of type</rdfs:label>
      <owl:inverseOf rdf:resource="http://erlangen-crm.org/current/P125i_was_type_of_object_used_in"/>
      <rdfs:domain rdf:resource="http://erlangen-crm.org/current/E7_Activity"/>
      <rdfs:range rdf:resource="http://erlangen-crm.org/current/E55_Type"/>
      <rdfs:superPropertyOf rdf:resource="http://erlangen-crm.org/current/P32_used_general_technique"/>
      <rdfs:comment>Quantification:
many to many (0,n:0,n)</rdfs:comment>
      <rdfs:comment>Scope note:
This property defines the kind of objects used in an E7 Activity, when the specific instance is either unknown or not of interest, such as use of "a hammer".</rdfs:comment>
      <rdfs:comment>Examples:
at the Battle of Agincourt (E7), the English archers used object of type long bow (E55)</rdfs:comment>
   </owl:ObjectProperty>
   <!--http://erlangen-crm.org/current/P127_has_broader_term-->
   <owl:ObjectProperty rdf:about="http://erlangen-crm.org/current/P127_has_broader_term">
      <rdfs:label xml:lang="en">P127 has broader term</rdfs:label>
      <owl:inverseOf rdf:resource="http://erlangen-crm.org/current/P127i_has_narrower_term"/>
      <rdfs:domain rdf:resource="http://erlangen-crm.org/current/E55_Type"/>
      <rdfs:range rdf:resource="http://erlangen-crm.org/current/E55_Type"/>
      <rdfs:comment>Quantification:
many to many (0,n:0,n)</rdfs:comment>
      <rdfs:comment>Scope note:
This property identifies a super-Type to which an E55 Type is related.It allows Types to be organised into hierarchies. This is the sense of "broader term generic (BTG)" as defined in ISO 2788.</rdfs:comment>
      <rdfs:comment>Examples:
dime (E55) has broader term coin (E55)</rdfs:comment>
   </owl:ObjectProperty>
   <!--http://erlangen-crm.org/current/P128_carries-->
   <owl:ObjectProperty rdf:about="http://erlangen-crm.org/current/P128_carries">
      <rdfs:label xml:lang="en">P128 carries</rdfs:label>
      <owl:inverseOf rdf:resource="http://erlangen-crm.org/current/P128i_is_carried_by"/>
      <rdfs:domain rdf:resource="http://erlangen-crm.org/current/E24_Physical_Man-Made_Thing"/>
      <rdfs:range rdf:resource="http://erlangen-crm.org/current/E90_Symbolic_Object"/>
      <rdfs:subPropertyOf rdf:resource="http://erlangen-crm.org/current/P130_shows_features_of"/>
      <rdfs:superPropertyOf rdf:resource="http://erlangen-crm.org/current/P65_shows_visual_item"/>
      <rdfs:comment>Quantification:
many to many (0,n:0,n)</rdfs:comment>
      <rdfs:comment>Scope note:
This property identifies an E90 Symbolic Object carried by an instance of E24 Physical Man-Made Thing.In general this would be an E84 Information Carrier. P65 shows visual item (is shown by) is a specialisation of P128 carries (is carried by) which should be used for carrying visual items.</rdfs:comment>
      <rdfs:comment>Examples:
Matthew’s paperback copy of Reach for the Sky (E84) carries the text of Reach for the Sky (E73)</rdfs:comment>
   </owl:ObjectProperty>
   <!--http://erlangen-crm.org/current/P129_is_about-->
   <owl:ObjectProperty rdf:about="http://erlangen-crm.org/current/P129_is_about">
      <rdfs:label xml:lang="en">P129 is about</rdfs:label>
      <owl:inverseOf rdf:resource="http://erlangen-crm.org/current/P129i_is_subject_of"/>
      <rdfs:domain rdf:resource="http://erlangen-crm.org/current/E89_Propositional_Object"/>
      <rdfs:range rdf:resource="http://erlangen-crm.org/current/E1_CRM_Entity"/>
      <rdfs:subPropertyOf rdf:resource="http://erlangen-crm.org/current/P67_refers_to"/>
      <rdfs:comment>Quantification:
many to many (0,n:0,n)</rdfs:comment>
      <rdfs:comment>Scope note:
This property documents that an E89 Propositional Object has as subject an instance of E1 CRM Entity.This differs from P67 refers to (is referred to by), which refers to an E1 CRM Entity, in that it describes the primary subject or subjects of an E89 Propositional Object.</rdfs:comment>
      <rdfs:comment>Examples:
The text entitled ‘Reach for the sky’ (E33) is about Douglas Bader (E21)</rdfs:comment>
   </owl:ObjectProperty>
   <!--http://erlangen-crm.org/current/P130_shows_features_of-->
   <owl:ObjectProperty rdf:about="http://erlangen-crm.org/current/P130_shows_features_of">
      <rdfs:label xml:lang="en">P130 shows features of</rdfs:label>
      <owl:inverseOf rdf:resource="http://erlangen-crm.org/current/P130i_features_are_also_found_on"/>
      <rdfs:domain rdf:resource="http://erlangen-crm.org/current/E70_Thing"/>
      <rdfs:range rdf:resource="http://erlangen-crm.org/current/E70_Thing"/>
      <rdfs:superPropertyOf rdf:resource="http://erlangen-crm.org/current/P73_has_translation"/>
      <rdfs:comment>Quantification:
many to many (0,n:0,n)</rdfs:comment>
      <rdfs:comment>Scope note:
This property generalises the notions of "copy of" and "similar to" into a dynamic, asymmetric relationship, where the domain expresses the derivative, if such a direction can be established.Otherwise, the relationship is symmetric. It is a shortcut of P15 was influenced by (influenced) in a creation or production, if such a reason for the similarity can be verified. Moreover it expresses similarity in cases that can be stated between two objects only, without historical knowledge about its reasons.</rdfs:comment>
      <rdfs:comment>Examples:
the Parthenon Frieze on the Acropolis in Athens (E22) shows features of the Original Parthenon Frieze in the British museum (E22). Kind of similarity: Copy (E55)Properties:P130.1 kind of similarity: E55 Type</rdfs:comment>
   </owl:ObjectProperty>
   <!--http://erlangen-crm.org/current/P131_is_identified_by-->
   <owl:ObjectProperty rdf:about="http://erlangen-crm.org/current/P131_is_identified_by">
      <rdfs:label xml:lang="en">P131 is identified by</rdfs:label>
      <owl:inverseOf rdf:resource="http://erlangen-crm.org/current/P131i_identifies"/>
      <rdfs:domain rdf:resource="http://erlangen-crm.org/current/E39_Actor"/>
      <rdfs:range rdf:resource="http://erlangen-crm.org/current/E82_Actor_Appellation"/>
      <rdfs:subPropertyOf rdf:resource="http://erlangen-crm.org/current/P1_is_identified_by"/>
      <rdfs:comment>Quantification:
many to many (0,n:0,n)</rdfs:comment>
      <rdfs:comment>Scope note:
This property identifies a name used specifically to identify an E39 Actor.This property is a specialisation of P1 is identified by (identifies) is identified by.</rdfs:comment>
      <rdfs:comment>Examples:
Tyler Withersopp IV (E39) is identified by US social security number “619-17-4204” (E82)</rdfs:comment>
   </owl:ObjectProperty>
   <!--http://erlangen-crm.org/current/P138_represents-->
   <owl:ObjectProperty rdf:about="http://erlangen-crm.org/current/P138_represents">
      <rdfs:label xml:lang="en">P138 represents</rdfs:label>
      <owl:inverseOf rdf:resource="http://erlangen-crm.org/current/P138i_has_representation"/>
      <rdfs:domain rdf:resource="http://erlangen-crm.org/current/E36_Visual_Item"/>
      <rdfs:range rdf:resource="http://erlangen-crm.org/current/E1_CRM_Entity"/>
      <rdfs:subPropertyOf rdf:resource="http://erlangen-crm.org/current/P67_refers_to"/>
      <rdfs:comment>Quantification:
many to many (0,n:0,n)</rdfs:comment>
      <rdfs:comment>Scope note:
This property establishes the relationship between an E36 Visual Item and the entity that it visually represents.Any entity may be represented visually. This property is part of the fully developed path from E24 Physical Man-Made Thing through P65 shows visual item (is shown by), E36 Visual Item, P138 represents (has representation) to E1 CRM Entity, which is shortcut by P62depicts (is depicted by). P138.1 mode of representation allows the nature of the representation to be refined.</rdfs:comment>
      <rdfs:comment>Examples:
the design on the reverse of a Swiss coin (E36) represents Helvetia (E28) mode of representation Profile (E55)Properties:P138.1 mode of representation: E55 Type</rdfs:comment>
   </owl:ObjectProperty>
   <!--http://erlangen-crm.org/current/P140_assigned_attribute_to-->
   <owl:ObjectProperty rdf:about="http://erlangen-crm.org/current/P140_assigned_attribute_to">
      <rdfs:label xml:lang="en">P140 assigned attribute to</rdfs:label>
      <owl:inverseOf rdf:resource="http://erlangen-crm.org/current/P140i_was_attributed_by"/>
      <rdfs:domain rdf:resource="http://erlangen-crm.org/current/E13_Attribute_Assignment"/>
      <rdfs:range rdf:resource="http://erlangen-crm.org/current/E1_CRM_Entity"/>
      <rdfs:superPropertyOf rdf:resource="http://erlangen-crm.org/current/P34_concerned"/>
      <rdfs:superPropertyOf rdf:resource="http://erlangen-crm.org/current/P39_measured"/>
      <rdfs:superPropertyOf rdf:resource="http://erlangen-crm.org/current/P41_classified"/>
      <rdfs:comment>Quantification:
many to many (0,n:0,n)</rdfs:comment>
      <rdfs:comment>Scope note:
This property indicates the item to which an attribute or relation is assigned.</rdfs:comment>
      <rdfs:comment>Examples:
February 1997 Current Ownership Assessment of Martin Doerr’s silver cup (E13) assigned attribute to Martin Doerr’s silver cup (E19) 01 June 1997 Identifier Assignment of the silver cup donated by Martin Doerr (E15) assigned attribute to silver cup 232 (E19)</rdfs:comment>
   </owl:ObjectProperty>
   <!--http://erlangen-crm.org/current/P141_assigned-->
   <owl:ObjectProperty rdf:about="http://erlangen-crm.org/current/P141_assigned">
      <rdfs:label xml:lang="en">P141 assigned</rdfs:label>
      <owl:inverseOf rdf:resource="http://erlangen-crm.org/current/P141i_was_assigned_by"/>
      <rdfs:domain rdf:resource="http://erlangen-crm.org/current/E13_Attribute_Assignment"/>
      <rdfs:range rdf:resource="http://erlangen-crm.org/current/E1_CRM_Entity"/>
      <rdfs:superPropertyOf rdf:resource="http://erlangen-crm.org/current/P35_has_identified"/>
      <rdfs:superPropertyOf rdf:resource="http://erlangen-crm.org/current/P37_assigned"/>
      <rdfs:superPropertyOf rdf:resource="http://erlangen-crm.org/current/P38_deassigned"/>
      <rdfs:superPropertyOf rdf:resource="http://erlangen-crm.org/current/P40_observed_dimension"/>
      <rdfs:superPropertyOf rdf:resource="http://erlangen-crm.org/current/P42_assigned"/>
      <rdfs:comment>Quantification:
many to many (0,n:0,n)</rdfs:comment>
      <rdfs:comment>Scope note:
This property indicates the attribute that was assigned or the item that was related to the item denoted by a property P140 assigned attribute to in an Attribute assignment action.</rdfs:comment>
      <rdfs:comment>Examples:
February 1997 Current Ownership Assessment of Martin Doerr’s silver cup (E13) assigned Martin Doerr (E21) 01 June 1997 Identifier Assignment of the silver cup donated by Martin Doerr (E15) assigned object identifier “232” (E42)</rdfs:comment>
   </owl:ObjectProperty>
   <!--http://erlangen-crm.org/current/P142_used_constituent-->
   <owl:ObjectProperty rdf:about="http://erlangen-crm.org/current/P142_used_constituent">
      <rdfs:label xml:lang="en">P142 used constituent</rdfs:label>
      <owl:inverseOf rdf:resource="http://erlangen-crm.org/current/P142i_was_used_in"/>
      <rdfs:domain rdf:resource="http://erlangen-crm.org/current/E15_Identifier_Assignment"/>
      <rdfs:range rdf:resource="http://erlangen-crm.org/current/E90_Symbolic_Object"/>
      <rdfs:subPropertyOf rdf:resource="http://erlangen-crm.org/current/P16_used_specific_object"/>
      <rdfs:comment>Quantification:
(0,n:0,n)</rdfs:comment>
      <rdfs:comment>Scope note:
This property associates the event of assigning an instance of E42 Identifier with the instances of E90 Symbolic Object that were used as constituents of the identifier.</rdfs:comment>
      <rdfs:comment>Examples:
On June 1, 2001 assigning the personal name identifier “Guillaume, de Machaut, ca. 1300-1377” (E15) used constituent “ca. 1300-1377” (E49) Assigning a uniform title to the anonymous textual work known as ‘The Adoration of the Shepherds’(E15) used constituent ‘Coventry’ (E48) Assigning a uniform title to Pina Bausch’s choreographic work entitled ‘Rite of spring’ (E15) used constituent ‘(Choreographic Work: Bausch)’(E90) Assigning a uniform title to the motion picture directed in 1933 by Merian C. Cooper and Ernest B. Schoedsack and entitled ‘King Kong’ (E15) used constituent ‘1933’ (E50) Assigning the corporate name identifier ‘Univerza v Ljubljani. Oddelek za bibliotekarstvo’ to The Department for library science of the University of Ljubljana (E15) used constituent ‘Univerza v Ljubljani’ (E42)</rdfs:comment>
   </owl:ObjectProperty>
   <!--http://erlangen-crm.org/current/P148_has_component-->
   <owl:ObjectProperty rdf:about="http://erlangen-crm.org/current/P148_has_component">
      <rdfs:label xml:lang="en">P148 has component</rdfs:label>
      <owl:inverseOf rdf:resource="http://erlangen-crm.org/current/P148i_is_component_of"/>
      <rdfs:domain rdf:resource="http://erlangen-crm.org/current/E89_Propositional_Object"/>
      <rdfs:range rdf:resource="http://erlangen-crm.org/current/E89_Propositional_Object"/>
      <rdfs:comment>Quantification:
(0,n:0,n)</rdfs:comment>
      <rdfs:comment>Scope note:
This property associates an instance of E89 Propositional Object with a structural part of it that is by itself an instance of E89 Propositional Object.</rdfs:comment>
      <rdfs:comment>Examples:
Dante’s “Divine Comedy” (E89) has component Dante’s “Hell” (E89)</rdfs:comment>
   </owl:ObjectProperty>
   <!--http://erlangen-crm.org/current/P151_was_formed_from-->
   <owl:ObjectProperty rdf:about="http://erlangen-crm.org/current/P151_was_formed_from">
      <rdfs:label xml:lang="en">P151 was formed from</rdfs:label>
      <owl:inverseOf rdf:resource="http://erlangen-crm.org/current/P151i_participated_in"/>
      <rdfs:domain rdf:resource="http://erlangen-crm.org/current/E66_Formation"/>
      <rdfs:range rdf:resource="http://erlangen-crm.org/current/E74_Group"/>
      <rdfs:subPropertyOf rdf:resource="http://erlangen-crm.org/current/P11_had_participant"/>
      <rdfs:comment>Quantification:
(0,n:0:n)</rdfs:comment>
      <rdfs:comment>Scope note:
This property associates an instance of E66 Formation with an instance of E74 Group from which the new group was formed preserving a sense of continuity such as in mission, membership or tradition.</rdfs:comment>
      <rdfs:comment>Examples:
The formation of the House of Bourbon-Conti in 1581 (E66) was formed from House of Condé (E74)</rdfs:comment>
   </owl:ObjectProperty>
   <!--http://erlangen-crm.org/current/P165_incorporates-->
   <owl:ObjectProperty rdf:about="http://erlangen-crm.org/current/P165_incorporates">
      <rdfs:label xml:lang="en">P165 incorporates</rdfs:label>
      <owl:inverseOf rdf:resource="http://erlangen-crm.org/current/P165i_is_incorporated_in"/>
      <rdfs:domain rdf:resource="http://erlangen-crm.org/current/E73_Information_Object"/>
      <rdfs:range rdf:resource="http://erlangen-crm.org/current/E90_Symbolic_Object"/>
      <rdfs:subPropertyOf rdf:resource="http://erlangen-crm.org/current/P106_is_composed_of"/>
      <rdfs:comment>Quantification:
(0,n:0,n)</rdfs:comment>
      <rdfs:comment>Scope note:
This property associates an instance of E73 Information Object with an instance of E90 Symbolic Object (or any of its subclasses) that was included in it.This property makes it possible to recognise the autonomous status of the incorporated signs, which were created in a distinct context, and can be incorporated in many distinct self-contained expressions, and to highlight the difference between structural and accidental whole-part relationships between conceptual entities.It accounts for many cultural facts that are quite frequent and significant: the inclusion of a poem in an anthology, the re-use of an operatic aria in a new opera, the use of a reproduction of a painting for a book cover or a CD booklet, the integration of textual quotations, the presence of lyrics in a song that sets those lyrics to music, the presence of the text of a play in a movie based on that play, etc.</rdfs:comment>
   </owl:ObjectProperty>
</rdf:RDF>
